@prefix :        <http://www.w3.org/2002/07/owl#> .
@prefix dc:      <http://purl.org/dc/elements/1.1/> .
@prefix rdfs:    <http://www.w3.org/2000/01/rdf-schema#> .
@prefix ns:      <http://woo.corp.yahoo.com/ns/> .
@prefix xsd:     <http://www.w3.org/2001/XMLSchema#> .
@prefix owl:     <http://www.w3.org/2002/07/owl#> .
@prefix rdf:     <http://www.w3.org/1999/02/22-rdf-syntax-ns#> .

ns:MusicGroup
      a       owl:Class ;
      rdfs:comment "A music group is a group of individuals who band together for the purpose of playing or creating music."@en ;
      owl:label "MusicGroup"@en ;
      owl:subClassOf
              [ a       owl:Class ;
                :intersectionOf (ns:Group ns:MusicArtist)
              ] .

ns:Ceremony
      a       owl:Class ;
      rdfs:comment "An event created to mark a special occasion or to give out awards. Examples: Oscars, Emmys, Tonys, Nobel. Not to be confused with the actual awards themselves."@en ;
      rdfs:label "Ceremony"@en ;
      owl:subClassOf ns:Event .

ns:connectionTo
      a       owl:ObjectProperty ;
      rdfs:comment "connectionTo connects an organization to the reified OrgAffiliation   (need to represent an entity's affiliation to org for time x)"@en ;
      rdfs:domain ns:Organization ;
      rdfs:label "connectionTo"@en ;
      rdfs:range ns:OrgAffiliation .

ns:url
      a       :FunctionalProperty , owl:DatatypeProperty ;
      rdfs:comment "Specific URL for a webpage."@en ;
      rdfs:domain
              [ a       owl:Class ;
                :unionOf (ns:EventVenue ns:Image ns:LocalEvent ns:OnlineAccount ns:Webpage)
              ] ;
      rdfs:label "url"@en ;
      rdfs:range xsd:anyURI ;
      owl:subPropertyOf :topDataProperty .

ns:publisher
      a       :FunctionalProperty , owl:ObjectProperty ;
      rdfs:comment "Connects a Media Work to its publisher."@en ;
      rdfs:domain
              [ a       owl:Class ;
                :unionOf (ns:MediaWork ns:Synopsis)
              ] ;
      rdfs:label "publisher"@en ;
      rdfs:range ns:Publisher ;
      :inverseOf ns:publisherOf .

ns:parking
      a       owl:DatatypeProperty ;
      rdfs:comment "Describes the type and availability of parking at a location. Allowed values: has_parking, free, paid, valet, no_parking "@en ;
      rdfs:domain
              [ a       owl:Class ;
                :unionOf (ns:LocalBusiness ns:Structure)
              ] ;
      rdfs:label "parking"@en ;
      rdfs:range owl:Literal ;
      rdfs:range
              [ a       owl:Datatype ;
                :oneOf  [ a       rdf:List ;
                          rdf:first "FREE"^^xsd:string ;
                          rdf:rest
                                  [ a       rdf:List ;
                                    rdf:first "HAS PARKING"^^xsd:string ;
                                    rdf:rest
                                            [ a       rdf:List ;
                                              rdf:first "NO PARKING"^^xsd:string ;
                                              rdf:rest
                                                      [ a       rdf:List ;
                                                        rdf:first "PAID"^^xsd:string ;
                                                        rdf:rest
                                                                [ a       rdf:List ;
                                                                  rdf:first "STREET"^^xsd:string ;
                                                                  rdf:rest
                                                                          [ a       rdf:List ;
                                                                            rdf:first "VALET"^^xsd:string ;
                                                                            rdf:rest ()
                                                                          ]
                                                                ]
                                                      ]
                                            ]
                                  ]
                        ]
              ] ;
      owl:subPropertyOf :topDataProperty .

ns:featureRating
      a       owl:DatatypeProperty ;
      rdfs:comment "Rating assigned to the special features available on a DVD."@en ;
      rdfs:domain ns:Video ;
      rdfs:label "featureRating"@en ;
      rdfs:range owl:Literal ;
      owl:subPropertyOf :topDataProperty .

ns:financeInstrumentName
      a       :FunctionalProperty , owl:DatatypeProperty ;
      rdfs:comment "financenstrumentName is the name (if any) for this quotable instrument. For example, Yahoo! Common Stock on NASDAQ. "@en ;
      rdfs:domain
              [ a       owl:Class ;
                :unionOf (ns:FinancialInstrument ns:QuotableInstrument)
              ] ;
      rdfs:label "financeInstrumentName"@en ;
      rdfs:range owl:Literal ;
      owl:subPropertyOf ns:name .

ns:stockExchange
      a       owl:ObjectProperty ;
      rdfs:comment "stockExchange connects a publicly traded company to its primary stock exchange"@en ;
      rdfs:domain ns:PublicCompany ;
      rdfs:label "stockExchange"@en ;
      rdfs:range ns:StockExchange ;
      :inverseOf ns:stockExchangeOf .

ns:SportGame
      a       owl:Class ;
      rdfs:comment "A sports game is a competitive event between individuals or teams."@en ;
      rdfs:label "SportGame"@en ;
      owl:subClassOf ns:LocalEvent .

ns:alcoholAllowed
      a       :FunctionalProperty , owl:DatatypeProperty ;
      rdfs:comment "Indicates if alcohol is available at a local business."@en ;
      rdfs:domain
              [ a       owl:Class ;
                :unionOf (ns:LocalBusiness ns:LocalEvent)
              ] ;
      rdfs:label "alcoholAllowed"@en ;
      rdfs:range xsd:boolean .

ns:deathDate
      a       :FunctionalProperty , owl:DatatypeProperty ;
      rdfs:comment "The date on which an individual becomes deceased."@en ;
      rdfs:domain ns:Person ;
      rdfs:label "deathDate"@en ;
      rdfs:range
              [ a       owl:Datatype ;
                :unionOf (xsd:date xsd:gYearMonth)
              ] ;
      owl:subPropertyOf ns:date .

ns:Director
      a       owl:Class ;
      rdfs:comment "A director is a person who directs the making or production of a film, television program, or play."@en ;
      rdfs:label "Director"@en ;
      owl:subClassOf ns:Person .

ns:healthcareFacilities
      a       owl:DatatypeProperty ;
      rdfs:comment "Enumerates the services offered by a hospital or other healthcare facility."@en ;
      rdfs:domain ns:Healthcare ;
      rdfs:label "healthcareFacilities"@en ;
      rdfs:range
              [ a       owl:Datatype ;
                :oneOf  [ a       rdf:List ;
                          rdf:first "AMBULANCE"^^xsd:string ;
                          rdf:rest
                                  [ a       rdf:List ;
                                    rdf:first "BLOOD BANK"^^xsd:string ;
                                    rdf:rest
                                            [ a       rdf:List ;
                                              rdf:first "CASUALTY"^^xsd:string ;
                                              rdf:rest
                                                      [ a       rdf:List ;
                                                        rdf:first "DIAGNOSTIC SERVICES"^^xsd:string ;
                                                        rdf:rest
                                                                [ a       rdf:List ;
                                                                  rdf:first "ICU"^^xsd:string ;
                                                                  rdf:rest
                                                                          [ a       rdf:List ;
                                                                            rdf:first "MEDICAL SHOP"^^xsd:string ;
                                                                            rdf:rest ()
                                                                          ]
                                                                ]
                                                      ]
                                            ]
                                  ]
                        ]
              ] ;
      owl:subPropertyOf :topDataProperty .

ns:productionStatus
      a       :FunctionalProperty , owl:DatatypeProperty ;
      rdfs:comment "Enumerates the status of a media work while in production."@en ;
      rdfs:domain ns:MediaWork ;
      rdfs:label "productionStatus"@en ;
      rdfs:range owl:Literal ;
      owl:subPropertyOf :topDataProperty .

ns:providerName
      a       owl:DatatypeProperty ;
      rdfs:comment "Name of the data provider"@en ;
      rdfs:domain ns:LocalBusiness ;
      rdfs:label "providerName"@en ;
      rdfs:range owl:Literal ;
      owl:subPropertyOf ns:name .

ns:nominated
      a       owl:ObjectProperty ;
      rdfs:comment "Connects a person, organization, or media work to the award nomination class."@en ;
      rdfs:domain
              [ a       owl:Class ;
                :unionOf (ns:MediaWork ns:Organization ns:Person)
              ] ;
      rdfs:label "nominated"@en ;
      rdfs:range ns:Nomination ;
      owl:subPropertyOf :topObjectProperty .

ns:uriErrorCode
      a       :FunctionalProperty , owl:DatatypeProperty ;
      rdfs:comment "Error code for the URI"@en ;
      rdfs:domain ns:Webpage ;
      rdfs:label "uriErrorCode"@en ;
      rdfs:range owl:Literal ;
      owl:subPropertyOf :topDataProperty .

ns:mediaMenu
      a       owl:DatatypeProperty ;
      rdfs:comment "Menu elements of a media product."@en ;
      rdfs:domain ns:MediaProduct ;
      rdfs:label "mediaMenu"@en ;
      rdfs:range owl:Literal ;
      owl:subPropertyOf :topDataProperty .

ns:contactNameLast
      a       :FunctionalProperty , owl:DatatypeProperty ;
      rdfs:comment "Last name of the contact person for a local business (for use with SingleLocationBusiness only)."@en ;
      rdfs:domain ns:SingleLocationBusiness ;
      rdfs:label "contactNameLast"@en ;
      rdfs:range owl:Literal .

ns:timeZone
      a       :FunctionalProperty , owl:DatatypeProperty ;
      rdfs:comment "timeZone is a region that has a uniform, legally mandated standard time"@en ;
      rdfs:domain ns:Address ;
      rdfs:label "timezone"@en ;
      rdfs:range owl:Literal .

ns:flag
      a       owl:DatatypeProperty ;
      rdfs:comment "One-character code(s) providing additional descriptive information for a DVD."@en ;
      rdfs:domain ns:Video ;
      rdfs:label "flag"@en ;
      rdfs:range owl:Literal ;
      owl:subPropertyOf :topDataProperty .

ns:compensationOf
      a       :FunctionalProperty , owl:ObjectProperty ;
      rdfs:comment "compensationOf connects the type of compensation the the financial person who receives it."@en ;
      rdfs:domain ns:Compensation ;
      rdfs:label "compensationOf"@en ;
      rdfs:range ns:FinancePerson .

ns:personalRelationship
      a       owl:ObjectProperty ;
      rdfs:comment "Connects a person to the reified PersonalRelationship class."@en ;
      rdfs:domain ns:Person ;
      rdfs:label "personalRelationship"@en ;
      rdfs:range ns:PersonalRelationship ;
      owl:subPropertyOf :topObjectProperty .

ns:rates
      a       :FunctionalProperty , owl:ObjectProperty ;
      rdfs:comment "Connects a rating system to the films it categorizes according to thematic and content suitability for certain audiences."@en ;
      rdfs:domain ns:MovieRating ;
      rdfs:label "rates"@en ;
      rdfs:range
              [ a       owl:Class ;
                :unionOf (ns:Movie ns:Video)
              ] ;
      owl:subPropertyOf :topObjectProperty ;
      :inverseOf ns:rated .

ns:affiliation
      a       owl:ObjectProperty ;
      rdfs:comment "affiliation connects the reified class OrgAffiliation to a person, organization or shareholder"@en ;
      rdfs:domain ns:OrgAffiliation ;
      rdfs:label "affiliation"@en ;
      rdfs:range
              [ a       owl:Class ;
                :unionOf (ns:Organization ns:Person)
              ] ;
      :inverseOf ns:affiliationWith .

ns:soldOut
      a       :FunctionalProperty , owl:DatatypeProperty ;
      rdfs:comment "Boolean attribute indicating if an event is sold out."@en ;
      rdfs:domain
              [ a       owl:Class ;
                :unionOf (ns:Deal ns:EventRegistration ns:LocalEventOccurrence)
              ] ;
      rdfs:label "soldOut"@en ;
      rdfs:range xsd:boolean .

ns:TQIAffiliation
      a       owl:Class ;
      rdfs:comment "TQIAffiliation is a reified class linking a tradeablequoteableinstrument to a ticker"@en ;
      rdfs:label "TQIAffiliation"@en ;
      owl:subClassOf ns:Event .

ns:dealShortTitle
      a       owl:DatatypeProperty ;
      rdfs:comment "Abbreviated title of a deal, coupon, or offer."@en ;
      rdfs:domain ns:Deal ;
      rdfs:label "dealShortTitle"@en ;
      rdfs:range owl:Literal ;
      owl:subPropertyOf ns:label .

ns:mtLists
      a       owl:ObjectProperty ;
      rdfs:comment "mtLists connects a market tier to the tradablequotable instruments that it lists"@en ;
      rdfs:domain ns:MarketTier ;
      rdfs:label "mtLists"@en ;
      rdfs:range ns:TradableQuotableInstrument ;
      :inverseOf ns:mtListedOn .

ns:openingDays
      a       :FunctionalProperty , owl:DatatypeProperty ;
      rdfs:comment "Number of days in a given week or weekend that a film was open."@en ;
      rdfs:domain
              [ a       owl:Class ;
                :unionOf (ns:BoxOfficeWeekend ns:BoxOfficeWeekly)
              ] ;
      rdfs:label "openingDays"@en ;
      rdfs:range xsd:int ;
      owl:subPropertyOf :topDataProperty .

ns:valueText
      a       owl:DatatypeProperty ;
      rdfs:comment "example: 99.00USD"@en , "Indicates the actual value of a deal or offer."@en ;
      rdfs:label "valueText"@en .

ns:Island
      a       owl:Class ;
      rdfs:comment "placetype code: 13"@en , "An Island. Example: Alcatraz."@en ;
      rdfs:label "Island"@en ;
      owl:subClassOf ns:Place .

ns:MusicRight
      a       owl:Class ;
      rdfs:comment "The type of right associated with the audio album/track "@en ;
      rdfs:label "MusicRight"@en ;
      owl:subClassOf ns:DistributionRight .

ns:kioskAt
      a       :FunctionalProperty , owl:ObjectProperty ;
      rdfs:comment "kioskAt connects a kiosk (ATM or Redbox for example) to the local business it is at (a Safeway of Walgreens for example)"@en ;
      rdfs:domain ns:Kiosk ;
      rdfs:label "kioskAt"@en ;
      rdfs:range ns:LocalBusiness .

ns:starAnalyst
      a       :FunctionalProperty , owl:DatatypeProperty ;
      rdfs:comment "starAnalyst indicates if an analyst is a star analyst or not"@en ;
      rdfs:domain ns:Analyst ;
      rdfs:label "starAnalyst"@en ;
      rdfs:range xsd:boolean .

ns:albumTrack
      a       owl:ObjectProperty ;
      rdfs:comment "The albumTrack property connects an album with the tracks that make up its constituent parts."@en ;
      rdfs:domain ns:Album ;
      rdfs:label "albumTrack"@en ;
      rdfs:range
              [ a       owl:Class ;
                :unionOf (ns:AlbumTrack ns:Song)
              ] .

ns:recurrenceRule
      a       :FunctionalProperty , owl:DatatypeProperty ;
      rdfs:comment "Conforms to the iCalendar standard: http://www.ietf.org/rfc/rfc2445.txt (page 116)"@en , "Indicates how often and when an event recurs as well as the recurrence end date if present, e.g., monthly, until January 2015."@en ;
      rdfs:domain ns:Event ;
      rdfs:label "recurrenceRule"@en ;
      rdfs:range ns:rRule .

ns:Producer
      a       owl:Class ;
      rdfs:comment "A producer is an individual responsible for the production of a film, television program, or musical album, composition, or song. This includes the executive producer credit."@en ;
      rdfs:label "Producer"@en ;
      owl:subClassOf ns:Person .

ns:primarySIC
      a       :FunctionalProperty , owl:DatatypeProperty ;
      rdfs:comment "This field contains the 6-digit standard industry classification code for the business's primary activity. IinfoUSA source data."@en ;
      rdfs:domain ns:SingleLocationBusiness ;
      rdfs:label "primarySIC"@en ;
      rdfs:range owl:Literal .

ns:areaCode
      a       :FunctionalProperty , owl:DatatypeProperty ;
      rdfs:comment "Area code of a phone number"@en ;
      rdfs:domain ns:Phone ;
      rdfs:label "areaCode"@en ;
      rdfs:range xsd:int ;
      owl:subPropertyOf :topDataProperty .

ns:gameVenueOf
      a       :FunctionalProperty , owl:ObjectProperty ;
      rdfs:comment "Connects a Game to the Venue it was played in."@en ;
      rdfs:domain ns:SportVenue ;
      rdfs:label "gameVenueOf"@en ;
      rdfs:range
              [ a       owl:Class ;
                :unionOf (ns:SportCompetitionInstance ns:SportGame)
              ] ;
      :inverseOf ns:gameVenue .

ns:memberOf
      a       owl:ObjectProperty ;
      rdfs:comment "The memberOf relation connects a group to the people or subgroups that comprise its membership."@en ;
      rdfs:domain
              [ a       owl:Class ;
                :unionOf (ns:Group ns:Person)
              ] ;
      rdfs:label "memberOf"@en ;
      rdfs:range ns:Group .

ns:Coach
      a       owl:Class ;
      rdfs:comment "A person who coaches either an individual athlete or a sports team."@en ;
      rdfs:label "Coach"@en ;
      owl:subClassOf ns:Person .

ns:finaleDate
      a       :FunctionalProperty , owl:DatatypeProperty ;
      rdfs:comment "original date the finale of a TV show aired. ISO 8601 extended."@en ;
      rdfs:domain
              [ a       owl:Class ;
                :unionOf (ns:TvSeason ns:TvSeries)
              ] ;
      rdfs:label "finaleDate"@en ;
      rdfs:range
              [ a       owl:Datatype ;
                :unionOf (xsd:date xsd:gYearMonth)
              ] ;
      owl:subPropertyOf ns:date .

ns:performerName
      a       :FunctionalProperty , owl:DatatypeProperty ;
      rdfs:comment "Name by which a performer is known."@en ;
      rdfs:domain ns:Performer ;
      rdfs:label "performerName"@en ;
      rdfs:range owl:Literal ;
      owl:subPropertyOf ns:name .

ns:newCar
      a       :FunctionalProperty , owl:DatatypeProperty ;
      rdfs:comment "Indicates if the make is currently in production (likely definition). This information is derived from model, trim details in the enrichment phase "@en ;
      rdfs:domain ns:AutoMake ;
      rdfs:label "newCar"@en ;
      rdfs:range xsd:boolean .

ns:county
      a       :FunctionalProperty , owl:DatatypeProperty ;
      rdfs:comment "The county of a physical location"@en ;
      rdfs:domain
              [ a       owl:Class ;
                :unionOf (ns:Address ns:SingleLocationBusiness)
              ] ;
      rdfs:label "county"@en ;
      rdfs:range owl:Literal ;
      owl:subPropertyOf :topDataProperty .

ns:uuid
      a       :FunctionalProperty , owl:DatatypeProperty ;
      rdfs:comment "Unique identifier for an object."@en ;
      rdfs:domain ns:Entity ;
      rdfs:label "uuid"@en ;
      rdfs:range owl:Literal ;
      owl:subPropertyOf ns:id .

ns:quotableInstrumentOf
      a       :FunctionalProperty , owl:ObjectProperty ;
      rdfs:comment "quoteableInstrumentOf connects a quoteable instruemnt to its financial instrument"@en ;
      rdfs:domain ns:QuotableInstrument ;
      rdfs:label "quoteableInstrumentOf"@en ;
      rdfs:range ns:FinancialInstrument ;
      :inverseOf ns:quotableInstrument .

ns:Organization
      a       owl:Class ;
      rdfs:comment " An organization is an organized body of members or people with a particular purpose."@en ;
      rdfs:label "Organization"@en ;
      owl:subClassOf ns:Entity .

ns:statusChangeType
      a       owl:DatatypeProperty ;
      rdfs:comment "statusChangeType captures the type of coroporate status change"@en ;
      rdfs:domain ns:OrganizationStatusChange ;
      rdfs:label "statusChangeType"@en ;
      rdfs:range owl:Literal .

ns:soundSystem
      a       owl:DatatypeProperty ;
      rdfs:comment "Indicates the type of sound system available at a venue."@en ;
      rdfs:domain
              [ a       owl:Class ;
                :unionOf (ns:MovieShowtime ns:MovieTheater)
              ] ;
      rdfs:label "soundSystem"@en ;
      rdfs:range owl:Literal ;
      owl:subPropertyOf :topDataProperty .

ns:contestantOn
      a       owl:ObjectProperty ;
      rdfs:comment "Connects a game show to a contestant who appeared on it."@en ;
      rdfs:domain ns:Contestant ;
      rdfs:label "contestantOn" ;
      rdfs:range
              [ a       owl:Class ;
                :unionOf (ns:TvEpisode ns:TvSeason ns:TvSeries ns:TvSpecial)
              ] ;
      owl:subPropertyOf :topObjectProperty ;
      :inverseOf ns:contestant .

[]    a       :AllDisjointClasses ;
      :members (ns:AthleticConference ns:SportDivision ns:SportLeague ns:SportTeam) .

ns:familyName
      a       :FunctionalProperty , owl:DatatypeProperty ;
      rdfs:comment "Note for Media V2 schema: Change to familyName to support Trailblazers globalization guidelines: http://twiki.corp.yahoo.com/view/TrailBlazers/PersonalNames"@en , "A family name is a surname added to a given name and is part of a personal name."@en ;
      rdfs:domain ns:Person ;
      rdfs:label "familyName"@en ;
      rdfs:range owl:Literal ;
      owl:subPropertyOf ns:name .

ns:astrologicalSign
      a       :FunctionalProperty , owl:DatatypeProperty ;
      rdfs:comment "Designates the astrological sign of a person. "@en ;
      rdfs:domain ns:Person ;
      rdfs:label "astrologicalSign"@en ;
      rdfs:range owl:Literal .

ns:ETN
      a       owl:Class ;
      rdfs:comment "ETN is exchange traded note"@en ;
      rdfs:label "ETN"@en ;
      owl:subClassOf ns:ETO .

ns:numEmployees
      a       :FunctionalProperty , owl:DatatypeProperty ;
      rdfs:comment "numEmployees indicates the number of full-time employees"@en ;
      rdfs:domain ns:Company ;
      rdfs:label "numEmployees"@en ;
      rdfs:range xsd:float .

ns:accessibilityDescription
      a       owl:DatatypeProperty ;
      rdfs:comment "Describes any special features of the wheelchair accessibilityof a business."@en ;
      rdfs:domain ns:LocalBusiness ;
      rdfs:label "accessibilityDescription"@en ;
      rdfs:range owl:Literal .

ns:Founder
      a       owl:Class ;
      rdfs:comment "Founder represents the person or persons who founded a company."@en ;
      rdfs:label "Founder"@en ;
      owl:subClassOf ns:FinancePerson .

ns:lyricsTo
      a       owl:ObjectProperty ;
      rdfs:comment "Attaches the lyrics class to its song or performance"@en ;
      rdfs:domain ns:Lyrics ;
      rdfs:label "lyricsTo"@en ;
      rdfs:range
              [ a       owl:Class ;
                :unionOf (ns:MusicPerformance ns:Song)
              ] ;
      owl:subPropertyOf :topObjectProperty ;
      :inverseOf ns:lyrics .

ns:PointOfInterest
      a       owl:Class ;
      rdfs:comment "Placetype: 20"@en , "A point of interest such as a school, hospital, tourist attraction. Example: statue of Liberty"@en ;
      rdfs:label "PointOfInterest"@en ;
      owl:subClassOf ns:Place .

ns:autoStreetPrice
      a       :FunctionalProperty , owl:DatatypeProperty ;
      rdfs:comment "The street price of a car is the price at which a car actually sells."@en ;
      rdfs:domain
              [ a       owl:Class ;
                :unionOf (ns:AutoMake ns:AutoModel ns:AutoTrim ns:Automobile)
              ] ;
      rdfs:label "autoStreetPrice"@en ;
      rdfs:range xsd:double .

ns:weekendGross
      a       :FunctionalProperty , owl:DatatypeProperty ;
      rdfs:comment "Gross box office receipts for a film in a given weekend."@en ;
      rdfs:domain ns:BoxOfficeWeekend ;
      rdfs:label "weekendGross"@en ;
      rdfs:range xsd:float ;
      owl:subPropertyOf :topDataProperty .

ns:lodgingDetailURL
      a       owl:DatatypeProperty ;
      rdfs:comment "URL at which lodging details about a local business may be accessed."@en ;
      rdfs:domain ns:Lodging ;
      rdfs:label "lodgingDetailURL"@en ;
      rdfs:range xsd:anyURI .

ns:endYear
      a       :FunctionalProperty , owl:DatatypeProperty ;
      rdfs:comment "Year that an event ends."@en ;
      rdfs:domain
              [ a       owl:Class ;
                :unionOf (ns:Event ns:Organization ns:TvSeason)
              ] ;
      rdfs:label "endYear"@en ;
      rdfs:range xsd:gYear ;
      owl:subPropertyOf ns:date .

ns:studentOf
      a       :FunctionalProperty , owl:ObjectProperty ;
      rdfs:comment "Connects an Education class to the EducationalInstitution where the study has been carried out."@en ;
      rdfs:domain ns:Education ;
      rdfs:label "studentOf"@en ;
      rdfs:range ns:EducationalInstitution ;
      owl:subPropertyOf :topObjectProperty .

ns:paymentType
      a       owl:DatatypeProperty ;
      rdfs:comment "Enumerates the types of payment accepted by a business."@en ;
      rdfs:domain
              [ a       owl:Class ;
                :unionOf (ns:LocalBusiness ns:LocalEvent)
              ] ;
      rdfs:label "paymentType"@en ;
      rdfs:range owl:Literal ;
      rdfs:range
              [ a       owl:Datatype ;
                :oneOf  [ a       rdf:List ;
                          rdf:first "CASH"^^xsd:string ;
                          rdf:rest
                                  [ a       rdf:List ;
                                    rdf:first "CHECK"^^xsd:string ;
                                    rdf:rest
                                            [ a       rdf:List ;
                                              rdf:first "COUPON ACCOR"^^xsd:string ;
                                              rdf:rest
                                                      [ a       rdf:List ;
                                                        rdf:first "COUPON SUDEXHO"^^xsd:string ;
                                                        rdf:rest
                                                                [ a       rdf:List ;
                                                                  rdf:first "COUPON TIMES TICKET"^^xsd:string ;
                                                                  rdf:rest
                                                                          [ a       rdf:List ;
                                                                            rdf:first "CREDIT CARD"^^xsd:string ;
                                                                            rdf:rest
                                                                                    [ a       rdf:List ;
                                                                                      rdf:first "DEBIT CARD"^^xsd:string ;
                                                                                      rdf:rest
                                                                                              [ a       rdf:List ;
                                                                                                rdf:first "GOOGLE CHECKOUT"^^xsd:string ;
                                                                                                rdf:rest
                                                                                                        [ a       rdf:List ;
                                                                                                          rdf:first "PAYPAL"^^xsd:string ;
                                                                                                          rdf:rest
                                                                                                                  [ a       rdf:List ;
                                                                                                                    rdf:first "TRAVELERS CHECK"^^xsd:string ;
                                                                                                                    rdf:rest
                                                                                                                            [ a       rdf:List ;
                                                                                                                              rdf:first "WIRE TRANSFER"^^xsd:string ;
                                                                                                                              rdf:rest ()
                                                                                                                            ]
                                                                                                                  ]
                                                                                                        ]
                                                                                              ]
                                                                                    ]
                                                                          ]
                                                                ]
                                                      ]
                                            ]
                                  ]
                        ]
              ] ;
      owl:subPropertyOf :topDataProperty .

ns:ETO
      a       owl:Class ;
      rdfs:comment "ETO (Exchange Traded Option )  An option traded on a regulated exchange where the terms of each option are standardized by the exchange"@en ;
      rdfs:label "ETO"@en ;
      owl:subClassOf ns:Fund .

ns:rawDateTime
      a       owl:DatatypeProperty ;
      rdfs:comment "Unparsed date/time information for an event or event occurrence."@en ;
      rdfs:domain ns:LocalEventOccurrence ;
      rdfs:label "rawDateTime"@en ;
      rdfs:range owl:Literal .

ns:ambiguous
      a       owl:DatatypeProperty ;
      rdfs:comment "Captures whether a record is equivocal or open to interpretation or multiple meanings."@en ;
      rdfs:domain
              [ a       owl:Class ;
                :unionOf (ns:Movie ns:Person)
              ] ;
      rdfs:label "ambiguous"@en ;
      rdfs:range xsd:boolean .

ns:appearance
      a       owl:ObjectProperty ;
      rdfs:comment "Connects the appearance to a tv show. "@en ;
      rdfs:domain
              [ a       owl:Class ;
                :unionOf (ns:TvEpisode ns:TvSeason ns:TvSeries ns:TvSpecial)
              ] ;
      rdfs:label "appearance"@en ;
      rdfs:range ns:AppearanceRole ;
      owl:subPropertyOf :topObjectProperty .

ns:businessStatus
      a       owl:DatatypeProperty ;
      rdfs:comment """Indicates the current status of the business. Should be a numeric value. The list of values are as follows:
'1' - 'maybe closed'
'2' - 'closed' """@en ;
      rdfs:domain ns:LocalBusiness ;
      rdfs:label "businessStatus"@en ;
      rdfs:range xsd:int .

ns:FinancePerson
      a       owl:Class ;
      rdfs:comment "FinancePerson is an organizational construct for those persons important to the finance sector."@en ;
      rdfs:label "FinancePerson"@en ;
      owl:subClassOf ns:Person .

ns:ConsumerProduct
      a       owl:Class ;
      rdfs:comment "A consumer product is a physical item that a consumer may buy. It includes items from the Yahoo Product taxonomy, and excludes such things as real estate and autos."@en ;
      rdfs:label "ConsumerProduct"@en ;
      owl:subClassOf ns:Entity .

ns:buildingNumber
      a       :FunctionalProperty , owl:DatatypeProperty ;
      rdfs:comment "Building number of an address listing."@en ;
      rdfs:domain
              [ a       owl:Class ;
                :unionOf (ns:Address ns:SingleLocationBusiness)
              ] ;
      rdfs:label "buildingNumber"@en ;
      rdfs:range owl:Literal ;
      owl:subPropertyOf :topDataProperty .

ns:runTime
      a       :FunctionalProperty , owl:DatatypeProperty ;
      rdfs:comment "The length of time a recording of media work takes to play from start to finish."@en ;
      rdfs:domain
              [ a       owl:Class ;
                :unionOf (ns:MediaProduct ns:MediaRelease ns:MediaWork)
              ] ;
      rdfs:label "runTime"@en ;
      rdfs:range xsd:duration .

ns:relatedness
      a       :FunctionalProperty , owl:DatatypeProperty ;
      rdfs:comment "The degree to which associated objects are related."@en ;
      rdfs:domain ns:Association ;
      rdfs:label "relatedness"@en ;
      rdfs:range owl:Literal .

ns:Option
      a       owl:Class ;
      rdfs:comment "Option a derivative financial instrument that establishes a contract between two parties concerning the buying or selling of an asset at a reference price during a specified time frame."@en ;
      rdfs:label "Option"@en ;
      owl:subClassOf ns:Derivative .

ns:businessSpecialty
      a       owl:DatatypeProperty ;
      rdfs:comment "Indicates areas of specialization or specialty features offered by a business."@en ;
      rdfs:domain ns:LocalBusiness ;
      rdfs:label "businessSpecialty"@en ;
      rdfs:range owl:Literal .

ns:competitorsOf
      a       owl:ObjectProperty ;
      rdfs:comment "Connects a game to the athletes that play in it."@en ;
      rdfs:domain ns:Athlete ;
      rdfs:label "competitorsOf"@en ;
      rdfs:range ns:SportGame ;
      owl:subPropertyOf :topObjectProperty .

ns:SeaGulf
      a       owl:Class ;
      rdfs:comment "placetype: 38"@en , "An area of open water that makes up part of an ocean such as a sea, bay, gulf, channel "@en ;
      rdfs:label "SeaGulf"@en ;
      owl:subClassOf ns:Place .

ns:locationLandmark
      a       owl:DatatypeProperty ;
      rdfs:comment "Used in Indian addresses in a way similar to the US cross street concept."@en ;
      rdfs:domain ns:Address ;
      rdfs:label "locationLandmark"@en ;
      rdfs:range owl:Literal ;
      owl:subPropertyOf :topDataProperty .

ns:associatedTo
      a       owl:ObjectProperty ;
      rdfs:comment "Connects the reified Association class to an individual, organization, or media work with which it is associated."@en ;
      rdfs:domain ns:Association ;
      rdfs:label "associatedTo"@en ;
      rdfs:range
              [ a       owl:Class ;
                :unionOf (ns:MediaWork ns:Organization ns:Performer ns:Person)
              ] ;
      owl:subPropertyOf :topObjectProperty ;
      :inverseOf ns:association .

ns:Writer
      a       owl:Class ;
      rdfs:comment "The Writer type includes anyone who creates a written work, though the word usually designates those who write creatively or professionally, as well as those who have written in many different forms."@en ;
      rdfs:label "Writer"@en ;
      owl:subClassOf ns:Person .

ns:latitude
      a       :FunctionalProperty , owl:DatatypeProperty ;
      rdfs:comment "Latitude of a location"@en ;
      rdfs:domain
              [ a       owl:Class ;
                :unionOf (ns:Address ns:EventVenue ns:Place ns:SingleLocationBusiness)
              ] ;
      rdfs:label "latitude"@en ;
      rdfs:range xsd:float ;
      owl:subPropertyOf :topDataProperty .

ns:BusinessListingCategory
      a       owl:Class ;
      rdfs:comment "Describes the Y! category for a listing."@en ;
      rdfs:label "BusinessListingCategory"@en ;
      owl:subClassOf ns:Category .

ns:audioURL
      a       owl:DatatypeProperty ;
      rdfs:comment "URL at which audio information about a Local Business may be accessed."@en ;
      rdfs:domain ns:LocalBusiness ;
      rdfs:label "audioURL"@en ;
      rdfs:range xsd:anyURI .

ns:HistoricalTown
      a       owl:Class ;
      rdfs:comment "A former/historial populated settlement Example: Montreal (Ohio)"@en , "placetype: 35"@en ;
      rdfs:label "HistoricalTown"@en ;
      owl:subClassOf ns:Place .

ns:Publisher
      a       owl:Class ;
      rdfs:comment "An organization or company that publishes written works, including books, periodicals, and online content."@en ;
      rdfs:label "Publisher"@en ;
      owl:subClassOf ns:Company .

ns:PersonalRelationship
      a       owl:Class ;
      rdfs:comment "Reified class defining relationships between persons. Generic relationship class differentiated by relationshipType data property. May include friendship, dating, business affiliation, influencers, etc."@en ;
      rdfs:label "PersonalRelationship"@en ;
      owl:subClassOf ns:Event .

ns:listingState
      a       :FunctionalProperty , owl:DatatypeProperty ;
      rdfs:comment "State of a listing. Possible values for published listing are active (ie. should be included in Vespa), inactive (i.e. should be removed from Vespa). For provider listing, it can also be perm_suppressed, urgent_deleted, etc. "@en ;
      rdfs:domain ns:LocalBusiness ;
      rdfs:label "listingState"@en ;
      rdfs:range owl:Literal ;
      owl:subPropertyOf :topDataProperty .

ns:politicalAffiliation
      a       owl:DatatypeProperty ;
      rdfs:comment "politicalAffiliation captures any political party a person is associated with"@en ;
      rdfs:domain ns:Person ;
      rdfs:label "politicalAffiliation"@en ;
      rdfs:range owl:Literal .

ns:seasonEpisode
      a       owl:ObjectProperty ;
      rdfs:comment "Connects a TV Season to an episode"@en ;
      rdfs:domain ns:TvSeason ;
      rdfs:label "seasonEpisode"@en ;
      rdfs:range ns:TvEpisode ;
      owl:subPropertyOf :topObjectProperty .

ns:airDate
      a       :FunctionalProperty , owl:DatatypeProperty ;
      rdfs:comment "The date on which a television episode first aired."@en ;
      rdfs:domain
              [ a       owl:Class ;
                :unionOf (ns:TvEpisode ns:TvSpecial)
              ] ;
      rdfs:label "airDate"@en ;
      rdfs:range
              [ a       owl:Datatype ;
                :unionOf (xsd:date xsd:gYearMonth)
              ] ;
      owl:subPropertyOf ns:date .

ns:mediaType
      a       :FunctionalProperty , owl:DatatypeProperty ;
      rdfs:comment "media content type. Eg: image/png "@en ;
      rdfs:domain ns:Image ;
      rdfs:label "mediaType"@en ;
      rdfs:range owl:Literal ;
      owl:subPropertyOf :topDataProperty .

ns:ticketUrl
      a       owl:DatatypeProperty ;
      rdfs:comment "Captures the URL where event registration may be completed online."@en ;
      rdfs:domain ns:EventRegistration ;
      rdfs:label "ticketUrl"@en ;
      rdfs:range xsd:anyURI .

ns:reviewTitle
      a       :FunctionalProperty , owl:DatatypeProperty ;
      rdfs:comment "Title of a critical or user review."@en ;
      rdfs:domain ns:Review ;
      rdfs:label "reviewTitle"@en ;
      rdfs:range owl:Literal ;
      owl:subPropertyOf ns:label .

ns:cateringURL
      a       owl:DatatypeProperty ;
      rdfs:comment "URL where catering information for a local business may be accessed."@en ;
      rdfs:domain ns:Restaurant ;
      rdfs:label "cateringURL"@en ;
      rdfs:range xsd:anyURI .

ns:capType
      a       owl:DatatypeProperty ;
      rdfs:comment "Describes the type of data as pulled from CAP or IY."@en ;
      rdfs:domain
              [ a       owl:Class ;
                :unionOf (ns:Movie ns:Person)
              ] ;
      rdfs:label "capType"@en ;
      rdfs:range owl:Literal .

<http://woo.corp.yahoo.com/ns/units/m>
      a       owl:Datatype .

ns:festival
      a       :FunctionalProperty , owl:DatatypeProperty ;
      rdfs:comment "Indicates if a film showtime occurs as part of a film festival."@en ;
      rdfs:domain ns:MovieShowtime ;
      rdfs:label "festival"@en ;
      rdfs:range owl:Literal ;
      owl:subPropertyOf :topDataProperty .

ns:Deal
      a       owl:Class ;
      rdfs:comment "Deals, offers, coupons and other short term sale offers."@en ;
      rdfs:label "Deal"@en ;
      owl:subClassOf ns:Event .

ns:rightsType
      a       :FunctionalProperty , owl:DatatypeProperty ;
      rdfs:comment "The type of right associated with the album/track, e.g. 'streaming'."@en ;
      rdfs:domain ns:MusicRight ;
      rdfs:label "rightsType"@en ;
      rdfs:range owl:Literal ;
      owl:subPropertyOf :topDataProperty .

ns:venueTypeName
      a       owl:DatatypeProperty ;
      rdfs:comment "Enumerated value capturing a venue's type."@en ;
      rdfs:domain ns:EventVenue ;
      rdfs:label "venueTypeName"@en ;
      rdfs:range owl:Literal .

ns:unitType
      a       :FunctionalProperty , owl:DatatypeProperty ;
      rdfs:comment "Unit, suite, apartment. EG, 'ste' in 1659 Branham Ln, Ste G"@en ;
      rdfs:domain
              [ a       owl:Class ;
                :unionOf (ns:Address ns:SingleLocationBusiness)
              ] ;
      rdfs:label "unitType"@en ;
      rdfs:range owl:Literal ;
      owl:subPropertyOf :topDataProperty .

ns:releaseDate
      a       :FunctionalProperty , owl:DatatypeProperty ;
      rdfs:comment "The date a media work is released for public distribution."@en , "Multiple formats acceptable: YYYY, YYYY-MM, YYYY-MM-DD. Should conform to ISO 8601."@en ;
      rdfs:domain
              [ a       owl:Class ;
                :unionOf (ns:BoxOfficeAllTime ns:MediaProduct ns:MediaRelease)
              ] ;
      rdfs:label "releaseDate"@en ;
      rdfs:range
              [ a       owl:Datatype ;
                :unionOf (xsd:date xsd:gYear xsd:gYearMonth)
              ] ;
      owl:subPropertyOf ns:date .

ns:KidsMovies
      a       owl:Class ;
      rdfs:comment "Creating the class of movies for children in order to capture that no movie can be both for kids and adults only."@en ;
      rdfs:label "Movies for Children"@en ;
      owl:subClassOf ns:Movie .

ns:creditGroup
      a       :FunctionalProperty , owl:DatatypeProperty ;
      rdfs:comment "Departmental designation of the type of work an individual contributed to the production of a media work."@en ;
      rdfs:domain
              [ a       owl:Class ;
                :unionOf (ns:CompanyRole ns:CrewRole)
              ] ;
      rdfs:label "creditGroup"@en ;
      rdfs:range owl:Literal ;
      owl:subPropertyOf :topDataProperty .

ns:dating
      a       owl:ObjectProperty ;
      rdfs:comment "The dating property connects a person to the reified Dating class."@en ;
      rdfs:domain ns:Person ;
      rdfs:label "dating"@en ;
      rdfs:range ns:Dating .

ns:LocalEventOccurrence
      a       owl:Class ;
      rdfs:comment "Single occurrence of a local event with multiple venues."@en ;
      rdfs:label "LocalEventOccurrence"@en ;
      owl:subClassOf ns:Event .

ns:LandFeature
      a       owl:Class ;
      rdfs:comment "A land feature such as a park, mountain, beach. Example: Golden Gate Park."@en , "placetype: 16"@en ;
      rdfs:label "LandFeature"@en ;
      owl:subClassOf ns:Place .

ns:AutoModel
      a       owl:Class ;
      rdfs:comment "A model is a specific car carried under a make. For example, a Mustang is a model of a Ford. Models are further broken down into generations classifying styling and platform changes. "@en ;
      rdfs:label "AutoModel"@en ;
      owl:subClassOf ns:Entity .

ns:FundManager
      a       owl:Class ;
      rdfs:comment "FundManager refers to the person(s) resposible for implementing a fund's investing strategy and managing its portfolio trading activities"@en ;
      rdfs:label "FundManager"@en ;
      owl:subClassOf ns:FinancePerson .

ns:paintType
      a       :FunctionalProperty , owl:DatatypeProperty ;
      rdfs:comment "Represents the type of the paint used for the car exterior. Applicable only if colorCategory is Exterior. Possible values: black, customised, metallic, gloss, mica, matt, pearl "@en ;
      rdfs:domain ns:Color ;
      rdfs:label "paintType"@en ;
      rdfs:range owl:Literal ;
      owl:subPropertyOf ns:colorHolding .

ns:endTime
      a       :FunctionalProperty , owl:DatatypeProperty ;
      rdfs:comment "The time at which an event ends."@en ;
      rdfs:domain ns:Event ;
      rdfs:label "endTime"@en ;
      rdfs:range xsd:time ;
      owl:subPropertyOf :topDataProperty .

ns:operatingHours
      a       :FunctionalProperty , owl:DatatypeProperty ;
      rdfs:comment "array of strings with each string of the format (,,*,*,*,*) as in http://wiki.pentaho.com/display/ServerDoc1x/05.+CRON+Expressions+in+Detail?showComments=false"@en ;
      rdfs:domain
              [ a       owl:Class ;
                :unionOf (ns:ContactInfo ns:LocalBusiness ns:SingleLocationBusiness)
              ] ;
      rdfs:label "operatingHours"@en ;
      rdfs:range owl:Literal ;
      owl:subPropertyOf :topDataProperty .

ns:shortDescription
      a       owl:DatatypeProperty ;
      rdfs:comment "Description snippet providing info about an entity."@en ;
      rdfs:domain
              [ a       owl:Class ;
                :unionOf (ns:Deal ns:LocalBusiness ns:LocalEvent)
              ] ;
      rdfs:label "shortDescription"@en ;
      rdfs:range owl:Literal .

ns:broadcastInstance
      a       owl:ObjectProperty ;
      rdfs:comment "Connects a movie or event to its televised broadcast via TVSpecial. "@en ;
      rdfs:domain
              [ a       owl:Class ;
                :unionOf (ns:Movie ns:SportCompetition ns:SportCompetitionInstance ns:SportGame)
              ] ;
      rdfs:label "broadcastInstance"@en ;
      rdfs:range ns:TvSpecial .

ns:photoCollection
      a       :FunctionalProperty , owl:DatatypeProperty ;
      rdfs:comment "Source information for photo collections."@en ;
      rdfs:domain ns:Image ;
      rdfs:label "photoCollection"@en ;
      rdfs:range xsd:anyURI ;
      owl:subPropertyOf :topDataProperty .

ns:Kiosk
      a       owl:Class ;
      rdfs:comment "Kiosk represents ATMs, Redbox, and any other kiosk that appears inside or outside of other local businesses."@en ;
      rdfs:label "Kiosk"@en ;
      owl:subClassOf ns:LocalBusiness .

ns:apr
      a       :FunctionalProperty , owl:DatatypeProperty ;
      rdfs:comment "annual percentage rate for a loan offer."@en ;
      rdfs:domain ns:AutoIncentive ;
      rdfs:label "apr"@en ;
      rdfs:range xsd:double .

ns:areaServed
      a       owl:DatatypeProperty ;
      rdfs:comment "Areas that a business serves."@en ;
      rdfs:domain ns:LocalBusiness ;
      rdfs:label "areaServed"@en ;
      rdfs:range owl:Literal ;
      owl:subPropertyOf :topDataProperty .

ns:countyCode
      a       :FunctionalProperty , owl:DatatypeProperty ;
      rdfs:comment "County Code"@en ;
      rdfs:domain
              [ a       owl:Class ;
                :unionOf (ns:Address ns:CountyAdminArea ns:SingleLocationBusiness)
              ] ;
      rdfs:label "countyCode"@en ;
      rdfs:range owl:Literal ;
      owl:subPropertyOf :topDataProperty .

ns:SportSchedulePeriod
      a       owl:Class ;
      rdfs:comment "Captures the schedule period for a competition. Example: preseason, postseason, regular."@en ;
      rdfs:label "SportSchedulePeriod"@en ;
      owl:subClassOf ns:Event .

ns:soundtrackOf
      a       owl:ObjectProperty ;
      rdfs:comment "connects a movie to its soundtrack album"@en ;
      rdfs:domain ns:Movie ;
      rdfs:label "soundtrackOf"@en ;
      rdfs:range ns:Album ;
      owl:subPropertyOf :topObjectProperty ;
      :inverseOf ns:soundtrack .

ns:normalizedUrl
      a       :FunctionalProperty , owl:DatatypeProperty ;
      rdfs:comment "Url in a normalized format."@en ;
      rdfs:domain ns:Webpage ;
      rdfs:label "normalizedUrl"@en ;
      rdfs:range xsd:anyURI ;
      owl:subPropertyOf :topDataProperty .

ns:MovieStudio
      a       owl:Class ;
      rdfs:comment "Company that produces filmed entertainment. Could be movies, films, or TV."@en ;
      rdfs:label "MovieStudio"@en ;
      owl:subClassOf ns:Company .

ns:competitionTeam
      a       owl:ObjectProperty ;
      rdfs:comment "Connects the teams with the competitions they are involved in."@en ;
      rdfs:domain ns:SportTeam ;
      rdfs:label "competitionTeam"@en ;
      rdfs:range ns:SportCompetitionInstance ;
      owl:subPropertyOf :topObjectProperty .

ns:Equity
      a       owl:Class ;
      rdfs:comment "Equity represents the compensation type equity. The securityID will be represented by the externalid relationship inheritied from the entity class."@en ;
      rdfs:label "Equity"@en ;
      owl:subClassOf ns:Compensation .

ns:relatedEntity
      a       owl:DatatypeProperty ;
      rdfs:comment "Offers movies, people, or other entites that have an association with the entity described."@en ;
      rdfs:domain
              [ a       owl:Class ;
                :unionOf (ns:Movie ns:Person)
              ] ;
      rdfs:label "relatedEntity"@en ;
      rdfs:range owl:Literal .

ns:OnlineAccount
      a       owl:Class ;
      rdfs:comment "Describes an online account held by a person, organization, place, or thing."@en ;
      rdfs:label "OnlineAccount"@en ;
      owl:subClassOf ns:Entity .

ns:orgName
      a       :FunctionalProperty , owl:DatatypeProperty ;
      rdfs:comment "The name of an organization."@en ;
      rdfs:domain
              [ a       owl:Class ;
                :unionOf (ns:FinancialInstrument ns:Organization ns:SportCompetition)
              ] ;
      rdfs:label "orgName"@en ;
      rdfs:range owl:Literal ;
      owl:subPropertyOf ns:name .

ns:theaterNumber
      a       :FunctionalProperty , owl:DatatypeProperty ;
      rdfs:comment "Number of theaters in which a film is shown in release."@en ;
      rdfs:domain ns:BoxOfficeWeekend ;
      rdfs:label "theaterNumber"@en ;
      rdfs:range xsd:int ;
      owl:subPropertyOf :topDataProperty .

ns:exchangeOf
      a       owl:ObjectProperty ;
      rdfs:comment "exchangeOf connects the exchange to the tradablequotable instrument or ticker entity which is traded on it"@en ;
      rdfs:domain ns:StockExchange ;
      rdfs:label "exchangeOf"@en ;
      rdfs:range
              [ a       owl:Class ;
                :unionOf (ns:Ticker ns:TradableQuotableInstrument)
              ] ;
      :inverseOf ns:tradesOnExchange .

ns:legalStructure
      a       :FunctionalProperty , owl:DatatypeProperty ;
      rdfs:comment "The legal structure of an organization"@en ;
      rdfs:domain ns:Organization ;
      rdfs:label "legalStructure"@en ;
      rdfs:range owl:Literal .

ns:QuotableInstrument
      a       owl:Class ;
      rdfs:comment "QuotableInstrument denotes those symbols by which a financial instrument can be discussed."@en ;
      rdfs:label "QuotableInstrument"@en ;
      owl:subClassOf ns:Entity .

ns:Warrant
      a       owl:Class ;
      rdfs:comment "Warrant a security that entitles the holder to buy the underlying stock of the issuing company at a fixed exercise price until the expiry date"@en ;
      rdfs:label "Warrant"@en ;
      owl:subClassOf ns:Derivative .

ns:businessSlogan
      a       owl:DatatypeProperty ;
      rdfs:comment "businessSlogan is the slogan of a business"@en ;
      rdfs:domain ns:Organization ;
      rdfs:label "businessSlogan"@en ;
      rdfs:range owl:Literal .

ns:AlternatePersonName
      a       owl:Class ;
      rdfs:comment "Reified class detailing alternate names by which a person may be known, includes stage, birth, nick, pen, and aka names."@en ;
      rdfs:label "AlternatePersonName"@en ;
      owl:subClassOf ns:Entity .

ns:packaging
      a       :FunctionalProperty , owl:DatatypeProperty ;
      rdfs:comment "Describes the packaging type of a consumer product."@en ;
      rdfs:domain ns:ConsumerProduct ;
      rdfs:label "packaging"@en ;
      rdfs:range owl:Literal ;
      owl:subPropertyOf :topDataProperty .

[]    a       :AllDisjointClasses ;
      :members (ns:Album ns:Composition ns:Movie ns:Song ns:TvEpisode ns:TvSeries) .

ns:id
      a       owl:DatatypeProperty ;
      rdfs:comment "Holding area for ID data properties."@en ;
      rdfs:label "idHolding" ;
      owl:subPropertyOf :topDataProperty .

ns:fuelEconomyCityMin
      a       :FunctionalProperty , owl:DatatypeProperty ;
      rdfs:comment "Indicates the minimum fuel economy for this model for city driving. This information is derived from trim details in the enrichment phase "@en ;
      rdfs:domain ns:AutoModel ;
      rdfs:label "fuelEconomyCityMin"@en ;
      rdfs:range xsd:float .

ns:financialInstrumentGroup
      a       :FunctionalProperty , owl:DatatypeProperty ;
      rdfs:comment "financialInstrumentGroup is the broad categorization of a financial instrument, for example, equity"@en ;
      rdfs:domain ns:FinancialInstrument ;
      rdfs:label "financialInstrumentGroup"@en ;
      rdfs:range owl:Literal .

ns:webpage
      a       owl:ObjectProperty ;
      rdfs:comment "Connects a thing to its webpage."@en , "Connected to Entity per Ticket 4192755"@en ;
      rdfs:domain ns:Entity ;
      rdfs:label "webpage"@en ;
      rdfs:range ns:Webpage ;
      owl:subPropertyOf :topObjectProperty ;
      :inverseOf ns:webpageOf .

ns:regionCode
      a       :FunctionalProperty , owl:DatatypeProperty ;
      rdfs:comment "Describes the region in which a media product will play."@en ;
      rdfs:domain ns:MediaProduct ;
      rdfs:label "regionCode"@en ;
      rdfs:range owl:Literal .

ns:boxoffice
      a       owl:ObjectProperty ;
      rdfs:comment "Connects a film to its box office receipts."@en ;
      rdfs:domain ns:Movie ;
      rdfs:label "boxoffice"@en ;
      rdfs:range
              [ a       owl:Class ;
                :unionOf (ns:BoxOfficeAllTime ns:BoxOfficeDaily ns:BoxOfficeWeekend ns:BoxOfficeWeekly)
              ] ;
      owl:subPropertyOf :topObjectProperty .

ns:AlternateTitle
      a       owl:Class ;
      rdfs:comment "Alternate names by which a media work may be known."@en ;
      rdfs:label "AlternateTitle"@en ;
      owl:subClassOf ns:Entity .

ns:TvSeries
      a       owl:Class ;
      rdfs:comment "TV Series rely on a continuing plot that unfolds in a sequential episode by episode fashion."@en ;
      rdfs:label "TvSeries"@en ;
      owl:subClassOf ns:MediaWork ;
      :hasKey (ns:createdBy ns:mediaTitle) .

ns:broaderEvent
      a       owl:ObjectProperty ;
      rdfs:comment "Connects an event that is part of a series or group to its broader, parent event. For example, game 1 of the Major League Baseball World Series to the series itself."@en ;
      rdfs:domain ns:LocalEvent ;
      rdfs:label "broaderEvent"@en ;
      rdfs:range ns:LocalEvent .

ns:musicType
      a       :FunctionalProperty , owl:DatatypeProperty ;
      rdfs:comment "Normalized value of the composition "@en ;
      rdfs:domain ns:Composition ;
      rdfs:label "musicType"@en ;
      rdfs:range owl:Literal .

<http://woo.corp.yahoo.com/ns/units/bytes>
      a       owl:Datatype .

ns:streetName
      a       :FunctionalProperty , owl:DatatypeProperty ;
      rdfs:comment "The name of the street in an address listing"@en ;
      rdfs:domain
              [ a       owl:Class ;
                :unionOf (ns:Address ns:SingleLocationBusiness)
              ] ;
      rdfs:label "streetName"@en ;
      rdfs:range owl:Literal ;
      owl:subPropertyOf ns:name .

ns:invoiceMax
      a       :FunctionalProperty , owl:DatatypeProperty ;
      rdfs:comment "Indicates the maximum invoice for this model. This information is derived from trim details in the enrichment phase "@en ;
      rdfs:domain ns:AutoModel ;
      rdfs:label "invoiceMax"@en ;
      rdfs:range xsd:double .

ns:DistributionRight
      a       owl:Class ;
      rdfs:comment "Describes the rights associated with a given media work."@en ;
      rdfs:label "DistributionRight"@en ;
      owl:subClassOf ns:Event .

ns:ticketAdult
      a       :FunctionalProperty , owl:DatatypeProperty ;
      rdfs:comment "Describes the cost of an adult ticket at a given theater."@en ;
      rdfs:domain ns:MovieTheater ;
      rdfs:label "ticketAdult"@en ;
      rdfs:range xsd:float ;
      owl:subPropertyOf :topDataProperty .

ns:offerCode
      a       owl:DatatypeProperty ;
      rdfs:comment "example: Reka09 "@en , "Code for a deal or offer."@en ;
      rdfs:domain ns:Deal ;
      rdfs:label "offerCode"@en ;
      rdfs:range owl:Literal .

ns:BoxOffice
      a       owl:Class ;
      rdfs:comment "Holding area for BoxOffice classes"@en ;
      rdfs:label "BoxOffice"@en ;
      owl:subClassOf ns:Entity .

ns:EmployeeAffiliation
      a       owl:Class ;
      rdfs:comment "EmployeeAffiliation is a reified class representing the time an person is an employee of an organization"@en ;
      rdfs:label "EmployeeAffiliation"@en ;
      owl:subClassOf ns:OrgAffiliation .

ns:rawFeedDataId
      a       owl:DatatypeProperty ;
      rdfs:comment "Captures the unique identifier assigned to an entity in the raw feed data. Not for display."@en ;
      rdfs:domain ns:Entity ;
      rdfs:label "rawFeedDataId"@en ;
      rdfs:range owl:Literal .

ns:lodgingRoomAmenities
      a       owl:DatatypeProperty ;
      rdfs:comment "Enumerates the types of features the hotel room offers"@en ;
      rdfs:domain ns:Lodging ;
      rdfs:label "lodgingRoomAmenities"@en ;
      rdfs:range owl:Literal ;
      rdfs:range
              [ a       owl:Datatype ;
                :oneOf  [ a       rdf:List ;
                          rdf:first "AIR CONDITIONING"^^xsd:string ;
                          rdf:rest
                                  [ a       rdf:List ;
                                    rdf:first "BALCONY OR TERRACE"^^xsd:string ;
                                    rdf:rest
                                            [ a       rdf:List ;
                                              rdf:first "BATHROBES"^^xsd:string ;
                                              rdf:rest
                                                      [ a       rdf:List ;
                                                        rdf:first "COFFEE MAKER"^^xsd:string ;
                                                        rdf:rest
                                                                [ a       rdf:List ;
                                                                  rdf:first "DATAPORT"^^xsd:string ;
                                                                  rdf:rest
                                                                          [ a       rdf:List ;
                                                                            rdf:first "DEADBOLTS OR LOCKS"^^xsd:string ;
                                                                            rdf:rest
                                                                                    [ a       rdf:List ;
                                                                                      rdf:first "DESK"^^xsd:string ;
                                                                                      rdf:rest
                                                                                              [ a       rdf:List ;
                                                                                                rdf:first "FAX"^^xsd:string ;
                                                                                                rdf:rest
                                                                                                        [ a       rdf:List ;
                                                                                                          rdf:first "FIREPLACE"^^xsd:string ;
                                                                                                          rdf:rest
                                                                                                                  [ a       rdf:List ;
                                                                                                                    rdf:first "FITNESS EQUIPMENT"^^xsd:string ;
                                                                                                                    rdf:rest
                                                                                                                            [ a       rdf:List ;
                                                                                                                              rdf:first "HAIR DRYER"^^xsd:string ;
                                                                                                                              rdf:rest
                                                                                                                                      [ a       rdf:List ;
                                                                                                                                        rdf:first "INTERNET ACCESS"^^xsd:string ;
                                                                                                                                        rdf:rest
                                                                                                                                                [ a       rdf:List ;
                                                                                                                                                  rdf:first "IRON"^^xsd:string ;
                                                                                                                                                  rdf:rest
                                                                                                                                                          [ a       rdf:List ;
                                                                                                                                                            rdf:first "IRONING BOARD"^^xsd:string ;
                                                                                                                                                            rdf:rest
                                                                                                                                                                    [ a       rdf:List ;
                                                                                                                                                                      rdf:first "KITCHEN OR KITCHENETTE"^^xsd:string ;
                                                                                                                                                                      rdf:rest
                                                                                                                                                                              [ a       rdf:List ;
                                                                                                                                                                                rdf:first "MICROWAVE OVEN"^^xsd:string ;
                                                                                                                                                                                rdf:rest
                                                                                                                                                                                        [ a       rdf:List ;
                                                                                                                                                                                          rdf:first "MINIBAR"^^xsd:string ;
                                                                                                                                                                                          rdf:rest
                                                                                                                                                                                                  [ a       rdf:List ;
                                                                                                                                                                                                    rdf:first "NEWSPAPER"^^xsd:string ;
                                                                                                                                                                                                    rdf:rest
                                                                                                                                                                                                            [ a       rdf:List ;
                                                                                                                                                                                                              rdf:first "NON-SMOKING ROOMS"^^xsd:string ;
                                                                                                                                                                                                              rdf:rest
                                                                                                                                                                                                                      [ a       rdf:List ;
                                                                                                                                                                                                                        rdf:first "PRINTER"^^xsd:string ;
                                                                                                                                                                                                                        rdf:rest
                                                                                                                                                                                                                                [ a       rdf:List ;
                                                                                                                                                                                                                                  rdf:first "PRIVATE BATH"^^xsd:string ;
                                                                                                                                                                                                                                  rdf:rest
                                                                                                                                                                                                                                          [ a       rdf:List ;
                                                                                                                                                                                                                                            rdf:first "RADIO OR ALARM CLOCK"^^xsd:string ;
                                                                                                                                                                                                                                            rdf:rest
                                                                                                                                                                                                                                                    [ a       rdf:List ;
                                                                                                                                                                                                                                                      rdf:first "REFRIGERATOR"^^xsd:string ;
                                                                                                                                                                                                                                                      rdf:rest
                                                                                                                                                                                                                                                              [ a       rdf:List ;
                                                                                                                                                                                                                                                                rdf:first "SAFE"^^xsd:string ;
                                                                                                                                                                                                                                                                rdf:rest
                                                                                                                                                                                                                                                                        [ a       rdf:List ;
                                                                                                                                                                                                                                                                          rdf:first "SHOWER"^^xsd:string ;
                                                                                                                                                                                                                                                                          rdf:rest
                                                                                                                                                                                                                                                                                  [ a       rdf:List ;
                                                                                                                                                                                                                                                                                    rdf:first "SOFABED"^^xsd:string ;
                                                                                                                                                                                                                                                                                    rdf:rest
                                                                                                                                                                                                                                                                                            [ a       rdf:List ;
                                                                                                                                                                                                                                                                                              rdf:first "TELEPHONE"^^xsd:string ;
                                                                                                                                                                                                                                                                                              rdf:rest
                                                                                                                                                                                                                                                                                                      [ a       rdf:List ;
                                                                                                                                                                                                                                                                                                        rdf:first "TELEPHONE DATAPORT"^^xsd:string ;
                                                                                                                                                                                                                                                                                                        rdf:rest
                                                                                                                                                                                                                                                                                                                [ a       rdf:List ;
                                                                                                                                                                                                                                                                                                                  rdf:first "TELEVISION CABLE OR SATELLITE"^^xsd:string ;
                                                                                                                                                                                                                                                                                                                  rdf:rest
                                                                                                                                                                                                                                                                                                                          [ a       rdf:List ;
                                                                                                                                                                                                                                                                                                                            rdf:first "TELEVISION MOVIES OR FREE"^^xsd:string ;
                                                                                                                                                                                                                                                                                                                            rdf:rest
                                                                                                                                                                                                                                                                                                                                    [ a       rdf:List ;
                                                                                                                                                                                                                                                                                                                                      rdf:first "TELEVISION MOVIES OR PAY"^^xsd:string ;
                                                                                                                                                                                                                                                                                                                                      rdf:rest
                                                                                                                                                                                                                                                                                                                                              [ a       rdf:List ;
                                                                                                                                                                                                                                                                                                                                                rdf:first "VCR"^^xsd:string ;
                                                                                                                                                                                                                                                                                                                                                rdf:rest
                                                                                                                                                                                                                                                                                                                                                        [ a       rdf:List ;
                                                                                                                                                                                                                                                                                                                                                          rdf:first "WAKEUP SERVICE"^^xsd:string ;
                                                                                                                                                                                                                                                                                                                                                          rdf:rest
                                                                                                                                                                                                                                                                                                                                                                  [ a       rdf:List ;
                                                                                                                                                                                                                                                                                                                                                                    rdf:first "WHIRLPOOL"^^xsd:string ;
                                                                                                                                                                                                                                                                                                                                                                    rdf:rest ()
                                                                                                                                                                                                                                                                                                                                                                  ]
                                                                                                                                                                                                                                                                                                                                                        ]
                                                                                                                                                                                                                                                                                                                                              ]
                                                                                                                                                                                                                                                                                                                                    ]
                                                                                                                                                                                                                                                                                                                          ]
                                                                                                                                                                                                                                                                                                                ]
                                                                                                                                                                                                                                                                                                      ]
                                                                                                                                                                                                                                                                                            ]
                                                                                                                                                                                                                                                                                  ]
                                                                                                                                                                                                                                                                        ]
                                                                                                                                                                                                                                                              ]
                                                                                                                                                                                                                                                    ]
                                                                                                                                                                                                                                          ]
                                                                                                                                                                                                                                ]
                                                                                                                                                                                                                      ]
                                                                                                                                                                                                            ]
                                                                                                                                                                                                  ]
                                                                                                                                                                                        ]
                                                                                                                                                                              ]
                                                                                                                                                                    ]
                                                                                                                                                          ]
                                                                                                                                                ]
                                                                                                                                      ]
                                                                                                                            ]
                                                                                                                  ]
                                                                                                        ]
                                                                                              ]
                                                                                    ]
                                                                          ]
                                                                ]
                                                      ]
                                            ]
                                  ]
                        ]
              ] ;
      owl:subPropertyOf :topDataProperty .

<http://woo.corp.yahoo.com/ns/units/in>
      a       owl:Datatype .

ns:valueNum
      a       owl:DatatypeProperty ;
      rdfs:comment "Value of a deal expressed numerically"@en ;
      rdfs:domain ns:Deal ;
      rdfs:label "valueNum"@en ;
      rdfs:range xsd:float .

ns:competitionAthlete
      a       owl:ObjectProperty ;
      rdfs:comment "Connects an individual athlete or player to the competition he or she participates in."@en ;
      rdfs:domain ns:Athlete ;
      rdfs:label "competitionAthlete"@en ;
      rdfs:range ns:SportCompetitionInstance .

ns:movieStudioFor
      a       owl:ObjectProperty ;
      rdfs:comment "Connects a studio to the films they've made."@en ;
      rdfs:domain ns:MovieStudio ;
      rdfs:label "movieStudioFor"@en ;
      rdfs:range
              [ a       owl:Class ;
                :unionOf (ns:MediaProduct ns:Movie ns:TvEpisode ns:TvSeason ns:TvSeries ns:TvSpecial)
              ] ;
      :inverseOf ns:movieStudio .

ns:extendedAddress
      a       :FunctionalProperty , owl:DatatypeProperty ;
      rdfs:comment "The second line of a street address, also known as addr2."@en ;
      rdfs:domain
              [ a       owl:Class ;
                :unionOf (ns:Address ns:SingleLocationBusiness)
              ] ;
      rdfs:label "extendedAddress"@en ;
      rdfs:range owl:Literal ;
      owl:subPropertyOf :topDataProperty .

ns:startText
      a       :FunctionalProperty , owl:DatatypeProperty ;
      rdfs:comment "Blob dataproperty containing textual representation of the beginning of a timerange."@en ;
      rdfs:domain ns:Event ;
      rdfs:label "startText"@en ;
      rdfs:range owl:Literal ;
      owl:subPropertyOf :topDataProperty .

ns:partyRoomAvailable
      a       :FunctionalProperty , owl:DatatypeProperty ;
      rdfs:comment "Denotes whether the venue has a room that can be reserved for parties."@en ;
      rdfs:domain ns:MovieTheater ;
      rdfs:label "partyRoomAvailable"@en ;
      rdfs:range xsd:boolean .

ns:eventStatus
      a       owl:DatatypeProperty ;
      rdfs:comment "Indicates the status of an event, e.g. recurrent, ongoing, cancelled."@en ;
      rdfs:domain
              [ a       owl:Class ;
                :unionOf (ns:LocalEvent ns:LocalEventOccurrence)
              ] ;
      rdfs:label "eventStatus"@en ;
      rdfs:range owl:Literal .

ns:representedBy
      a       owl:ObjectProperty ;
      rdfs:comment "representedBy connects the tradeablequoteable instrument to its ticker"@en ;
      rdfs:domain ns:TQIAffiliation ;
      rdfs:label "representedBy"@en ;
      rdfs:range ns:Ticker ;
      :inverseOf ns:represents .

ns:uriType
      a       :FunctionalProperty , owl:DatatypeProperty ;
      rdfs:comment "Enumerated values, which tells what the URI is for. Ex: 'RESERVATION', 'PROMOTIONAL_OFFER' "@en ;
      rdfs:domain ns:Webpage ;
      rdfs:label "uriType"@en ;
      rdfs:range owl:Literal ;
      rdfs:range
              [ a       owl:Datatype ;
                :oneOf  [ a       rdf:List ;
                          rdf:first "ADDITIONAL INFO"^^xsd:string ;
                          rdf:rest
                                  [ a       rdf:List ;
                                    rdf:first "APPLY ONLINE"^^xsd:string ;
                                    rdf:rest
                                            [ a       rdf:List ;
                                              rdf:first "AUDIO"^^xsd:string ;
                                              rdf:rest
                                                      [ a       rdf:List ;
                                                        rdf:first "CHECK INVENTORY"^^xsd:string ;
                                                        rdf:rest
                                                                [ a       rdf:List ;
                                                                  rdf:first "CONTACT US"^^xsd:string ;
                                                                  rdf:rest
                                                                          [ a       rdf:List ;
                                                                            rdf:first "COUPON"^^xsd:string ;
                                                                            rdf:rest
                                                                                    [ a       rdf:List ;
                                                                                      rdf:first "COURSE LISTINGS"^^xsd:string ;
                                                                                      rdf:rest
                                                                                              [ a       rdf:List ;
                                                                                                rdf:first "FEATURED"^^xsd:string ;
                                                                                                rdf:rest
                                                                                                        [ a       rdf:List ;
                                                                                                          rdf:first "GET DISCOUNT"^^xsd:string ;
                                                                                                          rdf:rest
                                                                                                                  [ a       rdf:List ;
                                                                                                                    rdf:first "GET QUOTE"^^xsd:string ;
                                                                                                                    rdf:rest
                                                                                                                            [ a       rdf:List ;
                                                                                                                              rdf:first "GIFT CERTIFICATE"^^xsd:string ;
                                                                                                                              rdf:rest
                                                                                                                                      [ a       rdf:List ;
                                                                                                                                        rdf:first "GUEST LIST"^^xsd:string ;
                                                                                                                                        rdf:rest
                                                                                                                                                [ a       rdf:List ;
                                                                                                                                                  rdf:first "HOMEPAGE"^^xsd:string ;
                                                                                                                                                  rdf:rest
                                                                                                                                                          [ a       rdf:List ;
                                                                                                                                                            rdf:first "LOGO"^^xsd:string ;
                                                                                                                                                            rdf:rest
                                                                                                                                                                    [ a       rdf:List ;
                                                                                                                                                                      rdf:first "MAKE RESERVATION"^^xsd:string ;
                                                                                                                                                                      rdf:rest
                                                                                                                                                                              [ a       rdf:List ;
                                                                                                                                                                                rdf:first "MENU"^^xsd:string ;
                                                                                                                                                                                rdf:rest
                                                                                                                                                                                        [ a       rdf:List ;
                                                                                                                                                                                          rdf:first "ONLINE SPECIAL"^^xsd:string ;
                                                                                                                                                                                          rdf:rest
                                                                                                                                                                                                  [ a       rdf:List ;
                                                                                                                                                                                                    rdf:first "ORDERING"^^xsd:string ;
                                                                                                                                                                                                    rdf:rest
                                                                                                                                                                                                            [ a       rdf:List ;
                                                                                                                                                                                                              rdf:first "PROFILE"^^xsd:string ;
                                                                                                                                                                                                              rdf:rest
                                                                                                                                                                                                                      [ a       rdf:List ;
                                                                                                                                                                                                                        rdf:first "RATES"^^xsd:string ;
                                                                                                                                                                                                                        rdf:rest
                                                                                                                                                                                                                                [ a       rdf:List ;
                                                                                                                                                                                                                                  rdf:first "REF SITE"^^xsd:string ;
                                                                                                                                                                                                                                  rdf:rest
                                                                                                                                                                                                                                          [ a       rdf:List ;
                                                                                                                                                                                                                                            rdf:first "REL SITE"^^xsd:string ;
                                                                                                                                                                                                                                            rdf:rest
                                                                                                                                                                                                                                                    [ a       rdf:List ;
                                                                                                                                                                                                                                                      rdf:first "SHOWTIMES"^^xsd:string ;
                                                                                                                                                                                                                                                      rdf:rest
                                                                                                                                                                                                                                                              [ a       rdf:List ;
                                                                                                                                                                                                                                                                rdf:first "SPECIAL OFFERS"^^xsd:string ;
                                                                                                                                                                                                                                                                rdf:rest
                                                                                                                                                                                                                                                                        [ a       rdf:List ;
                                                                                                                                                                                                                                                                          rdf:first "TICKETS"^^xsd:string ;
                                                                                                                                                                                                                                                                          rdf:rest
                                                                                                                                                                                                                                                                                  [ a       rdf:List ;
                                                                                                                                                                                                                                                                                    rdf:first "VIDEO"^^xsd:string ;
                                                                                                                                                                                                                                                                                    rdf:rest
                                                                                                                                                                                                                                                                                            [ a       rdf:List ;
                                                                                                                                                                                                                                                                                              rdf:first "YELLOW PAGES AD"^^xsd:string ;
                                                                                                                                                                                                                                                                                              rdf:rest
                                                                                                                                                                                                                                                                                                      [ a       rdf:List ;
                                                                                                                                                                                                                                                                                                        rdf:first "YELLOW PAGES HOSTED"^^xsd:string ;
                                                                                                                                                                                                                                                                                                        rdf:rest
                                                                                                                                                                                                                                                                                                                [ a       rdf:List ;
                                                                                                                                                                                                                                                                                                                  rdf:first "YELLOW PAGES LINK"^^xsd:string ;
                                                                                                                                                                                                                                                                                                                  rdf:rest ()
                                                                                                                                                                                                                                                                                                                ]
                                                                                                                                                                                                                                                                                                      ]
                                                                                                                                                                                                                                                                                            ]
                                                                                                                                                                                                                                                                                  ]
                                                                                                                                                                                                                                                                        ]
                                                                                                                                                                                                                                                              ]
                                                                                                                                                                                                                                                    ]
                                                                                                                                                                                                                                          ]
                                                                                                                                                                                                                                ]
                                                                                                                                                                                                                      ]
                                                                                                                                                                                                            ]
                                                                                                                                                                                                  ]
                                                                                                                                                                                        ]
                                                                                                                                                                              ]
                                                                                                                                                                    ]
                                                                                                                                                          ]
                                                                                                                                                ]
                                                                                                                                      ]
                                                                                                                            ]
                                                                                                                  ]
                                                                                                        ]
                                                                                              ]
                                                                                    ]
                                                                          ]
                                                                ]
                                                      ]
                                            ]
                                  ]
                        ]
              ] ;
      owl:subPropertyOf :topDataProperty .

ns:fiscalYearEnd
      a       :FunctionalProperty , owl:DatatypeProperty ;
      rdfs:comment "FiscalYearEnd is the end of the period used for calculating annual financial statements"@en ;
      rdfs:domain ns:Company ;
      rdfs:label "fiscalYearEnd"@en ;
      rdfs:range owl:Literal .

ns:Supername
      a       owl:Class ;
      rdfs:comment "Placetype19"@en , "An area covering multiple countries. Similar to colloquial or historical place, except for countries. Example: Indian Subcontinent, eurasia, USSR. "@en ;
      rdfs:label "Supername"@en ;
      owl:subClassOf ns:Place .

ns:RetailShop
      a       owl:Class ;
      rdfs:comment "A store where goods are sold to the public. Retail consists of the sale of goods or merchandise from a fixed location, such as a department store, boutique or kiosk, or by mail, in small or individual lots for direct consumption by the purchaser."@en ;
      rdfs:label "RetailShop"@en ;
      owl:subClassOf ns:LocalBusiness .

ns:kioskPlacement
      a       :FunctionalProperty , owl:DatatypeProperty ;
      rdfs:comment "kioskPlacement is a data property that captures where in reference to a local business the kiosk is (inside, outside,parking lot, etc.)"@en ;
      rdfs:domain ns:Kiosk ;
      rdfs:range owl:Literal .

ns:featured
      a       :FunctionalProperty , owl:DatatypeProperty ;
      rdfs:comment "Indicates whether a deal or offer is featured."@en ;
      rdfs:domain ns:Deal ;
      rdfs:label "featured"@en ;
      rdfs:range xsd:boolean .

ns:ticketMatinee
      a       :FunctionalProperty , owl:DatatypeProperty ;
      rdfs:comment "Describes the cost of a discount matinee ticket at a given theater."@en ;
      rdfs:domain ns:MovieTheater ;
      rdfs:label "ticketMatinee"@en ;
      rdfs:range xsd:float ;
      owl:subPropertyOf :topDataProperty .

ns:languageSpoken
      a       owl:DatatypeProperty ;
      rdfs:comment "List of languages spoken by a business or person."@en ;
      rdfs:domain
              [ a       owl:Class ;
                :unionOf (ns:ContactInfo ns:LocalBusiness ns:Person ns:SingleLocationBusiness)
              ] ;
      rdfs:label "languageSpoken"@en ;
      rdfs:range owl:Literal ;
      owl:subPropertyOf :topDataProperty .

<http://woo.corp.yahoo.com/ns/units/g>
      a       owl:Datatype .

ns:finalScore
      a       :FunctionalProperty , owl:DatatypeProperty ;
      rdfs:comment "Describes the final score recorded in a sports game at its finish."@en ;
      rdfs:domain ns:SportGame ;
      rdfs:label "finalScore"@en ;
      rdfs:range owl:Literal ;
      owl:subPropertyOf :topDataProperty .

ns:financialInstrumentOf
      a       :FunctionalProperty , owl:ObjectProperty ;
      rdfs:comment "financialInstrumentOf connects a trading instrument to the public company it was issued by"@en ;
      rdfs:domain ns:FinancialInstrument ;
      rdfs:label "financialInstrumentOf"@en ;
      rdfs:range ns:PublicCompany ;
      :inverseOf ns:financialInstrument .

ns:sportTeamPlaceOf
      a       owl:ObjectProperty ;
      rdfs:comment "Connects a place to the sports teams that represent it."@en ;
      rdfs:domain ns:SportTeam ;
      rdfs:label "sportTeamPlaceOf"@en ;
      rdfs:range ns:GeoPoliticalEntity ;
      :inverseOf ns:sportTeamPlace .

ns:CityTown
      a       owl:Class ;
      rdfs:comment "Placetype Code: 7"@en , "A populated settlement such as a city, town, village. example: Sunnyvale"@en ;
      rdfs:label "CityTown"@en ;
      owl:subClassOf ns:GeoPoliticalEntity .

ns:invoiceMin
      a       :FunctionalProperty , owl:DatatypeProperty ;
      rdfs:comment "Indicates the minimum invoice for this model. This information is derived from trim details in the enrichment phase "@en ;
      rdfs:domain ns:AutoModel ;
      rdfs:label "invoiceMin"@en ;
      rdfs:range xsd:double .

ns:CategoryAndGenre
      a       owl:Class ;
      rdfs:comment "Category and Genre will be the parent of all Genre and Category classes for ease of viewing.If needed we can move them out later."@en ;
      rdfs:label "CategoryAndGenre"@en ;
      owl:subClassOf ns:Entity .

ns:rightsSource
      a       :FunctionalProperty , owl:DatatypeProperty ;
      rdfs:comment "The source and/or ID for the rights provider"@en ;
      rdfs:domain ns:DistributionRight ;
      rdfs:label "rightsSource"@en ;
      rdfs:range owl:Literal ;
      owl:subPropertyOf :topDataProperty .

ns:issueDate
      a       :FunctionalProperty , owl:DatatypeProperty ;
      rdfs:comment "issueDate is the date a tradablequotable instrument was issued"@en ;
      rdfs:domain
              [ a       owl:Class ;
                :unionOf (ns:FinancialInstrument ns:QuotableInstrument)
              ] ;
      rdfs:label "issueDate"@en ;
      rdfs:range
              [ a       owl:Datatype ;
                :unionOf (xsd:date xsd:gYearMonth)
              ] ;
      owl:subPropertyOf ns:date .

ns:cyan
      a       :FunctionalProperty , owl:DatatypeProperty ;
      rdfs:comment "cyan component of the color representation per CMYK color system. "@en ;
      rdfs:domain ns:Color ;
      rdfs:label "cyan"@en ;
      rdfs:range owl:Literal ;
      owl:subPropertyOf ns:colorHolding .

ns:winnerOf
      a       owl:ObjectProperty ;
      rdfs:comment "The winnerOf object property connects an individual, organization, or media work to awards for which it has been nominated and won."@en ;
      rdfs:label "winnerOf"@en ;
      owl:subPropertyOf :topObjectProperty .

ns:competitionGroup
      a       owl:ObjectProperty ;
      rdfs:comment "Connects a competition organization group with the competition instances it puts on. NFL -> Super Bowl, FIFA -> World Cup"@en ;
      rdfs:domain ns:SportCompetitionInstance ;
      rdfs:label "competitionGroup"@en ;
      rdfs:range ns:SportCompetition .

ns:alternateGivenName
      a       :FunctionalProperty , owl:DatatypeProperty ;
      rdfs:comment "Note for Media V2 schema: Change to alternateGivenName to support Trailblazers globalization guidelines: http://twiki.corp.yahoo.com/view/TrailBlazers/PersonalNames"@en , "An alternate given name by which an individual may be known."@en ;
      rdfs:domain ns:AlternatePersonName ;
      rdfs:label "alternateGivenName"@en ;
      rdfs:range owl:Literal ;
      owl:subPropertyOf ns:name .

ns:contributingCompany
      a       owl:ObjectProperty ;
      rdfs:comment "Connects a media work to a company that contributed to the media work's production."@en ;
      rdfs:domain ns:MediaWork ;
      rdfs:label "contributingCompany"@en ;
      rdfs:range ns:Company ;
      owl:subPropertyOf :topObjectProperty ;
      :inverseOf ns:company .

ns:awardCategory
      a       :FunctionalProperty , owl:DatatypeProperty ;
      rdfs:comment "The subcategory for which an award is given (e.g., Best Picture)."@en ;
      rdfs:domain ns:AwardType ;
      rdfs:label "awardCategory"@en ;
      rdfs:range owl:Literal ;
      owl:subPropertyOf :topDataProperty .

ns:EventOrganizer
      a       owl:Class ;
      rdfs:comment "Group or individual that organizes a local event."@en ;
      rdfs:label "EventOrganizer"@en ;
      owl:subClassOf ns:Entity .

ns:contactNameMiddle
      a       :FunctionalProperty , owl:DatatypeProperty ;
      rdfs:comment "Middle name of the contact person for a local business (for use with SingleLocationBusiness only)."@en ;
      rdfs:domain ns:SingleLocationBusiness ;
      rdfs:label "contactNameMiddle"@en ;
      rdfs:range owl:Literal .

ns:logline
      a       :FunctionalProperty , owl:DatatypeProperty ;
      rdfs:comment "a brief summary of the television show or movie, used for promotion."@en ;
      rdfs:domain
              [ a       owl:Class ;
                :unionOf (ns:Movie ns:TvSeries ns:TvSpecial)
              ] ;
      rdfs:label "logline"@en ;
      rdfs:range owl:Literal ;
      owl:subPropertyOf :topDataProperty .

ns:vendorLink
      a       owl:DatatypeProperty ;
      rdfs:comment "Used by front-end to provide the link to feed-provider event page."@en ;
      rdfs:domain
              [ a       owl:Class ;
                :unionOf (ns:EventVenue ns:LocalEvent ns:Performer)
              ] ;
      rdfs:label "vendorLink"@en ;
      rdfs:range xsd:anyURI .

ns:PreferedStock
      a       owl:Class ;
      rdfs:comment "Preferred stcok  pecial equity security that has properties of both an equity and a debt instrument , senior to common stock"@en ;
      rdfs:label "PreferedStock"@en ;
      owl:subClassOf ns:FinancialInstrumentEquity .

ns:Ticker
      a       owl:Class ;
      rdfs:comment "Ticker represents an individual ticker entry"@en ;
      rdfs:label "Ticker"@en ;
      owl:subClassOf ns:Entity .

ns:StockExchange
      a       owl:Class ;
      rdfs:comment "StockExchange represents an entity which provides trading facilities for stock brokers and traders, to trade stocks and other securities"@en ;
      rdfs:label "StockExchange"@en ;
      owl:subClassOf ns:Exchange .

ns:educationLevel
      a       :FunctionalProperty , owl:DatatypeProperty ;
      rdfs:comment "Describes the level of education attained by a person."@en ;
      rdfs:domain ns:Person ;
      rdfs:label "educationLevel"@en ;
      rdfs:range owl:Literal .

ns:usedCarPriceMax
      a       :FunctionalProperty , owl:DatatypeProperty ;
      rdfs:comment "Applicable only if newModel=false. Indicates the maximum used car price (e.g. kbb price) for this model. This information is derived from trim details in the enrichment phase "@en ;
      rdfs:domain ns:AutoModel ;
      rdfs:label "usedCarPriceMax"@en ;
      rdfs:range xsd:double .

ns:teamGame
      a       owl:ObjectProperty ;
      rdfs:comment "Connects a game to the reified sport team role."@en ;
      rdfs:domain ns:SportGame ;
      rdfs:label "teamGame"@en ;
      rdfs:range ns:TeamGameRole .

ns:MovieRating
      a       owl:Class ;
      rdfs:comment "Rating system to categorize a film's thematic and content suitability for certain audiences."@en ;
      rdfs:label "MovieRating"@en ;
      owl:subClassOf ns:Entity .

ns:companyCompetitor
      a       owl:ObjectProperty ;
      rdfs:comment "Connects a company to its competitors."@en ;
      rdfs:domain ns:Company ;
      rdfs:label "companyCompetitor"@en ;
      rdfs:range ns:Company .

ns:birthday
      a       :FunctionalProperty , owl:DatatypeProperty ;
      rdfs:comment "The day and month on which an individual was born."@en ;
      rdfs:domain ns:Person ;
      rdfs:label "birthday"@en ;
      rdfs:range
              [ a       owl:Datatype ;
                :unionOf (ns:gMonthDay xsd:date)
              ] ;
      owl:subPropertyOf ns:date .

ns:autoModel
      a       owl:ObjectProperty ;
      rdfs:comment "Connects an auto model to its trim style"@en ;
      rdfs:domain ns:AutoTrim ;
      rdfs:label "autoModel"@en ;
      rdfs:range ns:AutoModel .

ns:name
      a       owl:DatatypeProperty ;
      rdfs:comment "this is a holding property for all organization and person name data properties."@en ;
      rdfs:label "name"@en ;
      owl:subPropertyOf ns:label .

ns:longitude
      a       :FunctionalProperty , owl:DatatypeProperty ;
      rdfs:comment "Longitude of a location"@en ;
      rdfs:domain
              [ a       owl:Class ;
                :unionOf (ns:Address ns:EventVenue ns:Place ns:SingleLocationBusiness)
              ] ;
      rdfs:label "longitude"@en ;
      rdfs:range xsd:float ;
      owl:subPropertyOf :topDataProperty .

ns:AlbumTrack
      a       owl:Class ;
      rdfs:comment "An audio file that makes up an audio album."@en ;
      rdfs:label "AlbumTrack"@en ;
      owl:subClassOf ns:MediaWork .

ns:NightClub
      a       owl:Class ;
      rdfs:comment "Nightclub is an entertainment venue which usually operates late into the night generally distinguished from bars, pubs or taverns by the inclusion of a dance floor and a DJ booth"@en ;
      rdfs:label "NightClub"@en ;
      owl:subClassOf ns:EventVenue .

ns:AutoTrim
      a       owl:Class ;
      rdfs:comment "A trim level is a version or level of a particular automotive model year.  Trim levels are usually defined by different combinations of dimensions, equipment, driveline, engine, transmission, top speed and acceleration. "@en ;
      rdfs:label "AutoTrim"@en ;
      owl:subClassOf ns:Entity .

ns:episodeType
      a       :FunctionalProperty , owl:DatatypeProperty ;
      rdfs:comment "whether or not this is an episode or pilot"@en ;
      rdfs:domain ns:TvEpisode ;
      rdfs:label "episodeType"@en ;
      rdfs:range owl:Literal ;
      owl:subPropertyOf :topDataProperty .

ns:businessHighlights
      a       owl:DatatypeProperty ;
      rdfs:comment "Featured highlights for a business, e.g. 'good for kids', 'good for seniors', etc."@en ;
      rdfs:domain ns:LocalBusiness ;
      rdfs:label "businessHighlights"@en ;
      rdfs:range owl:Literal .

ns:nearbyTransport
      a       owl:DatatypeProperty ;
      rdfs:comment "Outlines the transit options near a location. Free text. For example: 2km to nearest airport, metro station right around corner, etc. "@en ;
      rdfs:domain
              [ a       owl:Class ;
                :unionOf (ns:LocalBusiness ns:Structure)
              ] ;
      rdfs:label "nearbyTransport"@en ;
      rdfs:range owl:Literal ;
      owl:subPropertyOf :topDataProperty .

ns:parentalAdvisory
      a       owl:DatatypeProperty ;
      rdfs:comment "Parental advisory warning detailing thematic elements present in an audio media work."@en ;
      rdfs:domain
              [ a       owl:Class ;
                :unionOf (ns:Album ns:Song)
              ] ;
      rdfs:label "parentalAdvisory"@en ;
      rdfs:range owl:Literal ;
      owl:subPropertyOf :topDataProperty .

ns:reviewSource
      a       :FunctionalProperty , owl:DatatypeProperty ;
      rdfs:comment "Source from which a critical review originates."@en ;
      rdfs:domain ns:Review ;
      rdfs:label "reviewSource"@en ;
      rdfs:range owl:Literal .

ns:RecordLabel
      a       owl:Class ;
      rdfs:comment "A record label is an organization that coordinates the production, manufacture, distribution, marketing and promotion, and enforcement of copyright protection of sound recordings and music videos."@en ;
      rdfs:label "RecordLabel"@en ;
      owl:subClassOf ns:Company .

ns:departmentName
      a       :FunctionalProperty , owl:DatatypeProperty ;
      rdfs:comment "Department name for a business listing"@en ;
      rdfs:domain
              [ a       owl:Class ;
                :unionOf (ns:Address ns:ContactInfo ns:Phone ns:SingleLocationBusiness)
              ] ;
      rdfs:label "departmentName"@en ;
      rdfs:range owl:Literal ;
      owl:subPropertyOf ns:name .

ns:unitAddress
      a       :FunctionalProperty , owl:DatatypeProperty ;
      rdfs:comment "Unit value. Eg: G in 1659 Branham Ln Ste G"@en ;
      rdfs:domain
              [ a       owl:Class ;
                :unionOf (ns:Address ns:SingleLocationBusiness)
              ] ;
      rdfs:label "unitAddress"@en ;
      rdfs:range owl:Literal ;
      owl:subPropertyOf :topDataProperty .

ns:startYear
      a       :FunctionalProperty , owl:DatatypeProperty ;
      rdfs:comment "Year that an event begins or that an organization was established."@en ;
      rdfs:domain
              [ a       owl:Class ;
                :unionOf (ns:Event ns:Organization ns:TvSeason)
              ] ;
      rdfs:label "startYear"@en ;
      rdfs:range xsd:gYear ;
      owl:subPropertyOf ns:date .

ns:rated
      a       owl:ObjectProperty ;
      rdfs:comment "Connects a film to its rating for thematic and content suitability for certain audiences."@en ;
      rdfs:domain
              [ a       owl:Class ;
                :unionOf (ns:Movie ns:Video)
              ] ;
      rdfs:label "rated"@en ;
      rdfs:range ns:MovieRating ;
      owl:subPropertyOf :topObjectProperty .

ns:countyLocation
      a       owl:ObjectProperty ;
      rdfs:comment "Connects the county class to its address."@en ;
      rdfs:domain
              [ a       owl:Class ;
                :unionOf (ns:Address ns:Place)
              ] ;
      rdfs:label "countyLocation"@en ;
      rdfs:range ns:CountyAdminArea ;
      owl:subPropertyOf ns:location .

ns:operatingHoursNote
      a       owl:DatatypeProperty ;
      rdfs:comment "Examples: Closed on holidays, Open for all holidays except Christmas, etc "@en ;
      rdfs:domain
              [ a       owl:Class ;
                :unionOf (ns:ContactInfo ns:LocalBusiness ns:SingleLocationBusiness)
              ] ;
      rdfs:label "operatingHoursNote"@en ;
      rdfs:range owl:Literal ;
      owl:subPropertyOf :topDataProperty .

ns:eventOrganizer
      a       owl:ObjectProperty ;
      rdfs:comment "Connects an event to its sponsoring organization."@en ;
      rdfs:domain ns:LocalEvent ;
      rdfs:label "eventOrganizer"@en ;
      rdfs:range ns:EventOrganizer .

ns:biography
      a       owl:ObjectProperty ;
      rdfs:comment "Connects an individual to his or her biography."@en ;
      rdfs:domain ns:Person ;
      rdfs:label "biography"@en ;
      rdfs:range ns:Biography ;
      :inverseOf ns:biographyOf .

ns:imageWidth
      a       :FunctionalProperty , owl:DatatypeProperty ;
      rdfs:comment "width of image in pixels "@en ;
      rdfs:domain ns:Image ;
      rdfs:label "imageWidth"@en ;
      rdfs:range xsd:int ;
      owl:subPropertyOf :topDataProperty .

ns:listingCreationDate
      a       :FunctionalProperty , owl:DatatypeProperty ;
      rdfs:comment "listingCreationDate signifies when the listing is first generated"@en ;
      rdfs:domain ns:LocalBusiness ;
      rdfs:label "listingCreationDate"@en ;
      rdfs:range
              [ a       owl:Datatype ;
                :unionOf (xsd:date xsd:gYearMonth)
              ] ;
      owl:subPropertyOf ns:date .

ns:preferredParkingAvailable
      a       :FunctionalProperty , owl:DatatypeProperty ;
      rdfs:comment "Describes whether or not a theater or other venue offers preferred parking."@en ;
      rdfs:domain ns:MovieTheater ;
      rdfs:label "preferredParkingAvailable"@en ;
      rdfs:range xsd:boolean .

ns:analystRating
      a       :FunctionalProperty , owl:DatatypeProperty ;
      rdfs:comment "analyst rating how many stars (1-5) an anlyst rated for that stock"@en ;
      rdfs:domain ns:Analyst ;
      rdfs:label "analystRating"@en ;
      rdfs:range owl:Literal .

ns:countryCode
      a       :FunctionalProperty , owl:DatatypeProperty ;
      rdfs:comment "Standardized code to designate a country in an address or other location. Must conform to ISO 3166 country codes."@en ;
      rdfs:domain
              [ a       owl:Class ;
                :unionOf (ns:Address ns:Country ns:Currency ns:Organization ns:SingleLocationBusiness)
              ] ;
      rdfs:label "countryCode"@en ;
      rdfs:range owl:Literal ;
      owl:subPropertyOf :topDataProperty .

ns:Actor
      a       owl:Class ;
      rdfs:comment "Individual with at least one acting credit in a film, television series, or play."@en ;
      rdfs:label "Actor"@en ;
      owl:subClassOf ns:Person .

ns:trim
      a       owl:DatatypeProperty ;
      rdfs:comment "Describes the trim style and options of a particular automotive model."@en ;
      rdfs:domain
              [ a       owl:Class ;
                :unionOf (ns:AutoModel ns:AutoTrim)
              ] ;
      rdfs:label "trim"@en ;
      rdfs:range owl:Literal ;
      owl:subPropertyOf :topDataProperty .

ns:styleStatus
      a       :FunctionalProperty , owl:DatatypeProperty ;
      rdfs:comment "Style status of the Auto model. Sample values (New,Carryover,Freshen, Redesign, Reskin). "@en ;
      rdfs:domain ns:AutoModel ;
      rdfs:label "styleStatus"@en ;
      rdfs:range owl:Literal .

ns:accountProvider
      a       :FunctionalProperty , owl:DatatypeProperty ;
      rdfs:comment "Describes the organization generating an ID for an online account."@en ;
      rdfs:domain ns:OnlineAccount ;
      rdfs:label "accountProvider"@en ;
      rdfs:range owl:Literal ;
      owl:subPropertyOf :topDataProperty .

ns:releaseSubtitleLanguage
      a       :FunctionalProperty , owl:DatatypeProperty ;
      rdfs:comment "The language in which subtitles are available for a media release."@en ;
      rdfs:domain ns:MediaRelease ;
      rdfs:label "releaseSubtitleLanguage"@en ;
      rdfs:range owl:Literal .

ns:photographer
      a       :FunctionalProperty , owl:DatatypeProperty ;
      rdfs:comment "Photographer who created an image."@en ;
      rdfs:domain ns:Image ;
      rdfs:label "photographer"@en ;
      rdfs:range owl:Literal .

ns:showtimesURL
      a       owl:DatatypeProperty ;
      rdfs:comment "URL at which showtimes for a local business may be accessed."@en ;
      rdfs:domain
              [ a       owl:Class ;
                :unionOf (ns:Bar ns:EventVenue ns:MovieTheater ns:NightClub)
              ] ;
      rdfs:label "showtimesURL"@en .

ns:TertiaryAdminArea
      a       owl:Class ;
      rdfs:comment "Placetype: 10"@en , "A tertiary administrative area within a country. State = primary, County = secondary. example: London Borough of Greenwich"@en ;
      rdfs:label "TertiaryAdminArea"@en ;
      owl:subClassOf ns:GeoPoliticalEntity .

ns:FinancialInstrument
      a       owl:Class ;
      rdfs:comment """A Financial Instrument is a fungible, negotiable instrument representing financial value. Securities are broadly categorized into debt securities (such as banknotes, bonds and debentures) and equity securities, e.g., common stocks; and derivative contracts, such as forwards, futures, options and swaps.

Securities are financial instruments. """@en ;
      rdfs:label "FinancialInstrument"@en ;
      owl:subClassOf ns:Entity .

ns:endText
      a       :FunctionalProperty , owl:DatatypeProperty ;
      rdfs:comment "Blob dataproperty containing textual representation of the end of a timerange."@en ;
      rdfs:domain ns:Event ;
      rdfs:label "endText"@en ;
      rdfs:range owl:Literal ;
      owl:subPropertyOf :topDataProperty .

ns:urlContent
      a       owl:DatatypeProperty ;
      rdfs:comment "Content of the webpage"@en ;
      rdfs:domain ns:Webpage ;
      rdfs:label "urlContent"@en ;
      rdfs:range owl:Literal ;
      owl:subPropertyOf :topDataProperty .

ns:weekNumber
      a       :FunctionalProperty , owl:DatatypeProperty ;
      rdfs:comment "Numeric identifier for the calendar week in which box office revenue was received. Should be 1-52."@en ;
      rdfs:domain
              [ a       owl:Class ;
                :unionOf (ns:BoxOfficeWeekend ns:BoxOfficeWeekly)
              ] ;
      rdfs:label "weekNumber"@en ;
      rdfs:range xsd:int ;
      owl:subPropertyOf :topDataProperty .

ns:exPubCity
      a       :FunctionalProperty , owl:DatatypeProperty ;
      rdfs:comment "Amacai source data indicating the Published City as provided in Directory Source (e.g in WP or YP)."@en ;
      rdfs:domain ns:SingleLocationBusiness ;
      rdfs:label "exPubCity"@en ;
      rdfs:range owl:Literal .

ns:productTitle
      a       :FunctionalProperty , owl:DatatypeProperty ;
      rdfs:comment "Contains the main title of a media product."@en ;
      rdfs:domain ns:MediaProduct ;
      rdfs:label "productTitle"@en ;
      rdfs:range owl:Literal ;
      owl:subPropertyOf ns:label .

ns:influenced
      a       owl:ObjectProperty ;
      rdfs:comment "Connects a notable individual with people he or she has influenced."@en ;
      rdfs:domain ns:Person ;
      rdfs:label "influenced"@en ;
      rdfs:range ns:Person ;
      owl:subPropertyOf :topObjectProperty ;
      :inverseOf ns:influencedBy .

ns:businessCategoryAssignment
      a       owl:ObjectProperty ;
      rdfs:comment "businessCategoryAssignment connects LocalBusinessCategory to BusinessListingCategory"@en ;
      rdfs:domain ns:LocalBusinessCategory ;
      rdfs:label "businessCategoryAssignment"@en ;
      rdfs:range ns:BusinessListingCategory ;
      :inverseOf ns:businessCategoryAssignmentOf .

ns:orderOnlineURL
      a       owl:DatatypeProperty ;
      rdfs:comment "URL at which users may order goods or services from a local business."@en ;
      rdfs:domain ns:LocalBusiness ;
      rdfs:label "orderOnlineURL"@en ;
      rdfs:range xsd:anyURI .

ns:country
      a       :FunctionalProperty , owl:DatatypeProperty ;
      rdfs:comment "The country of a physical location or address."@en ;
      rdfs:domain
              [ a       owl:Class ;
                :unionOf (ns:Address ns:SingleLocationBusiness)
              ] ;
      rdfs:label "country"@en ;
      rdfs:range owl:Literal ;
      owl:subPropertyOf :topDataProperty .

ns:courseListingURL
      a       owl:DatatypeProperty ;
      rdfs:comment "URL at which course listings for an educational institution may be accessed."@en ;
      rdfs:domain ns:EducationalInstitution ;
      rdfs:label "courseListingURL"@en ;
      rdfs:range xsd:anyURI .

ns:criticalConsensus
      a       owl:DatatypeProperty ;
      rdfs:comment "Consensus about the quality of a film, as garnered from critical reviews."@en ;
      rdfs:domain ns:RottenTomatoesReview ;
      rdfs:label "criticalConsensus"@en ;
      rdfs:range owl:Literal ;
      owl:subPropertyOf :topDataProperty .

ns:localGlobalId
      a       :FunctionalProperty , owl:DatatypeProperty ;
      rdfs:comment "Global unique identifier assigned by Y! Local for Local Business."@en ;
      rdfs:domain ns:LocalBusiness ;
      rdfs:label "localGlobalId"@en ;
      rdfs:range owl:Literal ;
      owl:subPropertyOf ns:id .

ns:enrollment
      a       owl:DatatypeProperty ;
      rdfs:comment "Describes the enrollment at an educational institution."@en ;
      rdfs:domain ns:EducationalInstitution ;
      rdfs:label "enrollment"@en ;
      rdfs:range owl:Literal .

ns:teamGameIn
      a       owl:ObjectProperty ;
      rdfs:comment "Connects the team game role to the sport Game."@en ;
      rdfs:domain ns:TeamGameRole ;
      rdfs:label "teamGameIn"@en ;
      rdfs:range ns:SportGame ;
      :inverseOf ns:teamGame .

ns:recordLabelOf
      a       owl:ObjectProperty ;
      rdfs:comment "The label property connects a record label that released the album to the album itself."@en ;
      rdfs:domain ns:RecordLabel ;
      rdfs:label "recordLabelOf"@en ;
      rdfs:range ns:Album ;
      :inverseOf ns:recordLabel .

ns:homepage
      a       :FunctionalProperty , owl:DatatypeProperty ;
      rdfs:comment "The web page of an individual or group."@en ;
      rdfs:domain
              [ a       owl:Class ;
                :unionOf (ns:Group ns:Person ns:Structure)
              ] ;
      rdfs:label "homepage"@en ;
      rdfs:range xsd:anyURI .

ns:paymentCardAccepted
      a       owl:DatatypeProperty ;
      rdfs:comment "Brands of credit cards accepted by a business or other organization."@en ;
      rdfs:domain ns:LocalBusiness ;
      rdfs:label "paymentCardAccepted"@en ;
      rdfs:range owl:Literal ;
      rdfs:range
              [ a       owl:Datatype ;
                :oneOf  [ a       rdf:List ;
                          rdf:first "AMEX"^^xsd:string ;
                          rdf:rest
                                  [ a       rdf:List ;
                                    rdf:first "CARETE BLANCHE"^^xsd:string ;
                                    rdf:rest
                                            [ a       rdf:List ;
                                              rdf:first "DINERS CLUB"^^xsd:string ;
                                              rdf:rest
                                                      [ a       rdf:List ;
                                                        rdf:first "DISCOVER"^^xsd:string ;
                                                        rdf:rest
                                                                [ a       rdf:List ;
                                                                  rdf:first "ELECTRON"^^xsd:string ;
                                                                  rdf:rest
                                                                          [ a       rdf:List ;
                                                                            rdf:first "EUROCARD"^^xsd:string ;
                                                                            rdf:rest
                                                                                    [ a       rdf:List ;
                                                                                      rdf:first "JCB"^^xsd:string ;
                                                                                      rdf:rest
                                                                                              [ a       rdf:List ;
                                                                                                rdf:first "MASTERCARD"^^xsd:string ;
                                                                                                rdf:rest
                                                                                                        [ a       rdf:List ;
                                                                                                          rdf:first "OPTIMA"^^xsd:string ;
                                                                                                          rdf:rest
                                                                                                                  [ a       rdf:List ;
                                                                                                                    rdf:first "VISA"^^xsd:string ;
                                                                                                                    rdf:rest ()
                                                                                                                  ]
                                                                                                        ]
                                                                                              ]
                                                                                    ]
                                                                          ]
                                                                ]
                                                      ]
                                            ]
                                  ]
                        ]
              ] ;
      owl:subPropertyOf :topDataProperty .

ns:athleteParticipationIn
      a       owl:ObjectProperty ;
      rdfs:comment "connects a player to the reified AthleteGameRole class."@en ;
      rdfs:domain ns:Athlete ;
      rdfs:label "athleteParticipationIn"@en ;
      rdfs:range ns:AthleteGameRole ;
      :inverseOf ns:athleteParticipation .

ns:SportVenue
      a       owl:Class ;
      rdfs:comment "Covers stadiums, athletic fields, or basketball courts as well as any other place sports are played and practiced."@en ;
      rdfs:label "SportVenue"@en ;
      owl:subClassOf ns:EventVenue .

ns:gameId
      a       :FunctionalProperty , owl:DatatypeProperty ;
      rdfs:comment "Identifies a sporting event."@en ;
      rdfs:domain ns:SportGame ;
      rdfs:label "gameId"@en ;
      rdfs:range owl:Literal ;
      owl:subPropertyOf ns:id .

ns:SportCompetitionInstance
      a       owl:Class ;
      rdfs:comment "Core information about a competition made up of several games or an entire season of games, such as the English Premier League or Volleyball World Cup. "@en ;
      rdfs:label "SportCompetitionInstance"@en ;
      owl:subClassOf ns:LocalEvent .

ns:forum
      a       :FunctionalProperty , owl:DatatypeProperty ;
      rdfs:comment "Link to an online item's forum page."@en ;
      rdfs:domain ns:Entity ;
      rdfs:label "forum"@en ;
      rdfs:range xsd:anyURI ;
      owl:subPropertyOf :topDataProperty .

ns:topic
      a       owl:ObjectProperty ;
      rdfs:comment "connects the Topic class to the entity class."@en ;
      rdfs:domain ns:Topic ;
      rdfs:label "topic"@en ;
      rdfs:range ns:Entity .

ns:registration
      a       owl:ObjectProperty ;
      rdfs:comment "Connects an event to the registration class."@en ;
      rdfs:domain ns:LocalEventOccurrence ;
      rdfs:label "registration"@en ;
      rdfs:range ns:EventRegistration .

ns:rawFeedDataMarkup
      a       owl:DatatypeProperty ;
      rdfs:comment "Captures the data markup associated with an entity from the raw data feed. Not for display."@en ;
      rdfs:domain ns:Entity ;
      rdfs:label "rawFeedDataMarkup"@en ;
      rdfs:range owl:Literal .

ns:ETF
      a       owl:Class ;
      rdfs:comment "ETF is exchange traded fund"@en ;
      rdfs:label "ETF"@en ;
      owl:subClassOf ns:ETO .

ns:addressType
      a       owl:DatatypeProperty ;
      rdfs:comment "Type of address, like home, business, work, mailing, physical."@en ;
      rdfs:domain ns:Address ;
      rdfs:label "addressType"@en ;
      rdfs:range owl:Literal ;
      owl:subPropertyOf :topDataProperty .

ns:ageGroup
      a       :FunctionalProperty , owl:DatatypeProperty ;
      rdfs:comment "The age range of a sports competition or team."@en ;
      rdfs:domain
              [ a       owl:Class ;
                :unionOf (ns:SportCompetitionInstance ns:SportTeam)
              ] ;
      rdfs:label "ageGroup"@en ;
      rdfs:range owl:Literal ;
      owl:subPropertyOf :topDataProperty .

ns:courseList
      a       owl:DatatypeProperty ;
      rdfs:comment "courseList is a list of courses available at an educational institution"@en ;
      rdfs:domain ns:EducationalInstitution ;
      rdfs:label "courseList"@en ;
      rdfs:range owl:Literal .

ns:soundEncoding
      a       :FunctionalProperty , owl:DatatypeProperty ;
      rdfs:comment "Details the sound encoding present used on a media product."@en ;
      rdfs:domain ns:MediaProduct ;
      rdfs:label "soundEncoding"@en ;
      rdfs:range owl:Literal ;
      owl:subPropertyOf :topDataProperty .

ns:cityLocationOf
      a       :FunctionalProperty , owl:ObjectProperty ;
      rdfs:comment "Connects an address or other entity to its city."@en ;
      rdfs:domain ns:CityTown ;
      rdfs:label "cityLocationOf"@en ;
      rdfs:range
              [ a       owl:Class ;
                :unionOf (ns:Address ns:Place)
              ] ;
      owl:subPropertyOf ns:location ;
      :inverseOf ns:cityLocation .

ns:CompanyOfficer
      a       owl:Class ;
      rdfs:comment "CompanyOfficers repersents those persons who are executives in a company."@en ;
      rdfs:label "CompanyOfficers"@en ;
      owl:subClassOf ns:FinancePerson .

ns:rawFeedDataAltId
      a       owl:DatatypeProperty ;
      rdfs:comment "Alternate identifier assigned to an entity in the raw feed. Not for display."@en ;
      rdfs:domain ns:Entity ;
      rdfs:label "rawFeedDataAltId"@en ;
      rdfs:range owl:Literal .

ns:Bond
      a       owl:Class ;
      rdfs:comment "Bond is a debt security, in which the authorized issuer owes the holders a debt and, depending on the terms of the bond, is obliged to pay interest (the coupon) and/or to repay the principal at a later date, termed maturity"@en ;
      rdfs:label "Bond"@en ;
      owl:subClassOf ns:Debt .

ns:cityLocation
      a       owl:ObjectProperty ;
      rdfs:comment "Connects a city entity to its address."@en ;
      rdfs:domain
              [ a       owl:Class ;
                :unionOf (ns:Address ns:Place)
              ] ;
      rdfs:label "cityLocation"@en ;
      rdfs:range ns:CityTown ;
      owl:subPropertyOf ns:location .

ns:amount
      a       :FunctionalProperty , owl:DatatypeProperty ;
      rdfs:comment "Numerical value. In CCS, needs to include tuple with currency code and the value."@en ;
      rdfs:domain ns:BoxOfficeWeekend ;
      rdfs:label "amount"@en ;
      rdfs:range xsd:float ;
      owl:subPropertyOf :topDataProperty .

ns:Animal
      a       owl:Class ;
      rdfs:comment "Created by ace to support Milton mapping: http://twiki.corp.yahoo.com/view/P13nContextual/MiltonWooSchemaMap"@en , "Animals are a major group of mostly multicellular, eukaryotic organisms of the kingdom Animalia or Metazoa."@en ;
      rdfs:label "Animal"@en ;
      owl:subClassOf ns:Entity .

ns:BoxOfficeWeekly
      a       owl:Class ;
      rdfs:comment "The box office income for a film in theatrical release over the period of one week."@en ;
      rdfs:label "BoxOfficeWeekly"@en ;
      owl:subClassOf ns:BoxOffice .

ns:market
      a       owl:DatatypeProperty ;
      rdfs:comment "Describes the local market an organization serves."@en ;
      rdfs:domain
              [ a       owl:Class ;
                :unionOf (ns:LocalBusiness ns:MovieTheater)
              ] ;
      rdfs:label "market"@en ;
      rdfs:range owl:Literal .

ns:floorNumber
      a       :FunctionalProperty , owl:DatatypeProperty ;
      rdfs:comment "Designation of the building floor number for an address."@en ;
      rdfs:domain ns:Address ;
      rdfs:label "floorNumber"@en ;
      rdfs:range owl:Literal ;
      owl:subPropertyOf :topDataProperty .

ns:PostalZip
      a       owl:Class ;
      rdfs:comment "A partial or full postal code. Example: 94089, SW1 "@en , "placetype 11"@en ;
      rdfs:label "PostalZip"@en ;
      owl:subClassOf ns:Place .

:Thing
      a       owl:Class .

ns:reservationURL
      a       owl:DatatypeProperty ;
      rdfs:comment "URL by which users can make reservations at a local business."@en ;
      rdfs:domain ns:LocalBusiness ;
      rdfs:label "reservationURL"@en ;
      rdfs:range xsd:anyURI .

ns:vanityPhoneNumber
      a       :FunctionalProperty , owl:DatatypeProperty ;
      rdfs:comment "For a business that uses a mnemonic way of expressing their phone number. US data has quite a few cases of this type 1-800-4MYHOME, 1-800-MYAPPLE "@en ;
      rdfs:domain ns:Phone ;
      rdfs:label "vanityPhoneNumber"@en ;
      rdfs:range owl:Literal ;
      owl:subPropertyOf :topDataProperty .

ns:msrpMax
      a       :FunctionalProperty , owl:DatatypeProperty ;
      rdfs:comment "Indicates the maximum msrp for this model. This information is derived from trim details in the enrichment phase "@en ;
      rdfs:domain ns:AutoModel ;
      rdfs:label "msrpMax"@en ;
      rdfs:range xsd:float .

ns:schoolDistrict
      a       owl:DatatypeProperty ;
      rdfs:comment "Indicates the school district to which an educational institution belongs."@en ;
      rdfs:domain ns:EducationalInstitution ;
      rdfs:label "schoolDistrict"@en ;
      rdfs:range owl:Literal .

ns:ownerOfMarketTier
      a       owl:ObjectProperty ;
      rdfs:comment "ownerOfMarketTier connects an exchange to its market tiers"@en ;
      rdfs:domain ns:Exchange ;
      rdfs:label "ownerOfMarketTier"@en ;
      rdfs:range ns:MarketTier ;
      :inverseOf ns:marketTierOf .

ns:location
      a       owl:ObjectProperty ;
      rdfs:comment "Connects an event or thing to its physical location."@en ;
      rdfs:domain ns:Entity ;
      rdfs:label "location"@en ;
      rdfs:range ns:Place ;
      owl:subPropertyOf :topObjectProperty .

ns:Screenwriter
      a       owl:Class ;
      rdfs:comment "The screenwriter type includes people who have written screenplays for film or television."@en ;
      rdfs:label "Screenwriter"@en ;
      owl:subClassOf ns:Writer ;
      owl:subClassOf
              [ a       :Restriction ;
                :allValuesFrom
                        [ a       owl:Class ;
                          :unionOf (ns:Movie ns:TvEpisode ns:TvSeries)
                        ] ;
                :onProperty ns:written
              ] .

ns:tribuneID
      a       :FunctionalProperty , owl:DatatypeProperty ;
      rdfs:comment "Tribune ID for genres and categories"@en ;
      rdfs:domain ns:CategoryMovieTV ;
      rdfs:label "tribuneID"@en ;
      rdfs:range owl:Literal ;
      owl:subPropertyOf ns:id .

ns:keyBlack
      a       :FunctionalProperty , owl:DatatypeProperty ;
      rdfs:comment "Black, or Key, component of the color representation per CMYK color system"@en ;
      rdfs:label "keyBlack"@en ;
      owl:subPropertyOf ns:colorHolding .

ns:numOfListings
      a       :FunctionalProperty , owl:DatatypeProperty ;
      rdfs:comment "numOfListings is the number of entities listed on an exchange"@en ;
      rdfs:domain ns:Exchange ;
      rdfs:label "numOfListings"@en ;
      rdfs:range xsd:float .

ns:postalCode
      a       :FunctionalProperty , owl:DatatypeProperty ;
      rdfs:comment "The zip or postal code for a location's physical address."@en ;
      rdfs:domain
              [ a       owl:Class ;
                :unionOf (ns:Address ns:PostalZip ns:SingleLocationBusiness)
              ] ;
      rdfs:label "postalCode"@en ;
      rdfs:range owl:Literal .

ns:boardMember
      a       owl:ObjectProperty ;
      rdfs:comment "boardMember connects a company to its board member affiliation"@en ;
      rdfs:domain
              [ a       owl:Class ;
                :unionOf (ns:Company ns:Exchange)
              ] ;
      rdfs:label "boardMember"@en ;
      rdfs:range ns:BoardMemberAffiliation ;
      :inverseOf ns:boardMemberOf .

<http://woo.corp.yahoo.com/ns/currency/USD>
      a       owl:Datatype .

ns:modelMungedName
      a       :FunctionalProperty , owl:DatatypeProperty ;
      rdfs:comment "Munged name representation of Model as per http://twiki.corp.yahoo.com/view/Autos/GlobalMungedName. "@en ;
      rdfs:domain ns:AutoModel ;
      rdfs:label "modelMungedName"@en ;
      rdfs:range owl:Literal ;
      owl:subPropertyOf ns:name .

ns:Currency
      a       owl:Class ;
      rdfs:comment "Currency is money in any form when in actual use as a medium of exchange"@en ;
      rdfs:label "Currency"@en ;
      owl:subClassOf ns:Entity .

ns:castIn
      a       owl:ObjectProperty ;
      rdfs:comment "Connects a media work to the actors, contestants, hosts, or personalities that appear in it."@en ;
      rdfs:domain ns:Actor ;
      rdfs:label "castIn"@en ;
      rdfs:range
              [ a       owl:Class ;
                :unionOf (ns:Movie ns:TvEpisode ns:TvSeason ns:TvSeries ns:TvSpecial)
              ] ;
      owl:subPropertyOf :topObjectProperty ;
      :inverseOf ns:cast .

ns:alternateKey
      a       owl:DatatypeProperty ;
      rdfs:comment "data property to capture an external ID for a given piece of content, eg. DBpedia or Freebase ID."@en ;
      rdfs:domain ns:Entity ;
      rdfs:label "alternateKey"@en ;
      rdfs:range owl:Literal .

ns:Basketball
      a       owl:Class ;
      rdfs:comment "Basketball is a team sport in which two teams of five players try to score points by throwing or shooting a ball through the top of a basketball hoop while following a set of rules. "@en ;
      rdfs:label "Basketball"@en ;
      owl:subClassOf ns:Sport .

ns:releaseType
      a       :FunctionalProperty , owl:DatatypeProperty ;
      rdfs:comment "Describes the type of release for public distribution (eg theatrical, DVD, etc.)"@en ;
      rdfs:domain ns:MediaRelease ;
      rdfs:label "releaseType"@en ;
      rdfs:range owl:Literal ;
      owl:subPropertyOf :topDataProperty .

ns:originalUrl
      a       :FunctionalProperty , owl:DatatypeProperty ;
      rdfs:comment "Original url for a website."@en ;
      rdfs:domain ns:Webpage ;
      rdfs:label "originalUrl"@en ;
      rdfs:range xsd:anyURI ;
      owl:subPropertyOf :topDataProperty .

ns:organizerId
      a       owl:DatatypeProperty ;
      rdfs:comment "Unique identifier assigned by Events for Event organizers."@en ;
      rdfs:domain
              [ a       owl:Class ;
                :unionOf (ns:EventOrganizer ns:LocalEvent)
              ] ;
      rdfs:label "organizerId"@en ;
      rdfs:range owl:Literal ;
      owl:subPropertyOf ns:id .

ns:mediaworkGenre
      a       owl:ObjectProperty ;
      rdfs:comment "The genre relation connects an artwork to the Genres that it falls into."@en ;
      rdfs:domain
              [ a       owl:Class ;
                :unionOf (ns:MediaWork ns:MusicArtist)
              ] ;
      rdfs:label "mediaworkGenre"@en ;
      rdfs:range ns:Genre .

ns:Soccer
      a       owl:Class ;
      rdfs:comment "Association football, commonly known as football or soccer, is a sport played between two teams of eleven players with a spherical ball. It is the world's most popular sport."@en ;
      rdfs:label "Soccer"@en ;
      owl:subClassOf ns:Sport .

ns:industry
      a       owl:DatatypeProperty ;
      rdfs:comment "industry is what industry a fund invests in or characterizes a n organization"@en ;
      rdfs:domain
              [ a       owl:Class ;
                :unionOf (ns:Fund ns:Organization)
              ] ;
      rdfs:label "industry"@en ;
      rdfs:range owl:Literal .

ns:hearingDevicesAvailable
      a       :FunctionalProperty , owl:DatatypeProperty ;
      rdfs:comment "Indicates whether assistive listening devices are available for Deaf or hard of hearing patrons."@en ;
      rdfs:domain ns:MovieTheater ;
      rdfs:label "hearingDevicesAvailable"@en ;
      rdfs:range xsd:boolean .

ns:businessCategory
      a       owl:ObjectProperty ;
      rdfs:comment "businessCategory connects LocalBusiness to LocalBusinessCategory"@en ;
      rdfs:domain ns:LocalBusiness ;
      rdfs:label "businessCategory"@en ;
      rdfs:range ns:LocalBusinessCategory .

ns:categoryName
      a       owl:DatatypeProperty ;
      rdfs:comment "Y! category name "@en ;
      rdfs:domain
              [ a       owl:Class ;
                :unionOf (ns:BusinessListingCategory ns:Deal)
              ] ;
      rdfs:label "categoryName"@en ;
      rdfs:range owl:Literal ;
      owl:subPropertyOf ns:name .

ns:reviewOf
      a       :FunctionalProperty , owl:ObjectProperty ;
      rdfs:comment "Connects a critical review to the entity it evaluates."@en ;
      rdfs:domain ns:Review ;
      rdfs:label "reviewOf"@en ;
      rdfs:range
              [ a       owl:Class ;
                :unionOf (ns:LocalBusiness ns:MediaWork)
              ] ;
      owl:subPropertyOf :topObjectProperty .

ns:Milestone
      a       owl:Class ;
      rdfs:comment "The Milestone class describes notable events in an individual's life."@en ;
      rdfs:label "Milestone"@en ;
      owl:subClassOf ns:Event .

ns:discountUrl
      a       owl:DatatypeProperty ;
      rdfs:comment "URL for any local business discounts (use with SingleLocationBusiness only)"@en ;
      rdfs:domain ns:SingleLocationBusiness ;
      rdfs:label "discountUrl"@en ;
      rdfs:range xsd:anyURI .

ns:contactInfoType
      a       :FunctionalProperty , owl:DatatypeProperty ;
      rdfs:comment "contactInfoType indicates a place of business' type, eg. headquarters, branch, regional office, etc."@en ;
      rdfs:domain ns:ContactInfo ;
      rdfs:label "contactInfoType"@en ;
      rdfs:range owl:Literal .

ns:EstablishmentShow
      a       owl:Class ;
      rdfs:comment "EstablishmentShow is for those performances that occur in a bar, restaurant or nightclub"@en ;
      rdfs:label "EstablishmentShow"@en ;
      owl:subClassOf ns:LocalEvent .

ns:serviceAreaOf
      a       owl:ObjectProperty ;
      rdfs:comment "Connects a location with the businesses that serve it."@en ;
      rdfs:domain ns:Organization ;
      rdfs:label "serviceAreaOf"@en ;
      rdfs:range ns:GeoPoliticalEntity ;
      owl:subPropertyOf :topObjectProperty ;
      :inverseOf ns:serviceArea .

ns:HistoricalCounty
      a       owl:Class ;
      rdfs:comment "placetype: 27"@en , "Former or historical secondary administrative area within a country. Example: Avon County (England)"@en ;
      rdfs:label "HistoricalCounty"@en ;
      owl:subClassOf ns:Place .

ns:InsiderAffiliation
      a       owl:Class ;
      rdfs:comment "InsiderAffiliation represents those persons, orgs or shareholders that are related to an org with potential access to non-public information about the company"@en ;
      rdfs:label "InsiderAffiliation"@en ;
      owl:subClassOf ns:OrgAffiliation .

ns:Lyricist
      a       owl:Class ;
      rdfs:comment "The person who writes the words to a song or musical play."@en ;
      rdfs:label "Lyricist"@en ;
      owl:subClassOf ns:Writer .

ns:EventRegistration
      a       owl:Class ;
      rdfs:comment "Details registration information for a local event."@en ;
      rdfs:label "EventRegistration"@en ;
      owl:subClassOf ns:Entity .

ns:magenta
      a       :FunctionalProperty , owl:DatatypeProperty ;
      rdfs:comment "magenta component of the color representation per CMYK color system "@en ;
      rdfs:domain ns:Color ;
      rdfs:label "magenta"@en ;
      rdfs:range owl:Literal ;
      owl:subPropertyOf ns:colorHolding .

ns:Crew
      a       owl:Class ;
      rdfs:comment "The Crew class is a person who served as a crew member on a media work."@en ;
      rdfs:label "Crew"@en ;
      owl:subClassOf ns:Person .

ns:alternatePrefix
      a       :FunctionalProperty , owl:DatatypeProperty ;
      rdfs:comment "Alternate name prefixes by which an individual may be known."@en ;
      rdfs:domain ns:AlternatePersonName ;
      rdfs:label "alternatePrefix"@en ;
      rdfs:range owl:Literal ;
      owl:subPropertyOf ns:name .

ns:founder
      a       owl:DatatypeProperty ;
      rdfs:comment "founder is the founder of an organization"@en ;
      rdfs:domain ns:Organization ;
      rdfs:label "founder"@en ;
      rdfs:range owl:Literal .

ns:contributionFor
      a       :FunctionalProperty , owl:ObjectProperty ;
      rdfs:comment "The contributionFor property connects the reified CompanyRole class to the organization involved with the production of a media work."@en ;
      rdfs:domain ns:CompanyRole ;
      rdfs:label "contributionFor"@en ;
      rdfs:range ns:Movie ;
      owl:subPropertyOf :topObjectProperty ;
      :inverseOf ns:contribution .

ns:closedHolidays
      a       owl:DatatypeProperty ;
      rdfs:comment "Enumerates the holidays when an organization is closed. array of strings with each string of the format (,,*,*,*,*) as in http://wiki.pentaho.com/display/ServerDoc1x/05.+CRON+Expressions+in+Detail?showComments=false"@en ;
      rdfs:domain ns:ContactInfo ;
      rdfs:label "closedHolidays"@en ;
      rdfs:range owl:Literal ;
      owl:subPropertyOf :topDataProperty .

ns:Association
      a       owl:Class ;
      rdfs:comment "The Association class is a reified relationship connecting an individual, group, or media work to other individuals, groups, or media works that share similar traits. May include similar artists, similar films, or influences."@en ;
      rdfs:label "Association"@en ;
      owl:subClassOf ns:Entity .

ns:releaseLanguage
      a       :FunctionalProperty , owl:DatatypeProperty ;
      rdfs:comment "The language in which a media release's dialogue is spoken."@en ;
      rdfs:domain ns:MediaRelease ;
      rdfs:label "releaseLanguage"@en .

ns:issueEndDate
      a       :FunctionalProperty , owl:DatatypeProperty ;
      rdfs:comment "issueEndDate is the date an issue ends"@en ;
      rdfs:domain
              [ a       owl:Class ;
                :unionOf (ns:FinancialInstrument ns:QuotableInstrument)
              ] ;
      rdfs:label "issueEndDate"@en ;
      rdfs:range
              [ a       owl:Datatype ;
                :unionOf (xsd:date xsd:gYearMonth)
              ] ;
      owl:subPropertyOf ns:date .

ns:eventOccurrenceOf
      a       owl:ObjectProperty ;
      rdfs:comment "Connects a single event occurrence with a local event."@en ;
      rdfs:domain ns:LocalEventOccurrence ;
      rdfs:label "eventOccurrenceOf"@en ;
      rdfs:range ns:LocalEvent ;
      :inverseOf ns:eventOccurrence .

ns:companyOfficer
      a       owl:ObjectProperty ;
      rdfs:comment "companyOfficer connects a company to the companyofficeraffiliation"@en ;
      rdfs:domain ns:Company ;
      rdfs:label "companyOfficer"@en ;
      rdfs:range ns:CompanyOfficerAffiliation .

ns:tvShowType
      a       :FunctionalProperty , owl:DatatypeProperty ;
      rdfs:comment "Type of tv show. Examples: TV Series, Movie, Mini Series, Event "@en ;
      rdfs:domain
              [ a       owl:Class ;
                :unionOf (ns:TvSeries ns:TvSpecial)
              ] ;
      rdfs:label "tvShowType"@en ;
      rdfs:range owl:Literal ;
      owl:subPropertyOf :topDataProperty .

ns:appearanceIn
      a       owl:ObjectProperty ;
      rdfs:comment "Connects the reified AppearanceRole class to a TV Show."@en ;
      rdfs:domain ns:AppearanceRole ;
      rdfs:label "appearanceIn"@en ;
      rdfs:range
              [ a       owl:Class ;
                :unionOf (ns:TvEpisode ns:TvSeason ns:TvSeries ns:TvSpecial)
              ] ;
      owl:subPropertyOf :topObjectProperty ;
      :inverseOf ns:appearance .

ns:boxofficeOf
      a       :FunctionalProperty , owl:ObjectProperty ;
      rdfs:comment "Connects the box office class to the film for which it records receipts."@en ;
      rdfs:domain
              [ a       owl:Class ;
                :unionOf (ns:BoxOfficeAllTime ns:BoxOfficeDaily ns:BoxOfficeWeekend ns:BoxOfficeWeekly)
              ] ;
      rdfs:label "boxofficeOf"@en ;
      rdfs:range ns:Movie ;
      owl:subPropertyOf :topObjectProperty ;
      :inverseOf ns:boxoffice .

ns:Book
      a       owl:Class ;
      rdfs:comment "A written work or collection of works, in book form. May be paper or electronic."@en ;
      rdfs:label "Book"@en ;
      owl:subClassOf ns:MediaProduct .

ns:featuredPerformer
      a       owl:ObjectProperty , owl:DatatypeProperty ;
      rdfs:comment "Connects a featured performer to an event or musical performance."@en ;
      rdfs:domain ns:MusicPerformance ;
      rdfs:label "featuredPerformer"@en ;
      rdfs:range owl:Literal , ns:MusicArtist ;
      owl:subPropertyOf :topObjectProperty .

ns:scratchResistant
      a       :FunctionalProperty , owl:DatatypeProperty ;
      rdfs:comment "Is the exterior paint scratch resistant? Applicable only if colorCategory is Exterior"@en ;
      rdfs:domain ns:Color ;
      rdfs:label "scratchResistant"@en ;
      rdfs:range xsd:boolean ;
      owl:subPropertyOf ns:colorHolding .

ns:trackPerformanceOf
      a       owl:ObjectProperty ;
      rdfs:comment "Connects a musical perfomance to the album track it is on"@en ;
      rdfs:domain ns:MusicPerformance ;
      rdfs:label "trackPerformanceOf"@en ;
      rdfs:range ns:AlbumTrack ;
      owl:subPropertyOf :topObjectProperty ;
      :inverseOf ns:trackPerformance .

ns:deathYear
      a       :FunctionalProperty , owl:DatatypeProperty ;
      rdfs:comment "The year in which an individual died."@en ;
      rdfs:domain ns:Person ;
      rdfs:label "deathYear"@en ;
      rdfs:range xsd:gYear ;
      owl:subPropertyOf ns:date .

ns:competitors
      a       owl:ObjectProperty ;
      rdfs:comment "The competitors relation connects a game with the athletes that play in it."@en ;
      rdfs:domain ns:SportGame ;
      rdfs:label "competitors"@en ;
      rdfs:range ns:Athlete ;
      owl:subPropertyOf :topObjectProperty ;
      :inverseOf ns:competitorsOf .

ns:statusChangeOf
      a       owl:ObjectProperty ;
      rdfs:comment "statusChangeOf links the event class organizationStatusChange to an orgaization"@en ;
      rdfs:domain ns:OrganizationStatusChange ;
      rdfs:label "statusChangeOf"@en ;
      rdfs:range ns:Organization ;
      :inverseOf ns:statusChange .

ns:dealMobileTitle
      a       owl:DatatypeProperty ;
      rdfs:comment "Title of a deal, coupon, or offer formatted for easy display on a mobile device."@en ;
      rdfs:domain ns:Deal ;
      rdfs:label "dealMobileTitle"@en ;
      rdfs:range owl:Literal ;
      owl:subPropertyOf ns:label .

ns:valDate
      a       :FunctionalProperty , owl:DatatypeProperty ;
      rdfs:comment "Amacai source data indicating the date when the business is phone verified as active."@en ;
      rdfs:domain ns:SingleLocationBusiness ;
      rdfs:label "valDate"@en ;
      rdfs:range owl:Literal .

ns:majorShareholderOf
      a       owl:ObjectProperty ;
      rdfs:comment "majorShareholderOf connect a majorshoreholder affiliation to the financial instrument"@en ;
      rdfs:domain ns:MajorShareholderAffiliation ;
      rdfs:label "majorShareholderOf"@en ;
      rdfs:range ns:FinancialInstrument .

ns:lodgingClass
      a       owl:DatatypeProperty ;
      rdfs:comment "Describes the category of lodging type a local business falls into."@en ;
      rdfs:domain ns:Lodging ;
      rdfs:label "lodgingClass"@en ;
      rdfs:range owl:Literal .

ns:Country
      a       owl:Class ;
      rdfs:comment "Placetype code = 12"@en , "One of the countries or dependent territories defined by the ISO 3166-1 standard.  example: United States"@en ;
      rdfs:label "Country"@en ;
      owl:subClassOf ns:GeoPoliticalEntity .

ns:hashValue
      a       owl:DatatypeProperty ;
      rdfs:comment "contains the hash value of biz name or other entity for matching purposes. On published side, it's often optional."@en ;
      rdfs:domain ns:SingleLocationBusiness ;
      rdfs:label "hashValue"@en ;
      rdfs:range owl:Literal .

ns:LocalBusinessCategory
      a       owl:Class ;
      rdfs:comment "LocalBusinessCategory is a reified class connecting a LocaBusiness to BusinessLsitingCategory. Thie relationship has a weight and a primary category."@en ;
      rdfs:label "LocalBusinessCategory"@en ;
      owl:subClassOf ns:Entity .

ns:releaseFor
      a       :FunctionalProperty , owl:ObjectProperty ;
      rdfs:comment "Connects the reified Media Release class to a media work."@en ;
      rdfs:domain ns:MediaRelease ;
      rdfs:label "releaseFor"@en ;
      rdfs:range
              [ a       owl:Class ;
                :unionOf (ns:MediaProduct ns:MediaWork)
              ] ;
      owl:subPropertyOf :topObjectProperty .

ns:competitionGameOf
      a       owl:ObjectProperty ;
      rdfs:comment "Connects a competition to the individual games that made it up."@en ;
      rdfs:domain ns:SportCompetitionInstance ;
      rdfs:label "competitionGameOf"@en ;
      rdfs:range ns:SportGame ;
      owl:subPropertyOf :topObjectProperty ;
      :inverseOf ns:competitionGame .

ns:exchangeImportance
      a       :FunctionalProperty , owl:DatatypeProperty ;
      rdfs:comment "exchangeImportance is the ranking on the exchange "@en ;
      rdfs:domain ns:Exchange ;
      rdfs:label "exchangeImportance"@en ;
      rdfs:range xsd:int .

ns:releaseAttribute
      a       owl:DatatypeProperty ;
      rdfs:comment "Describes specific attributes of a media release, eg IMAX, 3D, Unrated, etc."@en ;
      rdfs:domain ns:MediaRelease ;
      rdfs:label "releaseAttribute"@en ;
      rdfs:range owl:Literal .

ns:analyserOf
      a       owl:ObjectProperty ;
      rdfs:comment "analyserOf connects the analyst to the org they analyze"@en ;
      rdfs:domain ns:AnalystAffiliation ;
      rdfs:label "analyserOf"@en ;
      rdfs:range ns:Company ;
      :inverseOf ns:analysedBy .

ns:boardAffiliationOf
      a       owl:ObjectProperty ;
      rdfs:comment "boardAffiliationOf connects a board member affiliation to a board member"@en ;
      rdfs:domain ns:BoardMemberAffiliation ;
      rdfs:label "boardAffiliationOf"@en ;
      rdfs:range ns:BoardMember ;
      :inverseOf ns:sitsOnBoard .

ns:officerAffiliationOf
      a       owl:ObjectProperty ;
      rdfs:comment "officerAffilaitionof connects the companyofficeraffiliation to the compay officer"@en ;
      rdfs:domain ns:CompanyOfficerAffiliation ;
      rdfs:label "officerAffiliationOf"@en ;
      rdfs:range ns:CompanyOfficer ;
      :inverseOf ns:officerAffiliated .

ns:marketCap
      a       :FunctionalProperty , owl:DatatypeProperty ;
      rdfs:comment "marketCap is a measurement of size of a business enterprise (corporation) equal to the share price times the number of shares outstandingis a measurement of size of a business enterprise (corporation) equal to the share price times the number of shares outstanding"@en ;
      rdfs:domain ns:Exchange ;
      rdfs:label "marketCap"@en ;
      rdfs:range owl:Literal .

ns:showing
      a       owl:ObjectProperty ;
      rdfs:comment "Connects a theater to the reified showtime class."@en ;
      rdfs:domain ns:MovieTheater ;
      rdfs:label "showing"@en ;
      rdfs:range ns:MovieShowtime ;
      owl:subPropertyOf :topObjectProperty .

ns:national
      a       :FunctionalProperty , owl:DatatypeProperty ;
      rdfs:comment "indicates whether a deal is national or not."@en ;
      rdfs:domain ns:Deal ;
      rdfs:label "national"@en ;
      rdfs:range xsd:boolean .

ns:centerLongitude
      a       :FunctionalProperty , owl:DatatypeProperty ;
      rdfs:comment "The longitude that leads to the central point of a location"@en ;
      rdfs:domain
              [ a       owl:Class ;
                :unionOf (ns:Address ns:Place)
              ] ;
      rdfs:label "centerLongitude"@en ;
      rdfs:range xsd:float ;
      owl:subPropertyOf :topDataProperty .

ns:operatingStatus
      a       :FunctionalProperty , owl:DatatypeProperty ;
      rdfs:comment "operatingStatus is for the current operating status of a company"@en ;
      rdfs:domain ns:Company ;
      rdfs:label "operatingStatus"@en ;
      rdfs:range owl:Literal .

ns:jobHeld
      a       owl:ObjectProperty ;
      rdfs:comment "Connects a person to the Occupational History reified class."@en ;
      rdfs:domain ns:Person ;
      rdfs:label "jobHeld"@en ;
      rdfs:range ns:OccupationalHistory ;
      owl:subPropertyOf :topObjectProperty .

ns:coachedBy
      a       owl:ObjectProperty ;
      rdfs:comment "Connects a team or athlete with the person who coaches it."@en ;
      rdfs:domain
              [ a       owl:Class ;
                :unionOf (ns:Athlete ns:SportTeam)
              ] ;
      rdfs:label "coachedBy"@en ;
      rdfs:range ns:Coach .

ns:logoImage
      a       :FunctionalProperty , owl:DatatypeProperty ;
      rdfs:comment "Logo Image URIs"@en ;
      rdfs:domain ns:Image ;
      rdfs:label "logoImage"@en ;
      rdfs:range owl:Literal ;
      owl:subPropertyOf :topDataProperty .

ns:discNumber
      a       :FunctionalProperty , owl:DatatypeProperty ;
      rdfs:comment "Indicates the disc on which a media product component appears."@en ;
      rdfs:domain
              [ a       owl:Class ;
                :unionOf (ns:AlbumTrack ns:MediaProduct)
              ] ;
      rdfs:label "discNumber"@en ;
      rdfs:range owl:Literal ;
      owl:subPropertyOf :topDataProperty .

ns:lastUpdatedDate
      a       owl:DatatypeProperty ;
      rdfs:comment "Date this record was last updated"@en ;
      rdfs:domain
              [ a       owl:Class ;
                :unionOf (ns:EventVenue ns:LocalEvent)
              ] ;
      rdfs:label "lastUpdatedDate"@en ;
      rdfs:range xsd:date ;
      owl:subPropertyOf ns:date .

ns:unparsed
      a       owl:DatatypeProperty ;
      rdfs:comment "Created per Peter, 11/29/2010, to resolve shared entity issues."@en , "Captures unstructured data associated with a class."@en ;
      rdfs:domain ns:Entity ;
      rdfs:label "unparsed"@en ;
      rdfs:range owl:Literal .

ns:Hockey
      a       owl:Class ;
      rdfs:comment "Hockey refers to a family of sports in which two teams play against each other by trying to maneuver a ball, or a puck, into the opponent's goal, using a hockey stick."@en ;
      rdfs:label "Hockey"@en ;
      owl:subClassOf ns:Sport .

ns:autoTrim
      a       owl:ObjectProperty ;
      rdfs:comment "Connects an automobile's trim style to the individual automobile offered for sale."@en ;
      rdfs:domain ns:Automobile ;
      rdfs:label "autoTrim"@en ;
      rdfs:range ns:AutoTrim ;
      :inverseOf ns:autoTrimOf .

ns:businessListingType
      a       :FunctionalProperty , owl:DatatypeProperty ;
      rdfs:comment "specifies whether the listing is a featured/enhanced/free listing"@en ;
      rdfs:domain ns:LocalBusiness ;
      rdfs:label "paidListing"@en ;
      rdfs:range owl:Literal ;
      owl:subPropertyOf :topDataProperty .

ns:departmentOf
      a       :FunctionalProperty , owl:ObjectProperty ;
      rdfs:comment "departmentOf connects one local business to another local business and indicates that the one is a department of the other. It does not imply the same address.For example, a particular Safeway Pharmacy is a department of a particular Safeway."@en ;
      rdfs:domain ns:LocalBusiness ;
      rdfs:label "departmentOf"@en ;
      rdfs:range ns:LocalBusiness .

ns:SportDivision
      a       owl:Class ;
      rdfs:comment "A division in sports consists of a group of teams which compete against one another for a divisional title. It is often part of a league system, which is a set of divisions, in which teams can move between differently ranked divisions."@en ;
      rdfs:label "SportDivision"@en ;
      owl:subClassOf
              [ a       owl:Class ;
                :intersectionOf (ns:Group ns:SportCompetition)
              ] .

ns:rawPhone
      a       owl:DatatypeProperty ;
      rdfs:comment "Raw, unparsed telephone number data."@en ;
      rdfs:domain
              [ a       owl:Class ;
                :unionOf (ns:Phone ns:SingleLocationBusiness)
              ] ;
      rdfs:label "rawPhone"@en ;
      rdfs:range owl:Literal .

ns:warrantyOf
      a       owl:ObjectProperty ;
      rdfs:comment "Connects a purchased item to its warranty object."@en ;
      rdfs:domain
              [ a       owl:Class ;
                :unionOf (ns:AutoTrim ns:ConsumerProduct)
              ] ;
      rdfs:label "warrantyOf"@en ;
      rdfs:range ns:Warranty ;
      :inverseOf ns:warranty .

ns:episode
      a       owl:ObjectProperty ;
      rdfs:comment "connects an episode of a tv show to the program"@en ;
      rdfs:domain
              [ a       owl:Class ;
                :unionOf (ns:TvSeries ns:TvSpecial)
              ] ;
      rdfs:label "episode"@en ;
      rdfs:range ns:TvEpisode ;
      owl:subPropertyOf :topObjectProperty ;
      :inverseOf ns:episodeOf .

ns:alternateFamilyName
      a       :FunctionalProperty , owl:DatatypeProperty ;
      rdfs:comment "Alternate surnames by which an individual may be known."@en , "Note for Media V2 schema: Change to alternateFamilyName to support Trailblazers globalization guidelines: http://twiki.corp.yahoo.com/view/TrailBlazers/PersonalNames"@en ;
      rdfs:domain ns:AlternatePersonName ;
      rdfs:label "alternateFamilyName"@en ;
      rdfs:range owl:Literal ;
      owl:subPropertyOf ns:name .

ns:capId
      a       owl:DatatypeProperty ;
      rdfs:comment "ID of an entity from the contextual analysis platform."@en ;
      rdfs:domain ns:Entity ;
      rdfs:label "capId"@en ;
      rdfs:range owl:Literal ;
      owl:subPropertyOf ns:id .

ns:gender
      a       :FunctionalProperty , owl:DatatypeProperty ;
      rdfs:comment "Gender refers to the personal inner-sex identity of an individual, irrespective of his or her outer sex, which is determined by his/her/hir sexual organs."@en ;
      rdfs:domain
              [ a       owl:Class ;
                :unionOf (ns:Animal ns:Person ns:SportCompetition)
              ] ;
      rdfs:label "gender"@en ;
      rdfs:range owl:Literal .

ns:Neighborhood
      a       owl:Class ;
      rdfs:comment "A subdivision of a town such as a quarter, suburb, or neighborhood. Example: Chinatown (San Francisco.)"@en , "Placetype: 22"@en ;
      rdfs:label "Subdivision"@en ;
      owl:subClassOf ns:Place .

ns:accountName
      a       :FunctionalProperty , owl:DatatypeProperty ;
      rdfs:comment "Unique name applied to an online account."@en ;
      rdfs:domain ns:OnlineAccount ;
      rdfs:label "accountName"@en ;
      rdfs:range owl:Literal ;
      owl:subPropertyOf ns:name .

ns:yellow
      a       :FunctionalProperty , owl:DatatypeProperty ;
      rdfs:comment "yellow component of the color representation per CMYK color system "@en ;
      rdfs:domain ns:Color ;
      rdfs:label "yellow"@en ;
      rdfs:range owl:Literal ;
      owl:subPropertyOf ns:colorHolding .

<http://woo.corp.yahoo.com/ns/units/kg>
      a       owl:Datatype .

ns:LocalBusiness
      a       owl:Class ;
      rdfs:comment "Organizations that have a localized area of operation. Includes local business subtypes."@en ;
      rdfs:label "LocalBusiness"@en ;
      owl:subClassOf ns:Organization .

ns:abstract
      a       :FunctionalProperty , owl:DatatypeProperty ;
      rdfs:comment "Short description of a text document or webpage."@en ;
      rdfs:domain ns:Webpage ;
      rdfs:label "abstract"@en ;
      rdfs:range owl:Literal ;
      owl:subPropertyOf :topDataProperty .

ns:address
      a       owl:ObjectProperty ;
      rdfs:comment "Connects an entity to its physical address."@en ;
      rdfs:domain
              [ a       owl:Class ;
                :unionOf (ns:ContactInfo ns:Person ns:Structure)
              ] ;
      rdfs:label "address"@en ;
      rdfs:range ns:Address ;
      owl:subPropertyOf :topObjectProperty .

ns:composer
      a       owl:ObjectProperty ;
      rdfs:comment "Connects a composer to his or her composition."@en ;
      rdfs:domain ns:Composer ;
      rdfs:label "composer"@en ;
      rdfs:range
              [ a       owl:Class ;
                :unionOf (ns:Composition ns:Song)
              ] ;
      owl:subPropertyOf :topObjectProperty ;
      :inverseOf ns:composedBy .

ns:maxValue
      a       :FunctionalProperty , owl:DatatypeProperty ;
      rdfs:comment "Maximum value of a deal or offer."@en ;
      rdfs:domain ns:Deal ;
      rdfs:label "maxValue"@en ;
      rdfs:range xsd:float .

ns:dateTrimIntroduced
      a       :FunctionalProperty , owl:DatatypeProperty ;
      rdfs:comment "represents the date the trim was introduced. "@en ;
      rdfs:domain ns:AutoTrim ;
      rdfs:label "dateTrimIntroduced"@en ;
      rdfs:range xsd:dateTime ;
      owl:subPropertyOf ns:date .

ns:budget
      a       :FunctionalProperty , owl:DatatypeProperty ;
      rdfs:comment "How much it costs to make a film."@en ;
      rdfs:domain ns:Movie ;
      rdfs:label "budget"@en ;
      rdfs:range xsd:float .

ns:zipPlusFour
      a       :FunctionalProperty , owl:DatatypeProperty ;
      rdfs:comment "Zip code suffix applied for greater specificity."@en ;
      rdfs:domain
              [ a       owl:Class ;
                :unionOf (ns:Address ns:SingleLocationBusiness)
              ] ;
      rdfs:label "zipPlusFour"@en ;
      rdfs:range owl:Literal .

ns:BoxOfficeDaily
      a       owl:Class ;
      rdfs:comment "The box office income for a film in theatrical release over the period of one day."@en ;
      rdfs:label "BoxOfficeDaily"@en ;
      owl:subClassOf ns:BoxOffice .

ns:vertical
      a       owl:DatatypeProperty ;
      rdfs:comment "List of verticals that apply to a listing, along with their schema."@en ;
      rdfs:domain ns:LocalBusiness ;
      rdfs:label "vertical"@en ;
      rdfs:range owl:Literal ;
      owl:subPropertyOf :topDataProperty .

ns:priority
      a       :FunctionalProperty , owl:DatatypeProperty ;
      rdfs:comment "Priority is used for merging rules, and is constructed with provider paid info."@en ;
      rdfs:domain ns:LocalBusiness ;
      rdfs:label "priority"@en ;
      rdfs:range owl:Literal ;
      owl:subPropertyOf :topDataProperty .

ns:chainName
      a       :FunctionalProperty , owl:DatatypeProperty ;
      rdfs:comment "Name of the chain organization with which a local business is associated."@en ;
      rdfs:domain ns:LocalBusiness ;
      rdfs:label "chainName"@en ;
      rdfs:range owl:Literal .

ns:headAdminEmail
      a       :FunctionalProperty , owl:DatatypeProperty ;
      rdfs:comment "Email address of the adminitrative contact at an educational institution."@en ;
      rdfs:domain ns:EducationalInstitution ;
      rdfs:label "headAdminEmail"@en ;
      rdfs:range owl:Literal .

ns:contestant
      a       owl:ObjectProperty ;
      rdfs:comment "Connects a reality or game show contestant to the series or episodes he or she appeared on."@en ;
      rdfs:domain
              [ a       owl:Class ;
                :unionOf (ns:TvEpisode ns:TvSeason ns:TvSeries ns:TvSpecial)
              ] ;
      rdfs:label "contestant"@en ;
      rdfs:range ns:Contestant ;
      owl:subPropertyOf :topObjectProperty .

ns:Zone
      a       owl:Class ;
      rdfs:comment "These regions share a context, like an MSA or area code, but are not legally incorporated as a city or town would be, nor are they legal administrative divisions like counties or sovereign entitites like states. "@en , "Placetype: 25"@en ;
      rdfs:label "Zone"@en ;
      owl:subClassOf ns:Place .

ns:yahooMovieID
      a       owl:DatatypeProperty ;
      rdfs:comment "ID used for Yahoo Movies"@en ;
      rdfs:domain ns:Movie ;
      rdfs:label "yahooMovieID"@en ;
      rdfs:range owl:Literal ;
      owl:subPropertyOf ns:id .

ns:imageOf
      a       owl:ObjectProperty ;
      rdfs:comment "Connects an entity with its image."@en ;
      rdfs:domain ns:Image ;
      rdfs:label "imageOf"@en ;
      rdfs:range ns:Entity ;
      owl:subPropertyOf :topObjectProperty ;
      :inverseOf ns:image .

ns:bodyStyle
      a       owl:DatatypeProperty ;
      rdfs:comment "List of body styles the make supports e.g. sedan. This information is derived from model, trim details in the enrichment phase "@en ;
      rdfs:domain
              [ a       owl:Class ;
                :unionOf (ns:AutoMake ns:AutoTrim)
              ] ;
      rdfs:label "bodyStyle"@en ;
      rdfs:range owl:Literal .

ns:Airport
      a       owl:Class ;
      rdfs:comment "Placetype: 14"@en , "An Airport, example San Jose International."@en ;
      rdfs:label "Airport"@en ;
      owl:subClassOf ns:Structure .

ns:relationType
      a       :FunctionalProperty , owl:DatatypeProperty ;
      rdfs:comment "Describes the type of interpersonal connection between two individuals."@en ;
      rdfs:domain ns:PersonalRelationship ;
      rdfs:label "relationType"@en ;
      rdfs:range owl:Literal .

ns:Genre
      a       owl:Class ;
      rdfs:comment "The genre class enumerates a loose set of criteria by which media works are classified by theme."@en ;
      rdfs:label "Genre"@en ;
      owl:subClassOf ns:CategoryAndGenre .

ns:roomRate
      a       owl:DatatypeProperty ;
      rdfs:comment "Details the room rates at a local business offering lodging."@en ;
      rdfs:domain ns:Lodging ;
      rdfs:label "roomRate"@en ;
      rdfs:range owl:Literal .

ns:theaterId
      a       :FunctionalProperty , owl:DatatypeProperty ;
      rdfs:comment "Unique identifier assigned to a theater by Yahoo! Movies."@en ;
      rdfs:domain ns:MovieTheater ;
      rdfs:label "theaterId"@en ;
      rdfs:range owl:Literal ;
      owl:subPropertyOf ns:id .

ns:analystSpecialty
      a       owl:DatatypeProperty ;
      rdfs:comment "specialty represents the area of expertise of an analyst"@en ;
      rdfs:domain ns:Analyst ;
      rdfs:range owl:Literal .

ns:Analyst
      a       owl:Class ;
      rdfs:comment "Analyst represents those people who research and rate a company's finacial health."@en ;
      rdfs:label "Analyst"@en ;
      owl:subClassOf ns:FinancePerson .

ns:phoneNumberOf
      a       owl:ObjectProperty ;
      rdfs:comment "Connects a person or organization to a phone number."@en ;
      rdfs:domain ns:Phone ;
      rdfs:label "phoneNumberOf"@en ;
      rdfs:range
              [ a       owl:Class ;
                :unionOf (ns:ContactInfo ns:LocalEvent ns:Person)
              ] ;
      owl:subPropertyOf :topObjectProperty .

ns:westLongitude
      a       :FunctionalProperty , owl:DatatypeProperty ;
      rdfs:comment "West longitude of the bounding box of a place "@en ;
      rdfs:domain ns:Place ;
      rdfs:label "westLongitude"@en ;
      rdfs:range xsd:float .

ns:CompositionPart
      a       owl:Class ;
      rdfs:comment "A Part is a music asset that refers to individual parts (movements or sections) of a composition. "@en ;
      rdfs:label "CompositionPart"@en ;
      owl:subClassOf ns:Composition .

ns:worksFor
      a       owl:ObjectProperty ;
      rdfs:comment "worksFor connects a person to the org that employs them"@en ;
      rdfs:domain ns:Person ;
      rdfs:label "worksFor"@en ;
      rdfs:range ns:EmployeeAffiliation ;
      :inverseOf ns:employs .

ns:eventType
      a       owl:DatatypeProperty ;
      rdfs:comment "Designates an event's type. Types may include production, tour, festival, etc."@en ;
      rdfs:domain ns:LocalEvent ;
      rdfs:label "eventType"@en ;
      rdfs:range owl:Literal .

ns:Hybrid
      a       owl:Class ;
      rdfs:comment "Hybrid securities are a broad group of securities that combine the elements of the two broader groups of securities, debt and equity"@en ;
      rdfs:label "Hybrid"@en ;
      owl:subClassOf ns:Security .

ns:Author
      a       owl:Class ;
      rdfs:comment "The Author type is used for anyone who has written prose (whether fiction, essay, journalism, or scholarship), poetry, drama, or written or edited a book of any sort. This therefore includes editors of anthologies, whether or not the editor has written any material included in the anthology, and also includes artists in other media such as the fine arts and music, who may have had monographs or songbooks (for example) published. It also can include businesses and organizations when a written work is credited to one, rather than to a person."@en ;
      rdfs:label "Author"@en ;
      owl:subClassOf ns:Writer .

ns:historicTickerSymbol
      a       owl:DatatypeProperty ;
      rdfs:comment "historicTickerSymbol is for indicating what ticker symbol a current ticker entity was know as in the past"@en ;
      rdfs:domain
              [ a       owl:Class ;
                :unionOf (ns:Ticker ns:TradableQuotableInstrument)
              ] ;
      rdfs:label "historicTickerSymbol"@en ;
      rdfs:range owl:Literal ;
      owl:subPropertyOf :topDataProperty .

ns:CategoryMovieTV
      a       owl:Class ;
      rdfs:comment "Grouping of movies and television programs based on attributes that are not necessarily related to the subject matter of the film or TV program. These will map Yahoo!, Baseline, Netflixand Tribune categories."@en ;
      rdfs:label "CategoryMovieTV"@en ;
      owl:subClassOf ns:MediaCategory .

ns:imageLength
      a       :FunctionalProperty , owl:DatatypeProperty ;
      rdfs:comment "Length of image in pixels "@en ;
      rdfs:domain ns:Image ;
      rdfs:label "imageLength"@en ;
      rdfs:range xsd:int ;
      owl:subPropertyOf :topDataProperty .

ns:modelYear
      a       :FunctionalProperty , owl:DatatypeProperty ;
      rdfs:comment "Describes the year in which an automotive model was released."@en ;
      rdfs:domain
              [ a       owl:Class ;
                :unionOf (ns:AutoModel ns:AutoTrim)
              ] ;
      rdfs:label "modelYear"@en ;
      rdfs:range xsd:gYear ;
      owl:subPropertyOf ns:date .

ns:Sport
      a       owl:Class ;
      rdfs:comment "A sport is commonly defined as an organized, competitive, and skillful physical activity requiring commitment and fair play."@en ;
      rdfs:label "Sport"@en ;
      owl:subClassOf ns:Entity .

ns:Group
      a       owl:Class ;
      rdfs:comment "Represents a set of individuals."@en ;
      rdfs:label "Group"@en ;
      owl:subClassOf ns:Organization ;
      :hasKey (ns:member ns:groupName) .

ns:alternateMiddleName
      a       :FunctionalProperty , owl:DatatypeProperty ;
      rdfs:comment "Alternate middle names by which an individual may be known."@en ;
      rdfs:domain ns:AlternatePersonName ;
      rdfs:label "alternateMiddleName"@en ;
      rdfs:range owl:Literal ;
      owl:subPropertyOf ns:name .

ns:sourceId
      a       :FunctionalProperty , owl:DatatypeProperty ;
      rdfs:comment "Identification code of a review's source."@en ;
      rdfs:domain ns:Review ;
      rdfs:label "sourceId"@en ;
      rdfs:range owl:Literal .

ns:originalReleaseDate
      a       :FunctionalProperty , owl:DatatypeProperty ;
      rdfs:comment "should conform to ISO 8601 - Multiple formats acceptable: YYYY, YYYY-MM, YYYY-MM-DD"@en , "The date that a media work was originally made available for public use and consumption."@en ;
      rdfs:domain ns:MediaWork ;
      rdfs:label "originalReleaseDate"@en ;
      rdfs:range
              [ a       owl:Datatype ;
                :unionOf (xsd:date xsd:gYear xsd:gYearMonth)
              ] ;
      owl:subPropertyOf ns:date .

ns:gameRoomOnPremises
      a       :FunctionalProperty , owl:DatatypeProperty ;
      rdfs:comment "Game room on the premises of the movie theater."@en ;
      rdfs:domain ns:MovieTheater ;
      rdfs:label "gameRoomOnPremises"@en ;
      rdfs:range xsd:boolean .

ns:rightsLocality
      a       :FunctionalProperty , owl:DatatypeProperty ;
      rdfs:comment "The ISO code for locality or localities to which this right is applicable."@en ;
      rdfs:domain ns:DistributionRight ;
      rdfs:label "rightsLocality"@en ;
      rdfs:range owl:Literal ;
      owl:subPropertyOf :topDataProperty .

ns:alternateNameType
      a       :FunctionalProperty , owl:DatatypeProperty ;
      rdfs:comment "Describes the type of alternate name by which an individual is known."@en ;
      rdfs:domain ns:AlternatePersonName ;
      rdfs:label "alternateNameType"@en ;
      rdfs:range owl:Literal ;
      owl:subPropertyOf :topDataProperty .

ns:eventName
      a       :FunctionalProperty , owl:DatatypeProperty ;
      rdfs:comment "The name by which an event is known."@en ;
      rdfs:domain ns:LocalEvent ;
      rdfs:label "eventName"@en ;
      rdfs:range owl:Literal ;
      owl:subPropertyOf ns:name .

ns:appeared
      a       owl:ObjectProperty ;
      rdfs:comment "Connects a person to the reified appearance class."@en ;
      rdfs:domain ns:Person ;
      rdfs:label "appeared"@en ;
      rdfs:range ns:AppearanceRole ;
      owl:subPropertyOf :topObjectProperty .

ns:Debt
      a       owl:Class ;
      rdfs:comment "debt refers to assets owed"@en ;
      rdfs:label "Debt"@en ;
      owl:subClassOf ns:Security .

ns:makeMungedName
      a       :FunctionalProperty , owl:DatatypeProperty ;
      rdfs:comment "Munged name representation of Make as per http://twiki.corp.yahoo.com/view/Autos/GlobalMungedName"@en ;
      rdfs:domain ns:AutoMake ;
      rdfs:label "makeMungedName"@en ;
      rdfs:range owl:Literal ;
      owl:subPropertyOf ns:name .

ns:releaseRegion
      a       :FunctionalProperty , owl:DatatypeProperty ;
      rdfs:comment "Region in which a media release is active."@en ;
      rdfs:domain
              [ a       owl:Class ;
                :unionOf (ns:BoxOfficeAllTime ns:BoxOfficeDaily ns:BoxOfficeWeekend ns:BoxOfficeWeekly ns:MediaRelease)
              ] ;
      rdfs:label "releaseRegion"@en ;
      rdfs:range owl:Literal ;
      owl:subPropertyOf :topDataProperty .

ns:studentTeacherRatio
      a       owl:DatatypeProperty ;
      rdfs:comment "Indicates the ratio of students to teachers at an educational institution."@en ;
      rdfs:domain ns:EducationalInstitution ;
      rdfs:label "studentTeacherRatio"@en ;
      rdfs:range owl:Literal .

ns:menuItem
      a       owl:DatatypeProperty ;
      rdfs:comment "Food items, should be at the menu detail level "@en ;
      rdfs:domain ns:Restaurant ;
      rdfs:label "menuItem"@en ;
      rdfs:range owl:Literal ;
      owl:subPropertyOf :topDataProperty .

ns:OrgAffiliation
      a       owl:Class ;
      rdfs:comment "OrgAffiliation is a reified event subclass that expresses a relationship between a person and an organization or a relationship between organizations."@en ;
      rdfs:label "OrgAffiliation"@en ;
      owl:subClassOf ns:Event .

ns:trackPerformance
      a       owl:ObjectProperty ;
      rdfs:comment "Connects a musical performance to the album track it's on."@en ;
      rdfs:domain ns:AlbumTrack ;
      rdfs:label "trackPerformance"@en ;
      rdfs:range ns:MusicPerformance ;
      owl:subPropertyOf :topObjectProperty .

ns:city
      a       :FunctionalProperty , owl:DatatypeProperty ;
      rdfs:comment "City where a place is located."@en ;
      rdfs:domain
              [ a       owl:Class ;
                :unionOf (ns:Address ns:SingleLocationBusiness)
              ] ;
      rdfs:label "city"@en ;
      rdfs:range owl:Literal ;
      owl:subPropertyOf :topDataProperty .

ns:instantMessageId
      a       owl:DatatypeProperty ;
      rdfs:comment "Instant messaging address assigned to a person, organization, or thing."@en ;
      rdfs:domain
              [ a       owl:Class ;
                :unionOf (ns:ContactInfo ns:Person ns:SingleLocationBusiness)
              ] ;
      rdfs:label "instantMessageId"@en ;
      rdfs:range owl:Literal .

ns:competitionTeamIn
      a       owl:ObjectProperty ;
      rdfs:comment "Connects a sports competition to the teams involved."@en ;
      rdfs:domain ns:SportCompetitionInstance ;
      rdfs:label "competitionTeamIn"@en ;
      rdfs:range ns:SportTeam ;
      owl:subPropertyOf :topObjectProperty ;
      :inverseOf ns:competitionTeam .

ns:movieStudio
      a       owl:ObjectProperty ;
      rdfs:comment "Connects a film to the studio that made it."@en ;
      rdfs:domain
              [ a       owl:Class ;
                :unionOf (ns:MediaProduct ns:Movie ns:TvEpisode ns:TvSeason ns:TvSeries ns:TvSpecial)
              ] ;
      rdfs:label "movieStudio"@en ;
      rdfs:range ns:MovieStudio .

<http://woo.corp.yahoo.com/ns/units/km>
      a       owl:Datatype .

ns:nationality
      a       owl:DatatypeProperty ;
      rdfs:comment "The nation where an individual was born or holds citizenship."@en ;
      rdfs:domain ns:Person ;
      rdfs:label "nationality"@en ;
      rdfs:range owl:Literal .

ns:insuranceInformation
      a       :FunctionalProperty , owl:DatatypeProperty ;
      rdfs:comment "Information about insurance requirements."@en ;
      rdfs:domain ns:Warranty ;
      rdfs:label "insuranceInformation"@en ;
      rdfs:range owl:Literal .

ns:boxofficeLocation
      a       :FunctionalProperty , owl:ObjectProperty ;
      rdfs:comment "boxofficeLocation connects a film to the place where its box office receipts were generated."@en ;
      rdfs:domain
              [ a       owl:Class ;
                :unionOf (ns:BoxOfficeAllTime ns:BoxOfficeDaily ns:BoxOfficeWeekend ns:BoxOfficeWeekly)
              ] ;
      rdfs:label "boxofficeLocation"@en ;
      rdfs:range ns:Place ;
      owl:subPropertyOf ns:location .

ns:biographyOf
      a       :FunctionalProperty , owl:ObjectProperty ;
      rdfs:comment "Connects a biography with the person it describes."@en ;
      rdfs:domain ns:Biography ;
      rdfs:label "biographyOf"@en ;
      rdfs:range ns:Person .

xsd:duration
      a       owl:Datatype .

ns:makeYear
      a       owl:DatatypeProperty ;
      rdfs:comment "List of years the make has available models e.g. sedan. This information is derived from model, trim details in the enrichment phase "@en ;
      rdfs:domain ns:AutoMake ;
      rdfs:label "makeYear"@en ;
      rdfs:range xsd:gYear ;
      owl:subPropertyOf ns:date .

ns:capacity
      a       :FunctionalProperty , owl:DatatypeProperty ;
      rdfs:comment "The number of people a venue or other location can hold."@en ;
      rdfs:domain
              [ a       owl:Class ;
                :unionOf (ns:EventVenue ns:Structure)
              ] ;
      rdfs:label "capacity"@en ;
      rdfs:range owl:Literal ;
      owl:subPropertyOf :topDataProperty .

ns:rRule
      a       owl:Datatype ;
      rdfs:label "rRule"@en .

ns:approxEnd
      a       owl:DatatypeProperty ;
      rdfs:comment "Approximate end time for an event or event occurrence."@en ;
      rdfs:domain ns:LocalEventOccurrence ;
      rdfs:label "approxEnd"@en ;
      rdfs:range owl:Literal .

ns:date
      a       owl:DatatypeProperty ;
      rdfs:comment "holding property to organize data property hierarchy."@en ;
      rdfs:label "dates"@en .

ns:chefName
      a       :FunctionalProperty , owl:DatatypeProperty ;
      rdfs:comment "chefName is the name of the executive chef for a restaurant"@en ;
      rdfs:domain
              [ a       owl:Class ;
                :unionOf (ns:EventVenue ns:Restaurant)
              ] ;
      rdfs:label "chefName"@en ;
      rdfs:range owl:Literal ;
      owl:subPropertyOf ns:name .

ns:TvSeason
      a       owl:Class ;
      rdfs:comment "Season of a television series."@en ;
      rdfs:label "TvSeason"@en ;
      owl:subClassOf ns:Event .

ns:accountProfileUrl
      a       :FunctionalProperty , owl:DatatypeProperty ;
      rdfs:comment "Describes the URL used to access the profile associated with an online account."@en ;
      rdfs:domain ns:OnlineAccount ;
      rdfs:label "accountProfileUrl"@en ;
      rdfs:range xsd:anyURI ;
      owl:subPropertyOf :topDataProperty .

ns:belongsToWoeEntity
      a       :FunctionalProperty , owl:DatatypeProperty ;
      rdfs:comment "map of most specfic woeid to which a place can be assigned. For example, belongs_to_woeentity:{woeid:789,typecode:22} "@en ;
      rdfs:domain
              [ a       owl:Class ;
                :unionOf (ns:Address ns:Place ns:SingleLocationBusiness)
              ] ;
      rdfs:label "belongsToWoeEntity"@en ;
      rdfs:range owl:Literal .

ns:recordLabel
      a       owl:ObjectProperty ;
      rdfs:comment "The label property connects a music album with the record label that released the album."@en ;
      rdfs:domain ns:Album ;
      rdfs:label "label"@en ;
      rdfs:range ns:RecordLabel .

ns:connection
      a       owl:ObjectProperty ;
      rdfs:comment "connection relates the reified class OrgAffiliation to an organization"@en ;
      rdfs:domain ns:OrgAffiliation ;
      rdfs:label "connection"@en ;
      rdfs:range ns:Organization ;
      :inverseOf ns:connectionTo .

ns:indexMembership
      a       :FunctionalProperty , owl:DatatypeProperty ;
      rdfs:comment "indexmembership indicates which indexes a public company is traded on"@en ;
      rdfs:domain ns:PublicCompany ;
      rdfs:label "indexMembership"@en ;
      rdfs:range owl:Literal .

ns:email
      a       owl:DatatypeProperty ;
      rdfs:comment "Email address assigned to a person, organization, or thing."@en ;
      rdfs:domain
              [ a       owl:Class ;
                :unionOf (ns:ContactInfo ns:Person ns:SingleLocationBusiness)
              ] ;
      rdfs:label "email"@en ;
      rdfs:range owl:Literal ;
      owl:subPropertyOf :topDataProperty .

ns:married
      a       owl:ObjectProperty ;
      rdfs:comment "The married property connects a married person to the reified Marriage class."@en ;
      rdfs:domain ns:Person ;
      rdfs:label "married"@en ;
      rdfs:range ns:Marriage ;
      owl:subPropertyOf :topObjectProperty ;
      :inverseOf ns:marriedTo .

ns:screenQuantity
      a       :FunctionalProperty , owl:DatatypeProperty ;
      rdfs:comment "Describes the number of screens a theater has."@en ;
      rdfs:domain ns:MovieTheater ;
      rdfs:label "screenQuantity"@en ;
      rdfs:range xsd:int ;
      owl:subPropertyOf :topDataProperty .

ns:ambiance
      a       owl:DatatypeProperty ;
      rdfs:comment "Describes the atmosphere for a restaurant or other business. Examples: Casual, classy, upscale"@en ;
      rdfs:domain
              [ a       owl:Class ;
                :unionOf (ns:Bar ns:EventVenue ns:NightClub ns:Restaurant)
              ] ;
      rdfs:label "ambiance"@en ;
      rdfs:range owl:Literal .

ns:category
      a       owl:DatatypeProperty ;
      rdfs:comment "A thematic category in which a film can be classified."@en , "Category into which a product may be classified."@en ;
      rdfs:domain ns:Movie ;
      rdfs:domain
              [ a       owl:Class ;
                :unionOf (ns:ConsumerProduct ns:Deal ns:Organization ns:Topic)
              ] ;
      rdfs:label "category"@en ;
      rdfs:range owl:Literal ;
      owl:subPropertyOf :topDataProperty .

ns:boxScore
      a       :FunctionalProperty , owl:DatatypeProperty ;
      rdfs:comment "detailed game score info."@en ;
      rdfs:domain ns:SportGame ;
      rdfs:label "boxScore"@en ;
      rdfs:range owl:Literal ;
      owl:subPropertyOf :topDataProperty .

ns:Future
      a       owl:Class ;
      rdfs:comment "Future a standardized contract between two parties to buy or sell a specified asset (eg.oranges, oil, gold) of standardized quantity and quality at a specified future date at a price agreed today"@en ;
      rdfs:label "Future"@en ;
      owl:subClassOf ns:Derivative .

ns:canonicalURL
      a       :FunctionalProperty , owl:DatatypeProperty ;
      rdfs:comment " canonicalURL is the authorized or main URL. multiple normalized URLS may end up really redirecting to the same page (e.g. the canonical url)"@en ;
      rdfs:domain ns:Webpage ;
      rdfs:label "canonicalURL"@en ;
      rdfs:range xsd:anyURI .

ns:MusicPerformance
      a       owl:Class ;
      rdfs:comment "Indicates the musical manifestation a person or group has created of a particular media work (song, role, story)"@en ;
      rdfs:label "MusicPerformance"@en ;
      owl:subClassOf ns:Entity .

ns:playsFor
      a       owl:ObjectProperty ;
      rdfs:comment "Connects an athlete with a team affiliation."@en ;
      rdfs:domain ns:Athlete ;
      rdfs:label "playsFor"@en ;
      rdfs:range ns:TeamAffiliation .

ns:mailStop
      a       :FunctionalProperty , owl:DatatypeProperty ;
      rdfs:comment "A mail stop is a four-digit code that shows up after a ZIP code in a postal address. "@en ;
      rdfs:domain ns:Address ;
      rdfs:label "mailStop"@en ;
      rdfs:range owl:Literal ;
      owl:subPropertyOf :topDataProperty .

ns:sedol
      a       :FunctionalProperty , owl:DatatypeProperty ;
      rdfs:comment "sedol is a list of security identifiers used in the United Kingdom and Ireland for clearing purposes"@en ;
      rdfs:domain ns:TradableQuotableInstrument ;
      rdfs:label "sedol"@en ;
      rdfs:range owl:Literal .

ns:SportCompetition
      a       owl:Class ;
      rdfs:comment "A sports competition is a class that encompasses discrete competitions (such as the World Cup) as well as leagues (such as the NBA.) The time-limited instances of these competitions (such as World Cup 2010 or the Final Four) are delinated under SportsCompetitionInstance."@en ;
      rdfs:label "SportCompetition"@en ;
      owl:subClassOf ns:Entity .

ns:thxCertified
      a       :FunctionalProperty , owl:DatatypeProperty ;
      rdfs:comment "THX-certified theaters provide a high-quality, predictable playback environment to ensure that any film soundtrack mixed in THX will sound as near as possible to the intentions of the mixing engineer. "@en ;
      rdfs:domain ns:MovieTheater ;
      rdfs:label "thxCertified"@en ;
      rdfs:range xsd:boolean .

ns:celebrity
      a       :FunctionalProperty , owl:DatatypeProperty ;
      rdfs:comment "celebrity captures whether a person is in the media spotlight (OMG definition)"@en ;
      rdfs:domain ns:Person ;
      rdfs:label "celebrity"@en ;
      rdfs:range xsd:boolean .

ns:categoryPath
      a       owl:DatatypeProperty ;
      rdfs:comment "Category path string in Y! category tree. Cat ids are from top to leaf, delimited by / "@en ;
      rdfs:domain ns:BusinessListingCategory ;
      rdfs:label "categoryPath"@en ;
      rdfs:range owl:Literal ;
      owl:subPropertyOf :topDataProperty .

ns:averageRating
      a       owl:DatatypeProperty ;
      rdfs:comment "Average rating awarded to a film."@en ;
      rdfs:domain ns:RottenTomatoesReview ;
      rdfs:label "averageRating"@en ;
      rdfs:range owl:Literal ;
      owl:subPropertyOf :topDataProperty .

ns:event
      a       owl:ObjectProperty ;
      rdfs:comment "Connects an establishment to the events or performances occurring there."@en ;
      rdfs:domain ns:EventVenue ;
      rdfs:label "event"@en ;
      rdfs:range ns:LocalEventOccurrence .

ns:Exchange
      a       owl:Class ;
      rdfs:comment "Exchange represents an exchange on which things are bought and sold."@en ;
      rdfs:label "Exchange"@en ;
      owl:subClassOf ns:Organization .

ns:musician
      a       owl:ObjectProperty ;
      rdfs:comment "The musician property connects a musical sound recording with the MusicArtists that contribute to the recording."@en ;
      rdfs:domain
              [ a       owl:Class ;
                :unionOf (ns:Album ns:Composition ns:Song)
              ] ;
      rdfs:label "musician"@en ;
      rdfs:range
              [ a       owl:Class ;
                :unionOf (ns:MusicArtist ns:MusicGroup ns:Musician)
              ] ;
      :inverseOf ns:musicianIn .

ns:sitsOnBoard
      a       owl:ObjectProperty ;
      rdfs:comment "sitsOnBoard connects a board member to their board member affiliation"@en ;
      rdfs:domain ns:BoardMember ;
      rdfs:label "sitsOnBoard"@en ;
      rdfs:range ns:BoardMemberAffiliation .

ns:parentCategoryOf
      a       :TransitiveProperty , owl:ObjectProperty ;
      rdfs:comment "parentCategoryOf connects a parent category to a sub category in order to represent a hierarchy."@en ;
      rdfs:domain ns:Category ;
      rdfs:label "parentCategoryOf"@en ;
      rdfs:range ns:Category ;
      owl:subPropertyOf :topObjectProperty ;
      :inverseOf ns:subCategoryOf .

ns:instrumentPlayed
      a       owl:DatatypeProperty ;
      rdfs:comment "The instrument that a music artist plays in general or on a given sound recording."@en ;
      rdfs:domain ns:Musician ;
      rdfs:label "instrumentPlayed"@en ;
      rdfs:range owl:Literal ;
      owl:subPropertyOf :topDataProperty .

ns:subtitleLanguage
      a       owl:DatatypeProperty ;
      rdfs:comment "The languages in which subtitles are available for a video product. Should conform to BCP 47 format."@en ;
      rdfs:domain ns:Video ;
      rdfs:label "subtitleLanguage"@en ;
      rdfs:range owl:Literal ;
      owl:subPropertyOf :topDataProperty .

ns:printAtHomeTicketing
      a       :FunctionalProperty , owl:DatatypeProperty ;
      rdfs:comment "Indicates if the theater offers patron the option of print at home ticketing."@en ;
      rdfs:domain ns:MovieTheater ;
      rdfs:label "printAtHomeTicketing"@en ;
      rdfs:range xsd:boolean .

ns:namePrefix
      a       :FunctionalProperty , owl:DatatypeProperty ;
      rdfs:comment "A prefix appended to the beginning of a personal name."@en ;
      rdfs:domain ns:Person ;
      rdfs:label "namePrefix"@en ;
      rdfs:range owl:Literal ;
      owl:subPropertyOf ns:name .

ns:contactPersonFor
      a       owl:ObjectProperty ;
      rdfs:comment "Links a person with the organization for which they are the contact person."@en ;
      rdfs:domain ns:Person ;
      rdfs:label "contactPersonFor"@en ;
      rdfs:range ns:Organization ;
      owl:subPropertyOf :topObjectProperty ;
      :inverseOf ns:contactPerson .

ns:distanceUnit
      a       :FunctionalProperty , owl:DatatypeProperty ;
      rdfs:comment "Unit for distance, miles or KM, for instance"@en ;
      rdfs:domain ns:Warranty ;
      rdfs:label "distanceUnit"@en ;
      rdfs:range owl:Literal .

ns:ratingReason
      a       :FunctionalProperty , owl:DatatypeProperty ;
      rdfs:comment "Text detailing the reasons a film was awarded a particular rating."@en ;
      rdfs:domain ns:MovieRating ;
      rdfs:label "ratingReason"@en ;
      rdfs:range owl:Literal .

ns:Contest
      a       owl:Class ;
      rdfs:comment "Contests, giveaways, and sweepstakes. A contest involves two or more people competing to win a prize, while giveaways and sweepstakes are more randomly chosen."@en ;
      rdfs:label "Contest"@en ;
      owl:subClassOf ns:Event .

ns:musicianIn
      a       owl:ObjectProperty ;
      rdfs:comment "The musicianIn relation connects a MusicArtist to sound recordings that s/he has played on."@en ;
      rdfs:domain
              [ a       owl:Class ;
                :unionOf (ns:MusicArtist ns:MusicGroup ns:Musician)
              ] ;
      rdfs:label "musicianIn"@en ;
      rdfs:range
              [ a       owl:Class ;
                :unionOf (ns:Album ns:Composition ns:Song)
              ] .

ns:seoMerchantName
      a       owl:DatatypeProperty ;
      rdfs:comment "Name of the SEO company representing a deals merchant"@en ;
      rdfs:domain ns:DealMerchant ;
      rdfs:label "seoMerchantName"@en ;
      rdfs:range owl:Literal ;
      owl:subPropertyOf ns:name .

ns:cast
      a       owl:ObjectProperty ;
      rdfs:comment "The cast property connects a media artwork to the actors that appear in it."@en ;
      rdfs:domain
              [ a       owl:Class ;
                :unionOf (ns:Movie ns:TvEpisode ns:TvSeason ns:TvSeries ns:TvSpecial)
              ] ;
      rdfs:label "cast"@en ;
      rdfs:range ns:Actor .

ns:managedBy
      a       owl:ObjectProperty ;
      rdfs:comment "managedBy connects an exchange to the organization that manges it"@en ;
      rdfs:domain ns:Exchange ;
      rdfs:label "managedBy"@en ;
      rdfs:range ns:Company .

ns:brandedIDOF
      a       :FunctionalProperty , owl:ObjectProperty ;
      rdfs:comment "brandedIDOF connects a brand to its company, for example Gap to Gap Inc."@en ;
      rdfs:domain ns:Company ;
      rdfs:label "brandedIDOF"@en ;
      rdfs:range ns:Company ;
      owl:subPropertyOf :topObjectProperty ;
      :inverseOf ns:brandedID .

ns:countryLocation
      a       owl:ObjectProperty ;
      rdfs:comment "Connects a country class to an address or other entity that requires it."@en ;
      rdfs:domain
              [ a       owl:Class ;
                :unionOf (ns:Address ns:Place)
              ] ;
      rdfs:label "countryLocation" ;
      rdfs:range ns:Country ;
      owl:subPropertyOf ns:location .

ns:onlineSpecialURL
      a       owl:DatatypeProperty ;
      rdfs:comment "URL for online specials offered by a local business."@en ;
      rdfs:domain ns:LocalBusiness ;
      rdfs:label "onlineSpecialURL"@en ;
      rdfs:range xsd:anyURI .

ns:colorHolding
      a       owl:DatatypeProperty ;
      rdfs:comment "Holding area for color data properties."@en ;
      rdfs:label "colorHolding"@en .

ns:partnerWith
      a       :FunctionalProperty , owl:ObjectProperty ;
      rdfs:comment "The parteredWith relation connects the reified Domestic Union class with the individuals engaged in the partnership."@en ;
      rdfs:domain ns:DomesticUnion ;
      rdfs:label "partnerWith"@en ;
      rdfs:range ns:Person ;
      :inverseOf ns:partner .

ns:awardName
      a       :FunctionalProperty , owl:DatatypeProperty ;
      rdfs:comment "The name by which an award is known."@en ;
      rdfs:domain ns:AwardType ;
      rdfs:label "awardName"@en ;
      rdfs:range owl:Literal ;
      owl:subPropertyOf ns:name .

ns:synonym
      a       owl:DatatypeProperty ;
      rdfs:comment "Added for Local BusinessListingCategory. For local, it refers to the synonyms provided with the providerCategory data property."@en , "Array of strings having synonyms "@en ;
      rdfs:domain
              [ a       owl:Class ;
                :unionOf (ns:BusinessListingCategory ns:Organization)
              ] ;
      rdfs:label "synonym"@en ;
      rdfs:range owl:Literal ;
      owl:subPropertyOf :topDataProperty .

ns:exclusionDate
      a       owl:DatatypeProperty ;
      rdfs:comment "Excluded Date of Recurrence. An explicit Date or Dates, with optional Time, excluded from the Recurrence rule. For example, if a regular monthly meeting coincides with public holidays, these can be excluded from the recurrence set using <exDate> "@en ;
      rdfs:domain ns:Event ;
      rdfs:label "exclusionDate"@en ;
      rdfs:range owl:Literal .

ns:previousName
      a       owl:DatatypeProperty ;
      rdfs:comment "previousName is for any historical names of an entity"@en ;
      rdfs:domain
              [ a       owl:Class ;
                :unionOf (ns:Currency ns:MarketTier ns:Organization ns:SportCompetition)
              ] ;
      rdfs:label "previousName"@en ;
      rdfs:range owl:Literal ;
      owl:subPropertyOf ns:name .

ns:countryLocationOf
      a       :FunctionalProperty , owl:ObjectProperty ;
      rdfs:comment "Connects an address to the country it's in."@en ;
      rdfs:domain ns:Country ;
      rdfs:label "countryLocationOf"@en ;
      rdfs:range
              [ a       owl:Class ;
                :unionOf (ns:Address ns:Place)
              ] ;
      owl:subPropertyOf ns:location ;
      :inverseOf ns:countryLocation .

ns:registrationFor
      a       owl:ObjectProperty ;
      rdfs:comment "Connects the registration class to an event."@en ;
      rdfs:domain ns:EventRegistration ;
      rdfs:label "registrationFor"@en ;
      rdfs:range ns:LocalEventOccurrence ;
      :inverseOf ns:registration .

ns:aspectRatio
      a       :FunctionalProperty , owl:DatatypeProperty ;
      rdfs:comment "The aspect ratio of an image is the ratio of the width of the image to its height, expressed as two numbers separated by a colon."@en ;
      rdfs:domain ns:Movie ;
      rdfs:label "aspectRatio" ;
      rdfs:range owl:Literal .

ns:alternatePersonName
      a       :FunctionalProperty , owl:DatatypeProperty ;
      rdfs:comment "Alternate names by which an individual may be known."@en ;
      rdfs:domain ns:AlternatePersonName ;
      rdfs:label "alternatePersonName"@en ;
      rdfs:range owl:Literal ;
      owl:subPropertyOf ns:name .

ns:Automobile
      a       owl:Class ;
      rdfs:comment "An individual instance of a motor vehicle, includes cars and light trucks. Autos as a class are covered under AutoMake, AutoModel and AutoTrim."@en ;
      rdfs:label "Automobile"@en ;
      owl:subClassOf ns:ConsumerProduct .

ns:warrantyDistance
      a       :FunctionalProperty , owl:DatatypeProperty ;
      rdfs:comment "Distance for which warranty is valid "@en ;
      rdfs:label "warrantyDistance"@en .

ns:teamRosterOf
      a       owl:ObjectProperty ;
      rdfs:comment "An association of a team to the teamaffiliation class."@en ;
      rdfs:domain ns:TeamAffiliation ;
      rdfs:label "teamRosterOf"@en ;
      rdfs:range ns:SportTeam ;
      owl:subPropertyOf :topObjectProperty ;
      :inverseOf ns:teamRoster .

ns:affiliationType
      a       owl:DatatypeProperty ;
      rdfs:comment "affiliationType expresses the type of relationship that exists between a person and an org or the relationship between organizations. May include subsidiary, limited partnership, takeover, etc."@en ;
      rdfs:domain ns:OrgAffiliation ;
      rdfs:label "affiliationType"@en ;
      rdfs:range owl:Literal .

ns:featureSetName
      a       owl:DatatypeProperty ;
      rdfs:comment "Name of the feature set on an automobile's trim.  i.e. technical specifications."@en ;
      rdfs:domain ns:AutoTrim ;
      rdfs:label "featureSetName"@en ;
      rdfs:range owl:Literal .

ns:CompanyRole
      a       owl:Class ;
      rdfs:comment "The Company role is a reified class connecting an organization with media works to which it has contributed."@en ;
      rdfs:label "CompanyRole"@en ;
      owl:subClassOf ns:Entity .

ns:TeamAffiliation
      a       owl:Class ;
      rdfs:comment "Reified class connecting an athlete with a team, includes duration of affiliation."@en ;
      rdfs:label "TeamAffiliation"@en ;
      owl:subClassOf ns:Event .

ns:northLatitude
      a       :FunctionalProperty , owl:DatatypeProperty ;
      rdfs:comment "North latitude of the bounding box of the place "@en ;
      rdfs:domain ns:Place ;
      rdfs:label "northLatitude"@en ;
      rdfs:range xsd:float .

ns:Football
      a       owl:Class ;
      rdfs:comment "American football, known in the United States simply as football and sometimes as gridiron outside the United States and Canada, is a sport played between two teams of eleven. The objective of the game is to score points by advancing the ball into the opposing team's end zone."@en ;
      rdfs:label "Football"@en ;
      owl:subClassOf ns:Sport .

ns:trademark
      a       owl:DatatypeProperty ;
      rdfs:comment "trademark lists the brands of a business"@en ;
      rdfs:domain ns:Organization ;
      rdfs:label "trademark"@en ;
      rdfs:range owl:Literal .

ns:vin
      a       :FunctionalProperty , owl:DatatypeProperty ;
      rdfs:comment "Vehicle Identification Number, used as a unique identifier by dealers or manufacturers of used or new cars."@en ;
      rdfs:domain ns:Automobile ;
      rdfs:label "vin"@en ;
      rdfs:range owl:Literal .

ns:studied
      a       owl:ObjectProperty ;
      rdfs:comment "Connects an individual to the reified education class."@en ;
      rdfs:domain ns:Person ;
      rdfs:label "studied"@en ;
      rdfs:range ns:Education ;
      owl:subPropertyOf :topObjectProperty .

ns:Song
      a       owl:Class ;
      rdfs:comment "A musical composition which might be performed. A song is the work itself, i.e. Hallelujah, by Leonard Cohen. A performance is the actual musical manifestation, i.e. Hallelujah, by Jeff Buckley would be connected to the Song property Hallelujah written by Leonard Cohen."@en ;
      rdfs:label "Song"@en ;
      owl:subClassOf ns:MediaWork .

ns:regionServed
      a       owl:DatatypeProperty ;
      rdfs:comment "ID of the region served by an organization. This follows ISO 3166"@en ;
      rdfs:domain
              [ a       owl:Class ;
                :unionOf (ns:ContactInfo ns:LocalBusiness ns:SingleLocationBusiness)
              ] ;
      rdfs:label "regionServed"@en ;
      rdfs:range owl:Literal ;
      owl:subPropertyOf :topDataProperty .

ns:neighborhood
      a       owl:DatatypeProperty ;
      rdfs:comment "Neighborhood of an address or other location. Usually an array."@en ;
      rdfs:domain
              [ a       owl:Class ;
                :unionOf (ns:Address ns:Place ns:SingleLocationBusiness)
              ] ;
      rdfs:label "neighborhood"@en ;
      rdfs:range owl:Literal ;
      owl:subPropertyOf :topDataProperty .

ns:eventParticipant
      a       owl:ObjectProperty ;
      rdfs:comment "Connects a local event to individuals or groups who participate in or perform at the event."@en ;
      rdfs:domain ns:LocalEvent ;
      rdfs:label "eventParticipant"@en ;
      rdfs:range ns:Performer .

ns:productColor
      a       owl:ObjectProperty ;
      rdfs:comment "Connects the color class to a product."@en ;
      rdfs:domain
              [ a       owl:Class ;
                :unionOf (ns:AutoTrim ns:ConsumerProduct)
              ] ;
      rdfs:label "productColor"@en ;
      rdfs:range ns:Color .

ns:exchangeOwner
      a       :FunctionalProperty , owl:DatatypeProperty ;
      rdfs:comment "exchangeOwner is the entity that owns an exchange"@en ;
      rdfs:domain ns:Exchange ;
      rdfs:label "exchangeOwner"@en ;
      rdfs:range owl:Literal .

ns:associationType
      a       :FunctionalProperty , owl:DatatypeProperty ;
      rdfs:comment "The type of association between two objects."@en ;
      rdfs:domain ns:Association ;
      rdfs:label "associationType"@en ;
      rdfs:range owl:Literal .

ns:products
      a       owl:DatatypeProperty ;
      rdfs:comment "Products sold at a retail outlet."@en ;
      rdfs:domain ns:RetailShop ;
      rdfs:label "products"@en ;
      rdfs:range owl:Literal ;
      owl:subPropertyOf :topDataProperty .

ns:CompanyOfficerAffiliation
      a       owl:Class ;
      rdfs:comment "CompanyOfficerAffiliation connects a company officer to org they are an officer of"@en ;
      rdfs:label "CompanyOfficerAffiliation"@en ;
      owl:subClassOf ns:InsiderAffiliation .

ns:phoneExtension
      a       :FunctionalProperty , owl:DatatypeProperty ;
      rdfs:comment "Extension number for a phone number"@en ;
      rdfs:domain
              [ a       owl:Class ;
                :unionOf (ns:Phone ns:SingleLocationBusiness)
              ] ;
      rdfs:label "phoneExtension"@en ;
      rdfs:range owl:Literal ;
      owl:subPropertyOf :topDataProperty .

ns:ageRestriction
      a       :FunctionalProperty , owl:DatatypeProperty ;
      rdfs:comment "Indicates if a business imposes any age restrictions for access."@en ;
      rdfs:domain
              [ a       owl:Class ;
                :unionOf (ns:LocalBusiness ns:LocalEvent)
              ] ;
      rdfs:label "ageRestriction"@en ;
      rdfs:range xsd:boolean .

ns:Webpage
      a       owl:Class ;
      rdfs:comment "Describes the website associated with a person, organization, place, or thing."@en ;
      rdfs:label "Webpage"@en ;
      owl:subClassOf ns:Entity .

ns:position
      a       owl:DatatypeProperty ;
      rdfs:comment "Describes the position or positions played by an athlete on a team."@en ;
      rdfs:domain
              [ a       owl:Class ;
                :unionOf (ns:AthleteGameRole ns:TeamAffiliation)
              ] ;
      rdfs:label "position"@en ;
      rdfs:range owl:Literal .

ns:EventVenue
      a       owl:Class ;
      rdfs:comment "Venue where local events are hosted. May include stadiums, theaters, amphitheaters, city parks, and music halls."@en ;
      rdfs:label "EventVenue"@en ;
      owl:subClassOf ns:LocalBusiness .

ns:NetworkAffiliation
      a       owl:Class ;
      rdfs:comment "Describes the relationship between a TV program and a network."@en ;
      rdfs:label "NetworkAffiliation"@en ;
      owl:subClassOf ns:Event .

xsd:date
      a       owl:Datatype .

ns:mtListedOn
      a       owl:ObjectProperty ;
      rdfs:comment "mtListedOn connects a tradablequotable instrument to its market tier"@en ;
      rdfs:domain ns:TradableQuotableInstrument ;
      rdfs:label "mtListedOn"@en ;
      rdfs:range ns:MarketTier .

ns:BoardMemberAffiliation
      a       owl:Class ;
      rdfs:comment "BoardMemberAffiliation connects a board member to their affiliation with a company."@en ;
      rdfs:label "BoardMemberAffiliation"@en ;
      owl:subClassOf ns:InsiderAffiliation .

<http://woo.corp.yahoo.com/ns/currency:xxx>
      a       owl:Datatype ;
      rdfs:comment "Generic currency datatype that allows substitution of currency code for xxx"@en ;
      rdfs:label "currency:xxx"@en .

ns:fuelEconomyCityMax
      a       :FunctionalProperty , owl:DatatypeProperty ;
      rdfs:comment "Indicates the maximum fuel economy for this model for city driving. This information is derived from trim details in the enrichment phase "@en ;
      rdfs:domain ns:AutoModel ;
      rdfs:label "fuelEconomyCityMax"@en ;
      rdfs:range xsd:float .

<http://woo.corp.yahoo.com/ns/units/cm>
      a       owl:Datatype .

ns:woeType
      a       :FunctionalProperty , owl:DatatypeProperty ;
      rdfs:comment "woeType is for the type of place attached to a woe id"@en ;
      rdfs:domain ns:Place ;
      rdfs:label "woeType"@en ;
      rdfs:range owl:Literal .

ns:countryCallingCode
      a       :FunctionalProperty , owl:DatatypeProperty ;
      rdfs:comment "Country calling code for a phone number"@en ;
      rdfs:domain ns:Phone ;
      rdfs:label "countryCallingCode" ;
      rdfs:range xsd:int ;
      owl:subPropertyOf :topDataProperty .

ns:causeOfDeath
      a       :FunctionalProperty , owl:DatatypeProperty ;
      rdfs:comment "Reason for a person's death. Car accident, cancer, heart attack."@en ;
      rdfs:domain ns:Person ;
      rdfs:label "causeOfDeath"@en ;
      rdfs:range owl:Literal ;
      owl:subPropertyOf :topDataProperty .

ns:edition
      a       :FunctionalProperty , owl:DatatypeProperty ;
      rdfs:comment "Describes the edition of a media product."@en ;
      rdfs:domain
              [ a       owl:Class ;
                :unionOf (ns:MediaProduct ns:MediaWork)
              ] ;
      rdfs:label "edition"@en ;
      rdfs:range owl:Literal ;
      owl:subPropertyOf :topDataProperty .

ns:currency
      a       owl:ObjectProperty ;
      rdfs:comment "currency connects a class with the currency its values are expressed in"@en ;
      rdfs:domain
              [ a       owl:Class ;
                :unionOf (ns:Exchange ns:Salary)
              ] ;
      rdfs:label "currency"@en ;
      rdfs:range ns:Currency .

ns:suppressAddress
      a       :FunctionalProperty , owl:DatatypeProperty ;
      rdfs:comment "Indicates if an address should be displayed or suppressed."@en ;
      rdfs:domain ns:Address ;
      rdfs:label "suppressAddress"@en ;
      rdfs:range xsd:boolean .

ns:winner
      a       :FunctionalProperty , owl:ObjectProperty ;
      rdfs:comment "Connects the Nomination class to an individual, organization, or media work that has been nominated for and won an award."@en ;
      rdfs:label "winner"@en ;
      owl:subPropertyOf :topObjectProperty .

ns:actingPerformanceIn
      a       :FunctionalProperty , owl:ObjectProperty ;
      rdfs:comment "Connects an Actor to the reified Performance class."@en ;
      rdfs:domain ns:ActingRole ;
      rdfs:label "actingPerformanceIn"@en ;
      rdfs:range
              [ a       owl:Class ;
                :unionOf (ns:Movie ns:TvEpisode ns:TvSeason ns:TvSeries ns:TvSpecial)
              ] ;
      owl:subPropertyOf :topObjectProperty ;
      :inverseOf ns:actingPerformance .

ns:OrganizerName
      a       :FunctionalProperty , owl:DatatypeProperty ;
      rdfs:comment "Name by which an event organizer is known."@en ;
      rdfs:domain ns:EventOrganizer ;
      rdfs:label "OrganizerName"@en ;
      rdfs:range owl:Literal ;
      owl:subPropertyOf ns:name .

ns:gameStatus
      a       :FunctionalProperty , owl:DatatypeProperty ;
      rdfs:comment "Status of a sports game"@en ;
      rdfs:domain ns:SportGame ;
      rdfs:label "gameStatus"@en ;
      rdfs:range owl:Literal ;
      owl:subPropertyOf :topDataProperty .

ns:nameSuffix
      a       :FunctionalProperty , owl:DatatypeProperty ;
      rdfs:comment "An educational (e.g., Ph.D.), generational (e.g., Jr, Sr, III), or other name suffix used by a person. "@en ;
      rdfs:domain ns:Person ;
      rdfs:label "nameSuffix"@en ;
      rdfs:range owl:Literal ;
      owl:subPropertyOf ns:name .

ns:company
      a       owl:ObjectProperty ;
      rdfs:comment "Connects a company to a media work."@en ;
      rdfs:domain ns:Company ;
      rdfs:label "company"@en ;
      rdfs:range ns:MediaWork ;
      owl:subPropertyOf :topObjectProperty .

ns:trimDate
      a       :FunctionalProperty , owl:DatatypeProperty ;
      rdfs:comment "represents the date an auto trim was introduced. "@en ;
      rdfs:domain
              [ a       owl:Class ;
                :unionOf (ns:AutoTrim ns:Warranty)
              ] ;
      rdfs:label "trimDate"@en ;
      rdfs:range xsd:date ;
      owl:subPropertyOf ns:date .

ns:currencyCode
      a       :FunctionalProperty , owl:DatatypeProperty ;
      rdfs:comment "currencyCode represents the type of currency something is in,  currency ISO-4217 currency code"@en ;
      rdfs:domain
              [ a       owl:Class ;
                :unionOf (ns:AutoIncentive ns:AutoMake ns:AutoModel ns:AutoTrim ns:Automobile ns:Color ns:ConsumerProduct ns:Currency ns:Deal ns:EventRegistration ns:Exchange ns:Salary)
              ] ;
      rdfs:label "currencyCode"@en ;
      rdfs:range owl:Literal .

ns:middleName
      a       :FunctionalProperty , owl:DatatypeProperty ;
      rdfs:comment "A type of personal name, placed between the first given name and the surname."@en ;
      rdfs:domain ns:Person ;
      rdfs:label "middleName"@en ;
      rdfs:range owl:Literal ;
      owl:subPropertyOf ns:name .

ns:submitterId
      a       :FunctionalProperty , owl:DatatypeProperty ;
      rdfs:comment "Unique identifier of the individual who submitted a review."@en ;
      rdfs:domain ns:Review ;
      rdfs:label "submitterId"@en ;
      rdfs:range owl:Literal .

ns:copyright
      a       :FunctionalProperty , owl:DatatypeProperty ;
      rdfs:comment "Copyright for an original work."@en ;
      rdfs:domain
              [ a       owl:Class ;
                :unionOf (ns:Biography ns:Image ns:MediaProduct ns:MediaWork ns:Review ns:Synopsis)
              ] ;
      rdfs:label "copyright"@en ;
      rdfs:range owl:Literal ;
      owl:subPropertyOf :topDataProperty .

ns:partner
      a       owl:ObjectProperty ;
      rdfs:comment "The partner property connects a person to the reified Domestic Union class."@en ;
      rdfs:domain ns:Person ;
      rdfs:label "partner"@en ;
      rdfs:range ns:DomesticUnion ;
      owl:subPropertyOf :topObjectProperty .

ns:teamGender
      a       :FunctionalProperty , owl:DatatypeProperty ;
      rdfs:comment "Gender of people who make up a sports team. Could be men, women, mixed, boys."@en ;
      rdfs:domain
              [ a       owl:Class ;
                :unionOf (ns:SportCompetitionInstance ns:SportTeam)
              ] ;
      rdfs:label "teamGender"@en ;
      rdfs:range owl:Literal ;
      owl:subPropertyOf :topDataProperty .

ns:anchorText
      a       owl:DatatypeProperty ;
      rdfs:comment "Anchortext for a webpage."@en ;
      rdfs:domain ns:Webpage ;
      rdfs:label "anchorText" ;
      rdfs:range owl:Literal ;
      owl:subPropertyOf :topDataProperty .

ns:salary
      a       :FunctionalProperty , owl:DatatypeProperty ;
      rdfs:comment "salary is the amount of salary a person is given"@en ;
      rdfs:domain ns:Salary ;
      rdfs:label "salary"@en ;
      rdfs:range xsd:float ;
      owl:subPropertyOf :topDataProperty .

ns:chain
      a       owl:ObjectProperty ;
      rdfs:comment "Connects a local business to its chain parent."@en ;
      rdfs:domain ns:LocalBusiness ;
      rdfs:label "chain"@en ;
      rdfs:range ns:Company ;
      owl:subPropertyOf :topObjectProperty .

ns:deathLocation
      a       :FunctionalProperty , owl:ObjectProperty ;
      rdfs:comment "Connects an individual to the place in which s/he becomes deceased."@en ;
      rdfs:domain ns:Person ;
      rdfs:label "deathLocation"@en ;
      rdfs:range ns:Place ;
      owl:subPropertyOf ns:location .

ns:chainOutlet
      a       owl:ObjectProperty ;
      rdfs:comment "Connects a chain organization to its local business locations."@en ;
      rdfs:domain ns:Company ;
      rdfs:label "chainOutlet"@en ;
      rdfs:range ns:LocalBusiness ;
      owl:subPropertyOf :topObjectProperty .

ns:Company
      a       owl:Class ;
      rdfs:comment "A Company (or corporation) is a legal entity formed which has a separate legal identity from its members, and is ordinarily incorporated to undertake commercial business. "@en ;
      rdfs:label "Company"@en ;
      owl:subClassOf ns:Organization .

ns:thumbnail
      a       :FunctionalProperty , owl:DatatypeProperty ;
      rdfs:comment "Source information for thumbnail images."@en ;
      rdfs:domain ns:Image ;
      rdfs:label "thumbnail"@en ;
      rdfs:range xsd:anyURI ;
      owl:subPropertyOf :topDataProperty .

ns:Restaurant
      a       owl:Class ;
      rdfs:comment "A restaurant prepares and serves food, drink and dessert to customers. Meals are generally served and eaten on premises, but many restaurants also offer take-out and food delivery services."@en ;
      rdfs:label "Restaurant"@en ;
      owl:subClassOf ns:LocalBusiness .

ns:analystOf
      a       owl:ObjectProperty ;
      rdfs:comment "Connects the reified AnalystAffiliation class to a financial analyst."@en ;
      rdfs:domain ns:AnalystAffiliation ;
      rdfs:label "analystOf"@en ;
      rdfs:range ns:Analyst ;
      :inverseOf ns:analyst .

ns:sportsSurface
      a       :FunctionalProperty , owl:DatatypeProperty ;
      rdfs:comment "The playing surface of a sports venue. Asphalt, grass, astroturf, etc."@en ;
      rdfs:domain ns:SportVenue ;
      rdfs:label "sportsSurface"@en ;
      rdfs:range owl:Literal ;
      owl:subPropertyOf :topDataProperty .

ns:VisualArtist
      a       owl:Class ;
      rdfs:comment "Created by ace to support Milton mapping: http://twiki.corp.yahoo.com/view/P13nContextual/MiltonWooSchemaMap"@en , "An individual who creates visual art, including painting, drawing, sculpture."@en ;
      rdfs:label "VisualArtist"@en ;
      owl:subClassOf ns:Person .

ns:productTypeOf
      a       owl:ObjectProperty ;
      rdfs:comment "Connects a media work to its product type."@en ;
      rdfs:domain ns:MediaProduct ;
      rdfs:label "productTypeOf"@en ;
      rdfs:range ns:MediaWork ;
      owl:subPropertyOf :topObjectProperty ;
      :inverseOf ns:productType .

ns:quantityRemaining
      a       owl:DatatypeProperty ;
      rdfs:comment "Number of items left in a deal, offer, or coupon"@en ;
      rdfs:domain ns:Deal ;
      rdfs:label "quantityRemaining"@en ;
      rdfs:range owl:Literal .

ns:priceRange
      a       owl:DatatypeProperty ;
      rdfs:comment "Indicates the possible price range of registration for an event occurrence."@en ;
      rdfs:domain ns:LocalEventOccurrence ;
      rdfs:label "priceRange"@en ;
      rdfs:range owl:Literal .

ns:videoInfo
      a       owl:DatatypeProperty ;
      rdfs:comment "Manufacturer's information about a video media product."@en ;
      rdfs:domain ns:Video ;
      rdfs:label "videoInfo"@en ;
      rdfs:range owl:Literal ;
      owl:subPropertyOf :topDataProperty .

ns:addressHash
      a       :FunctionalProperty , owl:DatatypeProperty ;
      rdfs:comment "FindLocation hash. Unique identifier generated by FindLocation for an address."@en ;
      rdfs:domain
              [ a       owl:Class ;
                :unionOf (ns:Address ns:Place ns:SingleLocationBusiness)
              ] ;
      rdfs:label "addressHash"@en ;
      rdfs:range owl:Literal ;
      owl:subPropertyOf :topDataProperty .

ns:tvSeason
      a       owl:ObjectProperty ;
      rdfs:comment "Connects a television season to its tv program"@en ;
      rdfs:domain ns:TvSeason ;
      rdfs:label "tvSeason"@en ;
      rdfs:range ns:TvSeries ;
      owl:subPropertyOf :topObjectProperty ;
      :inverseOf ns:tvSeasonOf .

[]    a       :AllDisjointClasses ;
      :members (ns:Dating ns:DomesticUnion ns:Group ns:Marriage ns:Organization ns:Person) .

ns:boardMemberOf
      a       owl:ObjectProperty ;
      rdfs:comment "boardMemberOf connects a board member affiliation to a company"@en ;
      rdfs:domain ns:BoardMemberAffiliation ;
      rdfs:label "boardMemberOf"@en ;
      rdfs:range
              [ a       owl:Class ;
                :unionOf (ns:Company ns:Exchange)
              ] .

ns:tvNetwork
      a       owl:ObjectProperty ;
      rdfs:comment "Connects a network to a TV show"@en ;
      rdfs:domain ns:TvNetwork ;
      rdfs:label "tvNetwork"@en ;
      rdfs:range
              [ a       owl:Class ;
                :unionOf (ns:TvSeries ns:TvSpecial)
              ] ;
      owl:subPropertyOf :topObjectProperty ;
      :inverseOf ns:tvNetworkOf .

ns:crewFor
      a       :FunctionalProperty , owl:ObjectProperty ;
      rdfs:comment "Connects the reified CrewRole class to a movie or TV show."@en ;
      rdfs:domain ns:CrewRole ;
      rdfs:label "crewFor"@en ;
      rdfs:range
              [ a       owl:Class ;
                :unionOf (ns:Movie ns:TvEpisode ns:TvSeason ns:TvSeries ns:TvSpecial)
              ] ;
      owl:subPropertyOf :topObjectProperty ;
      :inverseOf ns:crew .

ns:StateAdminArea
      a       owl:Class ;
      rdfs:comment "placetype code: 8."@en , "Refers to federated states which participate in a federal union. Can also encompass Canadian Provinces. A primary administrative area within a country. Examples: California, Ontario"@en ;
      rdfs:label "StateAdminArea"@en ;
      owl:subClassOf ns:GeoPoliticalEntity .

ns:showingAt
      a       :FunctionalProperty , owl:ObjectProperty ;
      rdfs:comment "Connects the reified showtime class to a theater."@en ;
      rdfs:domain ns:MovieShowtime ;
      rdfs:label "showingAt"@en ;
      rdfs:range ns:MovieTheater ;
      owl:subPropertyOf :topObjectProperty ;
      :inverseOf ns:showing .

ns:isin
      a       :FunctionalProperty , owl:DatatypeProperty ;
      rdfs:comment "International Securities Identification Number (ISIN) that uniquely identifies a security."@en ;
      rdfs:domain ns:Security ;
      rdfs:label "isin"@en ;
      rdfs:range owl:Literal .

ns:startDate
      a       :FunctionalProperty , owl:DatatypeProperty ;
      rdfs:comment "The time at which an event with duration begins."@en ;
      rdfs:domain
              [ a       owl:Class ;
                :unionOf (ns:Event ns:Organization)
              ] ;
      rdfs:label "startDate"@en ;
      rdfs:range xsd:date ;
      owl:subPropertyOf ns:date .

ns:quote
      a       owl:DatatypeProperty ;
      rdfs:comment "a pithy snippet of text that can be attributed to a person or media work."@en ;
      rdfs:domain
              [ a       owl:Class ;
                :unionOf (ns:Book ns:Movie ns:Person ns:TvEpisode ns:TvSeries ns:TvSpecial)
              ] ;
      rdfs:label "quote"@en ;
      rdfs:range owl:Literal ;
      owl:subPropertyOf :topDataProperty .

ns:accountId
      a       :FunctionalProperty , owl:DatatypeProperty ;
      rdfs:comment "The unique identifier assigned to an online account."@en ;
      rdfs:domain ns:OnlineAccount ;
      rdfs:label "accountId"@en ;
      rdfs:range owl:Literal ;
      owl:subPropertyOf ns:id .

ns:phoneNumberType
      a       :FunctionalProperty , owl:DatatypeProperty ;
      rdfs:comment "Type of phone number. Could be mobile, landline, tollfree, fax, etc."@en ;
      rdfs:domain ns:Phone ;
      rdfs:label "phoneNumberType"@en ;
      rdfs:range owl:Literal ;
      rdfs:range
              [ a       owl:Datatype ;
                :oneOf  [ a       rdf:List ;
                          rdf:first "AFTER HOURS"^^xsd:string ;
                          rdf:rest
                                  [ a       rdf:List ;
                                    rdf:first "EMERGENCY"^^xsd:string ;
                                    rdf:rest
                                            [ a       rdf:List ;
                                              rdf:first "FAX"^^xsd:string ;
                                              rdf:rest
                                                      [ a       rdf:List ;
                                                        rdf:first "LANDLINE"^^xsd:string ;
                                                        rdf:rest
                                                                [ a       rdf:List ;
                                                                  rdf:first "MOBILE"^^xsd:string ;
                                                                  rdf:rest
                                                                          [ a       rdf:List ;
                                                                            rdf:first "PAGER"^^xsd:string ;
                                                                            rdf:rest
                                                                                    [ a       rdf:List ;
                                                                                      rdf:first "PAGER PIN"^^xsd:string ;
                                                                                      rdf:rest
                                                                                              [ a       rdf:List ;
                                                                                                rdf:first "TOLLFREE"^^xsd:string ;
                                                                                                rdf:rest
                                                                                                        [ a       rdf:List ;
                                                                                                          rdf:first "TRACKING"^^xsd:string ;
                                                                                                          rdf:rest ()
                                                                                                        ]
                                                                                              ]
                                                                                    ]
                                                                          ]
                                                                ]
                                                      ]
                                            ]
                                  ]
                        ]
              ] ;
      owl:subPropertyOf :topDataProperty .

ns:TreasuryNote
      a       owl:Class ;
      rdfs:comment "Treasury note A marketable U.S. government debt security with a fixed interest rate and a maturity between one and 10 years."@en ;
      rdfs:label "TreasuryNote"@en ;
      owl:subClassOf ns:Debt .

ns:applyOnlineURL
      a       owl:DatatypeProperty ;
      rdfs:comment "URL that allows users to apply online for services offered by a local business."@en ;
      rdfs:domain ns:LocalBusiness ;
      rdfs:label "applyOnlineURL"@en ;
      rdfs:range xsd:anyURI .

ns:wheelchairAccessible
      a       :FunctionalProperty , owl:DatatypeProperty ;
      rdfs:comment "Denotes whether structures like ramps or elevators in order to permit people in wheelchairs (and those using crutches, canes, walkers and so forth, or those with unsupported walking disabilities) exist in the building."@en ;
      rdfs:domain
              [ a       owl:Class ;
                :unionOf (ns:LocalBusiness ns:LocalEvent ns:MovieTheater)
              ] ;
      rdfs:label "wheelchairAccessible"@en ;
      rdfs:range xsd:boolean .

ns:rightsLocation
      a       owl:ObjectProperty ;
      rdfs:comment "Connects the distribution rights to the place they are valid."@en ;
      rdfs:domain
              [ a       owl:Class ;
                :unionOf (ns:DistributionRight ns:MusicRight)
              ] ;
      rdfs:label "rightsLocation"@en ;
      rdfs:range ns:Place ;
      owl:subPropertyOf ns:location .

ns:SportLeague
      a       owl:Class ;
      rdfs:comment "League is a term commonly used to describe a group of sports teams or individual athletes that compete against each other in a specific sport."@en ;
      rdfs:label "SportLeague"@en ;
      owl:subClassOf
              [ a       owl:Class ;
                :intersectionOf (ns:Group ns:SportCompetition)
              ] .

ns:businessAffiliate
      a       owl:DatatypeProperty ;
      rdfs:comment "Lists name(s) of business(es) affiliated with a Local Business."@en ;
      rdfs:domain ns:LocalBusiness ;
      rdfs:label "businessAffiliate"@en ;
      rdfs:range owl:Literal .

ns:agent
      a       owl:ObjectProperty ;
      rdfs:comment "The agent relation connects an individual in the entertainment industry (actor, director, musician, athlete, etc.) to the talent agent who represents him or her."@en ;
      rdfs:domain
              [ a       owl:Class ;
                :unionOf (ns:Actor ns:Athlete ns:Director ns:Host ns:Musician ns:Screenwriter)
              ] ;
      rdfs:label "agent"@en ;
      rdfs:range ns:Agent ;
      :inverseOf ns:agentOf .

ns:urlErrorCode
      a       :FunctionalProperty , owl:DatatypeProperty ;
      rdfs:comment "error code for the web page."@en ;
      rdfs:domain ns:Webpage ;
      rdfs:label "urlErrorCode"@en ;
      rdfs:range xsd:int ;
      owl:subPropertyOf :topDataProperty .

ns:Album
      a       owl:Class ;
      rdfs:comment "A music album or record album is a collection of related audio or music tracks distributed to the public."@en ;
      rdfs:label "Album"@en ;
      owl:subClassOf ns:MediaWork .

ns:roomNumber
      a       :FunctionalProperty , owl:DatatypeProperty ;
      rdfs:comment "Number of rooms in a hotel property."@en ;
      rdfs:domain ns:Lodging ;
      rdfs:label "roomNumber"@en ;
      rdfs:range owl:Literal ;
      owl:subPropertyOf :topDataProperty .

ns:accountHomepage
      a       :FunctionalProperty , owl:DatatypeProperty ;
      rdfs:comment "URL of an online account provider."@en ;
      rdfs:domain ns:OnlineAccount ;
      rdfs:label "accountHomepage"@en ;
      rdfs:range xsd:anyURI ;
      owl:subPropertyOf :topDataProperty .

ns:screeningAt
      a       owl:ObjectProperty ;
      rdfs:comment "Connects the reified film showtime class with a film. "@en ;
      rdfs:domain ns:MovieShowtime ;
      rdfs:label "screeningAt"@en ;
      rdfs:range ns:Movie ;
      owl:subPropertyOf :topObjectProperty ;
      :inverseOf ns:screening .

ns:TravelAgency
      a       owl:Class ;
      rdfs:comment "Travel agencies help vacationers and other travellers book their tickets cheaply and efficiently."@en ;
      rdfs:label "TravelAgency"@en ;
      owl:subClassOf ns:LocalBusiness .

ns:vehicleCategory
      a       :FunctionalProperty , owl:DatatypeProperty ;
      rdfs:comment "an automobile's market class. Example: sedan, van, exotic."@en ;
      rdfs:domain
              [ a       owl:Class ;
                :unionOf (ns:AutoModel ns:AutoTrim ns:Automobile)
              ] ;
      rdfs:label "vehicleCategory"@en ;
      rdfs:range owl:Literal .

ns:exchangeSymbol
      a       :FunctionalProperty , owl:DatatypeProperty ;
      rdfs:comment "ExchangeSymbol symbol by which a stock exchange is identified."@en ;
      rdfs:domain ns:Exchange ;
      rdfs:label "exchangeSymbol"@en ;
      rdfs:range owl:Literal .

ns:Club
      a       owl:Class ;
      rdfs:comment "A club is an association of two or more people united by a common interest or goal. Includes book clubs or other informal leisure groups as well as service clubs such as the Elks."@en ;
      rdfs:label "Club"@en ;
      owl:subClassOf ns:Group .

ns:Lodging
      a       owl:Class ;
      rdfs:comment "A hotel, inn, campground, or bed & breakfast .Lodging (or a holiday accommodation) is a type of residential accommodation. "@en ;
      rdfs:label "Lodging"@en ;
      owl:subClassOf ns:LocalBusiness .

ns:broadcastInstanceOf
      a       :FunctionalProperty , owl:ObjectProperty ;
      rdfs:comment "Connects a TVSpecial to the event or movie for which it is a televised broadcast."@en ;
      rdfs:domain ns:TvSpecial ;
      rdfs:label "broadcastInstanceOf"@en ;
      rdfs:range
              [ a       owl:Class ;
                :unionOf (ns:Movie ns:SportCompetition ns:SportCompetitionInstance ns:SportGame)
              ] ;
      :inverseOf ns:broadcastInstance .

ns:producedBy
      a       owl:ObjectProperty ;
      rdfs:comment "The producedBy property connects a media artwork to the individual who produced it."@en ;
      rdfs:domain
              [ a       owl:Class ;
                :unionOf (ns:Album ns:Movie ns:Song ns:TvEpisode ns:TvSeason ns:TvSeries ns:TvSpecial)
              ] ;
      rdfs:label "producedBy"@en ;
      rdfs:range ns:Producer .

ns:weight
      a       :FunctionalProperty , owl:DatatypeProperty ;
      rdfs:comment "The physical mass of an individual. May be expressed in kilograms or pounds."@en ;
      rdfs:domain
              [ a       owl:Class ;
                :unionOf (ns:ConsumerProduct ns:Person)
              ] ;
      rdfs:label "weight"@en ;
      rdfs:range xsd:float ;
      owl:subPropertyOf :topDataProperty .

ns:contribution
      a       owl:ObjectProperty ;
      rdfs:comment "The contribution property connects organizations involved in the production of a media work to the reified CompanyRole class."@en ;
      rdfs:domain ns:Movie ;
      rdfs:label "contribution"@en ;
      rdfs:range ns:CompanyRole ;
      owl:subPropertyOf :topObjectProperty .

ns:coachesFor
      a       owl:ObjectProperty ;
      rdfs:comment "Connects a person to the team or athlete for which s/he coaches."@en ;
      rdfs:domain ns:Coach ;
      rdfs:label "coachesFor"@en ;
      rdfs:range
              [ a       owl:Class ;
                :unionOf (ns:Athlete ns:SportTeam)
              ] ;
      :inverseOf ns:coachedBy .

ns:Movie
      a       owl:Class ;
      rdfs:comment "Movies include feature-length and short-subject theatrical, video, and television releases."@en ;
      rdfs:label "Movie"@en ;
      owl:subClassOf ns:MediaWork .

ns:businessCategoryAssignmentOf
      a       owl:ObjectProperty ;
      rdfs:comment "businessCategoryAssignmentOf connects BusinessListingCategory to LocalBusinessCategory"@en ;
      rdfs:domain ns:BusinessListingCategory ;
      rdfs:label "businessCategoryAssignmentOf"@en ;
      rdfs:range ns:LocalBusinessCategory .

ns:MajorShareholderAffiliation
      a       owl:Class ;
      rdfs:comment "MajorShareholder owns 10% or more of a company's stock"@en ;
      rdfs:label "MajorShareholderAffiliation"@en ;
      owl:subClassOf ns:InsiderAffiliation .

ns:autoTrimOf
      a       owl:ObjectProperty ;
      rdfs:comment "Connects an individual automobile to the trim style it is a member of."@en ;
      rdfs:domain ns:AutoTrim ;
      rdfs:label "autoTrimOf"@en ;
      rdfs:range ns:Automobile .

ns:Audio
      a       owl:Class ;
      rdfs:comment "Consumer products that play sound recordings."@en ;
      rdfs:label "Audio"@en ;
      owl:subClassOf ns:MediaProduct .

ns:findLocationQuality
      a       owl:DatatypeProperty ;
      rdfs:comment "Quality score that determines whether a location is pinpointed on the SERP map."@en ;
      rdfs:domain
              [ a       owl:Class ;
                :unionOf (ns:Address ns:Place ns:SingleLocationBusiness)
              ] ;
      rdfs:label "findLocationQuality"@en ;
      rdfs:range owl:Literal ;
      owl:subPropertyOf :topDataProperty .

ns:infoboxContent
      a       owl:DatatypeProperty ;
      rdfs:comment "Content from a wikipedia or other infobox source."@en ;
      rdfs:domain ns:Topic ;
      rdfs:label "infoboxContent"@en ;
      rdfs:range owl:Literal .

ns:showDateTime
      a       :FunctionalProperty , owl:DatatypeProperty ;
      rdfs:comment "The date and time on which a movie showing or establishment event occurs."@en ;
      rdfs:domain
              [ a       owl:Class ;
                :unionOf (ns:EstablishmentShowTime ns:MovieShowtime)
              ] ;
      rdfs:label "showDateTime"@en ;
      rdfs:range xsd:dateTime ;
      owl:subPropertyOf ns:date .

ns:pastryChefName
      a       :FunctionalProperty , owl:DatatypeProperty ;
      rdfs:comment "pastryChefName is the name of the head pastry chef for a restaurant"@en ;
      rdfs:domain ns:Restaurant ;
      rdfs:label "pastryChefName"@en ;
      rdfs:range owl:Literal ;
      owl:subPropertyOf ns:name .

ns:travelAgentType
      a       owl:DatatypeProperty ;
      rdfs:comment "Type of travel agent, i.e. Domestic, International."@en ;
      rdfs:domain ns:TravelAgency ;
      rdfs:label "travelAgentType"@en ;
      rdfs:range owl:Literal ;
      rdfs:range
              [ a       owl:Datatype ;
                :oneOf  [ a       rdf:List ;
                          rdf:first "DOMESTIC"^^xsd:string ;
                          rdf:rest
                                  [ a       rdf:List ;
                                    rdf:first "INTERNATIONAL"^^xsd:string ;
                                    rdf:rest ()
                                  ]
                        ]
              ] ;
      owl:subPropertyOf :topDataProperty .

ns:teamNickname
      a       owl:DatatypeProperty ;
      rdfs:comment "The team nickname, Celtics, Chargers, Ducks"@en ;
      rdfs:domain ns:SportTeam ;
      rdfs:label "teamNickname"@en ;
      rdfs:range owl:Literal ;
      owl:subPropertyOf ns:name .

ns:competitionAthleteIn
      a       owl:ObjectProperty ;
      rdfs:comment "Connects a competition instance to the athletes who participated in it."@en ;
      rdfs:domain ns:SportCompetitionInstance ;
      rdfs:label "competitionAthleteIn"@en ;
      rdfs:range ns:Athlete ;
      :inverseOf ns:competitionAthlete .

ns:serviceArea
      a       owl:ObjectProperty ;
      rdfs:comment "Connects an organization with the cities it serves."@en ;
      rdfs:domain ns:GeoPoliticalEntity ;
      rdfs:label "serviceArea"@en ;
      rdfs:range ns:Organization ;
      owl:subPropertyOf :topObjectProperty .

ns:numFloor
      a       :FunctionalProperty , owl:DatatypeProperty ;
      rdfs:comment "indicates the number of floors in a building"@en ;
      rdfs:domain ns:Lodging ;
      rdfs:label "numFloor"@en ;
      rdfs:range xsd:float .

ns:productColorOf
      a       owl:ObjectProperty ;
      rdfs:comment "Connects the color class to the products it modifies."@en ;
      rdfs:domain ns:Color ;
      rdfs:label "productColorOf"@en ;
      rdfs:range
              [ a       owl:Class ;
                :unionOf (ns:AutoTrim ns:ConsumerProduct)
              ] ;
      :inverseOf ns:productColor .

ns:alternateTitleOf
      a       :FunctionalProperty , owl:ObjectProperty ;
      rdfs:comment "Connects the reified Alternate Title class to a media work."@en ;
      rdfs:domain ns:AlternateTitle ;
      rdfs:label "alternateTitleOf"@en ;
      rdfs:range ns:MediaWork ;
      owl:subPropertyOf :topObjectProperty ;
      :inverseOf ns:alternateTitle .

ns:AwardType
      a       owl:Class ;
      rdfs:comment "An award or prize offered in recognition of achievement."@en ;
      rdfs:label "AwardType"@en ;
      owl:subClassOf ns:Entity .

ns:isMajorCurrency
      a       :FunctionalProperty , owl:DatatypeProperty ;
      rdfs:comment "isMajorCurrency indicates whether a currency is major"@en ;
      rdfs:domain ns:Currency ;
      rdfs:label "isMajorCurrency"@en ;
      rdfs:range xsd:boolean .

ns:credit
      a       owl:ObjectProperty ;
      rdfs:comment "The credit property connects individuals involved with the production of a media work to the reified Crew class."@en ;
      rdfs:domain
              [ a       owl:Class ;
                :unionOf (ns:Actor ns:Company ns:Crew)
              ] ;
      rdfs:label "credit"@en ;
      rdfs:range
              [ a       owl:Class ;
                :unionOf (ns:ActingRole ns:CompanyRole ns:CrewRole)
              ] .

ns:operatingHoursText
      a       :FunctionalProperty , owl:DatatypeProperty ;
      rdfs:comment "Example: Open Mon till Fri, 08:00 am to 5:00 pm "@en ;
      rdfs:domain
              [ a       owl:Class ;
                :unionOf (ns:ContactInfo ns:LocalBusiness ns:SingleLocationBusiness)
              ] ;
      rdfs:label "operatingHoursText"@en ;
      rdfs:range owl:Literal ;
      owl:subPropertyOf :topDataProperty .

ns:sportSchedulePeriod
      a       owl:ObjectProperty ;
      rdfs:comment "Connects a game or competition instance to its sport schedule period."@en ;
      rdfs:domain
              [ a       owl:Class ;
                :unionOf (ns:SportCompetitionInstance ns:SportGame)
              ] ;
      rdfs:label "sportSchedulePeriod"@en ;
      rdfs:range ns:SportSchedulePeriod .

ns:nominee
      a       :FunctionalProperty , owl:ObjectProperty ;
      rdfs:comment "Connects the Nomination class to an individual, organization, or media work that has been nominated for an award."@en ;
      rdfs:domain ns:Nomination ;
      rdfs:label "nominee"@en ;
      rdfs:range
              [ a       owl:Class ;
                :unionOf (ns:MediaWork ns:Organization ns:Person)
              ] ;
      owl:subPropertyOf :topObjectProperty ;
      :inverseOf ns:nominated .

ns:Review
      a       owl:Class ;
      rdfs:comment "A review is any article or blurb that passes judgement on a business, performance, or other place or thing. It may be community-generated or part of a copyrighted work."@en ;
      rdfs:label "Review"@en ;
      owl:subClassOf ns:Entity .

ns:categoryBranch
      a       owl:DatatypeProperty ;
      rdfs:comment "This is a more structured representation of Cat_Path, including the current cat node."@en ;
      rdfs:domain ns:BusinessListingCategory ;
      rdfs:label "categoryBranch"@en ;
      rdfs:range owl:Literal ;
      owl:subPropertyOf :topDataProperty .

ns:sourceURL
      a       :FunctionalProperty , owl:DatatypeProperty ;
      rdfs:comment "Source URL for web-based content."@en ;
      rdfs:domain ns:Review ;
      rdfs:label "sourceURL"@en ;
      rdfs:range xsd:anyURI ;
      owl:subPropertyOf :topDataProperty .

ns:colorAvailability
      a       owl:DatatypeProperty ;
      rdfs:comment "Represents the availability of the color. Is it available standard with vehicle/ as option / as part of package. Possible values: built, option, pack, standard "@en ;
      rdfs:domain ns:Color ;
      rdfs:label "colorAvailability"@en ;
      rdfs:range owl:Literal ;
      owl:subPropertyOf ns:colorHolding .

ns:friend
      a       owl:ObjectProperty ;
      rdfs:comment "Connects an individual to the reified Friendship class."@en ;
      rdfs:domain ns:Person ;
      rdfs:label "friend"@en ;
      rdfs:range ns:Friendship ;
      owl:subPropertyOf :topObjectProperty .

ns:appearanceType
      a       owl:DatatypeProperty ;
      rdfs:comment "The type of appearance a person has made on a tv show."@en ;
      rdfs:domain ns:AppearanceRole ;
      rdfs:label "appearanceType"@en ;
      rdfs:range owl:Literal ;
      owl:subPropertyOf :topDataProperty .

ns:compositionPartOf
      a       :FunctionalProperty , owl:ObjectProperty ;
      rdfs:comment "ties a composition to its parts"@en ;
      rdfs:domain ns:CompositionPart ;
      rdfs:label "compositionPartOf"@en ;
      rdfs:range ns:Composition ;
      owl:subPropertyOf :topObjectProperty ;
      :inverseOf ns:compositionPart .

ns:ticketEndDate
      a       owl:DatatypeProperty ;
      rdfs:comment "Indicates the final date on which tickets may be purchased for an event."@en ;
      rdfs:domain
              [ a       owl:Class ;
                :unionOf (ns:EventRegistration ns:LocalEventOccurrence)
              ] ;
      rdfs:label "ticketEndDate"@en ;
      rdfs:range owl:Literal .

ns:phoneNumberBody
      a       :FunctionalProperty , owl:DatatypeProperty ;
      rdfs:comment "In a US phone number, this is the last 4 numbers of a phone number following the prefix."@en ;
      rdfs:domain ns:Phone ;
      rdfs:label "phoneNumberBody"@en ;
      rdfs:range xsd:int ;
      owl:subPropertyOf :topDataProperty .

ns:ratingLocation
      a       :FunctionalProperty , owl:ObjectProperty ;
      rdfs:comment "Location where a film rating system is in use. Should conform to ISO codes."@en ;
      rdfs:domain ns:MovieRating ;
      rdfs:label "ratingLocation"@en ;
      rdfs:range ns:Place ;
      owl:subPropertyOf ns:location .

ns:baseModelMungedName
      a       :FunctionalProperty , owl:DatatypeProperty ;
      rdfs:comment "Munged name representation of the base model (model without years) to which this model is part of "@en ;
      rdfs:domain ns:AutoModel ;
      rdfs:label "baseModelMungedName"@en ;
      rdfs:range owl:Literal ;
      owl:subPropertyOf ns:name .

ns:productTitleStripped
      a       :FunctionalProperty , owl:DatatypeProperty ;
      rdfs:comment "Media product title stripped of the leading article, to facilitate proper alphabetical sorting."@en ;
      rdfs:domain ns:MediaProduct ;
      rdfs:label "productTitleStripped"@en ;
      rdfs:range owl:Literal ;
      owl:subPropertyOf ns:label .

ns:crossStreet
      a       owl:DatatypeProperty ;
      rdfs:comment "Used to pinpoint a map or address location."@en ;
      rdfs:domain
              [ a       owl:Class ;
                :unionOf (ns:Address ns:SingleLocationBusiness)
              ] ;
      rdfs:label "crossStreet"@en ;
      rdfs:range owl:Literal ;
      owl:subPropertyOf :topDataProperty .

ns:featureValue
      a       owl:DatatypeProperty ;
      rdfs:comment "Represents the string value of an auto trim feature.. It is currently assumed that name is associated with a single string value. If multiple values are associated with the name, they would have to be combined into a single string value "@en ;
      rdfs:domain ns:AutoTrim ;
      rdfs:label "featureValue"@en ;
      rdfs:range owl:Literal .

ns:subCategoryOf
      a       :TransitiveProperty , owl:ObjectProperty ;
      rdfs:comment "subCategoryOf connects a sub category to a parent category in order to represent hierarchy."@en ;
      rdfs:domain ns:Category ;
      rdfs:label "subCategoryOf"@en ;
      rdfs:range ns:Category ;
      owl:subPropertyOf :topObjectProperty .

ns:historicJobPosition
      a       owl:DatatypeProperty ;
      rdfs:comment "historicJobPosition is a list of the past positions a person has held"@en ;
      rdfs:domain ns:Person ;
      rdfs:label "historicJobPosition"@en ;
      rdfs:range owl:Literal .

ns:streetAddress
      a       :FunctionalProperty , owl:DatatypeProperty ;
      rdfs:comment "The first line of a street address. Also known as Addr1."@en ;
      rdfs:domain
              [ a       owl:Class ;
                :unionOf (ns:Address ns:SingleLocationBusiness)
              ] ;
      rdfs:label "streetAddress"@en ;
      rdfs:range owl:Literal ;
      owl:subPropertyOf :topDataProperty .

ns:Structure
      a       owl:Class ;
      rdfs:comment "A man-made building or other structure."@en ;
      rdfs:label "Structure"@en ;
      owl:subClassOf ns:Place .

ns:usedCarPriceMin
      a       :FunctionalProperty , owl:DatatypeProperty ;
      rdfs:comment "Applicable only if newModel=false. Indicates the minimum used car price (e.g. kbb price) for this model. This information is derived from trim details in the enrichment phase "@en ;
      rdfs:domain ns:AutoModel ;
      rdfs:label "usedCarPriceMin"@en ;
      rdfs:range xsd:double .

ns:Phone
      a       owl:Class ;
      rdfs:comment "Describes the data associated with a phone listing."@en ;
      rdfs:label "Phone"@en ;
      owl:subClassOf ns:Entity .

ns:contactNameFirst
      a       :FunctionalProperty , owl:DatatypeProperty ;
      rdfs:comment "First name of the contact person for a local business (for use with SingleLocationBusiness only)."@en ;
      rdfs:domain ns:SingleLocationBusiness ;
      rdfs:label "contactNameFirst"@en ;
      rdfs:range owl:Literal .

ns:vestingSchedule
      a       :FunctionalProperty , owl:DatatypeProperty ;
      rdfs:comment "vesting schedule for equities used for compensation"@en ;
      rdfs:domain ns:Equity ;
      rdfs:label "vestingSchedule"@en ;
      rdfs:range owl:Literal ;
      owl:subPropertyOf :topDataProperty .

ns:Musician
      a       owl:Class ;
      rdfs:comment "A musician is an individual who plays music or contributes to a music album, composition, or track."@en ;
      rdfs:label "Musician"@en ;
      owl:subClassOf
              [ a       owl:Class ;
                :intersectionOf (ns:MusicArtist ns:Person)
              ] .

ns:distributionId
      a       owl:DatatypeProperty ;
      rdfs:comment "example: OPISNet-268694 "@en , "ID for a deal distributor"@en ;
      rdfs:domain ns:Deal ;
      rdfs:label "distributionId"@en ;
      rdfs:range owl:Literal ;
      owl:subPropertyOf ns:id .

ns:analysedBy
      a       owl:ObjectProperty ;
      rdfs:comment "analysedBy connects the org to the analyst"@en ;
      rdfs:domain ns:Company ;
      rdfs:label "analysedBy"@en ;
      rdfs:range ns:AnalystAffiliation .

ns:TimeZone
      a       owl:Class ;
      rdfs:comment "An area defined by the Olson standard TZ database. "@en , "Placetype: 31"@en ;
      rdfs:label "TimeZone"@en ;
      owl:subClassOf ns:Place .

ns:smokingAllowed
      a       :FunctionalProperty , owl:DatatypeProperty ;
      rdfs:comment "Indicates if smoking is allowed at a local business."@en ;
      rdfs:domain
              [ a       owl:Class ;
                :unionOf (ns:LocalBusiness ns:LocalEvent)
              ] ;
      rdfs:label "smokingAllowed"@en ;
      rdfs:range xsd:boolean .

ns:createdOn
      a       :FunctionalProperty , owl:DatatypeProperty ;
      rdfs:comment "Local listing source data indicating creation date of the record (for use with SingleLocationBusiness only)."@en ;
      rdfs:domain ns:SingleLocationBusiness ;
      rdfs:label "createdOn"@en ;
      rdfs:range owl:Literal .

ns:undecidedCount
      a       :FunctionalProperty , owl:DatatypeProperty ;
      rdfs:comment "Number of reviews for a given film that are undecided as positive or negative, calculated by Rotten Tomatoes."@en ;
      rdfs:domain ns:RottenTomatoesReview ;
      rdfs:label "undecidedCount"@en ;
      rdfs:range owl:Literal ;
      owl:subPropertyOf :topDataProperty .

ns:altText
      a       :FunctionalProperty , owl:DatatypeProperty ;
      rdfs:comment "Text used in image alt attribute "@en ;
      rdfs:domain ns:Image ;
      rdfs:label "altText"@en ;
      rdfs:range owl:Literal ;
      owl:subPropertyOf :topDataProperty .

ns:MediaWork
      a       owl:Class ;
      rdfs:comment "The media work superclass describes artwork created using various formats, including film, television, sound recording, and the written word."@en ;
      rdfs:label "MediaWork"@en ;
      owl:subClassOf ns:Entity .

ns:equityStreetPrice
      a       :FunctionalProperty , owl:DatatypeProperty ;
      rdfs:comment "street price of an equity"@en ;
      rdfs:domain ns:Equity ;
      rdfs:label "equityStreetPrice"@en ;
      rdfs:range xsd:float .

ns:minReservationSize
      a       owl:DatatypeProperty ;
      rdfs:comment "Indicates the minimum number of people for which a reservation may be made at a local business."@en ;
      rdfs:domain ns:Restaurant ;
      rdfs:label "minReservationSize"@en ;
      rdfs:range xsd:int .

ns:athleteGameIn
      a       :FunctionalProperty , owl:ObjectProperty ;
      rdfs:comment "Connects the athlete role class to the game played in."@en ;
      rdfs:domain ns:AthleteGameRole ;
      rdfs:label "athleteGameIn"@en ;
      rdfs:range ns:SportGame ;
      :inverseOf ns:athleteGame .

ns:CountyAdminArea
      a       owl:Class ;
      rdfs:comment "A county is a local level of government below the state (or federal territory). A secondary administrative area within a country. example: Santa Clara County."@en , "placetype code: 9"@en ;
      rdfs:label "CountyAdminArea"@en ;
      owl:subClassOf ns:GeoPoliticalEntity .

ns:seatingChart
      a       owl:DatatypeProperty ;
      rdfs:comment "Image file or URL at which the seating chart for a local business may be accessed."@en ;
      rdfs:domain
              [ a       owl:Class ;
                :unionOf (ns:Bar ns:EventVenue ns:NightClub)
              ] ;
      rdfs:label "seatingChart"@en ;
      rdfs:range owl:Literal .

ns:CriticalReview
      a       owl:Class ;
      rdfs:comment "A review is an evaluation of a media work; an event or performance; or a consumer product."@en ;
      rdfs:label "CriticalReview"@en ;
      owl:subClassOf ns:Review .

ns:ratingValue
      a       :FunctionalProperty , owl:DatatypeProperty ;
      rdfs:comment "Consumer or product rating value on a scale of 1-10"@en ;
      rdfs:domain ns:Review ;
      rdfs:label "ratingValue"@en ;
      rdfs:range xsd:int ;
      owl:subPropertyOf :topDataProperty .

ns:movieContributorFor
      a       owl:ObjectProperty ;
      rdfs:comment "Connects people who contribute to the making of a movie to the movie, including those whose contribution is unclear."@en ;
      rdfs:domain ns:Person ;
      rdfs:label "movieContributorFor"@en ;
      rdfs:range ns:Movie ;
      owl:subPropertyOf :topObjectProperty .

ns:releaseNumber
      a       :FunctionalProperty , owl:DatatypeProperty ;
      rdfs:comment "Unique identifier assigned to a given film release."@en ;
      rdfs:domain ns:BoxOfficeWeekend ;
      rdfs:label "releaseNumber"@en ;
      rdfs:range owl:Literal ;
      owl:subPropertyOf :topDataProperty .

ns:filmingLocation
      a       owl:ObjectProperty ;
      rdfs:comment "filmingLocation connects a film or television series to the place where it is shot."@en ;
      rdfs:domain
              [ a       owl:Class ;
                :unionOf (ns:Movie ns:TvEpisode ns:TvSeason ns:TvSeries ns:TvSpecial)
              ] ;
      rdfs:label "filmingLocation"@en ;
      rdfs:range
              [ a       owl:Class ;
                :unionOf (ns:Address ns:Place)
              ] ;
      owl:subPropertyOf ns:location .

ns:RottenTomatoesReview
      a       owl:Class ;
      rdfs:comment "Aggregated critical review for a film as provided by the Rotten Tomatoes website."@en ;
      rdfs:label "RottenTomatoesReview"@en ;
      owl:subClassOf ns:CriticalReview .

ns:recordedBy
      a       owl:ObjectProperty ;
      rdfs:comment "The recordedBy property connects an album to the music artist that recorded it."@en ;
      rdfs:domain
              [ a       owl:Class ;
                :unionOf (ns:Album ns:Song)
              ] ;
      rdfs:label "recordedBy"@en ;
      rdfs:range ns:MusicArtist ;
      :inverseOf ns:recorded .

ns:agentOf
      a       owl:ObjectProperty ;
      rdfs:comment "The agentOf property connects a talent agent to the individuals s/he represents."@en ;
      rdfs:domain ns:Agent ;
      rdfs:label "agentOf"@en ;
      rdfs:range
              [ a       owl:Class ;
                :unionOf (ns:Actor ns:Athlete ns:Director ns:Host ns:Musician ns:Screenwriter)
              ] .

ns:yctCategory
      a       owl:DatatypeProperty ;
      rdfs:comment "Category to which an entity can be assigned in the Yahoo Content Taxonomy."@en ;
      rdfs:domain ns:Entity ;
      rdfs:label "yctCategory"@en ;
      rdfs:range owl:Literal .

ns:Performer
      a       owl:Class ;
      rdfs:comment "An individual or group that participates in a Local Event. May include musicians, bands, musical groups, comedians, panel participants, or featured speakers."@en ;
      rdfs:label "Performer"@en ;
      owl:subClassOf ns:Entity .

ns:YearsActive
      a       owl:Class ;
      rdfs:comment "Captures the years a person or organization was active in a particular field."@en ;
      rdfs:label "YearsActive"@en ;
      owl:subClassOf ns:Event .

ns:seatingType
      a       owl:DatatypeProperty ;
      rdfs:comment "Describes the type of seating available at a venue."@en ;
      rdfs:domain ns:MovieTheater ;
      rdfs:label "seatingType"@en ;
      rdfs:range owl:Literal ;
      owl:subPropertyOf :topDataProperty .

ns:specialOfferURL
      a       owl:DatatypeProperty ;
      rdfs:comment "URL at which special offers from a local business may be accessed."@en ;
      rdfs:domain ns:LocalBusiness ;
      rdfs:label "specialOfferURL"@en ;
      rdfs:range owl:Literal .

ns:productService
      a       owl:DatatypeProperty ;
      rdfs:comment "Product services offered at a venue or business, e.g. Wedding Ceremony, Wedding Reception, Proms, Business Meetings, Seminars, Holiday Parties, Fundraisers, Business Conferences, Special Events, etc."@en ;
      rdfs:domain ns:EventVenue ;
      rdfs:label "productService"@en ;
      rdfs:range owl:Literal .

ns:CrewRole
      a       owl:Class ;
      rdfs:comment "The CrewRole class is a reified mediator connecting individuals affiliated with the production of a film or television program to the media work."@en ;
      rdfs:label "CrewRole"@en ;
      owl:subClassOf ns:Entity .

ns:Person
      a       owl:Class ;
      rdfs:comment "A person is a human being."@en ;
      rdfs:label "Person"@en ;
      owl:subClassOf ns:Entity ;
      :hasKey () .

ns:brandedID
      a       owl:ObjectProperty ;
      rdfs:comment "brandedID connects a company to its sub-brands. For example, Gap Inc. to Gap"@en ;
      rdfs:domain ns:Company ;
      rdfs:label "brandedID"@en ;
      rdfs:range ns:Company .

ns:pieceNumber
      a       :FunctionalProperty , owl:DatatypeProperty ;
      rdfs:comment "Number of pieces a media product includes (may include discs, cassettes, etc.)."@en ;
      rdfs:domain ns:MediaProduct ;
      rdfs:label "pieceNumber"@en ;
      rdfs:range xsd:int ;
      owl:subPropertyOf :topDataProperty .

ns:contactInfoProfile
      a       owl:DatatypeProperty ;
      rdfs:comment "contactInfoProfile contains descriptive profile information about a particular place of business."@en ;
      rdfs:domain ns:ContactInfo ;
      rdfs:label "contactInfoProfile"@en ;
      rdfs:range owl:Literal .

ns:Nomination
      a       owl:Class ;
      rdfs:comment "The Nomination class is a reified relationship that connects an individual, organization, or media work with an award for which it has been nominated."@en ;
      rdfs:label "Nomination"@en ;
      owl:subClassOf ns:Entity .

ns:Bar
      a       owl:Class ;
      rdfs:comment "bar is an establishment the serves alcoholic beverages to be consumed on the premises"@en ;
      rdfs:label "Bar"@en ;
      owl:subClassOf ns:EventVenue .

dc:creator
      a       :AnnotationProperty .

ns:Bonus
      a       owl:Class ;
      rdfs:comment "Bonus refers to the cash and gifts a person receives as compensation outside of salary and equities."@en ;
      rdfs:label "Bonus"@en ;
      owl:subClassOf ns:Compensation .

ns:coverCharge
      a       owl:DatatypeProperty ;
      rdfs:comment "coverCharge is the amount an establishment charges for entry when there is live entertainmet. It may or may not be a special show."@en ;
      rdfs:domain
              [ a       owl:Class ;
                :unionOf (ns:Bar ns:EstablishmentShowTime ns:EventVenue ns:NightClub ns:Restaurant)
              ] ;
      rdfs:label "coverCharge"@en ;
      rdfs:range xsd:float .

ns:imageCaption
      a       :FunctionalProperty , owl:DatatypeProperty ;
      rdfs:comment "Caption of images "@en ;
      rdfs:domain ns:Image ;
      rdfs:label "imageCaption"@en ;
      rdfs:range owl:Literal ;
      owl:subPropertyOf :topDataProperty .

ns:businessAssociation
      a       owl:DatatypeProperty ;
      rdfs:comment "businessAssociation are those formal associations a business belongs to"@en ;
      rdfs:domain ns:Organization ;
      rdfs:label "businessAssociation"@en ;
      rdfs:range owl:Literal .

ns:color
      a       :FunctionalProperty , owl:DatatypeProperty ;
      rdfs:comment "The color in which a film is presented. Usually full-color or black and white."@en ;
      rdfs:domain
              [ a       owl:Class ;
                :unionOf (ns:Color ns:Movie ns:Video)
              ] ;
      rdfs:label "color"@en ;
      rdfs:range owl:Literal ;
      owl:subPropertyOf ns:colorHolding .

ns:multicoat
      a       :FunctionalProperty , owl:DatatypeProperty ;
      rdfs:comment "Is the exterior paint finish multi-coat?(multi coat is a very high-quality and expensive finish in which several layers of paint are applied). Applicable only if category is Exterior"@en ;
      rdfs:domain ns:Color ;
      rdfs:label "multicoat"@en ;
      rdfs:range xsd:boolean ;
      owl:subPropertyOf ns:colorHolding .

ns:geoErrorCode
      a       owl:DatatypeProperty ;
      rdfs:comment "Geo Reporting code required for BLP."@en ;
      rdfs:domain
              [ a       owl:Class ;
                :unionOf (ns:Address ns:Place ns:SingleLocationBusiness)
              ] ;
      rdfs:label "geoErrorCode"@en ;
      rdfs:range owl:Literal .

ns:ColloquialPlace
      a       owl:Class ;
      rdfs:comment "A place known by a colloquial name. Example: Silicon Valley"@en , "Placetype: 24"@en ;
      rdfs:label "ColloquialPlace"@en ;
      owl:subClassOf ns:Place .

ns:approvedBrandOffered
      a       owl:DatatypeProperty ;
      rdfs:comment "Indicates the approved brands offered for sale at a local business."@en ;
      rdfs:domain
              [ a       owl:Class ;
                :unionOf (ns:EventVenue ns:RetailShop)
              ] ;
      rdfs:label "approvedBrandOffered"@en ;
      rdfs:range owl:Literal .

ns:givenName
      a       :FunctionalProperty , owl:DatatypeProperty ;
      rdfs:comment "Note for Media V2 schema: Change to givenName to support Trailblazers globalization guidelines: http://twiki.corp.yahoo.com/view/TrailBlazers/PersonalNames"@en , "A given name (or Christian name) is a personal name that specifies and differentiates between members of a group of individuals, especially in a family, all of whose members usually share the same family name (surname)."@en ;
      rdfs:domain ns:Person ;
      rdfs:label "givenName"@en ;
      rdfs:range owl:Literal ;
      owl:subPropertyOf ns:name .

ns:hostedAt
      a       owl:ObjectProperty ;
      rdfs:comment "hostedAt connects a show to the establishment"@en ;
      rdfs:domain ns:EstablishmentShow ;
      rdfs:label "hostedAt"@en ;
      rdfs:range ns:EstablishmentShowTime .

ns:Warranty
      a       owl:Class ;
      rdfs:comment "a warranty is an assurance by one party to the other party that certain facts or conditions are true or will happen; the other party is permitted to rely on that assurance and seek some type of remedy if it is not true or followed."@en ;
      rdfs:label "Warranty"@en ;
      owl:subClassOf ns:Entity .

ns:creditFor
      a       :FunctionalProperty , owl:ObjectProperty ;
      rdfs:comment "The creditFor property connects the reified Crew class to the individuals involved with the production of a media work."@en ;
      rdfs:domain
              [ a       owl:Class ;
                :unionOf (ns:ActingRole ns:CompanyRole ns:CrewRole)
              ] ;
      rdfs:label "creditFor"@en ;
      rdfs:range
              [ a       owl:Class ;
                :unionOf (ns:Actor ns:Company ns:Crew)
              ] ;
      owl:subPropertyOf :topObjectProperty ;
      :inverseOf ns:credit .

ns:USSenator
      a       owl:Class ;
      rdfs:comment "Created by ace to support Milton mapping: http://twiki.corp.yahoo.com/view/P13nContextual/MiltonWooSchemaMap"@en , "An individual elected to the United States Senate."@en ;
      rdfs:label "USSenator"@en ;
      owl:subClassOf ns:Politician .

ns:stateCode
      a       :FunctionalProperty , owl:DatatypeProperty ;
      rdfs:comment "standardized code to designate a state."@en ;
      rdfs:domain
              [ a       owl:Class ;
                :unionOf (ns:Address ns:SingleLocationBusiness ns:StateAdminArea)
              ] ;
      rdfs:label "stateCode"@en ;
      rdfs:range owl:Literal ;
      owl:subPropertyOf :topDataProperty .

ns:landmarkWithin
      a       :FunctionalProperty , owl:ObjectProperty ;
      rdfs:comment "landmarkWithin connects place or business landmarks to the place or business it exists within (for example, the Rodin Sculpture Garden  exists within Stanford University or Yosemite Falls  exists within Yosemite Park."@en ;
      rdfs:domain
              [ a       owl:Class ;
                :unionOf (ns:LocalBusiness ns:Place)
              ] ;
      rdfs:label "landmarkWithin"@en ;
      rdfs:range
              [ a       owl:Class ;
                :unionOf (ns:LocalBusiness ns:Place)
              ] .

ns:historicJobTitle
      a       owl:DatatypeProperty ;
      rdfs:comment "historicJobTitle is a list of past job titles a person has had"@en ;
      rdfs:domain ns:Person ;
      rdfs:label "historicJobTitle"@en ;
      rdfs:range owl:Literal .

<http://woo.corp.yahoo.com/ns/units/lb>
      a       owl:Datatype .

ns:priceValue
      a       owl:DatatypeProperty ;
      rdfs:comment "Price for an event registration."@en ;
      rdfs:domain ns:EventRegistration ;
      rdfs:label "priceValue"@en ;
      rdfs:range <http://woo.corp.yahoo.com/ns/currency:xxx> .

ns:giftCertificateURL
      a       owl:DatatypeProperty ;
      rdfs:comment "URL for gift certificates offered by a local business."@en ;
      rdfs:domain ns:LocalBusiness ;
      rdfs:label "giftCertificateURL"@en ;
      rdfs:range xsd:anyURI .

ns:sharesOwnedBy
      a       owl:ObjectProperty ;
      rdfs:comment "sharesOwnedBy connects the majorshareholderaffiliation to the person or organization that owns the shares"@en ;
      rdfs:domain ns:MajorShareholderAffiliation ;
      rdfs:label "sharesOwnedBy"@en ;
      rdfs:range
              [ a       owl:Class ;
                :unionOf (ns:Organization ns:Person)
              ] ;
      :inverseOf ns:ownsShares .

ns:InstallmentCredit
      a       owl:Class ;
      rdfs:comment "InstallmentCredit is credit with a fixed number of payments"@en ;
      rdfs:label "InstallmentCredit"@en ;
      owl:subClassOf ns:ConsumerCredit .

ns:abuseFlag
      a       owl:DatatypeProperty ;
      rdfs:comment "Includes PORN, HATE, SPAM "@en ;
      rdfs:domain ns:Webpage ;
      rdfs:label "abuseFlag"@en ;
      rdfs:range owl:Literal ;
      rdfs:range
              [ a       owl:Datatype ;
                :oneOf  [ a       rdf:List ;
                          rdf:first "HATE"^^xsd:string ;
                          rdf:rest
                                  [ a       rdf:List ;
                                    rdf:first "PORN"^^xsd:string ;
                                    rdf:rest
                                            [ a       rdf:List ;
                                              rdf:first "SPAM"^^xsd:string ;
                                              rdf:rest ()
                                            ]
                                  ]
                        ]
              ] ;
      owl:subPropertyOf :topDataProperty .

ns:eventAt
      a       :FunctionalProperty , owl:ObjectProperty ;
      rdfs:comment "eventAt connects an event or show to the establishment where it occurs"@en ;
      rdfs:domain ns:LocalEventOccurrence ;
      rdfs:label "eventAt"@en ;
      rdfs:range ns:EventVenue ;
      :inverseOf ns:event .

ns:mediaProduct
      a       :InverseFunctionalProperty , owl:ObjectProperty ;
      rdfs:comment "Connects a media work to its product."@en ;
      rdfs:domain ns:MediaWork ;
      rdfs:label "mediaProduct"@en ;
      rdfs:range ns:MediaProduct ;
      owl:subPropertyOf :topObjectProperty .

ns:providerAssetId
      a       owl:DatatypeProperty ;
      rdfs:comment "Data provider's asset ID, added for Local"@en ;
      rdfs:domain ns:LocalBusiness ;
      rdfs:label "providerAssetId"@en ;
      rdfs:range owl:Literal ;
      owl:subPropertyOf ns:id .

ns:Fund
      a       owl:Class ;
      rdfs:comment "Fund represents teh fund sub-class of financial instrument"@en ;
      rdfs:label "Fund"@en ;
      owl:subClassOf ns:FinancialInstrument .

rdfs:comment
      a       :AnnotationProperty .

ns:featureName
      a       owl:DatatypeProperty ;
      rdfs:comment "Name of feature, i.e. no of speakers."@en ;
      rdfs:label "featureName"@en .

ns:homeTeamId
      a       :FunctionalProperty , owl:DatatypeProperty ;
      rdfs:comment "Designates the home team of a sports game."@en ;
      rdfs:domain ns:SportGame ;
      rdfs:label "homeTeamId"@en ;
      rdfs:range owl:Literal ;
      owl:subPropertyOf ns:id .

ns:competitionGame
      a       owl:ObjectProperty ;
      rdfs:comment "Connects the individual games to the competitions involved (world cup 2010, etc)"@en ;
      rdfs:domain ns:SportGame ;
      rdfs:label "competitionGame"@en ;
      rdfs:range ns:SportCompetitionInstance ;
      owl:subPropertyOf :topObjectProperty .

ns:awardTo
      a       :FunctionalProperty , owl:ObjectProperty ;
      rdfs:comment "Connects the reified nomination class to the award for which the nomination is granted."@en ;
      rdfs:domain ns:AwardType ;
      rdfs:label "awardTo"@en ;
      rdfs:range ns:Nomination ;
      owl:subPropertyOf :topObjectProperty ;
      :inverseOf ns:award .

ns:SingleLocationBusiness
      a       owl:Class ;
      rdfs:comment "Local Business with only one location of operation. One address and phone. Created to support Local prototype. Business listings with complete info should use the ContactInfo relationship."@en ;
      rdfs:label "SingleLocationBusiness"@en ;
      owl:subClassOf ns:LocalBusiness .

ns:frontpageSafe
      a       :FunctionalProperty , owl:DatatypeProperty ;
      rdfs:comment "Indicates whether content is approved for display on frontpage."@en ;
      rdfs:domain ns:Deal ;
      rdfs:label "frontpageSafe"@en ;
      rdfs:range xsd:boolean .

ns:synopsis
      a       owl:ObjectProperty ;
      rdfs:comment "Links a Media Work to the synopsis that summarizes it."@en ;
      rdfs:domain ns:MediaWork ;
      rdfs:label "synopsis"@en ;
      rdfs:range ns:Synopsis ;
      :inverseOf ns:synopsisOf .

ns:distributedBy
      a       owl:ObjectProperty ;
      rdfs:comment "The distributedBy property connects a media title to the organization or person that distributes it."@en ;
      rdfs:domain
              [ a       owl:Class ;
                :unionOf (ns:MediaProduct ns:Movie ns:TvEpisode ns:TvSeason ns:TvSeries ns:TvSpecial)
              ] ;
      rdfs:label "distributedBy"@en ;
      rdfs:range ns:TheatricalDistributor ;
      :inverseOf ns:distributed .

ns:trimName
      a       :FunctionalProperty , owl:DatatypeProperty ;
      rdfs:comment "Name of the auto's trim. "@en ;
      rdfs:domain ns:AutoTrim ;
      rdfs:label "trimName"@en ;
      rdfs:range owl:Literal ;
      owl:subPropertyOf ns:name .

ns:statusChange
      a       owl:ObjectProperty ;
      rdfs:comment "statusChange links an organization to the event class OrganizationStatusChange"@en ;
      rdfs:domain ns:Organization ;
      rdfs:label "statusChange"@en ;
      rdfs:range ns:OrganizationStatusChange .

ns:submitTime
      a       :FunctionalProperty , owl:DatatypeProperty ;
      rdfs:comment "Timestamp indicating the time at which a review was submitted."@en ;
      rdfs:domain ns:Review ;
      rdfs:label "submitTime"@en ;
      rdfs:range xsd:dateTimeStamp .

ns:approxStart
      a       owl:DatatypeProperty ;
      rdfs:comment "Approximate start time for an event or event occurrence."@en ;
      rdfs:domain ns:LocalEventOccurrence ;
      rdfs:label "approxStart"@en ;
      rdfs:range owl:Literal .

ns:Entity
      a       owl:Class ;
      rdfs:comment "Entity is the common class of entities managed by WOO."@en ;
      rdfs:label "Entity"@en .

ns:Video
      a       owl:Class ;
      rdfs:comment "Consumer products that play video recordings."@en ;
      rdfs:label "Video"@en ;
      owl:subClassOf ns:MediaProduct .

ns:consumerRelatedBrand
      a       owl:ObjectProperty ;
      rdfs:label "consumerRelatedBrand"@en .

ns:Place
      a       owl:Class ;
      rdfs:comment "A Place is a position or point in physical space, which can be designated using a specific pairing of latitude and longitude. Distinct from Address in that it doesn't designate a building or place where mail is delivered. Distinct from GPE in that it is a fixed point and not a political construct."@en , "An area with definite or indefinite boundaries; a portion of space."@en ;
      rdfs:label "Place"@en ;
      owl:subClassOf ns:Entity .

ns:text
      a       :FunctionalProperty , owl:DatatypeProperty ;
      rdfs:comment "Text value of a written piece of media."@en ;
      rdfs:domain
              [ a       owl:Class ;
                :unionOf (ns:Biography ns:Review ns:Synopsis ns:Webpage)
              ] ;
      rdfs:label "text"@en ;
      rdfs:range owl:Literal ;
      owl:subPropertyOf :topDataProperty .

ns:soundtrack
      a       owl:ObjectProperty ;
      rdfs:comment "Connects a soundtrack album to the movie it is from."@en ;
      rdfs:domain ns:Album ;
      rdfs:label "soundtrack"@en ;
      rdfs:range ns:Movie ;
      owl:subPropertyOf :topObjectProperty .

ns:companyOfficerOf
      a       owl:ObjectProperty ;
      rdfs:comment "companyOfficerOf connects the companyofficeraffiliation to the compay"@en ;
      rdfs:domain ns:CompanyOfficerAffiliation ;
      rdfs:label "companyOfficerOf"@en ;
      rdfs:range ns:Company ;
      :inverseOf ns:companyOfficer .

ns:diningFeature
      a       owl:DatatypeProperty ;
      rdfs:comment "Describes the dining features offered at a restaurant or venue, e.g. healthy, outdoor, late night, takeout, catering, brunch, etc. May include multiple values, comma separated."@en ;
      rdfs:domain
              [ a       owl:Class ;
                :unionOf (ns:EventVenue ns:Restaurant)
              ] ;
      rdfs:label "diningFeature"@en ;
      rdfs:range owl:Literal .

ns:venueTypeId
      a       owl:DatatypeProperty ;
      rdfs:comment "Unique identifier assigned to a category of venue type."@en ;
      rdfs:domain ns:EventVenue ;
      rdfs:label "venueTypeId"@en ;
      rdfs:range owl:Literal .

ns:webpageOf
      a       :FunctionalProperty , owl:ObjectProperty ;
      rdfs:comment "Connects a webpage to the thing it describes."@en , "Connected to Entity per Ticket 4192755"@en ;
      rdfs:domain ns:Webpage ;
      rdfs:label "webpageOf"@en ;
      rdfs:range ns:Entity ;
      owl:subPropertyOf :topObjectProperty .

ns:quantitySold
      a       owl:DatatypeProperty ;
      rdfs:comment "Number of items sold in a deal or offer"@en ;
      rdfs:domain ns:Deal ;
      rdfs:label "quantitySold"@en ;
      rdfs:range owl:Literal .

ns:containsKiosk
      a       owl:ObjectProperty ;
      rdfs:comment "containsKiosk coects a local business to the kiosk(s) that operate in or just outside ofit."@en ;
      rdfs:domain ns:LocalBusiness ;
      rdfs:label "containsKiosk"@en ;
      rdfs:range ns:Kiosk ;
      :inverseOf ns:kioskAt .

ns:jobType
      a       :FunctionalProperty , owl:DatatypeProperty ;
      rdfs:comment "Type of employment that a person has held."@en ;
      rdfs:domain ns:OccupationalHistory ;
      rdfs:label "jobType"@en ;
      rdfs:range owl:Literal ;
      owl:subPropertyOf :topDataProperty .

ns:analyst
      a       owl:ObjectProperty ;
      rdfs:comment "Connects a financial analyst to the reified AnalystAffiliation class."@en ;
      rdfs:domain ns:Analyst ;
      rdfs:label "analyst"@en ;
      rdfs:range ns:AnalystAffiliation .

ns:dressCode
      a       :FunctionalProperty , owl:DatatypeProperty ;
      rdfs:comment "dressCode is the type of dress expected of the patrons of a restaurant"@en ;
      rdfs:domain
              [ a       owl:Class ;
                :unionOf (ns:Bar ns:EventVenue ns:NightClub ns:Restaurant)
              ] ;
      rdfs:label "dressCode"@en ;
      rdfs:range owl:Literal .

ns:teamParticipationIn
      a       owl:ObjectProperty ;
      rdfs:comment "Connects the reified TeamGameRole class to a sports team."@en ;
      rdfs:domain ns:TeamGameRole ;
      rdfs:label "teamParticipationIn"@en ;
      rdfs:range ns:SportTeam ;
      :inverseOf ns:teamParticipation .

ns:association
      a       owl:ObjectProperty ;
      rdfs:comment "Connects an individual, organization, or media work to other individuals, organizations, or media works to the reified Association class."@en ;
      rdfs:domain
              [ a       owl:Class ;
                :unionOf (ns:MediaWork ns:Organization ns:Performer ns:Person)
              ] ;
      rdfs:label "association"@en ;
      rdfs:range ns:Association ;
      owl:subPropertyOf :topObjectProperty .

ns:twoTone
      a       :FunctionalProperty , owl:DatatypeProperty ;
      rdfs:comment "Is the vehicle body is finished in two distinct colors or shades? Applicable only if category is Exterior"@en ;
      rdfs:domain ns:Color ;
      rdfs:label "twoTone"@en ;
      rdfs:range xsd:boolean ;
      owl:subPropertyOf ns:colorHolding .

ns:performerId
      a       owl:DatatypeProperty ;
      rdfs:comment "ID of the band, singer, or other performer for an event."@en ;
      rdfs:domain
              [ a       owl:Class ;
                :unionOf (ns:Event ns:LocalEvent)
              ] ;
      rdfs:label "performerId"@en ;
      rdfs:range owl:Literal ;
      owl:subPropertyOf ns:id .

rdfs:label
      a       :AnnotationProperty .

ns:associatedKioskBusiness
      a       :FunctionalProperty , owl:DatatypeProperty ;
      rdfs:comment "associatedKioskBusiness is for the name of the business a kiosk is associated with (Lucky's, Wlagreens,Safeway,etc.)"@en ;
      rdfs:domain ns:Kiosk ;
      rdfs:label "associatedKioskBusiness"@en ;
      rdfs:range owl:Literal .

ns:earningsPerShare
      a       :FunctionalProperty , owl:DatatypeProperty ;
      rdfs:comment "Earnings per share (EPS) is the amount of earnings per each outstanding share of a company's stock."@en ;
      rdfs:domain ns:Security ;
      rdfs:label "earningsPerShare"@en ;
      rdfs:range xsd:float .

ns:sportPlayed
      a       owl:ObjectProperty ;
      rdfs:comment "Connects an athlete, team, or division with the sport(s) s/he plays."@en ;
      rdfs:domain
              [ a       owl:Class ;
                :unionOf (ns:Athlete ns:AthleticConference ns:SportDivision ns:SportLeague ns:SportTeam ns:SportVenue)
              ] ;
      rdfs:label "sportPlayed"@en ;
      rdfs:range ns:Sport ;
      :inverseOf ns:playedBy .

ns:phoneNumber
      a       owl:ObjectProperty ;
      rdfs:comment "Connects a phone number to a location or person"@en ;
      rdfs:domain
              [ a       owl:Class ;
                :unionOf (ns:ContactInfo ns:LocalEvent ns:Person)
              ] ;
      rdfs:label "phoneNumber"@en ;
      rdfs:range ns:Phone ;
      owl:subPropertyOf :topObjectProperty ;
      :inverseOf ns:phoneNumberOf .

ns:Continent
      a       owl:Class ;
      rdfs:comment "placetype: 29"@en , "One of the seven major land masses on the Earth. Example: North America."@en ;
      rdfs:label "Continent"@en ;
      owl:subClassOf ns:Place .

ns:lyrics
      a       owl:ObjectProperty ;
      rdfs:comment "Attaches the lyrics class to its song or performance."@en ;
      rdfs:domain
              [ a       owl:Class ;
                :unionOf (ns:MusicPerformance ns:Song)
              ] ;
      rdfs:label "lyrics"@en ;
      rdfs:range ns:Lyrics ;
      owl:subPropertyOf :topObjectProperty .

ns:financialInstrument
      a       owl:ObjectProperty ;
      rdfs:comment "financial instrument connects a public company to it trading instrument"@en ;
      rdfs:domain ns:PublicCompany ;
      rdfs:label "financialInstrument"@en ;
      rdfs:range ns:FinancialInstrument .

ns:ratingSystem
      a       :FunctionalProperty , owl:DatatypeProperty ;
      rdfs:comment "The system used to indicate film's thematic and content suitability for certain audiences."@en ;
      rdfs:domain ns:MovieRating ;
      rdfs:label "ratingSystem"@en ;
      rdfs:range owl:Literal .

ns:MutualFund
      a       owl:Class ;
      rdfs:comment "MutualFund a professionally managed type of collective investment scheme that pools money from many investors and invests typically in investment securities"@en ;
      rdfs:label "MutualFund"@en ;
      owl:subClassOf ns:Fund .

ns:reviewScore
      a       :FunctionalProperty , owl:DatatypeProperty ;
      rdfs:comment "Score awarded to a media work by a critical reviewer (includes letter grades, number of stars, etc.)."@en ;
      rdfs:domain ns:Review ;
      rdfs:label "reviewScore"@en ;
      rdfs:range owl:Literal .

ns:busListingCategoryId
      a       owl:DatatypeProperty ;
      rdfs:comment "Integer array of unique identifier(s) for the Yahoo Business Listing category (or categories) to which a business listing is assigned."@en ;
      rdfs:domain ns:BusinessListingCategory ;
      rdfs:label "busListingCategoryId"@en ;
      rdfs:range owl:Literal ;
      owl:subPropertyOf ns:id .

ns:postOfficeBox
      a       :FunctionalProperty , owl:DatatypeProperty ;
      rdfs:comment "Post office box where mail may be delivered for an organization or person."@en ;
      rdfs:domain
              [ a       owl:Class ;
                :unionOf (ns:Address ns:SingleLocationBusiness)
              ] ;
      rdfs:label "postOfficeBox"@en ;
      rdfs:range owl:Literal .

ns:marketTierSymbol
      a       :FunctionalProperty , owl:DatatypeProperty ;
      rdfs:comment "marketTierSymbol is the symbol used to refer to a market tier. For example, NasdaqGS"@en ;
      rdfs:domain
              [ a       owl:Class ;
                :unionOf (ns:MarketTier ns:TradableQuotableInstrument)
              ] ;
      rdfs:label "marketTierSymbol"@en ;
      rdfs:range owl:Literal .

ns:marketTierProfile
      a       :FunctionalProperty , owl:DatatypeProperty ;
      rdfs:comment "marketTierProfile is the text that describes the market tier"@en ;
      rdfs:domain ns:MarketTier ;
      rdfs:label "marketTierProfile"@en ;
      rdfs:range owl:Literal .

ns:warranty
      a       owl:ObjectProperty ;
      rdfs:comment "Connects a Warranty object to the entity it covers."@en ;
      rdfs:domain ns:Warranty ;
      rdfs:label "warranty"@en ;
      rdfs:range
              [ a       owl:Class ;
                :unionOf (ns:AutoTrim ns:ConsumerProduct)
              ] .

ns:athleteGame
      a       owl:ObjectProperty ;
      rdfs:comment "Connects a game to the athlete role in it."@en ;
      rdfs:domain ns:SportGame ;
      rdfs:label "athleteGame"@en ;
      rdfs:range ns:AthleteGameRole .

ns:MovieShowtime
      a       owl:Class ;
      rdfs:comment "Reified relationship describing film showtimes. Establishes a relationship between a particular film and theater."@en ;
      rdfs:label "MovieShowtime"@en ;
      owl:subClassOf ns:Event .

ns:featureCategoryName
      a       owl:DatatypeProperty ;
      rdfs:comment "Name of the feature category described. I.e. 'audio'."@en ;
      rdfs:domain ns:AutoTrim ;
      rdfs:label "featureCategoryName"@en ;
      rdfs:range owl:Literal .

ns:unparsedPhoneNumber
      a       :FunctionalProperty , owl:DatatypeProperty ;
      rdfs:comment "Captures phone numbers that don't fall into any other phone number data property."@en ;
      rdfs:domain ns:Phone ;
      rdfs:label "unparsedPhoneNumber"@en ;
      rdfs:range owl:Literal ;
      owl:subPropertyOf ns:unparsed .

ns:FinanceEvent
      a       owl:Class ;
      rdfs:comment "FinanceEvent is a reified class created to capture events that are of interest in the finance world."@en ;
      rdfs:label "FinanceEvent"@en ;
      owl:subClassOf ns:Event .

ns:reservationPolicy
      a       :FunctionalProperty , owl:DatatypeProperty ;
      rdfs:comment "Enumerates the reservations accepted or not by a restaurant."@en ;
      rdfs:domain
              [ a       owl:Class ;
                :unionOf (ns:EventVenue ns:Restaurant)
              ] ;
      rdfs:label "reservationPolicy"@en ;
      rdfs:range owl:Literal ;
      rdfs:range
              [ a       owl:Datatype ;
                :oneOf  [ a       rdf:List ;
                          rdf:first "ACCEPTED"^^xsd:string ;
                          rdf:rest
                                  [ a       rdf:List ;
                                    rdf:first "NOT ACCEPTED"^^xsd:string ;
                                    rdf:rest
                                            [ a       rdf:List ;
                                              rdf:first "REQUIRED"^^xsd:string ;
                                              rdf:rest
                                                      [ a       rdf:List ;
                                                        rdf:first "REQUIRED LARGE PARTIES"^^xsd:string ;
                                                        rdf:rest
                                                                [ a       rdf:List ;
                                                                  rdf:first "SUGGESTED"^^xsd:string ;
                                                                  rdf:rest ()
                                                                ]
                                                      ]
                                            ]
                                  ]
                        ]
              ] ;
      owl:subPropertyOf :topDataProperty .

ns:award
      a       :FunctionalProperty , owl:ObjectProperty ;
      rdfs:comment "Connects an award to the reified nomination class."@en ;
      rdfs:domain ns:Nomination ;
      rdfs:label "award"@en ;
      rdfs:range ns:AwardType ;
      owl:subPropertyOf :topObjectProperty .

ns:brandName
      a       owl:DatatypeProperty ;
      rdfs:comment "example: Kool-Aid"@en , "Brand name of a particular deal or product."@en ;
      rdfs:domain ns:Deal ;
      rdfs:label "brandName"@en ;
      rdfs:range owl:Literal ;
      owl:subPropertyOf ns:name .

ns:musicRightsOf
      a       owl:ObjectProperty ;
      rdfs:comment "connects a musical work to its rights"@en ;
      rdfs:domain ns:MusicRight ;
      rdfs:label "musicRightsOf"@en ;
      rdfs:range ns:Album ;
      owl:subPropertyOf :topObjectProperty ;
      :inverseOf ns:musicRights .

ns:Contestant
      a       owl:Class ;
      rdfs:comment "A television contestant is a person who competes on a television game show or reality contest."@en ;
      rdfs:label "Contestant"@en ;
      owl:subClassOf ns:Person .

ns:trimMungedName
      a       :FunctionalProperty , owl:DatatypeProperty ;
      rdfs:comment "Munged name representing trim."@en ;
      rdfs:domain ns:AutoTrim ;
      rdfs:label "trimMungedName"@en ;
      rdfs:range owl:Literal ;
      owl:subPropertyOf ns:name .

ns:birthYear
      a       :FunctionalProperty , owl:DatatypeProperty ;
      rdfs:comment "The year in which an individual was born."@en ;
      rdfs:domain ns:Person ;
      rdfs:label "birthYear"@en ;
      rdfs:range xsd:gYear ;
      owl:subPropertyOf ns:date .

ns:seasonPhase
      a       :FunctionalProperty , owl:DatatypeProperty ;
      rdfs:comment "Identifies the type of seasonal game: preseason, regular season, post season"@en ;
      rdfs:domain ns:SportGame ;
      rdfs:label "seasonPhase"@en ;
      rdfs:range owl:Literal ;
      owl:subPropertyOf :topDataProperty .

ns:titlePrefix
      a       :FunctionalProperty , owl:DatatypeProperty ;
      rdfs:comment "Leading article from a media title (eg, the, an, a)."@en ;
      rdfs:domain
              [ a       owl:Class ;
                :unionOf (ns:AlternateTitle ns:MediaWork)
              ] ;
      rdfs:label "titlePrefix"@en ;
      rdfs:range owl:Literal ;
      owl:subPropertyOf :topDataProperty .

ns:department
      a       owl:ObjectProperty ;
      rdfs:comment "connects one local business to another, indicating that one is a department of the other. This does not imply the same address."@en ;
      rdfs:domain ns:LocalBusiness ;
      rdfs:label "department"@en ;
      rdfs:range ns:LocalBusiness ;
      :inverseOf ns:departmentOf .

ns:invoice
      a       :FunctionalProperty , owl:DatatypeProperty ;
      rdfs:comment "The invoice price of a car is the standard price the car manufacturer invoices a dealership for a vehicle. The invoice price is the cost of just the vehicle, without any added options. "@en ;
      rdfs:domain
              [ a       owl:Class ;
                :unionOf (ns:AutoMake ns:AutoModel ns:AutoTrim ns:Automobile)
              ] ;
      rdfs:label "invoice"@en ;
      rdfs:range xsd:double .

ns:Compensation
      a       owl:Class ;
      rdfs:comment "Compensation is for the Finance need to display the compensation of insiders"@en ;
      rdfs:label "Compensation"@en ;
      owl:subClassOf ns:Entity .

ns:marketTier
      a       :FunctionalProperty , owl:DatatypeProperty ;
      rdfs:comment "marketTier identifies if  this exchange has market tiers "@en ;
      rdfs:domain ns:Exchange ;
      rdfs:label "marketTier"@en ;
      rdfs:range xsd:boolean .

ns:TvSpecial
      a       owl:Class ;
      rdfs:comment "One-time special tv program such as award shows, sports events, olympics, and so on."@en ;
      rdfs:label "TvSpecial"@en ;
      owl:subClassOf ns:MediaWork .

ns:reviewCount
      a       :FunctionalProperty , owl:DatatypeProperty ;
      rdfs:comment "Number of critical reviews collated for a given film."@en ;
      rdfs:domain ns:RottenTomatoesReview ;
      rdfs:label "reviewCount"@en ;
      rdfs:range owl:Literal .

ns:alternateName
      a       owl:ObjectProperty ;
      rdfs:comment "An alternate name for a Person."@en ;
      rdfs:domain ns:Person ;
      rdfs:label "alternateName"@en ;
      rdfs:range ns:AlternatePersonName ;
      :inverseOf ns:alternateNameOf .

ns:relatedWikiUri
      a       owl:DatatypeProperty ;
      rdfs:comment "Contains uris related to the entity in question."@en ;
      rdfs:domain
              [ a       owl:Class ;
                :unionOf (ns:Movie ns:Person)
              ] ;
      rdfs:label "relatedWikiUri"@en ;
      rdfs:range owl:Literal .

ns:fallback
      a       owl:DatatypeProperty ;
      rdfs:comment "Removed from entity class on 10/20/10, per discussion."@en , "Blob dataproperty to contain unformatted fallback information."@en ;
      rdfs:label "fallback"@en .

ns:employs
      a       owl:ObjectProperty ;
      rdfs:comment "employs connects the org to the person it employs"@en ;
      rdfs:domain ns:EmployeeAffiliation ;
      rdfs:label "employs"@en ;
      rdfs:range ns:Person .

ns:alcoholDescription
      a       owl:DatatypeProperty ;
      rdfs:comment "Describes any special features of the alcohol policy of a business."@en ;
      rdfs:domain ns:LocalBusiness ;
      rdfs:label "alcoholDescription"@en ;
      rdfs:range owl:Literal .

ns:judged
      a       owl:ObjectProperty ;
      rdfs:comment "The judged property connects a televison judge with the programs that s/he has judged."@en ;
      rdfs:domain ns:ContestJudge ;
      rdfs:label "judged"@en ;
      rdfs:range
              [ a       owl:Class ;
                :unionOf (ns:TvEpisode ns:TvSeason ns:TvSeries ns:TvSpecial)
              ] .

ns:onlineAccountOf
      a       :FunctionalProperty , owl:ObjectProperty ;
      rdfs:comment "Connects an online account to the holder of the account."@en ;
      rdfs:domain ns:OnlineAccount ;
      rdfs:label "onlineAccountOf"@en ;
      rdfs:range
              [ a       owl:Class ;
                :unionOf (ns:MusicArtist ns:Organization ns:Performer ns:Person)
              ] .

ns:genre
      a       owl:DatatypeProperty ;
      rdfs:comment "the mediaGenre data property captures the free test entry for the genre of a media work or music artist"@en ;
      rdfs:domain
              [ a       owl:Class ;
                :unionOf (ns:MediaWork ns:MusicArtist ns:Performer)
              ] ;
      rdfs:label "genre"@en ;
      rdfs:range owl:Literal .

ns:addressOf
      a       owl:ObjectProperty ;
      rdfs:comment "Connects a physical address to the entity located there."@en ;
      rdfs:domain ns:Address ;
      rdfs:label "addressOf"@en ;
      rdfs:range
              [ a       owl:Class ;
                :unionOf (ns:ContactInfo ns:Person ns:Structure)
              ] ;
      owl:subPropertyOf :topObjectProperty ;
      :inverseOf ns:address .

ns:rating
      a       :FunctionalProperty , owl:DatatypeProperty ;
      rdfs:comment "The rating assigned to a film to indicate its thematic and content suitability for certain audiences."@en ;
      rdfs:domain
              [ a       owl:Class ;
                :unionOf (ns:MovieRating ns:RottenTomatoesReview)
              ] ;
      rdfs:label "rating"@en ;
      rdfs:range owl:Literal .

ns:Security
      a       owl:Class ;
      rdfs:comment "Security a fungible, negotiable instrument representing financial value"@en ;
      rdfs:label "Security"@en ;
      owl:subClassOf ns:FinancialInstrument .

ns:metaDescription
      a       :FunctionalProperty , owl:DatatypeProperty ;
      rdfs:comment "Meta description for a web page."@en ;
      rdfs:domain ns:Webpage ;
      rdfs:label "metaDescription"@en ;
      rdfs:range owl:Literal ;
      owl:subPropertyOf :topDataProperty .

ns:rebateAmountLow
      a       :FunctionalProperty , owl:DatatypeProperty ;
      rdfs:comment "Represents the lower end of rebate amount if rebate amount is provided as a range. If rebate amount is not a range, rebateAmountLow is used to represent the rebate amount "@en ;
      rdfs:domain ns:AutoIncentive ;
      rdfs:label "rebateAmountLow"@en ;
      rdfs:range xsd:double .

ns:teamVenueOf
      a       owl:ObjectProperty ;
      rdfs:comment "Connects a venue to the team that plays there."@en ;
      rdfs:domain ns:SportVenue ;
      rdfs:label "teamVenueOf"@en ;
      rdfs:range ns:SportTeam ;
      owl:subPropertyOf :topObjectProperty ;
      :inverseOf ns:teamVenue .

ns:starRating
      a       owl:DatatypeProperty ;
      rdfs:comment "Hotel's Star rating (1 star, 2 star, 3 star, 4 star, 5 star, 7 star) "@en ;
      rdfs:domain ns:Lodging ;
      rdfs:label "starRating"@en ;
      rdfs:range owl:Literal ;
      rdfs:range
              [ a       owl:Datatype ;
                :oneOf  [ a       rdf:List ;
                          rdf:first "1STAR"^^xsd:string ;
                          rdf:rest
                                  [ a       rdf:List ;
                                    rdf:first "2STAR"^^xsd:string ;
                                    rdf:rest
                                            [ a       rdf:List ;
                                              rdf:first "3STAR"^^xsd:string ;
                                              rdf:rest
                                                      [ a       rdf:List ;
                                                        rdf:first "4STAR"^^xsd:string ;
                                                        rdf:rest
                                                                [ a       rdf:List ;
                                                                  rdf:first "5STAR"^^xsd:string ;
                                                                  rdf:rest
                                                                          [ a       rdf:List ;
                                                                            rdf:first "6STAR"^^xsd:string ;
                                                                            rdf:rest
                                                                                    [ a       rdf:List ;
                                                                                      rdf:first "7STAR"^^xsd:string ;
                                                                                      rdf:rest ()
                                                                                    ]
                                                                          ]
                                                                ]
                                                      ]
                                            ]
                                  ]
                        ]
              ] ;
      owl:subPropertyOf :topDataProperty .

ns:chapter
      a       owl:DatatypeProperty ;
      rdfs:comment "A listing of the individual chapters of a media product."@en ;
      rdfs:domain ns:MediaProduct ;
      rdfs:label "chapter"@en ;
      rdfs:range owl:Literal ;
      owl:subPropertyOf :topDataProperty .

ns:alternateMediaTitle
      a       :FunctionalProperty , owl:DatatypeProperty ;
      rdfs:comment "Alternate title by which a media work may be known (includes translated titles, nicknames, and foreign titles)."@en , "There may be multiple alternate titles for a media work, but there is only one title per object association between the MediaWork and AlternateTitle classes."@en ;
      rdfs:domain ns:AlternateTitle ;
      rdfs:label "alternateMediaTitle"@en ;
      rdfs:range owl:Literal ;
      owl:subPropertyOf ns:label .

ns:rightsId
      a       :FunctionalProperty , owl:DatatypeProperty ;
      rdfs:comment "The source id associated with a media work's rights provider"@en ;
      rdfs:domain ns:DistributionRight ;
      rdfs:label "rightsId"@en ;
      rdfs:range owl:Literal ;
      owl:subPropertyOf ns:id .

ns:broadcast
      a       owl:ObjectProperty ;
      rdfs:comment "Connects a network affiliation to a television program."@en ;
      rdfs:domain
              [ a       owl:Class ;
                :unionOf (ns:TvEpisode ns:TvSeason ns:TvSeries ns:TvSpecial)
              ] ;
      rdfs:label "broadcast"@en ;
      rdfs:range ns:NetworkAffiliation ;
      owl:subPropertyOf :topObjectProperty .

ns:albumTrackOf
      a       owl:ObjectProperty ;
      rdfs:comment "The albumTrackOf property connects a song (musical track) with the album on which it appears."@en ;
      rdfs:domain
              [ a       owl:Class ;
                :unionOf (ns:AlbumTrack ns:Song)
              ] ;
      rdfs:label "albumTrackOf"@en ;
      rdfs:range ns:Album ;
      :inverseOf ns:albumTrack .

:topObjectProperty
      a       owl:ObjectProperty .

ns:AdultsOnlyMovies
      a       owl:Class ;
      rdfs:comment "Creating the class of movies for adults only in order to capture that no movie can be both for kids and adults only."@en ;
      rdfs:label "Adults Only Movies"@en ;
      owl:subClassOf ns:Movie ;
      :disjointWith ns:KidsMovies .

ns:competitionType
      a       :FunctionalProperty , owl:DatatypeProperty ;
      rdfs:comment "Type of sports competition, i.e. tournament or world cup"@en ;
      rdfs:domain ns:SportCompetitionInstance ;
      rdfs:label "competitionType"@en ;
      rdfs:range owl:Literal ;
      owl:subPropertyOf :topDataProperty .

ns:AppearanceRole
      a       owl:Class ;
      rdfs:comment "An appearance is when a person appears on a television show as themself, usually a talk show or news program."@en ;
      rdfs:label "AppearanceRole"@en ;
      owl:subClassOf ns:Entity .

ns:fictional
      a       :FunctionalProperty , owl:DatatypeProperty ;
      rdfs:comment "fictional captures whether a person is real or fictional"@en ;
      rdfs:domain ns:Person ;
      rdfs:label "fictional"@en ;
      rdfs:range xsd:boolean .

ns:jobPosition
      a       :FunctionalProperty , owl:DatatypeProperty ;
      rdfs:comment "jobPosition describes the position a person holds at their job."@en ;
      rdfs:domain ns:Person ;
      rdfs:label "jobPosition"@en ;
      rdfs:range owl:Literal .

ns:dealTitle
      a       owl:DatatypeProperty ;
      rdfs:comment "Title of a deal or coupon."@en ;
      rdfs:domain ns:Deal ;
      rdfs:label "dealTitle"@en ;
      rdfs:range owl:Literal ;
      owl:subPropertyOf ns:label .

ns:eventParticipantAt
      a       owl:ObjectProperty ;
      rdfs:comment "Connects individuals or groups who participate in or perform at a local event to the event."@en ;
      rdfs:domain ns:Performer ;
      rdfs:label "eventParticipantAt"@en ;
      rdfs:range ns:LocalEvent ;
      :inverseOf ns:eventParticipant .

ns:outstandingShares
      a       :FunctionalProperty , owl:DatatypeProperty ;
      rdfs:comment "common shares that have been authorized, issued, and purchased by investors"@en ;
      rdfs:domain ns:Security ;
      rdfs:label "outstandingShares"@en ;
      rdfs:range xsd:float .

ns:employee
      a       owl:ObjectProperty ;
      rdfs:comment "employee connects the organization to the person it employs"@en ;
      rdfs:domain ns:Company ;
      rdfs:label "employee"@en ;
      rdfs:range ns:EmployeeAffiliation .

ns:stateLocationOf
      a       :FunctionalProperty , owl:ObjectProperty ;
      rdfs:comment "Connects an address or location with the state class."@en ;
      rdfs:domain ns:StateAdminArea ;
      rdfs:label "stateLocationOf"@en ;
      rdfs:range
              [ a       owl:Class ;
                :unionOf (ns:Address ns:Place)
              ] ;
      owl:subPropertyOf ns:location .

ns:Estate
      a       owl:Class ;
      rdfs:comment "A housing development or subdivsion known by a name Example: Winchester Ranch Mobile Home Park (San Jose) "@en , "placetype 33"@en ;
      rdfs:label "Estate"@en ;
      owl:subClassOf ns:Place .

ns:directorOf
      a       owl:ObjectProperty ;
      rdfs:comment "The directorOf property connects a director to the films, television programs, or plays that s/he has directed."@en ;
      rdfs:domain ns:Director ;
      rdfs:label "directorOf"@en ;
      rdfs:range
              [ a       owl:Class ;
                :unionOf (ns:Movie ns:TvEpisode ns:TvSeason ns:TvSeries ns:TvSpecial)
              ] ;
      :inverseOf ns:directedBy .

ns:financialInstrumentType
      a       :FunctionalProperty , owl:DatatypeProperty ;
      rdfs:comment "financialInstrumentType identifies the type of financial instrument. For example, Common Equity, Preferred Equity"@en ;
      rdfs:domain ns:FinancialInstrument ;
      rdfs:label "financialInstrumentType"@en ;
      rdfs:range owl:Literal .

ns:OtherPlace
      a       owl:Class ;
      rdfs:comment "An uncategorized place, that does not fit into any of the other classes. Example: Area 51, US Military bases."@en , "placetype: 17"@en ;
      rdfs:label "OtherPlace"@en ;
      owl:subClassOf ns:Place .

ns:freshCount
      a       :FunctionalProperty , owl:DatatypeProperty ;
      rdfs:comment "Number of reviews for a given film identified as positive (or 'fresh'), calculated by Rotten Tomatoes."@en ;
      rdfs:domain ns:RottenTomatoesReview ;
      rdfs:label "freshCount"@en ;
      rdfs:range owl:Literal ;
      owl:subPropertyOf :topDataProperty .

ns:Swap
      a       owl:Class ;
      rdfs:comment "Swap a derivative in which counterparties exchange certain benefits of one party's financial instrument for those of the other party's financial instrument"@en ;
      rdfs:label "Swap"@en ;
      owl:subClassOf ns:Derivative .

ns:listPrice
      a       :FunctionalProperty , owl:DatatypeProperty ;
      rdfs:comment "represents the real (not symbolic) price of a product or business services"@en ;
      rdfs:domain
              [ a       owl:Class ;
                :unionOf (ns:ConsumerProduct ns:LocalBusiness)
              ] ;
      rdfs:label "listPrice"@en ;
      rdfs:range xsd:float ;
      owl:subPropertyOf :topDataProperty .

ns:plays
      a       owl:ObjectProperty ;
      rdfs:comment "Connects a team to its players."@en ;
      rdfs:domain ns:TeamAffiliation ;
      rdfs:label "plays"@en ;
      rdfs:range ns:Athlete ;
      owl:subPropertyOf :topObjectProperty ;
      :inverseOf ns:playsFor .

ns:productTitleArticle
      a       :FunctionalProperty , owl:DatatypeProperty ;
      rdfs:comment "Contains the leading article of a media product title (The, A, An, etc.)."@en ;
      rdfs:domain ns:MediaProduct ;
      rdfs:label "productTitleArticle"@en ;
      rdfs:range owl:Literal ;
      owl:subPropertyOf ns:label .

ns:quotableInstrument
      a       owl:ObjectProperty ;
      rdfs:comment "quoteableInstrument connects a financial instrument to its quoteable instrument"@en ;
      rdfs:domain ns:FinancialInstrument ;
      rdfs:label "quoteableInstrument"@en ;
      rdfs:range ns:QuotableInstrument .

ns:episodeOf
      a       :FunctionalProperty , owl:ObjectProperty ;
      rdfs:comment "connects a tv episode to the tv show."@en ;
      rdfs:domain ns:TvEpisode ;
      rdfs:label "episodeOf"@en ;
      rdfs:range
              [ a       owl:Class ;
                :unionOf (ns:TvSeries ns:TvSpecial)
              ] ;
      owl:subPropertyOf :topObjectProperty .

ns:MovieTheater
      a       owl:Class ;
      rdfs:comment "A facility for the screening of films."@en ;
      rdfs:label "MovieTheater"@en ;
      owl:subClassOf ns:EventVenue .

ns:reservationSize
      a       owl:DatatypeProperty ;
      rdfs:comment "Details the reservation size allowable/required at a local business."@en ;
      rdfs:domain ns:Restaurant ;
      rdfs:label "reservationSize"@en ;
      rdfs:range xsd:int .

ns:contactAddress
      a       owl:ObjectProperty ;
      rdfs:comment "connects an organization to its contact information."@en ;
      rdfs:domain
              [ a       owl:Class ;
                :unionOf (ns:EventOrganizer ns:Organization)
              ] ;
      rdfs:label "contactInfo"@en ;
      rdfs:range ns:ContactInfo ;
      :inverseOf ns:contactInfoOf .

ns:structureName
      a       :FunctionalProperty , owl:DatatypeProperty ;
      rdfs:comment "Name of a particular structure. I.e. Palace of Auburn Hills, Superdome, PacBell Park."@en ;
      rdfs:domain ns:Structure ;
      rdfs:label "structureName"@en ;
      rdfs:range owl:Literal ;
      owl:subPropertyOf ns:name .

ns:Host
      a       owl:Class ;
      rdfs:comment "A television judge is a person who judges a televised contest, game show, or reality competition."@en ;
      rdfs:label "Host"@en ;
      owl:subClassOf ns:Person .

ns:primary
      a       :FunctionalProperty , owl:DatatypeProperty ;
      rdfs:comment "Designates whether a record is the primary value for a set of records. For instance, primary contact or phone number."@en ;
      rdfs:domain
              [ a       owl:Class ;
                :unionOf (ns:EventRegistration ns:FinancialInstrument ns:LocalBusinessCategory ns:Person ns:Phone ns:QuotableInstrument ns:Webpage)
              ] ;
      rdfs:label "primary"@en ;
      rdfs:range xsd:boolean ;
      owl:subPropertyOf :topDataProperty .

ns:compensationDate
      a       :FunctionalProperty , owl:DatatypeProperty ;
      rdfs:comment "Date upon which an person received compensation."@en ;
      rdfs:domain ns:Compensation ;
      rdfs:label "compensationDate"@en ;
      rdfs:range xsd:date ;
      owl:subPropertyOf ns:date .

ns:contactName
      a       owl:DatatypeProperty ;
      rdfs:comment "Name of the contact person for a Local Business. (SingleLocationBusiness only)"@en ;
      rdfs:domain ns:SingleLocationBusiness ;
      rdfs:label "contactName"@en ;
      rdfs:range owl:Literal .

ns:mediaTitle
      a       :FunctionalProperty , owl:DatatypeProperty ;
      rdfs:comment "The title assigned to a media work."@en ;
      rdfs:domain ns:MediaWork ;
      rdfs:label "mediaTitle" ;
      rdfs:range owl:Literal ;
      owl:subPropertyOf ns:label .

ns:RevolvingCredit
      a       owl:Class ;
      rdfs:comment "RevolvingCredit is credit that does not have a fixed number of payments"@en ;
      rdfs:label "RevolvingCredit"@en ;
      owl:subClassOf ns:ConsumerCredit .

ns:productionNumber
      a       :FunctionalProperty , owl:DatatypeProperty ;
      rdfs:comment "Production number assigned by the network to a television episiode."@en ;
      rdfs:domain ns:TvEpisode ;
      rdfs:label "productionNumber" ;
      rdfs:range owl:Literal ;
      owl:subPropertyOf :topDataProperty .

ns:Synopsis
      a       owl:Class ;
      rdfs:comment "Brief outline of the plot elements of a Media Work."@en ;
      rdfs:label "Synopsis"@en ;
      owl:subClassOf ns:Entity .

ns:BoxSet
      a       owl:Class ;
      rdfs:comment "Describes a collected set of media products."@en ;
      rdfs:label "BoxSet"@en ;
      owl:subClassOf ns:MediaProduct .

ns:religion
      a       owl:DatatypeProperty ;
      rdfs:comment "Describes the religious beliefs an individual holds. May indicate membership in a religious organization."@en ;
      rdfs:domain ns:Person ;
      rdfs:label "religion"@en ;
      rdfs:range owl:Literal ;
      owl:subPropertyOf :topDataProperty .

ns:Employee
      a       owl:Class ;
      rdfs:comment "Employee aer those people who are employed by a company."@en ;
      rdfs:label "Employee"@en ;
      owl:subClassOf ns:FinancePerson .

ns:registrationRole
      a       owl:DatatypeProperty ;
      rdfs:comment "Designates the role an event participant has registered for. May include public, media, exhibitor, etc. "@en ;
      rdfs:domain ns:EventRegistration ;
      rdfs:label "registrationRole"@en ;
      rdfs:range owl:Literal .

ns:fuelEconomyHighwayMax
      a       :FunctionalProperty , owl:DatatypeProperty ;
      rdfs:comment "Indicates the maximum fuel economy for this model for highway driving. This information is derived from trim details in the enrichment phase "@en ;
      rdfs:domain ns:AutoModel ;
      rdfs:label "fuelEconomyHighwayMax"@en ;
      rdfs:range xsd:float .

ns:TvEpisode
      a       owl:Class ;
      rdfs:comment "The Episode class includes single segments of a serialized television program."@en ;
      rdfs:label "TvEpisode"@en ;
      owl:subClassOf ns:MediaWork .

ns:sportSchedulePeriodType
      a       :FunctionalProperty , owl:DatatypeProperty ;
      rdfs:comment "Enumerated value for the type of sports scheduling period - preseason, postseason, etc. "@en ;
      rdfs:domain ns:SportSchedulePeriod ;
      rdfs:label "sportSchedulePeriodType"@en ;
      rdfs:range owl:Literal .

ns:Scientist
      a       owl:Class ;
      rdfs:comment "a scientist is an individual who uses the scientific method in his or her profession."@en ;
      rdfs:label "Scientist"@en ;
      owl:subClassOf ns:Person .

ns:teamParticipation
      a       owl:ObjectProperty ;
      rdfs:comment "Connects a sports team to the reified TeamGameRole class"@en ;
      rdfs:domain ns:SportTeam ;
      rdfs:label "teamParticipation"@en ;
      rdfs:range ns:TeamGameRole .

ns:lodgingHotelAmenities
      a       owl:DatatypeProperty ;
      rdfs:comment "Enumerates features of the hotel in general."@en ;
      rdfs:domain ns:Lodging ;
      rdfs:label "lodgingHotelAmenities"@en ;
      rdfs:range owl:Literal ;
      rdfs:range
              [ a       owl:Datatype ;
                :oneOf  [ a       rdf:List ;
                          rdf:first "AIR CONDITIONING"^^xsd:string ;
                          rdf:rest
                                  [ a       rdf:List ;
                                    rdf:first "ATM OR BANK"^^xsd:string ;
                                    rdf:rest
                                            [ a       rdf:List ;
                                              rdf:first "AV EQUIPMENT"^^xsd:string ;
                                              rdf:rest
                                                      [ a       rdf:List ;
                                                        rdf:first "BABYSITTING CHILDCARE"^^xsd:string ;
                                                        rdf:rest
                                                                [ a       rdf:List ;
                                                                  rdf:first "BUSINESS CENTER"^^xsd:string ;
                                                                  rdf:rest
                                                                          [ a       rdf:List ;
                                                                            rdf:first "CAR RENTAL"^^xsd:string ;
                                                                            rdf:rest
                                                                                    [ a       rdf:List ;
                                                                                      rdf:first "COMPLIMENTARY BREAKFAST"^^xsd:string ;
                                                                                      rdf:rest
                                                                                              [ a       rdf:List ;
                                                                                                rdf:first "COMPLIMENTARY COFFEE"^^xsd:string ;
                                                                                                rdf:rest
                                                                                                        [ a       rdf:List ;
                                                                                                          rdf:first "COMPUTER USE AVAILABLE"^^xsd:string ;
                                                                                                          rdf:rest
                                                                                                                  [ a       rdf:List ;
                                                                                                                    rdf:first "CONCIERGE SERVICES"^^xsd:string ;
                                                                                                                    rdf:rest
                                                                                                                            [ a       rdf:List ;
                                                                                                                              rdf:first "CURRENCY EXCHANGE"^^xsd:string ;
                                                                                                                              rdf:rest
                                                                                                                                      [ a       rdf:List ;
                                                                                                                                        rdf:first "DEPOSIT BOX"^^xsd:string ;
                                                                                                                                        rdf:rest
                                                                                                                                                [ a       rdf:List ;
                                                                                                                                                  rdf:first "DINING"^^xsd:string ;
                                                                                                                                                  rdf:rest
                                                                                                                                                          [ a       rdf:List ;
                                                                                                                                                            rdf:first "DOCTOR ON CALL"^^xsd:string ;
                                                                                                                                                            rdf:rest
                                                                                                                                                                    [ a       rdf:List ;
                                                                                                                                                                      rdf:first "DRY CLEANING"^^xsd:string ;
                                                                                                                                                                      rdf:rest
                                                                                                                                                                              [ a       rdf:List ;
                                                                                                                                                                                rdf:first "ELECTRONIC KEY"^^xsd:string ;
                                                                                                                                                                                rdf:rest
                                                                                                                                                                                        [ a       rdf:List ;
                                                                                                                                                                                          rdf:first "ELEVATORS"^^xsd:string ;
                                                                                                                                                                                          rdf:rest
                                                                                                                                                                                                  [ a       rdf:List ;
                                                                                                                                                                                                    rdf:first "EXPRESS CHECKOUT"^^xsd:string ;
                                                                                                                                                                                                    rdf:rest
                                                                                                                                                                                                            [ a       rdf:List ;
                                                                                                                                                                                                              rdf:first "FAX"^^xsd:string ;
                                                                                                                                                                                                              rdf:rest
                                                                                                                                                                                                                      [ a       rdf:List ;
                                                                                                                                                                                                                        rdf:first "FITNESS FACILITY"^^xsd:string ;
                                                                                                                                                                                                                        rdf:rest
                                                                                                                                                                                                                                [ a       rdf:List ;
                                                                                                                                                                                                                                  rdf:first "FRONT DESK 24HR"^^xsd:string ;
                                                                                                                                                                                                                                  rdf:rest
                                                                                                                                                                                                                                          [ a       rdf:List ;
                                                                                                                                                                                                                                            rdf:first "GIFT SHOP"^^xsd:string ;
                                                                                                                                                                                                                                            rdf:rest
                                                                                                                                                                                                                                                    [ a       rdf:List ;
                                                                                                                                                                                                                                                      rdf:first "HEARING IMPAIRED FACILITIES"^^xsd:string ;
                                                                                                                                                                                                                                                      rdf:rest
                                                                                                                                                                                                                                                              [ a       rdf:List ;
                                                                                                                                                                                                                                                                rdf:first "INTERNET ACCESS KIOSK"^^xsd:string ;
                                                                                                                                                                                                                                                                rdf:rest
                                                                                                                                                                                                                                                                        [ a       rdf:List ;
                                                                                                                                                                                                                                                                          rdf:first "LAUNDRY OR DRY CLEANING SERVICE"^^xsd:string ;
                                                                                                                                                                                                                                                                          rdf:rest
                                                                                                                                                                                                                                                                                  [ a       rdf:List ;
                                                                                                                                                                                                                                                                                    rdf:first "LAUNDRY ROOM"^^xsd:string ;
                                                                                                                                                                                                                                                                                    rdf:rest
                                                                                                                                                                                                                                                                                            [ a       rdf:List ;
                                                                                                                                                                                                                                                                                              rdf:first "MEALS"^^xsd:string ;
                                                                                                                                                                                                                                                                                              rdf:rest
                                                                                                                                                                                                                                                                                                      [ a       rdf:List ;
                                                                                                                                                                                                                                                                                                        rdf:first "MEETING FACILITIES"^^xsd:string ;
                                                                                                                                                                                                                                                                                                        rdf:rest
                                                                                                                                                                                                                                                                                                                [ a       rdf:List ;
                                                                                                                                                                                                                                                                                                                  rdf:first "MEETING ROOMS"^^xsd:string ;
                                                                                                                                                                                                                                                                                                                  rdf:rest
                                                                                                                                                                                                                                                                                                                          [ a       rdf:List ;
                                                                                                                                                                                                                                                                                                                            rdf:first "MODEMS GUEST ACCESS"^^xsd:string ;
                                                                                                                                                                                                                                                                                                                            rdf:rest
                                                                                                                                                                                                                                                                                                                                    [ a       rdf:List ;
                                                                                                                                                                                                                                                                                                                                      rdf:first "NEWSSTAND"^^xsd:string ;
                                                                                                                                                                                                                                                                                                                                      rdf:rest
                                                                                                                                                                                                                                                                                                                                              [ a       rdf:List ;
                                                                                                                                                                                                                                                                                                                                                rdf:first "PARKING"^^xsd:string ;
                                                                                                                                                                                                                                                                                                                                                rdf:rest
                                                                                                                                                                                                                                                                                                                                                        [ a       rdf:List ;
                                                                                                                                                                                                                                                                                                                                                          rdf:first "PARKING AREA WELL LIT"^^xsd:string ;
                                                                                                                                                                                                                                                                                                                                                          rdf:rest
                                                                                                                                                                                                                                                                                                                                                                  [ a       rdf:List ;
                                                                                                                                                                                                                                                                                                                                                                    rdf:first "PETS ALLOWED"^^xsd:string ;
                                                                                                                                                                                                                                                                                                                                                                    rdf:rest
                                                                                                                                                                                                                                                                                                                                                                            [ a       rdf:List ;
                                                                                                                                                                                                                                                                                                                                                                              rdf:first "PHOTOCOPY SERVICE"^^xsd:string ;
                                                                                                                                                                                                                                                                                                                                                                              rdf:rest
                                                                                                                                                                                                                                                                                                                                                                                      [ a       rdf:List ;
                                                                                                                                                                                                                                                                                                                                                                                        rdf:first "POST OR PARCEL SERVICE"^^xsd:string ;
                                                                                                                                                                                                                                                                                                                                                                                        rdf:rest
                                                                                                                                                                                                                                                                                                                                                                                                [ a       rdf:List ;
                                                                                                                                                                                                                                                                                                                                                                                                  rdf:first "RESTAURANT"^^xsd:string ;
                                                                                                                                                                                                                                                                                                                                                                                                  rdf:rest
                                                                                                                                                                                                                                                                                                                                                                                                          [ a       rdf:List ;
                                                                                                                                                                                                                                                                                                                                                                                                            rdf:first "ROOM SERVICE"^^xsd:string ;
                                                                                                                                                                                                                                                                                                                                                                                                            rdf:rest
                                                                                                                                                                                                                                                                                                                                                                                                                    [ a       rdf:List ;
                                                                                                                                                                                                                                                                                                                                                                                                                      rdf:first "SECRETARIAL SERVICE"^^xsd:string ;
                                                                                                                                                                                                                                                                                                                                                                                                                      rdf:rest
                                                                                                                                                                                                                                                                                                                                                                                                                              [ a       rdf:List ;
                                                                                                                                                                                                                                                                                                                                                                                                                                rdf:first "SECURITY 24HR"^^xsd:string ;
                                                                                                                                                                                                                                                                                                                                                                                                                                rdf:rest
                                                                                                                                                                                                                                                                                                                                                                                                                                        [ a       rdf:List ;
                                                                                                                                                                                                                                                                                                                                                                                                                                          rdf:first "SHOPS OR COMMERCIAL SERVICES"^^xsd:string ;
                                                                                                                                                                                                                                                                                                                                                                                                                                          rdf:rest
                                                                                                                                                                                                                                                                                                                                                                                                                                                  [ a       rdf:List ;
                                                                                                                                                                                                                                                                                                                                                                                                                                                    rdf:first "SMOKE ALARM IN ROOMS"^^xsd:string ;
                                                                                                                                                                                                                                                                                                                                                                                                                                                    rdf:rest
                                                                                                                                                                                                                                                                                                                                                                                                                                                            [ a       rdf:List ;
                                                                                                                                                                                                                                                                                                                                                                                                                                                              rdf:first "SPRINKLER IN ROOMS"^^xsd:string ;
                                                                                                                                                                                                                                                                                                                                                                                                                                                              rdf:rest
                                                                                                                                                                                                                                                                                                                                                                                                                                                                      [ a       rdf:List ;
                                                                                                                                                                                                                                                                                                                                                                                                                                                                        rdf:first "SWIMMING POOL"^^xsd:string ;
                                                                                                                                                                                                                                                                                                                                                                                                                                                                        rdf:rest
                                                                                                                                                                                                                                                                                                                                                                                                                                                                                [ a       rdf:List ;
                                                                                                                                                                                                                                                                                                                                                                                                                                                                                  rdf:first "TENNIS COURT"^^xsd:string ;
                                                                                                                                                                                                                                                                                                                                                                                                                                                                                  rdf:rest
                                                                                                                                                                                                                                                                                                                                                                                                                                                                                          [ a       rdf:List ;
                                                                                                                                                                                                                                                                                                                                                                                                                                                                                            rdf:first "WHEELCHAIR ACCESS"^^xsd:string ;
                                                                                                                                                                                                                                                                                                                                                                                                                                                                                            rdf:rest ()
                                                                                                                                                                                                                                                                                                                                                                                                                                                                                          ]
                                                                                                                                                                                                                                                                                                                                                                                                                                                                                ]
                                                                                                                                                                                                                                                                                                                                                                                                                                                                      ]
                                                                                                                                                                                                                                                                                                                                                                                                                                                            ]
                                                                                                                                                                                                                                                                                                                                                                                                                                                  ]
                                                                                                                                                                                                                                                                                                                                                                                                                                        ]
                                                                                                                                                                                                                                                                                                                                                                                                                              ]
                                                                                                                                                                                                                                                                                                                                                                                                                    ]
                                                                                                                                                                                                                                                                                                                                                                                                          ]
                                                                                                                                                                                                                                                                                                                                                                                                ]
                                                                                                                                                                                                                                                                                                                                                                                      ]
                                                                                                                                                                                                                                                                                                                                                                            ]
                                                                                                                                                                                                                                                                                                                                                                  ]
                                                                                                                                                                                                                                                                                                                                                        ]
                                                                                                                                                                                                                                                                                                                                              ]
                                                                                                                                                                                                                                                                                                                                    ]
                                                                                                                                                                                                                                                                                                                          ]
                                                                                                                                                                                                                                                                                                                ]
                                                                                                                                                                                                                                                                                                      ]
                                                                                                                                                                                                                                                                                            ]
                                                                                                                                                                                                                                                                                  ]
                                                                                                                                                                                                                                                                        ]
                                                                                                                                                                                                                                                              ]
                                                                                                                                                                                                                                                    ]
                                                                                                                                                                                                                                          ]
                                                                                                                                                                                                                                ]
                                                                                                                                                                                                                      ]
                                                                                                                                                                                                            ]
                                                                                                                                                                                                  ]
                                                                                                                                                                                        ]
                                                                                                                                                                              ]
                                                                                                                                                                    ]
                                                                                                                                                          ]
                                                                                                                                                ]
                                                                                                                                      ]
                                                                                                                            ]
                                                                                                                  ]
                                                                                                        ]
                                                                                              ]
                                                                                    ]
                                                                          ]
                                                                ]
                                                      ]
                                            ]
                                  ]
                        ]
              ] ;
      owl:subPropertyOf :topDataProperty .

ns:gMonthDay
      a       owl:Datatype ;
      rdfs:label "gMonthDay"@en .

ns:Ocean
      a       owl:Class ;
      rdfs:comment "placetype: 37"@en , "One of the five major bodies of water on the Earth "@en ;
      rdfs:label "Ocean"@en ;
      owl:subClassOf ns:Place .

ns:collectionDate
      a       :FunctionalProperty , owl:DatatypeProperty ;
      rdfs:comment "The date on which data was collected."@en ;
      rdfs:domain
              [ a       owl:Class ;
                :unionOf (ns:BoxOfficeAllTime ns:BoxOfficeDaily)
              ] ;
      rdfs:label "collectionDate"@en ;
      rdfs:range xsd:date ;
      owl:subPropertyOf ns:date .

ns:actorType
      a       :FunctionalProperty , owl:DatatypeProperty ;
      rdfs:comment "Describes the type of credit an actor receives (eg cameo, voice, featured, guest star)."@en ;
      rdfs:domain ns:ActingRole ;
      rdfs:label "actorType"@en ;
      rdfs:range owl:Literal ;
      owl:subPropertyOf :topDataProperty .

ns:passValidity
      a       :FunctionalProperty , owl:DatatypeProperty ;
      rdfs:comment "Indicates if passes are valid for a given film showtime, and if so, what kind of passes are allowed."@en ;
      rdfs:domain ns:MovieShowtime ;
      rdfs:label "passValidity"@en ;
      rdfs:range owl:Literal ;
      owl:subPropertyOf :topDataProperty .

ns:consumerRelatedBrandOf
      a       owl:ObjectProperty ;
      rdfs:comment "connects one sub brand to another parent brand as viewed by a consumer , for example, Gap (not Gap Inc see brandedIDOf)  to Gap Kids This is for the markup performed by Local"@en ;
      rdfs:domain ns:LocalBusiness ;
      rdfs:label "consumerRelatedBrandOf"@en ;
      rdfs:range ns:LocalBusiness ;
      :inverseOf ns:consumerRelatedBrand .

ns:datingWith
      a       :FunctionalProperty , owl:ObjectProperty ;
      rdfs:comment "The datingWith relation connects the reified Dating class to the individuals engaged in the dating courtship."@en ;
      rdfs:domain ns:Dating ;
      rdfs:label "datingWith"@en ;
      rdfs:range ns:Person .

ns:couponURL
      a       owl:DatatypeProperty ;
      rdfs:comment "URL at which coupons offered by a local business may be accessed."@en ;
      rdfs:domain ns:LocalBusiness ;
      rdfs:label "couponURL"@en ;
      rdfs:range xsd:anyURI .

ns:wifi
      a       owl:DatatypeProperty ;
      rdfs:comment "wifi contains any information regarding a business providing wifi"@en ;
      rdfs:domain ns:LocalBusiness ;
      rdfs:label "wifi"@en ;
      rdfs:range owl:Literal .

ns:currencyOf
      a       owl:ObjectProperty ;
      rdfs:comment "currencyOf connects a currency to the class that uses it"@en ;
      rdfs:domain ns:Currency ;
      rdfs:label "currencyOf"@en ;
      rdfs:range
              [ a       owl:Class ;
                :unionOf (ns:Exchange ns:Salary)
              ] .

ns:featureDisplayName
      a       owl:DatatypeProperty ;
      rdfs:comment "Represents a display oriented name of auto trim feature name. "@en ;
      rdfs:domain ns:AutoTrim ;
      rdfs:label "featureDisplayName"@en ;
      rdfs:range owl:Literal .

ns:ConsumerCredit
      a       owl:Class ;
      rdfs:comment "ConsumerCredit money, goods or services provided to an individual in lieu of payment"@en ;
      rdfs:label "ConsumerCredit"@en ;
      owl:subClassOf ns:FinancialInstrument .

ns:businessAmenity
      a       owl:DatatypeProperty ;
      rdfs:comment "businessAmenity lists those amenties that a business has"@en ;
      rdfs:domain ns:LocalBusiness ;
      rdfs:label "businessAmenity"@en ;
      rdfs:range owl:Literal .

ns:screenId
      a       :FunctionalProperty , owl:DatatypeProperty ;
      rdfs:comment "Indicates the screen(s) on which a film is playing for a particular showing."@en ;
      rdfs:domain ns:MovieShowtime ;
      rdfs:label "screenId"@en ;
      rdfs:range owl:Literal ;
      owl:subPropertyOf ns:id .

ns:abbreviation
      a       :FunctionalProperty , owl:DatatypeProperty ;
      rdfs:comment "A team abbreviation that is unique to a league "@en ;
      rdfs:domain ns:SportTeam ;
      rdfs:label "abbreviation"@en ;
      rdfs:range owl:Literal ;
      owl:subPropertyOf :topDataProperty .

ns:alternateSuffix
      a       :FunctionalProperty , owl:DatatypeProperty ;
      rdfs:comment "Alternate name suffixes by which an individual may be known."@en ;
      rdfs:domain ns:AlternatePersonName ;
      rdfs:label "alternateSuffix"@en ;
      rdfs:range owl:Literal ;
      owl:subPropertyOf ns:name .

ns:bandRoster
      a       owl:ObjectProperty ;
      rdfs:comment "The bandRoster relation connects a Music Group with the Band Affiliation of its members."@en ;
      rdfs:domain ns:MusicGroup ;
      rdfs:label "bandRoster"@en ;
      rdfs:range ns:BandAffiliation .

ns:contactURL
      a       owl:DatatypeProperty ;
      rdfs:comment "URL by which a local business can be contacted."@en ;
      rdfs:domain
              [ a       owl:Class ;
                :unionOf (ns:ContactInfo ns:LocalBusiness)
              ] ;
      rdfs:label "contactURL"@en ;
      rdfs:range xsd:anyURI .

<http://woo.corp.yahoo.com/ns/units/ft>
      a       owl:Datatype .

ns:LocalEvent
      a       owl:Class ;
      rdfs:comment "An event with relevance for a local audience. May include musical concerts, plays, standup comedy, conferences, festivals, etc."@en ;
      rdfs:label "LocalEvent"@en ;
      owl:subClassOf ns:Entity .

ns:free
      a       :FunctionalProperty , owl:DatatypeProperty ;
      rdfs:comment "Boolean attribute indicating if attendance at a Local Event Occurrence is free or paid."@en ;
      rdfs:domain
              [ a       owl:Class ;
                :unionOf (ns:EventRegistration ns:LocalEventOccurrence)
              ] ;
      rdfs:label "free"@en ;
      rdfs:range xsd:boolean .

ns:rebateAmountHigh
      a       :FunctionalProperty , owl:DatatypeProperty ;
      rdfs:comment "Represents the higher end of rebate amount if rebate amount is provided as a range. Value is 0 if rebate amount is not a range. "@en ;
      rdfs:domain ns:AutoIncentive ;
      rdfs:label "rebateAmountHigh"@en ;
      rdfs:range xsd:double .

ns:publisherOf
      a       owl:ObjectProperty ;
      rdfs:comment "Connects the Publisher class with media works it has published."@en ;
      rdfs:domain ns:Publisher ;
      rdfs:label "publisherOf"@en ;
      rdfs:range
              [ a       owl:Class ;
                :unionOf (ns:MediaWork ns:Synopsis)
              ] .

ns:upc
      a       :FunctionalProperty , owl:DatatypeProperty ;
      rdfs:comment "A universal product code (UPC) is a 12-digit barcode number used to track consumer products."@en ;
      rdfs:domain ns:ConsumerProduct ;
      rdfs:label "upc"@en ;
      rdfs:range xsd:int .

ns:categoryDepth
      a       owl:DatatypeProperty ;
      rdfs:comment "Depth of cat node, from top "@en ;
      rdfs:domain ns:BusinessListingCategory ;
      rdfs:label "categoryDepth"@en ;
      rdfs:range xsd:int ;
      owl:subPropertyOf :topDataProperty .

ns:personalRelationshipSource
      a       owl:ObjectProperty ;
      rdfs:comment "This property indicates that the given Person is the source of a directed relationship between two people. Example: in a parent-son relationship, the parent is the source, and the son is the target."@en ;
      rdfs:label "personalRelationshipSource"@en ;
      owl:subPropertyOf ns:personalRelationship .

ns:contactPerson
      a       owl:ObjectProperty ;
      rdfs:comment "Connects an organization with its contact person."@en ;
      rdfs:domain ns:Organization ;
      rdfs:label "contactPerson"@en ;
      rdfs:range ns:Person ;
      owl:subPropertyOf :topObjectProperty .

ns:teamPlayIn
      a       owl:ObjectProperty ;
      rdfs:comment "Connects the game to the teams that played in it."@en ;
      rdfs:domain ns:SportGame ;
      rdfs:label "teamPlayIn"@en ;
      rdfs:range ns:SportTeam ;
      owl:subPropertyOf :topObjectProperty ;
      :inverseOf ns:teamPlay .

ns:awayTeamId
      a       :FunctionalProperty , owl:DatatypeProperty ;
      rdfs:comment "Designates the away team of a sports game."@en ;
      rdfs:domain ns:SportGame ;
      rdfs:label "awayTeamId"@en ;
      rdfs:range owl:Literal ;
      owl:subPropertyOf ns:id .

ns:stateLocation
      a       owl:ObjectProperty ;
      rdfs:comment "Connects a state to the address or other location class."@en ;
      rdfs:domain
              [ a       owl:Class ;
                :unionOf (ns:Address ns:Place)
              ] ;
      rdfs:label "stateLocation"@en ;
      rdfs:range ns:StateAdminArea ;
      owl:subPropertyOf ns:location ;
      :inverseOf ns:stateLocationOf .

ns:ticketSenior
      a       :FunctionalProperty , owl:DatatypeProperty ;
      rdfs:comment "Describes the cost of a senior citizen's ticket at a given theater."@en ;
      rdfs:domain ns:MovieTheater ;
      rdfs:label "ticketSenior"@en ;
      rdfs:range xsd:float ;
      owl:subPropertyOf :topDataProperty .

ns:Topic
      a       owl:Class ;
      rdfs:comment "Information about a topic, taken from Wikipedia or other broad data source."@en ;
      rdfs:label "Topic"@en ;
      owl:subClassOf ns:Entity .

ns:centerLatitude
      a       :FunctionalProperty , owl:DatatypeProperty ;
      rdfs:comment "The latitude that will lead to the center point of a location."@en ;
      rdfs:domain
              [ a       owl:Class ;
                :unionOf (ns:Address ns:Place)
              ] ;
      rdfs:label "centerLatitude"@en ;
      rdfs:range xsd:float ;
      owl:subPropertyOf :topDataProperty .

ns:gameVenue
      a       :FunctionalProperty , owl:ObjectProperty ;
      rdfs:comment "Connects a SportVenue to the game played therein"@en ;
      rdfs:domain
              [ a       owl:Class ;
                :unionOf (ns:SportCompetitionInstance ns:SportGame)
              ] ;
      rdfs:label "gameVenue"@en ;
      rdfs:range ns:SportVenue .

ns:represents
      a       owl:ObjectProperty ;
      rdfs:comment "represents connects the ticker to the tradeablequoteable instrument it represents"@en ;
      rdfs:domain ns:Ticker ;
      rdfs:label "represents"@en ;
      rdfs:range ns:TQIAffiliation .

ns:Color
      a       owl:Class ;
      rdfs:comment "Represents the colors or paint available for a given trim or other product."@en ;
      rdfs:label "Color"@en ;
      owl:subClassOf ns:Entity .

ns:image
      a       owl:ObjectProperty ;
      rdfs:comment "Connects an entity with its image."@en ;
      rdfs:domain ns:Entity ;
      rdfs:label "image"@en ;
      rdfs:range ns:Image ;
      owl:subPropertyOf :topObjectProperty .

ns:yearsActive
      a       :FunctionalProperty , owl:DatatypeProperty ;
      rdfs:comment "The time span an individual, group, or other entity was active in a profession or activity"@en ;
      rdfs:domain ns:MusicArtist ;
      rdfs:label "yearsActive"@en ;
      rdfs:range owl:Literal ;
      owl:subPropertyOf :topDataProperty .

ns:BoxOfficeAllTime
      a       owl:Class ;
      rdfs:comment "The cumulative box office income for a film in theatrical release."@en ;
      rdfs:label "BoxOfficeAllTime"@en ;
      owl:subClassOf ns:BoxOffice .

ns:makeModel
      a       owl:ObjectProperty ;
      rdfs:comment "Connects the auto make class to the auto model class."@en ;
      rdfs:domain ns:AutoMake ;
      rdfs:label "makeModel"@en ;
      rdfs:range ns:AutoModel .

ns:featureCategoryList
      a       owl:DatatypeProperty ;
      rdfs:comment "Represents the list of features associated with the particular category. i.e. number of speakers "@en ;
      rdfs:domain ns:AutoTrim ;
      rdfs:label "featureCategoryList"@en ;
      rdfs:range owl:Literal .

ns:ratingElement
      a       :FunctionalProperty , owl:DatatypeProperty ;
      rdfs:comment "Product or service rating element name."@en ;
      rdfs:domain ns:Review ;
      rdfs:label "ratingElement"@en ;
      rdfs:range owl:Literal ;
      owl:subPropertyOf :topDataProperty .

ns:Salary
      a       owl:Class ;
      rdfs:comment "Salary represents the compensation type salary"@en ;
      rdfs:label "Salary"@en ;
      owl:subClassOf ns:Compensation .

ns:sportTeamPlace
      a       owl:ObjectProperty ;
      rdfs:comment "Connects a sportsteam to the place (city, state) that they represent."@en ;
      rdfs:domain ns:GeoPoliticalEntity ;
      rdfs:label "sportTeamPlace"@en ;
      rdfs:range ns:SportTeam .

ns:autoIncentive
      a       owl:ObjectProperty ;
      rdfs:comment "Connects an auto trim style to the incentive class."@en ;
      rdfs:domain ns:AutoTrim ;
      rdfs:label "autoIncentive"@en ;
      rdfs:range ns:AutoIncentive .

ns:trackingURL
      a       :FunctionalProperty , owl:DatatypeProperty ;
      rdfs:comment "tracking URL is for tracking click-thru referrals "@en ;
      rdfs:domain ns:Webpage ;
      rdfs:label "trackingURL"@en ;
      rdfs:range xsd:anyURI .

ns:fuelEconomyHighwayMin
      a       :FunctionalProperty , owl:DatatypeProperty ;
      rdfs:comment "Indicates the minimum fuel economy for this model for highway driving. This information is derived from trim details in the enrichment phase "@en ;
      rdfs:domain ns:AutoModel ;
      rdfs:label "fuelEconomyHighwayMin"@en ;
      rdfs:range xsd:float .

ns:warrantyDuration
      a       :FunctionalProperty , owl:DatatypeProperty ;
      rdfs:comment "Duration for which warranty is valid "@en ;
      rdfs:domain ns:Warranty ;
      rdfs:label "warrantyDuration"@en ;
      rdfs:range xsd:duration .

ns:warrantyCategory
      a       owl:DatatypeProperty ;
      rdfs:comment "Name of the area a warranty covers. i.e. Powertrain"@en ;
      rdfs:domain ns:Warranty ;
      rdfs:label "warrantyCategory"@en ;
      rdfs:range owl:Literal .

ns:EstablishmentShowTime
      a       owl:Class ;
      rdfs:comment "EstablishmentShowTime is a reified relationship that connects shows to the  bars, restaurants, nightclubs, etc where they occur"@en ;
      rdfs:label "EstablishmentShowTime"@en ;
      owl:subClassOf ns:LocalEventOccurrence .

ns:manages
      a       owl:ObjectProperty ;
      rdfs:comment "manages connects an organization to the exchange it manages"@en ;
      rdfs:domain ns:Company ;
      rdfs:label "manages"@en ;
      rdfs:range ns:Exchange ;
      :inverseOf ns:managedBy .

ns:submissionYUID
      a       :FunctionalProperty , owl:DatatypeProperty ;
      rdfs:comment "submisionYUID is the yahoo! id of the submitter of a businesslisting"@en ;
      rdfs:domain ns:LocalBusiness ;
      rdfs:label "submissionYUID"@en ;
      rdfs:range owl:Literal .

ns:jobTitle
      a       :FunctionalProperty , owl:DatatypeProperty ;
      rdfs:comment "jobTitle is for the title a person holds for their job"@en ;
      rdfs:domain ns:Person ;
      rdfs:label "jobTitle"@en ;
      rdfs:range owl:Literal .

ns:menuURL
      a       owl:DatatypeProperty ;
      rdfs:comment "URL at which a restaurant's menu may be accessed."@en ;
      rdfs:domain ns:Restaurant ;
      rdfs:label "menuURL"@en ;
      rdfs:range xsd:anyURI .

ns:sportSchedulePeriodOf
      a       owl:ObjectProperty ;
      rdfs:comment "connects a sport schedule period to the games or competiton instances it is related to."@en ;
      rdfs:domain ns:SportSchedulePeriod ;
      rdfs:label "sportSchedulePeriodOf"@en ;
      rdfs:range
              [ a       owl:Class ;
                :unionOf (ns:SportCompetitionInstance ns:SportGame)
              ] .

ns:endDate
      a       :FunctionalProperty , owl:DatatypeProperty ;
      rdfs:comment "The time at which an event with duration ends."@en ;
      rdfs:domain
              [ a       owl:Class ;
                :unionOf (ns:Event ns:Organization)
              ] ;
      rdfs:label "endDate"@en ;
      rdfs:range xsd:date ;
      owl:subPropertyOf ns:date .

ns:displayAddress
      a       :FunctionalProperty , owl:DatatypeProperty ;
      rdfs:comment "Full address to be displayed on SRP "@en ;
      rdfs:domain ns:Address ;
      rdfs:label "displayAddress"@en ;
      rdfs:range owl:Literal ;
      owl:subPropertyOf :topDataProperty .

ns:OrganizationStatusChange
      a       owl:Class ;
      rdfs:comment "OrganizationStatusChange is a reified class created to capture the legal status change eventsin the corporate world."@en ;
      rdfs:label "OrganizationStatusChange"@en ;
      owl:subClassOf ns:FinanceEvent .

ns:Agent
      a       owl:Class ;
      rdfs:comment "An agent is a person who provides professional representation for an individual in various entertainment fields, including television, film, music, and sports."@en ;
      rdfs:label "Agent"@en ;
      owl:subClassOf ns:Person .

ns:trackNumber
      a       :FunctionalProperty , owl:DatatypeProperty ;
      rdfs:comment "The number of the audio track, which reflects the order of the tracks on the disc."@en ;
      rdfs:domain ns:AlbumTrack ;
      rdfs:label "trackNumber"@en ;
      rdfs:range xsd:int ;
      owl:subPropertyOf :topDataProperty .

ns:eventDuration
      a       :FunctionalProperty , owl:DatatypeProperty ;
      rdfs:comment "Length of time an event lasts."@en ;
      rdfs:domain ns:Event ;
      rdfs:label "eventDuration"@en ;
      rdfs:range xsd:duration .

ns:eventGuestParticipant
      a       owl:ObjectProperty ;
      rdfs:comment "Connects an event ocurrence to a guest or featured participant."@en ;
      rdfs:domain ns:LocalEventOccurrence ;
      rdfs:label "eventGuestParticipant"@en ;
      rdfs:range ns:Performer ;
      :inverseOf ns:eventGuestParticipantAt .

ns:cumulativeReceipt
      a       :FunctionalProperty , owl:DatatypeProperty ;
      rdfs:comment "Cumulative box office receipts."@en ;
      rdfs:domain ns:BoxOfficeAllTime ;
      rdfs:label "cumulativeReceipt"@en ;
      rdfs:range xsd:float ;
      owl:subPropertyOf :topDataProperty .

ns:minValue
      a       :FunctionalProperty , owl:DatatypeProperty ;
      rdfs:comment "Minimum value of a deal or offer."@en ;
      rdfs:domain ns:Deal ;
      rdfs:label "minValue"@en ;
      rdfs:range xsd:float .

ns:produced
      a       owl:ObjectProperty ;
      rdfs:comment "The produced property connects a producer with media artworks that s/he has produced."@en ;
      rdfs:domain ns:Producer ;
      rdfs:label "produced"@en ;
      rdfs:range
              [ a       owl:Class ;
                :unionOf (ns:Album ns:Movie ns:Song ns:TvEpisode ns:TvSeason ns:TvSeries ns:TvSpecial)
              ] ;
      :inverseOf ns:producedBy .

ns:displayName
      a       :FunctionalProperty , owl:DatatypeProperty ;
      rdfs:comment "Describes the display name of an entity."@en , "For Sports teams, a unique, recognizable team name typically derived from teamFirstName, teamNickname, or both. I.e. Los Angeles Lakers, Arsenal."@en ;
      rdfs:domain
              [ a       owl:Class ;
                :unionOf (ns:OnlineAccount ns:Organization)
              ] ;
      rdfs:label "displayName"@en ;
      rdfs:range owl:Literal ;
      owl:subPropertyOf ns:name .

ns:funding
      a       owl:DatatypeProperty ;
      rdfs:comment "Describes the funding at an educational institution."@en ;
      rdfs:domain ns:EducationalInstitution ;
      rdfs:label "funding"@en ;
      rdfs:range owl:Literal .

ns:numTeacher
      a       owl:DatatypeProperty ;
      rdfs:comment "Indicates the number of teachers at an educational institution."@en ;
      rdfs:domain ns:EducationalInstitution ;
      rdfs:label "numTeacher"@en ;
      rdfs:range xsd:int .

<http://woo.corp.yahoo.com/ns/units/oz>
      a       owl:Datatype .

ns:ContestJudge
      a       owl:Class ;
      rdfs:comment "A television judge is a person who judges a televised contest, game show, or reality competition."@en ;
      rdfs:label "ContestJudge"@en ;
      owl:subClassOf ns:Person .

ns:quotableInstrumentStatus
      a       :FunctionalProperty , owl:DatatypeProperty ;
      rdfs:comment "quoteableInstrument status is the status of a quotable instrument"@en ;
      rdfs:domain ns:QuotableInstrument ;
      rdfs:label "quotableInstrumentStatus"@en ;
      rdfs:range owl:Literal .

ns:musicPerformance
      a       owl:ObjectProperty ;
      rdfs:comment "Connects a musical work to a particular performance."@en ;
      rdfs:domain
              [ a       owl:Class ;
                :unionOf (ns:Composition ns:CompositionPart ns:Song)
              ] ;
      rdfs:label "musicPerformance"@en ;
      rdfs:range ns:MusicPerformance ;
      owl:subPropertyOf :topObjectProperty ;
      :inverseOf ns:musicPerformanceOf .

ns:review
      a       owl:ObjectProperty ;
      rdfs:comment "Connects an entity to its critical review."@en ;
      rdfs:domain
              [ a       owl:Class ;
                :unionOf (ns:LocalBusiness ns:MediaWork)
              ] ;
      rdfs:label "review"@en ;
      rdfs:range ns:Review ;
      owl:subPropertyOf :topObjectProperty ;
      :inverseOf ns:reviewOf .

ns:MarketTier
      a       owl:Class ;
      rdfs:comment "MarketTier tiers and exchange uses for different markets"@en ;
      rdfs:label "MarketTier"@en ;
      owl:subClassOf ns:Entity .

ns:ageRestrictionDesc
      a       :FunctionalProperty , owl:DatatypeProperty ;
      rdfs:comment "Describes any age restrictions applicable for access to a local business, e.g. 21 and over, 18 and over, all ages, etc."@en ;
      rdfs:domain
              [ a       owl:Class ;
                :unionOf (ns:LocalBusiness ns:LocalEvent)
              ] ;
      rdfs:label "ageRestrictionDesc"@en ;
      rdfs:range owl:Literal .

ns:kioskForTicketPickup
      a       :FunctionalProperty , owl:DatatypeProperty ;
      rdfs:comment "Offers patrons the option to purchase tickets online and pick up at the theater via kiosk."@en ;
      rdfs:domain ns:MovieTheater ;
      rdfs:label "kioskForTicketPickup"@en ;
      rdfs:range xsd:boolean .

ns:Category
      a       owl:Class ;
      rdfs:comment "Category is for those classes that contain classification information for a domain."@en ;
      rdfs:label "Category"@en ;
      owl:subClassOf ns:CategoryAndGenre .

ns:imageSize
      a       owl:DatatypeProperty ;
      rdfs:comment "Enumerates the image sizes possible."@en ;
      rdfs:domain ns:Image ;
      rdfs:label "imageSize"@en ;
      rdfs:range owl:Literal ;
      rdfs:range
              [ a       owl:Datatype ;
                :oneOf  [ a       rdf:List ;
                          rdf:first "FULL"^^xsd:string ;
                          rdf:rest
                                  [ a       rdf:List ;
                                    rdf:first "LARGE"^^xsd:string ;
                                    rdf:rest
                                            [ a       rdf:List ;
                                              rdf:first "MEDIUM"^^xsd:string ;
                                              rdf:rest
                                                      [ a       rdf:List ;
                                                        rdf:first "ORIGINAL"^^xsd:string ;
                                                        rdf:rest
                                                                [ a       rdf:List ;
                                                                  rdf:first "THUMB"^^xsd:string ;
                                                                  rdf:rest ()
                                                                ]
                                                      ]
                                            ]
                                  ]
                        ]
              ] ;
      owl:subPropertyOf :topDataProperty .

ns:superMake
      a       :FunctionalProperty , owl:DatatypeProperty ;
      rdfs:comment "List of munged names of super models associated with make (if any) This information is derived from model details in the enrichment phase "@en ;
      rdfs:domain ns:AutoMake ;
      rdfs:label "superMake"@en ;
      rdfs:range owl:Literal ;
      owl:subPropertyOf :topDataProperty .

ns:attendable
      a       :FunctionalProperty , owl:DatatypeProperty ;
      rdfs:comment "Describes if an event may be attended."@en ;
      rdfs:domain ns:LocalEvent ;
      rdfs:label "attendable"@en ;
      rdfs:range xsd:boolean .

ns:legged
      a       :FunctionalProperty , owl:DatatypeProperty ;
      rdfs:comment "Designates whether an athlete is right or left legged."@en ;
      rdfs:domain ns:Athlete ;
      rdfs:label "legged"@en ;
      rdfs:range owl:Literal ;
      owl:subPropertyOf :topDataProperty .

ns:marketServed
      a       owl:DatatypeProperty ;
      rdfs:comment "Describes the local market served by a business."@en ;
      rdfs:domain ns:LocalBusiness ;
      rdfs:label "marketServed"@en ;
      rdfs:range owl:Literal .

ns:Event
      a       owl:Class ;
      rdfs:comment "An event is a topic that can be described by the time or date at which it happened. Long-lasting events may be described as occurring between two dates."@en ;
      rdfs:label "Event"@en ;
      owl:subClassOf ns:Entity .

ns:menuImage
      a       owl:DatatypeProperty ;
      rdfs:comment "Contains image info for restaurant menu items."@en ;
      rdfs:domain ns:Restaurant ;
      rdfs:label "menuImage"@en ;
      rdfs:range owl:Literal .

ns:ticketAvailability
      a       owl:DatatypeProperty ;
      rdfs:comment "Indicates if tickets are available for a Local Event Occurrence."@en ;
      rdfs:domain ns:LocalEventOccurrence ;
      rdfs:label "ticketAvailability"@en ;
      rdfs:range xsd:boolean .

ns:exchangeType
      a       :FunctionalProperty , owl:DatatypeProperty ;
      rdfs:comment "exchangeType refers what type an exchange is"@en ;
      rdfs:domain ns:Exchange ;
      rdfs:label "exchangeType"@en ;
      rdfs:range owl:Literal .

ns:language
      a       owl:DatatypeProperty ;
      rdfs:comment "For organizations, the languages in which an org operates. For media works, the language in which the work's dialogue is spoken. Should conform to ISO codes."@en ;
      rdfs:domain
              [ a       owl:Class ;
                :unionOf (ns:MediaWork ns:Organization)
              ] ;
      rdfs:label "language"@en ;
      rdfs:range owl:Literal .

ns:majorShareholder
      a       owl:ObjectProperty ;
      rdfs:comment "majorShareholderOf connects a financial instrument to the majorshareholder affiliation"@en ;
      rdfs:domain ns:FinancialInstrument ;
      rdfs:label "majorShareholder"@en ;
      rdfs:range ns:MajorShareholderAffiliation ;
      :inverseOf ns:majorShareholderOf .

ns:personalRelationshipWith
      a       :FunctionalProperty , owl:ObjectProperty ;
      rdfs:comment "Connects the reified PersonalRelationship class to a person."@en ;
      rdfs:domain ns:PersonalRelationship ;
      rdfs:label "personalRelationshipWith"@en ;
      rdfs:range ns:Person ;
      owl:subPropertyOf :topObjectProperty .

ns:Friendship
      a       owl:Class ;
      rdfs:comment "Reified class connecting individuals who share a platonic relationship."@en ;
      rdfs:label "Friendship"@en ;
      owl:subClassOf ns:PersonalRelationship .

ns:showingWith
      a       :SymmetricProperty , owl:ObjectProperty ;
      rdfs:comment "Connects showtimes for films that are screened together."@en ;
      rdfs:domain ns:MovieShowtime ;
      rdfs:label "showingWith"@en ;
      rdfs:range ns:MovieShowtime ;
      owl:subPropertyOf :topObjectProperty .

ns:msrpMin
      a       :FunctionalProperty , owl:DatatypeProperty ;
      rdfs:comment "Indicates the minimum msrp for this model. This information is derived from trim details in the enrichment phase "@en ;
      rdfs:domain ns:AutoModel ;
      rdfs:label "msrpMin"@en ;
      rdfs:range xsd:float .

ns:narrowerEvent
      a       owl:ObjectProperty ;
      rdfs:comment "Connects a parent event with its narrower, child event(s)."@en ;
      rdfs:domain ns:LocalEvent ;
      rdfs:label "narrowerEvent"@en ;
      rdfs:range ns:LocalEvent .

ns:ticker
      a       owl:ObjectProperty ;
      rdfs:comment "ticker connects a tradablequotable instrument to its ticker"@en ;
      rdfs:domain ns:TradableQuotableInstrument ;
      rdfs:label "ticker"@en ;
      rdfs:range ns:TQIAffiliation ;
      :inverseOf ns:tickerOf .

ns:releaseTitle
      a       :FunctionalProperty , owl:DatatypeProperty ;
      rdfs:comment "Stores the release title of a media release if is different from the canonical media work (Tangled IMAX 3D vs. Tangled). Distinct from alternate title as both movie names are valid release names used for display when showing movies playing in theaters. "@en ;
      rdfs:domain ns:MediaRelease ;
      rdfs:label "releaseTitle"@en ;
      rdfs:range owl:Literal ;
      owl:subPropertyOf ns:label .

ns:onlineAccount
      a       owl:ObjectProperty ;
      rdfs:comment "Connects a thing to its online account."@en ;
      rdfs:domain
              [ a       owl:Class ;
                :unionOf (ns:MusicArtist ns:Organization ns:Performer ns:Person)
              ] ;
      rdfs:label "onlineAccount"@en ;
      rdfs:range ns:OnlineAccount ;
      owl:subPropertyOf :topObjectProperty ;
      :inverseOf ns:onlineAccountOf .

ns:containsLandmark
      a       owl:ObjectProperty ;
      rdfs:comment "containsLandmark connects a place or local business to the landmarks it contains (place or local business) for example Yosemite contains Yosemite Falls or Stanford University contains the Rodin Sculpture Garden."@en ;
      rdfs:domain
              [ a       owl:Class ;
                :unionOf (ns:LocalBusiness ns:Place)
              ] ;
      rdfs:label "containsLandmark"@en ;
      rdfs:range
              [ a       owl:Class ;
                :unionOf (ns:LocalBusiness ns:Place)
              ] ;
      :inverseOf ns:landmarkWithin .

ns:AutoMake
      a       owl:Class ;
      rdfs:comment "An automotive make is a specific car line a manufacturer produces. For example, Pontiac, Chevrolet, Audi and Volkswagen are all makes. "@en ;
      rdfs:label "AutoMake"@en ;
      owl:subClassOf ns:Entity .

ns:marketTierOf
      a       owl:ObjectProperty ;
      rdfs:comment "marketTierOf connects a market tier to the exchange to which it belongs"@en ;
      rdfs:domain ns:MarketTier ;
      rdfs:label "marketTierOf"@en ;
      rdfs:range ns:Exchange .

ns:lastRenovationDate
      a       :FunctionalProperty , owl:DatatypeProperty ;
      rdfs:comment "date the facility was last renovated"@en ;
      rdfs:domain ns:Lodging ;
      rdfs:label "lastRenovationDate"@en ;
      rdfs:range xsd:date ;
      owl:subPropertyOf ns:date .

ns:price
      a       :FunctionalProperty , owl:DatatypeProperty ;
      rdfs:comment "Indicates the price of a product or service."@en ;
      rdfs:domain
              [ a       owl:Class ;
                :unionOf (ns:ConsumerProduct ns:Deal ns:EventRegistration ns:LocalEventOccurrence)
              ] ;
      rdfs:label "price"@en ;
      rdfs:range owl:Literal .

ns:student
      a       owl:ObjectProperty ;
      rdfs:comment "Connects an educational institution with the Education class."@en ;
      rdfs:domain ns:EducationalInstitution ;
      rdfs:label "student"@en ;
      rdfs:range ns:Education ;
      owl:subPropertyOf :topObjectProperty ;
      :inverseOf ns:studentOf .

ns:jobHeldBy
      a       :FunctionalProperty , owl:ObjectProperty ;
      rdfs:comment "Connects the reified Occupational History class to a person."@en ;
      rdfs:domain ns:OccupationalHistory ;
      rdfs:label "jobHeldBy"@en ;
      rdfs:range ns:Person ;
      owl:subPropertyOf :topObjectProperty ;
      :inverseOf ns:jobHeld .

ns:distributed
      a       owl:ObjectProperty ;
      rdfs:comment "The distributed property connects a media distribution organization with media titles that it has distributed."@en ;
      rdfs:domain ns:TheatricalDistributor ;
      rdfs:label "distributed"@en ;
      rdfs:range
              [ a       owl:Class ;
                :unionOf (ns:MediaProduct ns:Movie ns:TvEpisode ns:TvSeason ns:TvSeries ns:TvSpecial)
              ] .

ns:summaryText
      a       :FunctionalProperty , owl:DatatypeProperty ;
      rdfs:comment "summaryText is the text that summarizes an organization's profile"@en ;
      rdfs:domain ns:Organization ;
      rdfs:label "summaryText"@en ;
      rdfs:range owl:Literal .

ns:discount
      a       owl:DatatypeProperty ;
      rdfs:comment "discounted price of an offer or deal."@en ;
      rdfs:domain ns:Deal ;
      rdfs:label "discount"@en ;
      rdfs:range owl:Literal .

ns:franchiseCodePrimary
      a       :FunctionalProperty , owl:DatatypeProperty ;
      rdfs:comment "Primary local listing franchise code. Indicates the franchise status/affiliation. (for SingleLocationBusiness only)"@en ;
      rdfs:domain ns:SingleLocationBusiness ;
      rdfs:label "franchiseCodePrimary"@en ;
      rdfs:range owl:Literal .

ns:cuisine
      a       owl:DatatypeProperty ;
      rdfs:comment "The various kind of food served. Precise item should go in menuItem"@en ;
      rdfs:domain
              [ a       owl:Class ;
                :unionOf (ns:EventVenue ns:Restaurant)
              ] ;
      rdfs:label "cuisine"@en ;
      rdfs:range owl:Literal ;
      owl:subPropertyOf :topDataProperty .

ns:productType
      a       owl:ObjectProperty ;
      rdfs:comment "Connects a media work to its consumer product type."@en ;
      rdfs:domain ns:MediaWork ;
      rdfs:label "productType"@en ;
      rdfs:range ns:MediaProduct ;
      owl:subPropertyOf :topObjectProperty .

ns:degree
      a       :FunctionalProperty , owl:DatatypeProperty ;
      rdfs:comment "Describes an educational degree awarded to an individual."@en ;
      rdfs:domain ns:Education ;
      rdfs:label "degree"@en ;
      rdfs:range owl:Literal ;
      owl:subPropertyOf :topDataProperty .

ns:recurrence
      a       owl:DatatypeProperty ;
      rdfs:comment "Specific date and/or time on which an event recurs."@en ;
      rdfs:domain ns:Event ;
      rdfs:label "recurrence"@en ;
      rdfs:range owl:Literal .

<http://woo.corp.yahoo.com/ns/units/mi>
      a       owl:Datatype .

ns:keyword
      a       owl:DatatypeProperty ;
      rdfs:comment "Array of specific keyword names (string) and their weights."@en , "Added for Local BusinessListingCategory. This connects to the providerCategory property."@en ;
      rdfs:domain
              [ a       owl:Class ;
                :unionOf (ns:BusinessListingCategory ns:Image ns:LocalBusiness ns:LocalEvent ns:Performer ns:SingleLocationBusiness)
              ] ;
      rdfs:label "keyword"@en ;
      rdfs:range owl:Literal ;
      owl:subPropertyOf :topDataProperty .

ns:topicName
      a       owl:DatatypeProperty ;
      rdfs:comment "Canonical name of a topic."@en ;
      rdfs:domain ns:Topic ;
      rdfs:label "topicName"@en ;
      rdfs:range owl:Literal ;
      owl:subPropertyOf ns:name .

ns:DomesticUnion
      a       owl:Class ;
      rdfs:comment "A domestic partnership is a personal relationship between two individuals who live together and share a common domestic life but are neither joined by marriage nor a civil union."@en ;
      rdfs:label "DomesticUnion"@en ;
      owl:subClassOf ns:PersonalRelationship .

ns:productName
      a       :FunctionalProperty , owl:DatatypeProperty ;
      rdfs:comment "Trademarked name by which a consumer product is known."@en ;
      rdfs:domain ns:ConsumerProduct ;
      rdfs:label "productName"@en ;
      rdfs:range owl:Literal ;
      owl:subPropertyOf ns:name .

ns:rawFeedDataRank
      a       owl:DatatypeProperty ;
      rdfs:comment "Captures feed ranking. Can be scaled across providers and can be used for ranking in the search results. Not for display."@en ;
      rdfs:domain ns:Entity ;
      rdfs:label "rawFeedDataRank"@en ;
      rdfs:range owl:Literal .

ns:merchantUrl
      a       owl:DatatypeProperty ;
      rdfs:comment "URL for a merchant offering a deal."@en ;
      rdfs:domain ns:DealMerchant ;
      rdfs:label "merchantUrl"@en ;
      rdfs:range owl:Literal .

ns:composedBy
      a       owl:ObjectProperty ;
      rdfs:comment "Connects a composition to its composer"@en ;
      rdfs:domain
              [ a       owl:Class ;
                :unionOf (ns:Composition ns:Song)
              ] ;
      rdfs:label "composedBy"@en ;
      rdfs:range ns:Composer ;
      owl:subPropertyOf :topObjectProperty .

ns:cafeOnPremises
      a       :FunctionalProperty , owl:DatatypeProperty ;
      rdfs:comment "Indicates the presence of a cafe on a venue's premises."@en ;
      rdfs:domain ns:MovieTheater ;
      rdfs:label "cafeOnPremises"@en ;
      rdfs:range xsd:boolean .

ns:employeeOf
      a       owl:ObjectProperty ;
      rdfs:comment "employeeOf connects a person to an org of which they are an employee"@en ;
      rdfs:domain ns:EmployeeAffiliation ;
      rdfs:label "employeeOf"@en ;
      rdfs:range ns:Company ;
      :inverseOf ns:employee .

ns:height
      a       :FunctionalProperty , owl:DatatypeProperty ;
      rdfs:comment "The length of a person's body, typically measured by an individual's vertical distance from the ground."@en ;
      rdfs:domain ns:Person ;
      rdfs:label "height"@en ;
      rdfs:range xsd:float ;
      owl:subPropertyOf :topDataProperty .

ns:influencedBy
      a       owl:ObjectProperty ;
      rdfs:comment "Connects an individual with other individuals who have had a a professional or personal influence on that person."@en ;
      rdfs:domain ns:Person ;
      rdfs:label "influencedBy"@en ;
      rdfs:range ns:Person ;
      owl:subPropertyOf :topObjectProperty .

ns:birthLocation
      a       :FunctionalProperty , owl:ObjectProperty ;
      rdfs:comment "birthLocation connects an individual to the place where s/he was born."@en ;
      rdfs:domain ns:Person ;
      rdfs:label "birthLocation"@en ;
      rdfs:range ns:Place ;
      owl:subPropertyOf ns:location .

ns:PublicCompany
      a       owl:Class ;
      rdfs:comment "PublicCompany are those companies who sell shares of thier stock to the public."@en ;
      rdfs:label "PublicCompany"@en ;
      owl:subClassOf ns:Company .

ns:subcategoryName
      a       owl:DatatypeProperty ;
      rdfs:domain ns:Deal ;
      rdfs:label "subcategoryName"@en ;
      rdfs:range owl:Literal ;
      owl:subPropertyOf ns:name .

ns:Derivative
      a       owl:Class ;
      rdfs:comment "Derivative is the class of those financial instruments that have a value based on the expected future price movements of the asset to which it is linked"@en ;
      rdfs:label "Derivative"@en ;
      owl:subClassOf ns:FinancialInstrument .

ns:movieContributor
      a       owl:ObjectProperty ;
      rdfs:comment "Connects a film to any of the people involved in its making, including those whose contribution is unclear."@en ;
      rdfs:domain ns:Movie ;
      rdfs:label "movieContributor"@en ;
      rdfs:range ns:Person ;
      owl:subPropertyOf :topObjectProperty ;
      :inverseOf ns:movieContributorFor .

ns:MusicArtist
      a       owl:Class ;
      rdfs:comment "An individual or group that produces music."@en ;
      rdfs:label "MusicArtist"@en ;
      owl:subClassOf ns:Entity .

ns:maxPrice
      a       owl:DatatypeProperty ;
      rdfs:comment "Indicates the maximum price of a product or service."@en ;
      rdfs:domain
              [ a       owl:Class ;
                :unionOf (ns:Deal ns:EventRegistration ns:LocalEventOccurrence)
              ] ;
      rdfs:label "maxPrice"@en ;
      rdfs:range xsd:int .

ns:nominationYear
      a       :FunctionalProperty , owl:DatatypeProperty ;
      rdfs:comment "The year in which an individual, organization, or media work is nominated for an award."@en ;
      rdfs:domain ns:Nomination ;
      rdfs:label "nominationYear"@en ;
      rdfs:range xsd:gYear ;
      owl:subPropertyOf ns:date .

ns:topicOf
      a       owl:ObjectProperty ;
      rdfs:comment "Connects an entity to topic data."@en ;
      rdfs:domain ns:Entity ;
      rdfs:label "topicOf"@en ;
      rdfs:range ns:Topic ;
      :inverseOf ns:topic .

ns:TradableQuotableInstrument
      a       owl:Class ;
      rdfs:comment "TradeableQuotableInstrument is the symbols by which a financial instrument is tradedon any particular exchange."@en ;
      rdfs:label "TradeableQuoteableInstrument"@en ;
      owl:subClassOf ns:QuotableInstrument .

ns:TvNetwork
      a       owl:Class ;
      rdfs:comment "A company that creates and broadcasts television content."@en ;
      rdfs:label "TvNetwork"@en ;
      owl:subClassOf ns:Company .

ns:ncesURL
      a       owl:DatatypeProperty ;
      rdfs:comment "URL at which the National Center for Education Statistics information for an educational institution may be accessed."@en ;
      rdfs:domain ns:EducationalInstitution ;
      rdfs:label "ncesURL"@en ;
      rdfs:range xsd:anyURI .

ns:BandAffiliation
      a       owl:Class ;
      rdfs:comment "The BandAffiliation class is a reified relationship that connects a music group with the music artists that comprise it."@en ;
      rdfs:label "BandAffiliation"@en ;
      owl:subClassOf ns:Event .

ns:BankNote
      a       owl:Class ;
      rdfs:comment "Bank Note is a kind of negotiable instrument, a promissory note made by a bank payable to the bearer on demand"@en ;
      rdfs:label "BankNote"@en ;
      owl:subClassOf ns:Debt .

ns:IndividualPerformer
      a       owl:Class ;
      rdfs:comment "An individual who performs at a local event."@en ;
      rdfs:label "IndividualPerformer"@en ;
      owl:subClassOf
              [ a       owl:Class ;
                :intersectionOf (ns:Performer ns:Person)
              ] .

ns:ticketChild
      a       :FunctionalProperty , owl:DatatypeProperty ;
      rdfs:comment "Describes the cost of a child's ticket at a given theater."@en ;
      rdfs:domain ns:MovieTheater ;
      rdfs:label "ticketChild"@en ;
      rdfs:range xsd:float ;
      owl:subPropertyOf :topDataProperty .

ns:updatedOn
      a       :FunctionalProperty , owl:DatatypeProperty ;
      rdfs:comment "Local listing source data indicating update date of the record (for use with SingleLocationBusiness only)."@en ;
      rdfs:domain ns:LocalBusiness ;
      rdfs:label "updatedOn"@en ;
      rdfs:range owl:Literal .

ns:primaryUrlScore
      a       :FunctionalProperty , owl:DatatypeProperty ;
      rdfs:comment "Primary url score"@en ;
      rdfs:domain ns:Webpage ;
      rdfs:label "primaryUrlScore" ;
      rdfs:range xsd:int ;
      owl:subPropertyOf :topDataProperty .

ns:eventOffer
      a       owl:DatatypeProperty ;
      rdfs:comment "Text value of special offers available from an Event Registration service, for particular events."@en ;
      rdfs:domain ns:EventRegistration ;
      rdfs:label "eventOffer"@en ;
      rdfs:range owl:Literal .

ns:alias
      a       owl:DatatypeProperty ;
      rdfs:comment "Alternate name by which an entity may be known. Suitable for unparsed data only. Normalized data should use either AlternatePersonName Class or alternateOrgName data property."@en ;
      rdfs:domain
              [ a       owl:Class ;
                :unionOf (ns:EventOrganizer ns:Performer ns:Topic)
              ] ;
      rdfs:label "alias"@en ;
      rdfs:range owl:Literal ;
      owl:subPropertyOf ns:name .

ns:manufacturer
      a       owl:ObjectProperty ;
      rdfs:comment "Connects a product with the company that manufactures it."@en ;
      rdfs:domain
              [ a       owl:Class ;
                :unionOf (ns:AutoMake ns:ConsumerProduct)
              ] ;
      rdfs:label "manufacturer"@en ;
      rdfs:range ns:Company .

ns:degreeYear
      a       :FunctionalProperty , owl:DatatypeProperty ;
      rdfs:comment "The year in which a degree was awarded."@en ;
      rdfs:domain ns:Education ;
      rdfs:label "degreeYear"@en ;
      rdfs:range xsd:gYear ;
      owl:subPropertyOf ns:date .

ns:eventGuestParticipantAt
      a       owl:ObjectProperty ;
      rdfs:comment "Connects a featured or guest participant with the event ocurrence at which he/she/it is featured."@en ;
      rdfs:domain ns:Performer ;
      rdfs:label "eventGuestParticipantAt"@en ;
      rdfs:range ns:LocalEventOccurrence .

ns:compensation
      a       owl:ObjectProperty ;
      rdfs:comment "compensation connects a financial person to the type of compensation they receive."@en ;
      rdfs:domain ns:FinancePerson ;
      rdfs:label "compensation"@en ;
      rdfs:range ns:Compensation ;
      :inverseOf ns:compensationOf .

ns:alternateTitle
      a       owl:ObjectProperty ;
      rdfs:comment "Connects a media work to the reified alternate title class."@en ;
      rdfs:domain ns:MediaWork ;
      rdfs:label "alternateTitle"@en ;
      rdfs:range ns:AlternateTitle ;
      owl:subPropertyOf :topObjectProperty .

ns:reportTemplate
      a       :FunctionalProperty , owl:DatatypeProperty ;
      rdfs:comment "reportTemplate is the template in which a company's financials were collected "@en ;
      rdfs:domain ns:Organization ;
      rdfs:label "reportTemplate"@en ;
      rdfs:range owl:Literal .

ns:recordingLocation
      a       owl:ObjectProperty ;
      rdfs:comment "Location where and album or track or song was recorded. Should conform to ISO codes."@en ;
      rdfs:domain
              [ a       owl:Class ;
                :unionOf (ns:Album ns:Composition ns:Song)
              ] ;
      rdfs:label "recordingLocation"@en ;
      rdfs:range ns:Place ;
      owl:subPropertyOf ns:location .

ns:showComment
      a       owl:DatatypeProperty ;
      rdfs:comment "Descriptive commentary about a film showing, as provided by the theater."@en ;
      rdfs:domain ns:MovieShowtime ;
      rdfs:label "showComment"@en ;
      rdfs:range owl:Literal ;
      owl:subPropertyOf :topDataProperty .

ns:woeId
      a       :FunctionalProperty , owl:DatatypeProperty ;
      rdfs:comment "Unique identifier assigned to a place by Where on Earth. WOE types include: Town, Zip, State, County, Colloquial, Time Zone, POI, Land feature, DMA, MMA, and Country"@en ;
      rdfs:domain
              [ a       owl:Class ;
                :unionOf (ns:EventVenue ns:Place)
              ] ;
      rdfs:label "woeId"@en ;
      rdfs:range owl:Literal ;
      owl:subPropertyOf ns:id .

ns:primaryExchange
      a       :FunctionalProperty , owl:DatatypeProperty ;
      rdfs:comment "primaryExchange is the primary exchange upon which a publicly traded company trades."@en ;
      rdfs:domain ns:PublicCompany ;
      rdfs:label "primaryExchange"@en ;
      rdfs:range owl:Literal .

ns:altitude
      a       owl:DatatypeProperty ;
      rdfs:comment "Captures a place's height above sea level."@en ;
      rdfs:domain
              [ a       owl:Class ;
                :unionOf (ns:EventVenue ns:Place)
              ] ;
      rdfs:label "altitude"@en ;
      rdfs:range xsd:int .

ns:replacedBy
      a       :FunctionalProperty , owl:DatatypeProperty ;
      rdfs:comment "Where On Earth Identifier of the place that replaces the place "@en ;
      rdfs:domain ns:Place ;
      rdfs:label "replacedBy"@en ;
      rdfs:range owl:Literal .

ns:dataSource
      a       :FunctionalProperty , owl:DatatypeProperty ;
      rdfs:comment " Source of this data. Can be either the provider name ('infobel', 'infousa', etc) or the site where this data is extracted (www.somewhere.com, for example)."@en ;
      rdfs:domain ns:Webpage ;
      rdfs:label "dataSource"@en ;
      rdfs:range owl:Literal ;
      owl:subPropertyOf :topDataProperty .

ns:metaKeywords
      a       owl:DatatypeProperty ;
      rdfs:comment "Meta-keywords for a website."@en ;
      rdfs:domain ns:Webpage ;
      rdfs:label "metaKeywords"@en ;
      rdfs:range owl:Literal ;
      owl:subPropertyOf :topDataProperty .

ns:eventOrganizerOf
      a       owl:ObjectProperty ;
      rdfs:comment "Connects an event organizer to events that it has arranged or sponsored."@en ;
      rdfs:domain ns:EventOrganizer ;
      rdfs:label "eventOrganizerOf"@en ;
      rdfs:range ns:LocalEvent ;
      :inverseOf ns:eventOrganizer .

ns:startTime
      a       :FunctionalProperty , owl:DatatypeProperty ;
      rdfs:comment "The time at which an event begins."@en ;
      rdfs:domain ns:Event ;
      rdfs:label "startTime"@en ;
      rdfs:range xsd:time ;
      owl:subPropertyOf :topDataProperty .

ns:eventCategory
      a       owl:DatatypeProperty ;
      rdfs:comment "Designates the categories into which an event may be classified."@en ;
      rdfs:domain ns:LocalEvent ;
      rdfs:label "eventCategory"@en ;
      rdfs:range owl:Literal .

ns:holidayWeekend
      a       :FunctionalProperty , owl:DatatypeProperty ;
      rdfs:comment "Indicates if a period for which box office receipts was recorded is a holiday weekend."@en ;
      rdfs:domain
              [ a       owl:Class ;
                :unionOf (ns:BoxOfficeDaily ns:BoxOfficeWeekend ns:BoxOfficeWeekly)
              ] ;
      rdfs:label "holidayWeekend"@en ;
      rdfs:range owl:Literal ;
      owl:subPropertyOf :topDataProperty .

ns:boardMemberList
      a       owl:DatatypeProperty ;
      rdfs:comment "boardMemberList are allthose who are on the board of a company"@en ;
      rdfs:domain
              [ a       owl:Class ;
                :unionOf (ns:Company ns:Exchange)
              ] ;
      rdfs:label "boardMemberList"@en ;
      rdfs:range owl:Literal .

ns:Healthcare
      a       owl:Class ;
      rdfs:comment "A healthcare organization includes hospitals, doctor's offices, blood banks."@en ;
      rdfs:label "Healthcare"@en ;
      owl:subClassOf ns:LocalBusiness .

ns:service
      a       owl:DatatypeProperty ;
      rdfs:comment "list of services offered by a business."@en ;
      rdfs:domain ns:LocalBusiness ;
      rdfs:label "service"@en ;
      rdfs:range owl:Literal ;
      owl:subPropertyOf :topDataProperty .

ns:PrivateCompany
      a       owl:Class ;
      rdfs:comment "PrivateCompany are those companies whose stock is privately owned."@en ;
      rdfs:label "PrivateCompany"@en ;
      owl:subClassOf ns:Company .

ns:screenNumber
      a       :FunctionalProperty , owl:DatatypeProperty ;
      rdfs:comment "Number of screens on which a film is shown in release."@en ;
      rdfs:domain ns:BoxOfficeWeekend ;
      rdfs:label "screenNumber"@en ;
      rdfs:range xsd:int ;
      owl:subPropertyOf :topDataProperty .

ns:ticketStartDate
      a       owl:DatatypeProperty ;
      rdfs:comment "Indicates the first date on which tickets may be purchased for an event."@en ;
      rdfs:domain
              [ a       owl:Class ;
                :unionOf (ns:EventRegistration ns:LocalEventOccurrence)
              ] ;
      rdfs:label "ticketStartDate"@en ;
      rdfs:range owl:Literal .

ns:tag
      a       owl:DatatypeProperty ;
      rdfs:comment "Array of specific tag names (string) and their weights"@en ;
      rdfs:domain
              [ a       owl:Class ;
                :unionOf (ns:Deal ns:LocalBusiness)
              ] ;
      rdfs:label "tag"@en ;
      rdfs:range owl:Literal ;
      owl:subPropertyOf :topDataProperty .

ns:awardWinner
      a       :FunctionalProperty , owl:DatatypeProperty ;
      rdfs:comment "Designates whether the reified nomination to award relationship ended up a winner."@en ;
      rdfs:domain ns:Nomination ;
      rdfs:label "awardWinner"@en ;
      rdfs:range xsd:boolean .

ns:description
      a       :FunctionalProperty , owl:DatatypeProperty ;
      rdfs:comment "Text describing an object. Contains free text and may be used for a wide variety of object types, including media works, relationships, educational milestones, or biography events, e.g. how two persons have met."@en ;
      rdfs:domain ns:Entity ;
      rdfs:label "description"@en ;
      rdfs:range owl:Literal ;
      owl:subPropertyOf :topDataProperty .

ns:containsCompany
      a       owl:ObjectProperty ;
      rdfs:comment "containsCompany connects a local business to the companies that it contains (does not imly organizational hierarchy) for example a particlur Safeway conatins a particulr Starbucks or BOA location)"@en ;
      rdfs:domain ns:LocalBusiness ;
      rdfs:label "containsCompany"@en ;
      rdfs:range ns:LocalBusiness ;
      :inverseOf ns:companyWithin .

ns:franchiseCode4
      a       :FunctionalProperty , owl:DatatypeProperty ;
      rdfs:comment "Local listing franchise code. Indicates the franchise status/affiliation. (for SingleLocationBusiness only)"@en ;
      rdfs:domain ns:SingleLocationBusiness ;
      rdfs:label "franchiseCode4"@en ;
      rdfs:range owl:Literal .

ns:imageSourceType
      a       :FunctionalProperty , owl:DatatypeProperty ;
      rdfs:comment "imageSourceType indicates the source of an image, user, licensed, crawled, merchant"@en ;
      rdfs:domain ns:Image ;
      rdfs:label "imageSourceType"@en ;
      rdfs:range owl:Literal .

ns:theaterClosed
      a       :FunctionalProperty , owl:DatatypeProperty ;
      rdfs:comment "Describes reason why a theater may be closed, i.e. 1 - temp closed, 2 - permanently closed, 3 - relocated."@en ;
      rdfs:domain ns:MovieTheater ;
      rdfs:label "theaterClosed"@en ;
      rdfs:range owl:Literal ;
      owl:subPropertyOf :topDataProperty .

xsd:gYearMonth
      a       owl:Datatype .

ns:teamFirstName
      a       :FunctionalProperty , owl:DatatypeProperty ;
      rdfs:comment "Typically the city in which the team is based. Arsenal, Los Angeles, Chicago."@en ;
      rdfs:domain ns:SportTeam ;
      rdfs:label "teamFirstName"@en ;
      rdfs:range owl:Literal ;
      owl:subPropertyOf ns:name .

ns:CommonStock
      a       owl:Class ;
      rdfs:comment "Common stock a form of corporate equity ownership, a type of security"@en ;
      rdfs:label "CommonStock"@en ;
      owl:subClassOf ns:FinancialInstrumentEquity .

ns:ncesCode
      a       owl:DatatypeProperty ;
      rdfs:comment "Identification code assigned to an educational institution by the National Center for Education Statistics."@en ;
      rdfs:label "ncesCode"@en .

ns:worksFrom
      a       owl:ObjectProperty ;
      rdfs:comment "worksFrom connects a person local business (doctor or lawyer for example) to the local business they work from. For example a doctor may have office hours at several different clinics but not work for any of them."@en ;
      rdfs:domain
              [ a       owl:Class ;
                :unionOf (ns:LocalBusiness ns:Person)
              ] ;
      rdfs:label "worksFrom"@en ;
      rdfs:range ns:LocalBusiness .

ns:DealMerchant
      a       owl:Class ;
      rdfs:label "DealMerchant"@en ;
      owl:subClassOf ns:Company .

ns:teamRoster
      a       owl:ObjectProperty ;
      rdfs:comment "An association of a team to the reified team affiliation class"@en ;
      rdfs:domain ns:SportTeam ;
      rdfs:label "teamRoster"@en ;
      rdfs:range ns:TeamAffiliation .

ns:SportTeam
      a       owl:Class ;
      rdfs:comment "A competitive athletic group comprised of athletes."@en ;
      rdfs:label "SportTeam"@en ;
      owl:subClassOf ns:Group .

ns:analystRanking
      a       :FunctionalProperty , owl:DatatypeProperty ;
      rdfs:comment "analyst ranking is where the analyst ranks compared to the other analysts for that stock"@en ;
      rdfs:domain ns:Analyst ;
      rdfs:label "analystRanking"@en ;
      rdfs:range owl:Literal .

ns:Composition
      a       owl:Class ;
      rdfs:comment "A musical composition is a piece of music that exists in written form."@en ;
      rdfs:label "Composition"@en ;
      owl:subClassOf ns:MediaWork .

ns:crew
      a       owl:ObjectProperty ;
      rdfs:comment "Connects a movie or TV show to the reified CrewRole class."@en ;
      rdfs:domain
              [ a       owl:Class ;
                :unionOf (ns:Movie ns:TvEpisode ns:TvSeason ns:TvSeries ns:TvSpecial)
              ] ;
      rdfs:label "crew"@en ;
      rdfs:range ns:CrewRole ;
      owl:subPropertyOf :topObjectProperty .

ns:crc
      a       :FunctionalProperty , owl:DatatypeProperty ;
      rdfs:comment "Cyclic redundancy code added for Webpage/URI"@en ;
      rdfs:domain ns:Webpage ;
      rdfs:label "crc"@en ;
      rdfs:range owl:Literal ;
      owl:subPropertyOf :topDataProperty .

ns:approvedMenuItem
      a       owl:DatatypeProperty ;
      rdfs:comment "Describes approved items on a restaurant's menu."@en ;
      rdfs:domain ns:Restaurant ;
      rdfs:label "approvedMenuItem"@en ;
      rdfs:range owl:Literal .

ns:Education
      a       owl:Class ;
      rdfs:comment "The education class lists the educational history of an individual, including any degrees earned, field of study, and time of study."@en ;
      rdfs:label "Education"@en ;
      owl:subClassOf ns:Entity .

ns:handed
      a       :FunctionalProperty , owl:DatatypeProperty ;
      rdfs:comment "Designates whether an athlete or other person is right or left handed."@en ;
      rdfs:domain ns:Person ;
      rdfs:label "handed"@en ;
      rdfs:range owl:Literal ;
      owl:subPropertyOf :topDataProperty .

ns:BoxOfficeWeekend
      a       owl:Class ;
      rdfs:comment "The box office income for a film in theatrical release over the period of one weekend."@en ;
      rdfs:label "BoxOfficeWeekend"@en ;
      owl:subClassOf ns:BoxOffice .

ns:percentageScore
      a       :FunctionalProperty , owl:DatatypeProperty ;
      rdfs:comment "Percentage score awarded to an entity."@en ;
      rdfs:domain ns:RottenTomatoesReview ;
      rdfs:label "percentageScore"@en ;
      rdfs:range owl:Literal ;
      owl:subPropertyOf :topDataProperty .

ns:screening
      a       owl:ObjectProperty ;
      rdfs:comment "Connects a film with the reified showtime class. "@en ;
      rdfs:domain ns:Movie ;
      rdfs:label "screening"@en ;
      rdfs:range ns:MovieShowtime ;
      owl:subPropertyOf :topObjectProperty .

ns:incentiveType
      a       owl:DatatypeProperty ;
      rdfs:comment "Represents the type of incentive offered to auto buyers."@en ;
      rdfs:domain ns:AutoIncentive ;
      rdfs:label "incentiveType"@en ;
      rdfs:range owl:Literal .

ns:businessWorkedFrom
      a       owl:ObjectProperty ;
      rdfs:comment "businessWorkedFrom connects a local business to the local business or person that works out of the office. For example Stanford Clinic may have doctors who work out of the Stanford Clinic offices."@en ;
      rdfs:domain ns:LocalBusiness ;
      rdfs:label "businessWorkedFrom"@en ;
      rdfs:range
              [ a       owl:Class ;
                :unionOf (ns:LocalBusiness ns:Person)
              ] ;
      :inverseOf ns:worksFrom .

ns:videoURL
      a       owl:DatatypeProperty ;
      rdfs:comment "URL at which video information about a local business may be accessed."@en ;
      rdfs:domain ns:LocalBusiness ;
      rdfs:label "videoURL"@en ;
      rdfs:range xsd:anyURI .

ns:mediaworkGenreOf
      a       owl:ObjectProperty ;
      rdfs:comment "The genreOf relation connects an genre to the media work or artist it describes."@en ;
      rdfs:domain ns:Genre ;
      rdfs:label "mediaworkGenreOf"@en ;
      rdfs:range
              [ a       owl:Class ;
                :unionOf (ns:MediaWork ns:MusicArtist)
              ] ;
      owl:subPropertyOf :topObjectProperty ;
      :inverseOf ns:mediaworkGenre .

ns:ticketStudent
      a       :FunctionalProperty , owl:DatatypeProperty ;
      rdfs:comment "Describes the cost of a student's ticket at a given theater."@en ;
      rdfs:domain ns:MovieTheater ;
      rdfs:label "ticketStudent"@en ;
      rdfs:range xsd:float ;
      owl:subPropertyOf :topDataProperty .

ns:AutoIncentive
      a       owl:Class ;
      rdfs:comment "Covers the special rebates, incentives and financing packages offered to encourage people to buy Autos."@en ;
      rdfs:label "AutoIncentive"@en ;
      owl:subClassOf ns:Event .

ns:franchiseCode2
      a       :FunctionalProperty , owl:DatatypeProperty ;
      rdfs:comment "Local listing franchise code. Indicates the franchise status/affiliation. (for SingleLocationBusiness only)"@en ;
      rdfs:domain ns:SingleLocationBusiness ;
      rdfs:label "franchiseCode2"@en ;
      rdfs:range owl:Literal .

ns:AthleticConference
      a       owl:Class ;
      rdfs:comment "An athletic conference is a collection of sports teams, playing competitively against each other."@en ;
      rdfs:label "AthleticConference"@en ;
      owl:subClassOf
              [ a       owl:Class ;
                :intersectionOf (ns:Group ns:SportCompetition)
              ] .

ns:exclusionRule
      a       owl:DatatypeProperty ;
      rdfs:comment "Indicates exclusions to the recurrence rules for an event."@en ;
      rdfs:domain ns:Event ;
      rdfs:label "exclusionRule"@en ;
      rdfs:range ns:rRule .

ns:lyricsText
      a       :FunctionalProperty , owl:DatatypeProperty ;
      rdfs:comment "The words that make up a song."@en ;
      rdfs:domain ns:Lyrics ;
      rdfs:label "lyrics"@en ;
      rdfs:range owl:Literal .

ns:hosts
      a       owl:ObjectProperty ;
      rdfs:comment "hosts connects the establishment to the show its hosting"@en ;
      rdfs:domain ns:EstablishmentShowTime ;
      rdfs:label "hosts"@en ;
      rdfs:range ns:EstablishmentShow ;
      :inverseOf ns:hostedAt .

ns:Politician
      a       owl:Class ;
      rdfs:comment "Created by ace to support Milton mapping: http://twiki.corp.yahoo.com/view/P13nContextual/MiltonWooSchemaMap"@en , "A politician or political leader is an individual who is involved in influencing public policy and decision making. This includes people who hold decision-making positions in government, and people who seek those positions, whether by means of election, coup d'etat, appointment, electoral fraud, conquest, right of inheritance or other means."@en ;
      rdfs:label "Politician"@en ;
      owl:subClassOf ns:Person .

ns:tradesOnExchange
      a       owl:ObjectProperty ;
      rdfs:comment "connects the tradablequotable instrument or ticker entity with the exchange on which it is traded"@en ;
      rdfs:domain
              [ a       owl:Class ;
                :unionOf (ns:Ticker ns:TradableQuotableInstrument)
              ] ;
      rdfs:label "tradesOnExchange"@en ;
      rdfs:range ns:StockExchange .

ns:studiedBy
      a       :FunctionalProperty , owl:ObjectProperty ;
      rdfs:comment "Connects the education class to an individual who has been educated."@en ;
      rdfs:domain ns:Education ;
      rdfs:label "studiedBy"@en ;
      rdfs:range ns:Person ;
      owl:subPropertyOf :topObjectProperty ;
      :inverseOf ns:studied .

ns:telephone
      a       :FunctionalProperty , owl:DatatypeProperty ;
      rdfs:comment "Full telephone number of an organization or person. Preferable to use the Phone class."@en ;
      rdfs:domain
              [ a       owl:Class ;
                :unionOf (ns:ContactInfo ns:Person ns:Phone ns:SingleLocationBusiness)
              ] ;
      rdfs:label "telephone"@en ;
      rdfs:range owl:Literal ;
      owl:subPropertyOf :topDataProperty .

ns:parkingAvailable
      a       :FunctionalProperty , owl:DatatypeProperty ;
      rdfs:comment "Indicates if parking is available at a business."@en ;
      rdfs:domain
              [ a       owl:Class ;
                :unionOf (ns:LocalBusiness ns:LocalEvent)
              ] ;
      rdfs:label "parkingAvailable"@en ;
      rdfs:range xsd:boolean .

ns:HistoricalState
      a       owl:Class ;
      rdfs:comment "placetype: 26"@en , "A former or historical primary administrative area for a country. Example: Grand Cayman, Oregon Country"@en ;
      rdfs:label "HistoricalState"@en ;
      owl:subClassOf ns:Place .

ns:franchiseCode3
      a       :FunctionalProperty , owl:DatatypeProperty ;
      rdfs:comment "Local listing franchise code. Indicates the franchise status/affiliation. (for SingleLocationBusiness only)"@en ;
      rdfs:domain ns:SingleLocationBusiness ;
      rdfs:label "franchiseCode3"@en ;
      rdfs:range owl:Literal .

ns:countyLocationOf
      a       :FunctionalProperty , owl:ObjectProperty ;
      rdfs:comment "Connects a physical address to its county"@en ;
      rdfs:domain ns:CountyAdminArea ;
      rdfs:label "countyLocationOf"@en ;
      rdfs:range
              [ a       owl:Class ;
                :unionOf (ns:Address ns:Place)
              ] ;
      owl:subPropertyOf ns:location ;
      :inverseOf ns:countyLocation .

ns:profileURL
      a       owl:DatatypeProperty ;
      rdfs:comment "URL at which the profile for a local business may be accessed."@en ;
      rdfs:domain ns:LocalBusiness ;
      rdfs:label "profileURL"@en ;
      rdfs:range xsd:anyURI .

ns:brandsSold
      a       owl:DatatypeProperty ;
      rdfs:comment "Brands sold at a retail outlet."@en ;
      rdfs:domain
              [ a       owl:Class ;
                :unionOf (ns:EventVenue ns:RetailShop)
              ] ;
      rdfs:label "brandsSold"@en ;
      rdfs:range owl:Literal ;
      owl:subPropertyOf :topDataProperty .

ns:TheatricalDistributor
      a       owl:Class ;
      rdfs:comment "A film distributor is an independent company, a subsidiary company or occasionally an individual, which acts as the final agent between a film production company or some intermediary agent, and a film exhibitor, to the end of securing placement of the producer's film on the exhibitor's screen."@en ;
      rdfs:label "TheatricalDistributor"@en ;
      owl:subClassOf ns:Company .

ns:chainId
      a       :FunctionalProperty , owl:DatatypeProperty ;
      rdfs:comment "Identifier of the chain a local business is associated with."@en ;
      rdfs:domain ns:LocalBusiness ;
      rdfs:label "chainId"@en ;
      rdfs:range owl:Literal .

ns:pricing
      a       owl:DatatypeProperty ;
      rdfs:comment "Captures how expensive a restaurant or hotel or other venue is. Symbolic representation, i.e. number of dollar signs signifying general price category."@en ;
      rdfs:domain ns:LocalBusiness ;
      rdfs:label "pricing"@en ;
      rdfs:range owl:Literal ;
      owl:subPropertyOf :topDataProperty .

ns:compositionPartNumber
      a       :FunctionalProperty , owl:DatatypeProperty ;
      rdfs:comment "Ordering of the part within the composition "@en ;
      rdfs:domain ns:CompositionPart ;
      rdfs:label "compositionPartNumber"@en ;
      rdfs:range xsd:int ;
      owl:subPropertyOf :topDataProperty .

ns:BodyOfWater
      a       owl:Class ;
      rdfs:comment "placetype: 15"@en , "A landlocked water body not associated with an ocean such as a river, canal, lake. Example: Lake Tahoe. Oceans are separate."@en ;
      rdfs:label "BodyOfWater"@en ;
      owl:subClassOf ns:Place .

ns:merchantId
      a       owl:DatatypeProperty ;
      rdfs:comment "ID of a merchant offering a deal."@en ;
      rdfs:domain ns:DealMerchant ;
      rdfs:label "merchantId"@en ;
      rdfs:range owl:Literal ;
      owl:subPropertyOf ns:id .

ns:alternateNameOf
      a       :FunctionalProperty , owl:ObjectProperty ;
      rdfs:comment "The Person this alternate name belongs to."@en ;
      rdfs:domain ns:AlternatePersonName ;
      rdfs:label "alternateNameOf"@en ;
      rdfs:range ns:Person .

ns:contactInfoOf
      a       :FunctionalProperty , owl:ObjectProperty ;
      rdfs:comment "contactInfoOf connects the ContactInfo class to the organization to which it belongs."@en ;
      rdfs:domain ns:ContactInfo ;
      rdfs:label "contactInfoOf"@en ;
      rdfs:range
              [ a       owl:Class ;
                :unionOf (ns:EventOrganizer ns:Organization)
              ] .

ns:performedMusicBy
      a       owl:ObjectProperty ;
      rdfs:comment "Connects a performer to a musical performance"@en ;
      rdfs:domain ns:MusicPerformance ;
      rdfs:label "performedMusicBy"@en ;
      rdfs:range ns:MusicArtist ;
      owl:subPropertyOf :topObjectProperty ;
      :inverseOf ns:performedMusic .

ns:categoryWeight
      a       owl:DatatypeProperty ;
      rdfs:comment "Weight of this Y! category "@en ;
      rdfs:domain ns:LocalBusinessCategory ;
      rdfs:label "categoryWeight"@en ;
      rdfs:range xsd:int ;
      owl:subPropertyOf :topDataProperty .

ns:TeamGameRole
      a       owl:Class ;
      rdfs:comment "Reified class describes the actions of a team in a particular game."@en ;
      rdfs:label "TeamGameRole"@en ;
      owl:subClassOf ns:Entity .

ns:synopsisOf
      a       :FunctionalProperty , owl:ObjectProperty ;
      rdfs:comment "Links the Synopsis class to the Media work it summarizes."@en ;
      rdfs:domain ns:Synopsis ;
      rdfs:label "synopsisOf"@en ;
      rdfs:range ns:MediaWork .

ns:screenFormat
      a       :FunctionalProperty , owl:DatatypeProperty ;
      rdfs:comment "Y! normalized array of strings for provider screen code. May include 3D, B&W, Color, etc."@en ;
      rdfs:domain ns:Video ;
      rdfs:label "screenFormat"@en ;
      rdfs:range owl:Literal ;
      owl:subPropertyOf :topDataProperty .

ns:onlineDeal
      a       :FunctionalProperty , owl:DatatypeProperty ;
      rdfs:comment "Indicates whether a deal or offer is online-only"@en ;
      rdfs:domain ns:Deal ;
      rdfs:label "onlineDeal"@en ;
      rdfs:range xsd:boolean .

ns:groupName
      a       :FunctionalProperty , owl:DatatypeProperty ;
      rdfs:comment "The name by which a group is identified."@en ;
      rdfs:domain ns:Group ;
      rdfs:label "groupName"@en ;
      rdfs:range owl:Literal ;
      owl:subPropertyOf ns:name .

ns:financialInstrumentSubType
      a       :FunctionalProperty , owl:DatatypeProperty ;
      rdfs:comment "financialInstrumentSubType is the sub type the financial instrument belongs to. For example, Common Stock, Preferred Stock"@en ;
      rdfs:domain ns:FinancialInstrument ;
      rdfs:label "financialInstrumentSubType"@en ;
      rdfs:range owl:Literal .

ns:awardWon
      a       owl:ObjectProperty ;
      rdfs:comment "Direct connection between an individual, media work, or organization to an award won by that entity."@en ;
      rdfs:domain
              [ a       owl:Class ;
                :unionOf (ns:MediaWork ns:Organization ns:Person)
              ] ;
      rdfs:label "awardWon"@en ;
      rdfs:range ns:AwardType ;
      owl:subPropertyOf :topObjectProperty .

ns:colorCode
      a       :FunctionalProperty , owl:DatatypeProperty ;
      rdfs:comment "Code representing the color, i.e. BLU"@en ;
      rdfs:domain ns:Color ;
      rdfs:label "colorCode"@en ;
      rdfs:range owl:Literal ;
      owl:subPropertyOf ns:colorHolding .

ns:tickerOf
      a       :FunctionalProperty , owl:ObjectProperty ;
      rdfs:comment "tickerOf connects a ticker to the tradablequotable instrument it represents"@en ;
      rdfs:domain ns:TQIAffiliation ;
      rdfs:label "tickerOf"@en ;
      rdfs:range ns:TradableQuotableInstrument .

ns:exclusiveDeal
      a       :FunctionalProperty , owl:DatatypeProperty ;
      rdfs:comment "Indicates the exclusivity of a deal."@en ;
      rdfs:domain ns:Deal ;
      rdfs:label "exclusiveDeal"@en ;
      rdfs:range xsd:boolean .

ns:expired
      a       owl:DatatypeProperty ;
      rdfs:comment "indicates whether a deal or offer has expired."@en ;
      rdfs:domain ns:Deal ;
      rdfs:label "expired"@en ;
      rdfs:range xsd:boolean .

ns:franchiseCode1
      a       :FunctionalProperty , owl:DatatypeProperty ;
      rdfs:comment "Local listing franchise code. Indicates the franchise status/affiliation. (for SingleLocationBusiness only)"@en ;
      rdfs:domain ns:SingleLocationBusiness ;
      rdfs:label "franchiseCode1"@en ;
      rdfs:range owl:Literal .

ns:precisePostalCode
      a       :FunctionalProperty , owl:DatatypeProperty ;
      rdfs:comment "Precise zip code if any. Else, similar to postalCode. This corresponds to \"postal\" from FindLocation. For example: 95089-1019 "@en ;
      rdfs:domain
              [ a       owl:Class ;
                :unionOf (ns:Address ns:PostalZip ns:SingleLocationBusiness)
              ] ;
      rdfs:label "precisePostalCode"@en ;
      rdfs:range owl:Literal .

<http://woo.corp.yahoo.com/ns/units/mm>
      a       owl:Datatype .

ns:headAdminName
      a       :FunctionalProperty , owl:DatatypeProperty ;
      rdfs:comment "Name of the head administrator at an educational institution."@en ;
      rdfs:domain ns:EducationalInstitution ;
      rdfs:label "headAdminName"@en ;
      rdfs:range owl:Literal .

ns:musicRights
      a       owl:ObjectProperty ;
      rdfs:comment "connects a musical work to its rights rules."@en ;
      rdfs:domain ns:Album ;
      rdfs:label "musicRights"@en ;
      rdfs:range ns:MusicRight ;
      owl:subPropertyOf :topObjectProperty .

ns:quoteableInstruments
      a       :FunctionalProperty , owl:DatatypeProperty ;
      rdfs:comment "UUIDs for the quotable instruments "@en ;
      rdfs:domain ns:Security ;
      rdfs:label "quoteableInstruments"@en ;
      rdfs:range owl:Literal .

ns:stadiumSeating
      a       :FunctionalProperty , owl:DatatypeProperty ;
      rdfs:comment "In stadium seating, most or all seats are placed higher than the seats immediately in front of them so that the occupants of further-back seats have less of their views blocked by those further forward."@en ;
      rdfs:domain ns:MovieTheater ;
      rdfs:label "stadiumSeating"@en ;
      rdfs:range xsd:boolean .

xsd:gYear
      a       owl:Datatype .

ns:MediaCategory
      a       owl:Class ;
      rdfs:comment "Grouping of media based on attributes that are not necessarily related to the subject matter."@en ;
      rdfs:label "MediaCategory"@en ;
      owl:subClassOf ns:Category .

<http://www.w3.org/2002/07/owl>
      a       owl:Ontology ;
      rdfs:comment "The Web of Objects schema"@en ;
      rdfs:label "Web of Objects (WOO)"@en ;
      dc:creator "Anneliese Eisentraut"@en , "Jennifer Eaton"@en , "Peter Mika"@en , "Anton Yulo"@en , "Alice Swanberg"@en .

ns:currencyName
      a       :FunctionalProperty , owl:DatatypeProperty ;
      rdfs:comment "currencyName is the name of a currency"@en ;
      rdfs:domain ns:Currency ;
      rdfs:label "currencyName"@en ;
      rdfs:range owl:Literal ;
      owl:subPropertyOf ns:name .

ns:milestone
      a       owl:ObjectProperty ;
      rdfs:comment "Connects an individual to milestone events in his or her life."@en ;
      rdfs:domain ns:Person ;
      rdfs:label "milestone"@en ;
      rdfs:range ns:Milestone ;
      owl:subPropertyOf :topObjectProperty .

ns:Dating
      a       owl:Class ;
      rdfs:comment "Dating is a form of courtship, and may include any social activity undertaken by, typically, two persons with the aim of each assessing the other's suitability as a partner in an intimate relationship or as a spouse."@en ;
      rdfs:label "Dating"@en ;
      owl:subClassOf ns:PersonalRelationship .

ns:placeType
      a       :FunctionalProperty , owl:DatatypeProperty ;
      rdfs:comment "Code for type of the place "@en ;
      rdfs:domain ns:Place ;
      rdfs:label "placeType"@en ;
      rdfs:range owl:Literal .

ns:parValue
      a       :FunctionalProperty , owl:DatatypeProperty ;
      rdfs:comment "The par value of a stock was the share price upon initial offering."@en ;
      rdfs:domain ns:Security ;
      rdfs:label "parValue"@en ;
      rdfs:range xsd:float .

ns:manufacturerOf
      a       owl:ObjectProperty ;
      rdfs:comment "Connects a company with the products it manufactures."@en ;
      rdfs:domain ns:Company ;
      rdfs:label "manufacturerOf"@en ;
      rdfs:range
              [ a       owl:Class ;
                :unionOf (ns:AutoMake ns:ConsumerProduct)
              ] ;
      :inverseOf ns:manufacturer .

ns:state
      a       :FunctionalProperty , owl:DatatypeProperty ;
      rdfs:comment "State or province where a place is located."@en ;
      rdfs:domain
              [ a       owl:Class ;
                :unionOf (ns:Address ns:SingleLocationBusiness)
              ] ;
      rdfs:label "state"@en ;
      rdfs:range owl:Literal ;
      owl:subPropertyOf :topDataProperty .

ns:domed
      a       :FunctionalProperty , owl:DatatypeProperty ;
      rdfs:comment "Designates whether a venue is indoor or outdoor."@en ;
      rdfs:domain ns:SportVenue ;
      rdfs:label "domed" ;
      rdfs:range xsd:boolean ;
      owl:subPropertyOf :topDataProperty .

ns:seasonNumber
      a       :FunctionalProperty , owl:DatatypeProperty ;
      rdfs:comment "sequence number of a TV Show season "@en ;
      rdfs:domain ns:TvSeason ;
      rdfs:label "seasonNumber"@en ;
      rdfs:range owl:Literal ;
      owl:subPropertyOf :topDataProperty .

ns:maxReservationSize
      a       owl:DatatypeProperty ;
      rdfs:comment "Indicates the maximum number of people allowed for a reservation at a local business."@en ;
      rdfs:domain ns:Restaurant ;
      rdfs:label "maxReservationSize"@en ;
      rdfs:range xsd:int .

ns:note
      a       owl:DatatypeProperty ;
      rdfs:comment "Administrative note on an entity. Not for display."@en ;
      rdfs:domain
              [ a       owl:Class ;
                :unionOf (ns:EventOrganizer ns:LocalEvent ns:Performer)
              ] ;
      rdfs:label "note"@en ;
      rdfs:range owl:Literal .

ns:appearedIn
      a       :FunctionalProperty , owl:ObjectProperty ;
      rdfs:comment "Connects the reified AppearanceRole class to a person."@en ;
      rdfs:domain ns:AppearanceRole ;
      rdfs:label "appearedIn"@en ;
      rdfs:range ns:Person ;
      owl:subPropertyOf :topObjectProperty ;
      :inverseOf ns:appeared .

ns:smokingPolicy
      a       :FunctionalProperty , owl:DatatypeProperty ;
      rdfs:comment "smokingPolicy is the policy a business has with regards to smoking"@en ;
      rdfs:domain ns:LocalBusiness ;
      rdfs:label "smokingPolicy"@en ;
      rdfs:range owl:Literal .

ns:Marriage
      a       owl:Class ;
      rdfs:comment "Marriage is a social union or legal contract between individuals that creates kinship."@en ;
      rdfs:label "Marriage"@en ;
      owl:subClassOf ns:PersonalRelationship .

ns:contactNameTitle
      a       :FunctionalProperty , owl:DatatypeProperty ;
      rdfs:comment "Title of the contact person for a local business (for use with SingleLocationBusiness only)."@en ;
      rdfs:domain ns:SingleLocationBusiness ;
      rdfs:label "contactNameTitle"@en ;
      rdfs:range owl:Literal .

ns:baselineID
      a       :FunctionalProperty , owl:DatatypeProperty ;
      rdfs:comment "Baseline ID for genres and categories"@en ;
      rdfs:domain ns:CategoryMovieTV ;
      rdfs:label "baselineID"@en ;
      rdfs:range owl:Literal ;
      owl:subPropertyOf ns:id .

ns:numOfShare
      a       :FunctionalProperty , owl:DatatypeProperty ;
      rdfs:comment "The number of shares a person or company owns."@en ;
      rdfs:domain
              [ a       owl:Class ;
                :unionOf (ns:Equity ns:MajorShareholderAffiliation)
              ] ;
      rdfs:label "numOfShare"@en ;
      rdfs:range xsd:float .

ns:uniformNumber
      a       :FunctionalProperty , owl:DatatypeProperty ;
      rdfs:comment "The number of a player's team uniform."@en ;
      rdfs:domain
              [ a       owl:Class ;
                :unionOf (ns:AthleteGameRole ns:TeamAffiliation)
              ] ;
      rdfs:label "uniformNumber"@en ;
      rdfs:range xsd:int ;
      owl:subPropertyOf :topDataProperty .

ns:msrp
      a       :FunctionalProperty , owl:DatatypeProperty ;
      rdfs:comment "MSRP is the Manufacturer's Suggested Retail Price. The maker of the automobile suggests this price. "@en ;
      rdfs:domain
              [ a       owl:Class ;
                :unionOf (ns:AutoMake ns:AutoModel ns:AutoTrim ns:Automobile)
              ] ;
      rdfs:label "msrp"@en ;
      rdfs:range xsd:float .

ns:analystScore
      a       :FunctionalProperty , owl:DatatypeProperty ;
      rdfs:comment "analyst score How well the analyst did overall analyzing a stock"@en ;
      rdfs:domain ns:Analyst ;
      rdfs:label "analystScore"@en ;
      rdfs:range owl:Literal .

ns:soundtrackArtist
      a       owl:ObjectProperty ;
      rdfs:comment "The soundtrack relation connects a music artist to films for which s/he has contributed musical tracks."@en ;
      rdfs:domain ns:Movie ;
      rdfs:label "soundtrackArtist"@en ;
      rdfs:range
              [ a       owl:Class ;
                :unionOf (ns:MusicArtist ns:MusicGroup ns:Musician)
              ] .

ns:locationName
      a       :FunctionalProperty , owl:DatatypeProperty ;
      rdfs:comment "String value for a location's or place's name."@en ;
      rdfs:domain ns:Place ;
      rdfs:label "locationName"@en ;
      rdfs:range owl:Literal ;
      owl:subPropertyOf ns:name .

ns:major
      a       owl:DatatypeProperty ;
      rdfs:comment "Describes an individual's area of study."@en ;
      rdfs:domain ns:Education ;
      rdfs:label "major"@en ;
      rdfs:range owl:Literal .

ns:releaseStatus
      a       :FunctionalProperty , owl:DatatypeProperty ;
      rdfs:comment "details the status of a media release, e.g. Released, Announced, Awaiting Release."@en ;
      rdfs:domain ns:MediaRelease ;
      rdfs:label "releaseStatus"@en ;
      rdfs:range owl:Literal .

ns:listingExchange
      a       :FunctionalProperty , owl:DatatypeProperty ;
      rdfs:comment "listingExchange is the Exchange on which a tradablequotable instrument is listed"@en ;
      rdfs:domain ns:TradableQuotableInstrument ;
      rdfs:label "listingExchange"@en ;
      rdfs:range owl:Literal .

ns:milestoneOf
      a       :FunctionalProperty , owl:ObjectProperty ;
      rdfs:comment "Connects the milestone class to the person class."@en ;
      rdfs:domain ns:Milestone ;
      rdfs:label "milestoneOf"@en ;
      rdfs:range ns:Person ;
      owl:subPropertyOf :topObjectProperty ;
      :inverseOf ns:milestone .

ns:teamVenue
      a       owl:ObjectProperty ;
      rdfs:comment "Connects a team to the location it plays."@en ;
      rdfs:domain ns:SportTeam ;
      rdfs:label "teamVenue"@en ;
      rdfs:range ns:SportVenue ;
      owl:subPropertyOf :topObjectProperty .

ns:nominatedWork
      a       :FunctionalProperty , owl:ObjectProperty ;
      rdfs:comment "The work for which an individual or organization is nominated for an award."@en ;
      rdfs:domain ns:Nomination ;
      rdfs:label "nominatedWork"@en ;
      rdfs:range ns:MediaWork ;
      owl:subPropertyOf :topObjectProperty ;
      :inverseOf ns:nominated .

ns:eastLongitude
      a       :FunctionalProperty , owl:DatatypeProperty ;
      rdfs:comment "East longitude of the bounding box of the place "@en ;
      rdfs:domain ns:Place ;
      rdfs:label "eastLongitude"@en ;
      rdfs:range xsd:float .

ns:guestlistURL
      a       owl:DatatypeProperty ;
      rdfs:comment "URL at which the guestlist for a local business may be accessed."@en ;
      rdfs:domain
              [ a       owl:Class ;
                :unionOf (ns:Bar ns:EventVenue ns:NightClub)
              ] ;
      rdfs:label "guestlistURL"@en ;
      rdfs:range xsd:anyURI .

ns:OccupationalHistory
      a       owl:Class ;
      rdfs:comment "The occupational history class lists types of employment that an individual has held."@en ;
      rdfs:label "OccupationalHistory"@en ;
      owl:subClassOf ns:Event .

ns:personName
      a       :FunctionalProperty , owl:DatatypeProperty ;
      rdfs:comment "A personal name identifies a specific unique and identifiable individual person, and may or may not include a middle name."@en ;
      rdfs:domain ns:Person ;
      rdfs:label "personName"@en ;
      rdfs:range owl:Literal ;
      owl:subPropertyOf ns:name .

ns:providerId
      a       owl:DatatypeProperty ;
      rdfs:comment "ID of the Data provider"@en ;
      rdfs:domain
              [ a       owl:Class ;
                :unionOf (ns:Deal ns:LocalBusiness)
              ] ;
      rdfs:label "providerId"@en ;
      rdfs:range owl:Literal ;
      owl:subPropertyOf ns:id .

ns:tvNetworkOf
      a       owl:ObjectProperty ;
      rdfs:comment "Connects a TV Show to its network"@en ;
      rdfs:domain
              [ a       owl:Class ;
                :unionOf (ns:TvSeries ns:TvSpecial)
              ] ;
      rdfs:label "tvNetworkOf"@en ;
      rdfs:range ns:TvNetwork ;
      owl:subPropertyOf :topObjectProperty .

ns:logoLink
      a       owl:DatatypeProperty ;
      rdfs:comment "Captures the URL where an image of a vendor's logo is stored."@en ;
      rdfs:domain ns:EventRegistration ;
      rdfs:label "logoLink"@en ;
      rdfs:range xsd:anyURI .

ns:offerId
      a       owl:DatatypeProperty ;
      rdfs:comment "example: 14538002"@en , "ID of a deal or offer."@en ;
      rdfs:domain ns:Deal ;
      rdfs:label "offerId"@en ;
      rdfs:range owl:Literal ;
      owl:subPropertyOf ns:id .

ns:ssic4
      a       :FunctionalProperty , owl:DatatypeProperty ;
      rdfs:comment "Standard industry classification code for Local business (for use with SingleLocationBusiness only)."@en ;
      rdfs:domain ns:SingleLocationBusiness ;
      rdfs:label "ssic4"@en ;
      rdfs:range owl:Literal .

ns:showAttribute
      a       owl:DatatypeProperty ;
      rdfs:comment "Describes particular features of a film showtime."@en ;
      rdfs:domain ns:MovieShowtime ;
      rdfs:label "showAttribute"@en ;
      rdfs:range owl:Literal ;
      owl:subPropertyOf :topDataProperty .

ns:broadcastOn
      a       owl:ObjectProperty ;
      rdfs:comment "connects a TV series to a network affiliation"@en ;
      rdfs:domain ns:NetworkAffiliation ;
      rdfs:label "broadcastOn"@en ;
      rdfs:range
              [ a       owl:Class ;
                :unionOf (ns:TvEpisode ns:TvSeason ns:TvSeries ns:TvSpecial)
              ] ;
      owl:subPropertyOf :topObjectProperty ;
      :inverseOf ns:broadcast .

ns:fuelUnit
      a       :FunctionalProperty , owl:DatatypeProperty ;
      rdfs:comment "Unit for fuel economy, i.e. MPG. priceUnit in CCM"@en ;
      rdfs:domain ns:AutoModel ;
      rdfs:label "fuelUnit"@en ;
      rdfs:range owl:Literal .

ns:GeoPoliticalEntity
      a       owl:Class ;
      rdfs:comment "A geographical area which is associated with some sort of political structure - a country, city, municipality."@en ;
      rdfs:label "GeoPoliticalEntity"@en ;
      owl:subClassOf ns:Place .

ns:participantRole
      a       :FunctionalProperty , owl:DatatypeProperty ;
      rdfs:comment "Specifies the role an event participant plays, e.g. singer, guitarist, keynote speaker, etc." ;
      rdfs:domain ns:Performer ;
      rdfs:label "participantRole"@en ;
      rdfs:range owl:Literal .

ns:Management
      a       owl:Class ;
      rdfs:comment "Management refers to those employees who are managers"@en ;
      rdfs:label "Management"@en ;
      owl:subClassOf ns:Employee .

ns:trailer
      a       :FunctionalProperty , owl:DatatypeProperty ;
      rdfs:comment "URL for a film trailer page."@en ;
      rdfs:domain
              [ a       owl:Class ;
                :unionOf (ns:Movie ns:RottenTomatoesReview)
              ] ;
      rdfs:label "trailer"@en ;
      rdfs:range xsd:anyURI ;
      owl:subPropertyOf :topDataProperty .

ns:homeService
      a       owl:DatatypeProperty ;
      rdfs:comment "Field also known as Is_Service_delivered_home in CCM or home delivery"@en ;
      rdfs:domain ns:LocalBusiness ;
      rdfs:label "homeService"@en ;
      rdfs:range xsd:boolean ;
      owl:subPropertyOf :topDataProperty .

ns:Biography
      a       owl:Class ;
      rdfs:comment "The biography class lists the personal history of an individual."@en ;
      rdfs:label "Biography"@en ;
      owl:subClassOf ns:Entity .

ns:seasonEpisodeOf
      a       :FunctionalProperty , owl:ObjectProperty ;
      rdfs:comment "Connects a television episode to its season"@en ;
      rdfs:domain ns:TvEpisode ;
      rdfs:label "seasonEpisodeOf" ;
      rdfs:range ns:TvSeason ;
      owl:subPropertyOf :topObjectProperty ;
      :inverseOf ns:seasonEpisode .

ns:ssic3
      a       :FunctionalProperty , owl:DatatypeProperty ;
      rdfs:comment "Standard industry classification code for Local business (for use with SingleLocationBusiness only)."@en ;
      rdfs:domain ns:SingleLocationBusiness ;
      rdfs:label "ssic3"@en ;
      rdfs:range owl:Literal .

ns:productionLocation
      a       owl:ObjectProperty ;
      rdfs:comment "Connects a film to the place where it was produced."@en ;
      rdfs:domain ns:Movie ;
      rdfs:label "productionLocation"@en ;
      rdfs:range ns:Place ;
      owl:subPropertyOf ns:location .

ns:categoryOf
      a       owl:ObjectProperty ;
      rdfs:comment "categoryOf connects the Category class with the MusicArtist or MediaWork it describes."@en ;
      rdfs:domain ns:Category ;
      rdfs:label "categoryOf"@en ;
      rdfs:range
              [ a       owl:Class ;
                :unionOf (ns:MediaWork ns:MusicArtist)
              ] .

ns:bannedInMarket
      a       owl:DatatypeProperty ;
      rdfs:comment "Indicates a market or country in which information about an entity has been banned. May include media works (book, movie, TV show, etc.), people, or any entity type. Entries must conform to ISO-3166 country codes."@en ;
      rdfs:domain ns:Entity ;
      rdfs:label "bannedInMarket"@en ;
      rdfs:range owl:Literal .

ns:eventApproximate
      a       owl:DatatypeProperty ;
      rdfs:comment "Captures whether an event's start or end times are approximate."@en ;
      rdfs:domain ns:LocalEventOccurrence ;
      rdfs:label "eventApproximate"@en ;
      rdfs:range xsd:boolean .

ns:busListingCategoryKeyword
      a       owl:DatatypeProperty ;
      rdfs:comment "Keywords associated with a business listing category."@en ;
      rdfs:domain
              [ a       owl:Class ;
                :unionOf (ns:BusinessListingCategory ns:LocalBusiness)
              ] ;
      rdfs:label "busListingCategoryKeyword"@en ;
      rdfs:range owl:Literal .

ns:cusip
      a       :FunctionalProperty , owl:DatatypeProperty ;
      rdfs:comment "cusip is the CUSIP for a security "@en ;
      rdfs:domain ns:Security ;
      rdfs:label "cusip"@en ;
      rdfs:range owl:Literal .

ns:athleteParticipation
      a       owl:ObjectProperty ;
      rdfs:comment "Connects a player to the reified AthleteGameRole class."@en ;
      rdfs:domain ns:AthleteGameRole ;
      rdfs:label "athleteParticipation"@en ;
      rdfs:range ns:Athlete .

ns:rottenCount
      a       :FunctionalProperty , owl:DatatypeProperty ;
      rdfs:comment "Number of reviews for a given film identified as negative (or 'rotten'), calculated by Rotten Tomatoes."@en ;
      rdfs:domain ns:RottenTomatoesReview ;
      rdfs:label "rottenCount"@en ;
      rdfs:range owl:Literal ;
      owl:subPropertyOf :topDataProperty .

ns:FinancialInstrumentEquity
      a       owl:Class ;
      rdfs:comment "Equity represents the remaining interest in assets of a company"@en ;
      rdfs:label "FinancialInstrumentEquity"@en ;
      owl:subClassOf ns:Security .

ns:newTrim
      a       :FunctionalProperty , owl:DatatypeProperty ;
      rdfs:comment "Boolean representing whether the trim represents a new vehicle or used."@en ;
      rdfs:domain ns:AutoTrim ;
      rdfs:label "newTrim"@en ;
      rdfs:range xsd:boolean .

ns:Address
      a       owl:Class ;
      rdfs:comment "Describes the location of a structure or a plot of land, generally using political boundaries and street names as references, along with other identifiers such as house or apartment numbers. May also include a mailing address different from the physical address, but where mail can delivered, eg, post office box."@en ;
      rdfs:label "Address"@en ;
      owl:subClassOf ns:Entity .

ns:ssic2
      a       :FunctionalProperty , owl:DatatypeProperty ;
      rdfs:comment "Standard industry classification code for Local business (for use with SingleLocationBusiness only)."@en ;
      rdfs:domain ns:SingleLocationBusiness ;
      rdfs:label "ssic2"@en ;
      rdfs:range owl:Literal .

ns:birthDate
      a       :FunctionalProperty , owl:DatatypeProperty ;
      rdfs:comment "The date on which an individual is born."@en ;
      rdfs:domain ns:Person ;
      rdfs:label "birthDate"@en ;
      rdfs:range
              [ a       owl:Datatype ;
                :unionOf (xsd:date xsd:gYearMonth)
              ] ;
      owl:subPropertyOf ns:date .

ns:releaseLocation
      a       :FunctionalProperty , owl:ObjectProperty ;
      rdfs:comment "The location in which a media work is released for public distribution."@en ;
      rdfs:domain
              [ a       owl:Class ;
                :unionOf (ns:MediaRelease ns:MediaWork)
              ] ;
      rdfs:label "releaseLocation"@en ;
      rdfs:range ns:Place ;
      owl:subPropertyOf ns:location .

ns:companyWithin
      a       owl:ObjectProperty ;
      rdfs:comment "companyWithin connects a local business to the local business it operates from within  ( a mall store to the mall, Starbucks to a Safeway, BOA in a Safeway) but does not imply organizational affiliation."@en ;
      rdfs:domain ns:LocalBusiness ;
      rdfs:label "companyWithin"@en ;
      rdfs:range ns:LocalBusiness .

ns:numberEpisodes
      a       :FunctionalProperty , owl:DatatypeProperty ;
      rdfs:comment "The number of episodes in a television season"@en ;
      rdfs:domain ns:TvSeason ;
      rdfs:label "numberEpisodes"@en ;
      rdfs:range xsd:int ;
      owl:subPropertyOf :topDataProperty .

ns:boardRank
      a       :FunctionalProperty , owl:DatatypeProperty ;
      rdfs:comment "boardRank is the rank of a board member"@en ;
      rdfs:domain ns:BoardMember ;
      rdfs:label "boardRank"@en ;
      rdfs:range owl:Literal .

ns:ContactInfo
      a       owl:Class ;
      rdfs:comment "Reified class that describes the contact address, phone number, and operating details for a business or organization. An entity may have multiple sets of ContactInfo."@en ;
      rdfs:label "ContactInfo"@en ;
      owl:subClassOf ns:Entity .

ns:Image
      a       owl:Class ;
      rdfs:comment "This class scheduled for deletion - images not needed for WOO"@en , "Describes the data associated with an image."@en ;
      rdfs:label "Image"@en ;
      owl:subClassOf ns:Entity .

ns:writtenBy
      a       owl:ObjectProperty ;
      rdfs:comment "The writtenBy property connects a written work to the individual or organization that created it."@en ;
      rdfs:domain
              [ a       owl:Class ;
                :unionOf (ns:Biography ns:MediaWork ns:Review ns:Synopsis)
              ] ;
      rdfs:label "writtenBy"@en ;
      rdfs:range ns:Writer .

ns:ssic1
      a       :FunctionalProperty , owl:DatatypeProperty ;
      rdfs:comment "Standard industry classification code for Local business (for use with SingleLocationBusiness only)."@en ;
      rdfs:domain ns:SingleLocationBusiness ;
      rdfs:label "ssic1"@en ;
      rdfs:range owl:Literal .

ns:areaOfCoverage
      a       owl:DatatypeProperty ;
      rdfs:comment "Describes the areas a warranty covers."@en ;
      rdfs:domain ns:Warranty ;
      rdfs:label "areaOfCoverage"@en ;
      rdfs:range owl:Literal .

ns:officerAffiliated
      a       owl:ObjectProperty ;
      rdfs:comment "officerAffiliated connects a company officer to the companyofficeraffiliation"@en ;
      rdfs:domain ns:CompanyOfficer ;
      rdfs:label "officerAffiliated"@en ;
      rdfs:range ns:CompanyOfficerAffiliation .

ns:countryOfOrigin
      a       :FunctionalProperty , owl:ObjectProperty ;
      rdfs:comment "countryOfOrigin connects an entity to its country of origin."@en ;
      rdfs:domain
              [ a       owl:Class ;
                :unionOf (ns:Movie ns:TvSeries ns:TvSpecial)
              ] ;
      rdfs:label "countryOfOrigin"@en ;
      rdfs:range ns:Country ;
      owl:subPropertyOf ns:location .

ns:personalRelationshipTarget
      a       owl:ObjectProperty ;
      rdfs:comment "This property indicates that the given Person is the target of a directed relationship between two people. Example: in a parent-son relationship, the parent is the source, and the son is the target."@en ;
      rdfs:label "personalRelationshipTarget"@en ;
      owl:subPropertyOf ns:personalRelationship .

ns:aprDuration
      a       :FunctionalProperty , owl:DatatypeProperty ;
      rdfs:comment "Represents the duration (in months) for which the financing rate is applicable"@en ;
      rdfs:domain ns:AutoIncentive ;
      rdfs:label "aprDuration"@en ;
      rdfs:range owl:Literal .

ns:kidFriendly
      a       owl:DatatypeProperty ;
      rdfs:comment "Designates whether an event or local venue is child-appropriate."@en ;
      rdfs:domain
              [ a       owl:Class ;
                :unionOf (ns:LocalBusiness ns:LocalEvent)
              ] ;
      rdfs:label "kidFriendly"@en ;
      rdfs:range xsd:boolean .

ns:created
      a       owl:ObjectProperty ;
      rdfs:comment "The created property connects a television creator with the programs s/he has created."@en ;
      rdfs:domain ns:ProgramCreator ;
      rdfs:label "created"@en ;
      rdfs:range
              [ a       owl:Class ;
                :unionOf (ns:TvSeries ns:TvSpecial)
              ] .

ns:colorCategory
      a       owl:DatatypeProperty ;
      rdfs:comment "Represents the are of the product the color belongs to, i.e. interior, exterior"@en ;
      rdfs:domain ns:Color ;
      rdfs:label "colorCategory"@en ;
      rdfs:range owl:Literal ;
      owl:subPropertyOf ns:colorHolding .

ns:GroupPerformer
      a       owl:Class ;
      rdfs:comment "A group that performs at a local event."@en ;
      rdfs:label "GroupPerformer"@en ;
      owl:subClassOf
              [ a       owl:Class ;
                :intersectionOf (ns:Organization ns:Performer)
              ] .

ns:quantity
      a       owl:DatatypeProperty ;
      rdfs:comment "Gives the number of items available for a deal or offer."@en ;
      rdfs:domain ns:Deal ;
      rdfs:label "quantity"@en ;
      rdfs:range owl:Literal .

ns:valFlag
      a       :FunctionalProperty , owl:DatatypeProperty ;
      rdfs:comment "Amacai source data for local business listing. It has value C if business is validated as connect."@en ;
      rdfs:domain ns:SingleLocationBusiness ;
      rdfs:label "valFlag"@en ;
      rdfs:range owl:Literal .

ns:catalogNumber
      a       :FunctionalProperty , owl:DatatypeProperty ;
      rdfs:comment "Describes the catalog number assigned to a media product."@en ;
      rdfs:domain ns:MediaProduct ;
      rdfs:label "catalogNumber"@en ;
      rdfs:range owl:Literal ;
      owl:subPropertyOf :topDataProperty .

ns:primaryTickerSymbol
      a       :FunctionalProperty , owl:DatatypeProperty ;
      rdfs:comment "primaryTickerSymbol of a public company's primary trading instrument"@en ;
      rdfs:domain ns:PublicCompany ;
      rdfs:label "primaryTickerSymbol"@en ;
      rdfs:range owl:Literal .

ns:matchName
      a       owl:DatatypeProperty ;
      rdfs:comment "Similar to display name, added to support Local team"@en ;
      rdfs:domain ns:Organization ;
      rdfs:label "matchName"@en ;
      rdfs:range owl:Literal ;
      owl:subPropertyOf ns:name .

ns:shippingDetails
      a       owl:DatatypeProperty ;
      rdfs:comment "Describes the shipping cost and other details of a deal or product."@en ;
      rdfs:domain ns:Deal ;
      rdfs:label "shippingDetails"@en ;
      rdfs:range owl:Literal .

ns:checkoutAndIn
      a       owl:DatatypeProperty ;
      rdfs:comment "Free text containing checkout and checkin details for the business "@en ;
      rdfs:domain ns:Lodging ;
      rdfs:label "checkoutAndIn"@en ;
      rdfs:range owl:Literal ;
      owl:subPropertyOf :topDataProperty .

ns:volume
      a       :FunctionalProperty , owl:DatatypeProperty ;
      rdfs:comment "volume is the amount of trades"@en ;
      rdfs:domain ns:Exchange ;
      rdfs:label "volume"@en ;
      rdfs:range owl:Literal .

ns:MediaRelease
      a       owl:Class ;
      rdfs:comment "Contains data about a media work's release for public distribution."@en ;
      rdfs:label "MediaRelease"@en ;
      owl:subClassOf ns:Entity .

ns:periodicity
      a       :FunctionalProperty , owl:DatatypeProperty ;
      rdfs:comment "Length of time between events. For instance, annual or every 4 years."@en ;
      rdfs:domain ns:SportCompetitionInstance ;
      rdfs:label "periodicity"@en ;
      rdfs:range xsd:duration ;
      owl:subPropertyOf :topDataProperty .

ns:ethnicity
      a       owl:DatatypeProperty ;
      rdfs:comment "ethnicity designates a group of people whose members identify with each other, through a common heritage, consisting of a common language, a common culture (often including a shared religion) and a tradition of common ancestry"@en ;
      rdfs:domain ns:Person ;
      rdfs:label "ethnicity"@en ;
      rdfs:range owl:Literal ;
      owl:subPropertyOf :topDataProperty .

ns:greatSchoolsURL
      a       owl:DatatypeProperty ;
      rdfs:comment "URL where the Great Schools information about an educational institution may be accessed."@en ;
      rdfs:domain ns:EducationalInstitution ;
      rdfs:label "greatSchoolsURL"@en ;
      rdfs:range owl:Literal .

ns:providerCategory
      a       :FunctionalProperty , owl:DatatypeProperty ;
      rdfs:comment "Contains the list of provider_category. Provider_category contains the name, UUID of taxonomy object and weight "@en ;
      rdfs:domain ns:BusinessListingCategory ;
      rdfs:label "providerCategory"@en ;
      rdfs:range owl:Literal ;
      owl:subPropertyOf :topDataProperty .

ns:buildDate
      a       :FunctionalProperty , owl:DatatypeProperty ;
      rdfs:comment "The data a particular building was built."@en ;
      rdfs:domain ns:Structure ;
      rdfs:label "buildDate"@en ;
      rdfs:range xsd:date ;
      owl:subPropertyOf ns:date .

ns:stockExchangeOf
      a       owl:ObjectProperty ;
      rdfs:comment "stockExchangeOf connects a stock exchange to the company that is traded on it"@en ;
      rdfs:domain ns:StockExchange ;
      rdfs:label "stockExchangeOf"@en ;
      rdfs:range ns:PublicCompany .

ns:southLatitude
      a       :FunctionalProperty , owl:DatatypeProperty ;
      rdfs:comment "South latitude of the bounding box of a place "@en ;
      rdfs:domain ns:Place ;
      rdfs:label "southLatitude"@en ;
      rdfs:range xsd:float .

ns:Lyrics
      a       owl:Class ;
      rdfs:comment "The words to a song."@en ;
      rdfs:label "Lyrics"@en ;
      owl:subClassOf ns:MediaWork .

ns:disclaimer
      a       owl:DatatypeProperty ;
      rdfs:comment "Limits on a deal or offer."@en , "Example: Limit one per person."@en ;
      rdfs:domain ns:Deal ;
      rdfs:label "disclaimer"@en ;
      rdfs:range owl:Literal .

ns:host
      a       owl:ObjectProperty ;
      rdfs:comment "connects a host to his or her television program."@en ;
      rdfs:domain
              [ a       owl:Class ;
                :unionOf (ns:TvEpisode ns:TvSeason ns:TvSeries ns:TvSpecial)
              ] ;
      rdfs:label "host"@en ;
      rdfs:range ns:Host ;
      owl:subPropertyOf :topObjectProperty .

ns:directedBy
      a       owl:ObjectProperty ;
      rdfs:comment "The directedBy property connects a media artwork to the individual that directed it."@en ;
      rdfs:domain
              [ a       owl:Class ;
                :unionOf (ns:Movie ns:TvEpisode ns:TvSeason ns:TvSeries ns:TvSpecial)
              ] ;
      rdfs:label "directedBy"@en ;
      rdfs:range ns:Director .

ns:ActingRole
      a       owl:Class ;
      rdfs:comment "The ActingRole class is a reified relationship that connects an actor with the media works in which s/he performs."@en ;
      rdfs:label "ActingRole"@en ;
      owl:subClassOf ns:Entity .

ns:makeName
      a       :FunctionalProperty , owl:DatatypeProperty ;
      rdfs:comment "Describes the make of an automobile, the specific product line into which the auto falls."@en ;
      rdfs:domain
              [ a       owl:Class ;
                :unionOf (ns:AutoMake ns:AutoTrim)
              ] ;
      rdfs:label "makeName"@en ;
      rdfs:range owl:Literal ;
      owl:subPropertyOf ns:name .

ns:localEventRank
      a       owl:DatatypeProperty ;
      rdfs:comment "Added for Events team. Added to preserve the raw data stored in the feed."@en ;
      rdfs:domain ns:LocalEvent ;
      rdfs:label "localEventRank"@en ;
      rdfs:range xsd:float .

ns:bonus
      a       owl:DatatypeProperty ;
      rdfs:comment "bonus holds those things a person receives as a bonus, cash and gifts."@en ;
      rdfs:domain ns:Bonus ;
      rdfs:label "bonus"@en ;
      rdfs:range owl:Literal .

ns:postTown
      a       :FunctionalProperty , owl:DatatypeProperty ;
      rdfs:comment "Unique to British mailing addresses."@en ;
      rdfs:domain ns:Address ;
      rdfs:label "postTown"@en ;
      rdfs:range owl:Literal ;
      owl:subPropertyOf :topDataProperty .

ns:modelName
      a       :FunctionalProperty , owl:DatatypeProperty ;
      rdfs:comment "Describes the particular model or a consumer product."@en ;
      rdfs:domain
              [ a       owl:Class ;
                :unionOf (ns:AutoModel ns:AutoTrim)
              ] ;
      rdfs:label "modelName"@en ;
      rdfs:range owl:Literal ;
      owl:subPropertyOf ns:name .

ns:restaurantFeatures
      a       owl:DatatypeProperty ;
      rdfs:comment "Enumerates the types of amenities a restaurant or other food service establishment offers."@en ;
      rdfs:domain ns:Restaurant ;
      rdfs:label "restaurantFeatures"@en ;
      rdfs:range owl:Literal ;
      rdfs:range
              [ a       owl:Datatype ;
                :oneOf  [ a       rdf:List ;
                          rdf:first "BAR"^^xsd:string ;
                          rdf:rest
                                  [ a       rdf:List ;
                                    rdf:first "BRUNCH"^^xsd:string ;
                                    rdf:rest
                                            [ a       rdf:List ;
                                              rdf:first "BUFFET"^^xsd:string ;
                                              rdf:rest
                                                      [ a       rdf:List ;
                                                        rdf:first "CATERING"^^xsd:string ;
                                                        rdf:rest
                                                                [ a       rdf:List ;
                                                                  rdf:first "DANCING"^^xsd:string ;
                                                                  rdf:rest
                                                                          [ a       rdf:List ;
                                                                            rdf:first "ENTERTAINMENT"^^xsd:string ;
                                                                            rdf:rest
                                                                                    [ a       rdf:List ;
                                                                                      rdf:first "GREAT BEER LIST"^^xsd:string ;
                                                                                      rdf:rest
                                                                                              [ a       rdf:List ;
                                                                                                rdf:first "GREAT WINE LIST"^^xsd:string ;
                                                                                                rdf:rest
                                                                                                        [ a       rdf:List ;
                                                                                                          rdf:first "HEALTHY OPTIONS"^^xsd:string ;
                                                                                                          rdf:rest
                                                                                                                  [ a       rdf:List ;
                                                                                                                    rdf:first "LATE NIGHT"^^xsd:string ;
                                                                                                                    rdf:rest
                                                                                                                            [ a       rdf:List ;
                                                                                                                              rdf:first "OUTDOOR SEATING"^^xsd:string ;
                                                                                                                              rdf:rest
                                                                                                                                      [ a       rdf:List ;
                                                                                                                                        rdf:first "PRIVATE ROOMS"^^xsd:string ;
                                                                                                                                        rdf:rest
                                                                                                                                                [ a       rdf:List ;
                                                                                                                                                  rdf:first "SERVES ALCOHOL"^^xsd:string ;
                                                                                                                                                  rdf:rest
                                                                                                                                                          [ a       rdf:List ;
                                                                                                                                                            rdf:first "TAKEOUT"^^xsd:string ;
                                                                                                                                                            rdf:rest
                                                                                                                                                                    [ a       rdf:List ;
                                                                                                                                                                      rdf:first "VIEW"^^xsd:string ;
                                                                                                                                                                      rdf:rest ()
                                                                                                                                                                    ]
                                                                                                                                                          ]
                                                                                                                                                ]
                                                                                                                                      ]
                                                                                                                            ]
                                                                                                                  ]
                                                                                                        ]
                                                                                              ]
                                                                                    ]
                                                                          ]
                                                                ]
                                                      ]
                                            ]
                                  ]
                        ]
              ] ;
      owl:subPropertyOf :topDataProperty .

ns:judgedBy
      a       owl:ObjectProperty ;
      rdfs:comment "The judgedBy property connects a television program to a person who has served as talent judge on the program."@en ;
      rdfs:domain
              [ a       owl:Class ;
                :unionOf (ns:TvEpisode ns:TvSeason ns:TvSeries ns:TvSpecial)
              ] ;
      rdfs:label "judgedBy"@en ;
      rdfs:range ns:ContestJudge ;
      :inverseOf ns:judged .

ns:format
      a       :FunctionalProperty , owl:DatatypeProperty ;
      rdfs:comment "Describes the format of a media product."@en ;
      rdfs:domain ns:MediaProduct ;
      rdfs:label "format"@en ;
      rdfs:range owl:Literal ;
      owl:subPropertyOf :topDataProperty .

ns:ticketing
      a       :FunctionalProperty , owl:DatatypeProperty ;
      rdfs:comment "Indicates whether online ticketing is available at a given theater."@en ;
      rdfs:domain ns:MovieTheater ;
      rdfs:label "ticketing"@en ;
      rdfs:range owl:Literal ;
      owl:subPropertyOf :topDataProperty .

ns:historicCurrencyOf
      a       :FunctionalProperty , owl:DatatypeProperty ;
      rdfs:comment "historicCurrencyOf is any currency an exchange traded in in the past"@en ;
      rdfs:domain ns:Exchange ;
      rdfs:label "historicCurrencyOf"@en ;
      rdfs:range owl:Literal .

ns:recorded
      a       owl:ObjectProperty ;
      rdfs:comment "The recorded property connects a music artist with the albums s/he has created, aka discography."@en ;
      rdfs:domain ns:MusicArtist ;
      rdfs:label "recorded"@en ;
      rdfs:range
              [ a       owl:Class ;
                :unionOf (ns:Album ns:Song)
              ] .

ns:publishDate
      a       :FunctionalProperty , owl:DatatypeProperty ;
      rdfs:comment "The date on which a review or other piece of media was published. May also be used as an administrative attribute that indicates the date on which a listing was published to help faciliate updating of records."@en ;
      rdfs:domain
              [ a       owl:Class ;
                :unionOf (ns:Deal ns:Image ns:LocalEvent ns:Review)
              ] ;
      rdfs:label "publishDate"@en ;
      rdfs:range
              [ a       owl:Datatype ;
                :unionOf (xsd:date xsd:gYearMonth)
              ] ;
      owl:subPropertyOf ns:date .

ns:hostOf
      a       owl:ObjectProperty ;
      rdfs:comment "Connects a host to the television program he or she hosts."@en ;
      rdfs:domain ns:Host ;
      rdfs:label "hostOf"@en ;
      rdfs:range
              [ a       owl:Class ;
                :unionOf (ns:TvEpisode ns:TvSeason ns:TvSeries ns:TvSpecial)
              ] ;
      owl:subPropertyOf :topObjectProperty ;
      :inverseOf ns:host .

ns:tickerSymbol
      a       :FunctionalProperty , owl:DatatypeProperty ;
      rdfs:comment "tickerSymbol Ticker a security trades with on a specific exchange"@en ;
      rdfs:domain
              [ a       owl:Class ;
                :unionOf (ns:Ticker ns:TradableQuotableInstrument)
              ] ;
      rdfs:label "tickerSymbol"@en ;
      rdfs:range owl:Literal .

ns:submissionDate
      a       :FunctionalProperty , owl:DatatypeProperty ;
      rdfs:comment "submissionDate is the date a business listing was submitted"@en ;
      rdfs:domain ns:LocalBusiness ;
      rdfs:label "submissionDate"@en ;
      rdfs:range
              [ a       owl:Datatype ;
                :unionOf (xsd:date xsd:gYearMonth)
              ] ;
      owl:subPropertyOf ns:date .

ns:createdBy
      a       owl:ObjectProperty ;
      rdfs:comment "The createdBy relation connects a Television Program with the person who created the program."@en ;
      rdfs:domain
              [ a       owl:Class ;
                :unionOf (ns:TvSeries ns:TvSpecial)
              ] ;
      rdfs:label "createdBy"@en ;
      rdfs:range ns:ProgramCreator ;
      :inverseOf ns:created .

xsd:time
      a       owl:Datatype .

ns:transferability
      a       :FunctionalProperty , owl:DatatypeProperty ;
      rdfs:comment "Text describing transferability of warranty example: 	Transferable to family members at no additional cost"@en ;
      rdfs:domain ns:Warranty ;
      rdfs:label "transferability"@en ;
      rdfs:range owl:Literal .

ns:EducationalInstitution
      a       owl:Class ;
      rdfs:comment "An institution created for the purpose of education."@en ;
      rdfs:label "EducationalInstitution"@en ;
      owl:subClassOf ns:LocalBusiness .

ns:soundFormat
      a       owl:DatatypeProperty ;
      rdfs:comment "Code(s) that indicate the available audio tracks for languages on a media product. For less common languages, the full name of the language may be indicated in this field."@en ;
      rdfs:domain
              [ a       owl:Class ;
                :unionOf (ns:MediaProduct ns:MediaWork)
              ] ;
      rdfs:label "soundFormat"@en ;
      rdfs:range owl:Literal ;
      owl:subPropertyOf :topDataProperty .

ns:Athlete
      a       owl:Class ;
      rdfs:comment "A person who participates regularly in a sport. An athlete can be amateur or professional."@en ;
      rdfs:label "Athlete"@en ;
      owl:subClassOf ns:Person .

ns:boxofficeRank
      a       :FunctionalProperty , owl:DatatypeProperty ;
      rdfs:comment "Position held by a film's box office receipts in a ranking of weekly  or daily receipts."@en ;
      rdfs:domain
              [ a       owl:Class ;
                :unionOf (ns:BoxOfficeDaily ns:BoxOfficeWeekend ns:BoxOfficeWeekly)
              ] ;
      rdfs:label "boxofficeRank"@en ;
      rdfs:range xsd:int ;
      owl:subPropertyOf :topDataProperty .

ns:alternateOrgName
      a       owl:DatatypeProperty ;
      rdfs:comment "Alternative names for a business or other organization."@en ;
      rdfs:domain
              [ a       owl:Class ;
                :unionOf (ns:Organization ns:SportCompetition)
              ] ;
      rdfs:label "alternateOrgName"@en ;
      rdfs:range owl:Literal ;
      owl:subPropertyOf ns:name .

ns:yearsNew
      a       owl:DatatypeProperty ;
      rdfs:comment "List of years for which make is considered new e.g. sedan. This information is derived from model, trim details in the enrichment phase "@en ;
      rdfs:domain ns:AutoMake ;
      rdfs:label "yearsNew"@en ;
      rdfs:range xsd:gYear .

ns:actingPerformance
      a       owl:ObjectProperty ;
      rdfs:comment "Connects the reified performance class to an actor or performer."@en ;
      rdfs:domain
              [ a       owl:Class ;
                :unionOf (ns:Movie ns:TvEpisode ns:TvSeason ns:TvSeries ns:TvSpecial)
              ] ;
      rdfs:label "actingPerformance"@en ;
      rdfs:range ns:ActingRole ;
      owl:subPropertyOf :topObjectProperty .

ns:MusicalPerformer
      a       owl:Class ;
      rdfs:comment "A musician or music group that performs at a local event."@en ;
      rdfs:label "MusicalPerformer"@en ;
      owl:subClassOf
              [ a       owl:Class ;
                :intersectionOf (ns:MusicArtist ns:Performer)
              ] .

ns:Commodity
      a       owl:Class ;
      rdfs:comment "Commodity good for which there is demand, but which is supplied without qualitative differentiation across a market (for example gold or copper)"@en ;
      rdfs:label "Commodity"@en ;
      owl:subClassOf ns:Future .

ns:affiliationWith
      a       owl:ObjectProperty ;
      rdfs:comment "affiliationWith connects a person, organization, or shareholder to the reified OrgAffiliation class"@en ;
      rdfs:domain
              [ a       owl:Class ;
                :unionOf (ns:Organization ns:Person)
              ] ;
      rdfs:label "affiliationWith"@en ;
      rdfs:range ns:OrgAffiliation .

ns:friendOf
      a       :FunctionalProperty , owl:ObjectProperty ;
      rdfs:comment "Connects the reified Friendship class to an individual."@en ;
      rdfs:domain ns:Friendship ;
      rdfs:label "friendOf"@en ;
      rdfs:range ns:Person ;
      owl:subPropertyOf :topObjectProperty ;
      :inverseOf ns:friend .

ns:AnalystAffiliation
      a       owl:Class ;
      rdfs:comment "AnalystAffiliation is a reified class representing the time an analyst is analyzes a particular organization"@en ;
      rdfs:label "AnalystAffiliation"@en ;
      owl:subClassOf ns:OrgAffiliation .

ns:autoModelOf
      a       owl:ObjectProperty ;
      rdfs:comment "Connects a trim style to the auto model it differentiates."@en ;
      rdfs:domain ns:AutoModel ;
      rdfs:label "autoModelOf"@en ;
      rdfs:range ns:AutoTrim ;
      :inverseOf ns:autoModel .

ns:Composer
      a       owl:Class ;
      rdfs:comment "An individual who writes music."@en ;
      rdfs:label "Composer"@en ;
      owl:subClassOf ns:Person .

ns:MediaProduct
      a       owl:Class ;
      rdfs:comment "The Media Product class includes multimedia consumer products."@en ;
      rdfs:label "MediaProduct"@en ;
      owl:subClassOf ns:ConsumerProduct .

ns:eventOccurrence
      a       owl:ObjectProperty ;
      rdfs:comment "Connects a local event to a single occurrence of that event."@en ;
      rdfs:domain ns:LocalEvent ;
      rdfs:label "eventOccurrence"@en ;
      rdfs:range ns:LocalEventOccurrence .

ns:sector
      a       :FunctionalProperty , owl:DatatypeProperty ;
      rdfs:comment "sector is what market sector a fund invests in or an organization is categorized by"@en ;
      rdfs:domain
              [ a       owl:Class ;
                :unionOf (ns:Fund ns:Organization)
              ] ;
      rdfs:label "sector"@en ;
      rdfs:range owl:Literal .

ns:titleType
      a       :FunctionalProperty , owl:DatatypeProperty ;
      rdfs:comment "Type of alternate title by which a media work is know (eg, translation, AKA, etc.)."@en ;
      rdfs:domain ns:AlternateTitle ;
      rdfs:label "titleType"@en ;
      rdfs:range owl:Literal ;
      owl:subPropertyOf :topDataProperty .

ns:BoardMember
      a       owl:Class ;
      rdfs:comment "BoardMember represents those people who are members of a company's board of directors."@en ;
      rdfs:label "BoardMember"@en ;
      owl:subClassOf ns:FinancePerson .

ns:series
      a       :FunctionalProperty , owl:DatatypeProperty ;
      rdfs:comment "Describes series information about a video product, eg. \"Hollywood Classics.\" "@en ;
      rdfs:domain ns:Video ;
      rdfs:label "series"@en ;
      rdfs:range owl:Literal ;
      owl:subPropertyOf :topDataProperty .

ns:preciseGeo
      a       :FunctionalProperty , owl:DatatypeProperty ;
      rdfs:comment "Is this geo location precise? (India has specific usecases around this) "@en ;
      rdfs:domain ns:Place ;
      rdfs:label "preciseGeo"@en ;
      rdfs:range owl:Literal ;
      owl:subPropertyOf :topDataProperty .

ns:feature
      a       owl:DatatypeProperty ;
      rdfs:comment "A listing of special features that appear on a media product."@en ;
      rdfs:domain
              [ a       owl:Class ;
                :unionOf (ns:AutoTrim ns:MediaProduct)
              ] ;
      rdfs:label "feature"@en ;
      rdfs:range owl:Literal ;
      owl:subPropertyOf :topDataProperty .

ns:rawAddress
      a       owl:DatatypeProperty ;
      rdfs:comment "Raw, unparsed address data."@en ;
      rdfs:domain
              [ a       owl:Class ;
                :unionOf (ns:Address ns:SingleLocationBusiness)
              ] ;
      rdfs:label "rawAddress"@en ;
      rdfs:range owl:Literal .

ns:redeemFromHome
      a       :FunctionalProperty , owl:DatatypeProperty ;
      rdfs:comment "Indicates whether a deal or offer can be redeemed from home."@en ;
      rdfs:domain ns:Deal ;
      rdfs:label "redeemFromHome"@en ;
      rdfs:range xsd:boolean .

ns:gradeLevel
      a       owl:DatatypeProperty ;
      rdfs:comment "Describes the grade level taught at an educational institution."@en ;
      rdfs:domain ns:EducationalInstitution ;
      rdfs:label "gradeLevel"@en ;
      rdfs:range owl:Literal .

ns:release
      a       owl:ObjectProperty ;
      rdfs:comment "Connects a media work to the reified media release class."@en ;
      rdfs:domain
              [ a       owl:Class ;
                :unionOf (ns:MediaProduct ns:MediaWork)
              ] ;
      rdfs:label "release"@en ;
      rdfs:range ns:MediaRelease ;
      owl:subPropertyOf :topObjectProperty ;
      :inverseOf ns:releaseFor .

ns:competitionGroupFor
      a       owl:ObjectProperty ;
      rdfs:comment "Connects a competition instance with the competition organization that organizes it."@en ;
      rdfs:domain ns:SportCompetition ;
      rdfs:label "competitionGroupFor"@en ;
      rdfs:range ns:SportCompetitionInstance ;
      :inverseOf ns:competitionGroup .

ns:ratingCount
      a       :FunctionalProperty , owl:DatatypeProperty ;
      rdfs:comment "Number of consumer product ratings."@en ;
      rdfs:domain ns:Review ;
      rdfs:label "ratingCount"@en ;
      rdfs:range xsd:int ;
      owl:subPropertyOf :topDataProperty .

ns:theaterAttribute
      a       owl:DatatypeProperty ;
      rdfs:comment "Describes features of a theater and services offered, including wheelchair accessibility, seating type, parking, etc."@en ;
      rdfs:domain ns:MovieTheater ;
      rdfs:label "theaterAttribute"@en ;
      rdfs:range owl:Literal ;
      owl:subPropertyOf :topDataProperty .

ns:phonePrefix
      a       :FunctionalProperty , owl:DatatypeProperty ;
      rdfs:comment "Prefix code of a phone number"@en ;
      rdfs:domain ns:Phone ;
      rdfs:label "phonePrefix"@en ;
      rdfs:range owl:Literal ;
      owl:subPropertyOf :topDataProperty .

ns:news
      a       :FunctionalProperty , owl:DatatypeProperty ;
      rdfs:comment "Link to an online item's news page."@en ;
      rdfs:domain ns:Entity ;
      rdfs:label "news"@en ;
      rdfs:range xsd:anyURI ;
      owl:subPropertyOf :topDataProperty .

ns:musicPerformanceOf
      a       owl:ObjectProperty ;
      rdfs:comment "Connects a recorded performance to a musical work."@en ;
      rdfs:domain ns:MusicPerformance ;
      rdfs:label "musicPerformanceOf"@en ;
      rdfs:range
              [ a       owl:Class ;
                :unionOf (ns:Composition ns:CompositionPart ns:Song)
              ] ;
      owl:subPropertyOf :topObjectProperty .

ns:relatedEvent
      a       owl:ObjectProperty ;
      rdfs:comment "Connects local events that are related in some way."@en ;
      rdfs:domain ns:LocalEvent ;
      rdfs:label "relatedEvent"@en ;
      rdfs:range ns:LocalEvent .

ns:playsWith
      a       owl:ObjectProperty ;
      rdfs:comment "The playsWith relation connects a MusicArtist to his/her BandAffiliation."@en ;
      rdfs:domain ns:Musician ;
      rdfs:label "playsWith"@en ;
      rdfs:range ns:BandAffiliation .

ns:parentCategory
      a       :FunctionalProperty , owl:DatatypeProperty ;
      rdfs:comment "Parent category name in Y! category tree "@en ;
      rdfs:domain ns:BusinessListingCategory ;
      rdfs:label "parentCategory"@en ;
      rdfs:range owl:Literal ;
      owl:subPropertyOf :topDataProperty .

ns:written
      a       owl:ObjectProperty ;
      rdfs:comment "The written property connects an individual or organization to a written work that he/she/it has created."@en ;
      rdfs:domain ns:Writer ;
      rdfs:label "written"@en ;
      rdfs:range
              [ a       owl:Class ;
                :unionOf (ns:Biography ns:MediaWork ns:Review ns:Synopsis)
              ] ;
      :inverseOf ns:writtenBy .

ns:creditType
      a       :FunctionalProperty , owl:DatatypeProperty ;
      rdfs:comment "The role for which an individual was credited in a film or television program."@en ;
      rdfs:domain
              [ a       owl:Class ;
                :unionOf (ns:CompanyRole ns:CrewRole)
              ] ;
      rdfs:label "creditType"@en ;
      rdfs:range owl:Literal ;
      owl:subPropertyOf :topDataProperty .

ns:eventGroup
      a       owl:DatatypeProperty ;
      rdfs:comment "Captures if an event occurs as part of a larger grouping of events. Eg, Game One in the MLB World Series or one stop on a musical tour."@en ;
      rdfs:domain ns:LocalEvent ;
      rdfs:label "eventGroup"@en ;
      rdfs:range xsd:boolean .

ns:playedBy
      a       owl:ObjectProperty ;
      rdfs:comment "Connects a sport to the athletes that play it."@en ;
      rdfs:domain ns:Sport ;
      rdfs:label "playedBy"@en ;
      rdfs:range
              [ a       owl:Class ;
                :unionOf (ns:Athlete ns:AthleticConference ns:SportDivision ns:SportLeague ns:SportTeam)
              ] .

ns:USCongressperson
      a       owl:Class ;
      rdfs:comment "Created by ace to support Milton mapping: http://twiki.corp.yahoo.com/view/P13nContextual/MiltonWooSchemaMap"@en , "An individual elected to the United States House of Representatives."@en ;
      rdfs:label "USCongressperson"@en ;
      owl:subClassOf ns:Politician .

ns:minPrice
      a       owl:DatatypeProperty ;
      rdfs:comment "Indicates the minimum price for a product or service."@en ;
      rdfs:domain
              [ a       owl:Class ;
                :unionOf (ns:Deal ns:EventRegistration ns:LocalEventOccurrence)
              ] ;
      rdfs:label "minPrice"@en ;
      rdfs:range xsd:int .

ns:marriedTo
      a       :FunctionalProperty , owl:ObjectProperty ;
      rdfs:comment "The marriedTo property connects the reified Marriage class to the individuals engaged in the marriage."@en ;
      rdfs:domain ns:Marriage ;
      rdfs:label "marriedTo"@en ;
      rdfs:range ns:Person .

ns:ProgramCreator
      a       owl:Class ;
      rdfs:comment "This type is for people who are credited with creating a TV series. They may or may not also be directors, writers, and producers of the series"@en ;
      rdfs:label "ProgramCreator"@en ;
      owl:subClassOf ns:Person .

ns:extendedWarranty
      a       owl:DatatypeProperty ;
      rdfs:comment "An extended warranty, sometimes called a service agreement, a service contract, or a maintenance agreement, is a prolonged warranty offered to consumers. Example Isuzu Protection Plan offers various plans with coverage up to 84 months/100,000 miles."@en ;
      rdfs:domain ns:Warranty ;
      rdfs:label "extendedWarranty"@en ;
      rdfs:range owl:Literal .

ns:performedMusic
      a       owl:ObjectProperty ;
      rdfs:comment "Connects a performer to a musical performance"@en ;
      rdfs:domain ns:MusicArtist ;
      rdfs:label "performedMusic"@en ;
      rdfs:range ns:MusicPerformance ;
      owl:subPropertyOf :topObjectProperty .

ns:teamPlay
      a       owl:ObjectProperty ;
      rdfs:comment "Connects a game to the teams that played in it"@en ;
      rdfs:domain ns:SportTeam ;
      rdfs:label "teamPlay"@en ;
      rdfs:range ns:SportGame ;
      owl:subPropertyOf :topObjectProperty .

ns:marketTierName
      a       :FunctionalProperty , owl:DatatypeProperty ;
      rdfs:comment "marketTierName is the name of a market tier, for example Nasdaq Global Market"@en ;
      rdfs:domain
              [ a       owl:Class ;
                :unionOf (ns:MarketTier ns:TradableQuotableInstrument)
              ] ;
      rdfs:label "marketTiername"@en ;
      rdfs:range owl:Literal ;
      owl:subPropertyOf ns:name .

ns:autoIncentiveOf
      a       :FunctionalProperty , owl:ObjectProperty ;
      rdfs:comment "Connects the auto trim class to its incentive class"@en ;
      rdfs:domain ns:AutoIncentive ;
      rdfs:label "autoIncentiveOf"@en ;
      rdfs:range ns:AutoTrim ;
      :inverseOf ns:autoIncentive .

ns:establishedDate
      a       :FunctionalProperty , owl:DatatypeProperty ;
      rdfs:comment "Year or date on which a business was established."@en ;
      rdfs:domain ns:LocalBusiness ;
      rdfs:label "establishedDate"@en ;
      rdfs:range
              [ a       owl:Datatype ;
                :unionOf (xsd:date xsd:gYear)
              ] ;
      owl:subPropertyOf ns:date .

ns:characterName
      a       :FunctionalProperty , owl:DatatypeProperty ;
      rdfs:comment "The name of a fictional character."@en ;
      rdfs:domain ns:ActingRole ;
      rdfs:label "characterName"@en ;
      rdfs:range owl:Literal ;
      owl:subPropertyOf ns:name .

ns:priceNumber
      a       owl:DatatypeProperty ;
      rdfs:comment "Price expressed as a number."@en ;
      rdfs:domain ns:Deal ;
      rdfs:label "priceNumber"@en ;
      rdfs:range xsd:float .

ns:mediaProductOf
      a       :FunctionalProperty , owl:ObjectProperty ;
      rdfs:comment "Connects a media product to the media work it represents."@en ;
      rdfs:domain ns:MediaProduct ;
      rdfs:label "mediaProductOf"@en ;
      rdfs:range ns:MediaWork ;
      owl:subPropertyOf :topObjectProperty ;
      :inverseOf ns:mediaProduct .

ns:Debenture
      a       owl:Class ;
      rdfs:comment "Debenture is an unsecured corporate bond"@en ;
      rdfs:label "Debenture"@en ;
      owl:subClassOf ns:Debt .

ns:GovernmentAgency
      a       owl:Class ;
      rdfs:comment "a permanent or semi-permanent organization in the machinery of government that is responsible for the oversight and administration of specific functions, such as an intelligence agency."@en ;
      rdfs:label "GovernmentAgency"@en ;
      owl:subClassOf ns:Organization .

ns:extraCost
      a       owl:DatatypeProperty ;
      rdfs:comment "Represents the additional cost for colors or other features that are available as additional option "@en ;
      rdfs:domain ns:Color ;
      rdfs:label "extraCost"@en ;
      rdfs:range xsd:double .

ns:label
      a       :FunctionalProperty , owl:DatatypeProperty ;
      rdfs:comment "Generic label property used when multiple titles/names/etc are needed. More specific properties are movie title, person name etc. "@en , "Describes the title of an entity."@en ;
      rdfs:domain ns:Entity ;
      rdfs:label "label"@en ;
      rdfs:range owl:Literal ;
      owl:subPropertyOf :topDataProperty .

ns:AthleteGameRole
      a       owl:Class ;
      rdfs:comment "Reified class describes the activity of a player in a particular game or competition."@en ;
      rdfs:label "AthleteGameRole"@en ;
      owl:subClassOf ns:Entity .

ns:popularity
      a       owl:DatatypeProperty ;
      rdfs:comment "indicates the popularity of a particular deal"@en ;
      rdfs:domain ns:Deal ;
      rdfs:label "popularity"@en ;
      rdfs:range owl:Literal .

:topDataProperty
      a       owl:DatatypeProperty .

ns:member
      a       owl:ObjectProperty ;
      rdfs:comment "The member relation connects an individual with the groups in which s/he has membership."@en ;
      rdfs:domain ns:Group ;
      rdfs:label "member"@en ;
      rdfs:range
              [ a       owl:Class ;
                :unionOf (ns:Group ns:Person)
              ] ;
      :inverseOf ns:memberOf .

ns:tvSeasonOf
      a       owl:ObjectProperty ;
      rdfs:comment "Connects a tv program to its seasons."@en ;
      rdfs:domain ns:TvSeries ;
      rdfs:label "tvSeasonOf"@en ;
      rdfs:range ns:TvSeason ;
      owl:subPropertyOf :topObjectProperty .

ns:ownsShares
      a       owl:ObjectProperty ;
      rdfs:comment "ownsShares connects a person or organization to the majorshareholderaffiliation"@en ;
      rdfs:domain
              [ a       owl:Class ;
                :unionOf (ns:Organization ns:Person)
              ] ;
      rdfs:label "ownsShares"@en ;
      rdfs:range ns:MajorShareholderAffiliation .

ns:streetType
      a       :FunctionalProperty , owl:DatatypeProperty ;
      rdfs:comment "Avenue, lane, etc"@en ;
      rdfs:domain
              [ a       owl:Class ;
                :unionOf (ns:Address ns:SingleLocationBusiness)
              ] ;
      rdfs:label "streetType"@en ;
      rdfs:range owl:Literal ;
      owl:subPropertyOf :topDataProperty .

ns:compositionPart
      a       owl:ObjectProperty ;
      rdfs:comment "Ties a compositon to its parts"@en ;
      rdfs:domain ns:Composition ;
      rdfs:label "compositionPart"@en ;
      rdfs:range ns:CompositionPart ;
      owl:subPropertyOf :topObjectProperty .

ns:makeModelOf
      a       owl:ObjectProperty ;
      rdfs:comment "Connects the auto model class to the auto make class."@en ;
      rdfs:domain ns:AutoModel ;
      rdfs:label "makeModelOf"@en ;
      rdfs:range ns:AutoMake ;
      :inverseOf ns:makeModel .

ns:Fundraiser
      a       owl:Class ;
      rdfs:comment "Event to raise funds for a cause. Includes benefits."@en ;
      rdfs:label "Fundraiser"@en ;
      owl:subClassOf ns:Event .

ns:businessCategoryOf
      a       owl:ObjectProperty ;
      rdfs:comment "businessCategoryOf conntects LocalBusinessCategory to LocalBusiness"@en ;
      rdfs:domain ns:LocalBusinessCategory ;
      rdfs:label "businessCategoryOf"@en ;
      rdfs:range ns:LocalBusiness ;
      :inverseOf ns:businessCategory .
